@prefix : <http://FYP-ASHS21/csonto/> .
@prefix owl: <http://www.w3.org/2002/07/owl#> .
@prefix rdf: <http://www.w3.org/1999/02/22-rdf-syntax-ns#> .
@prefix xml: <http://www.w3.org/XML/1998/namespace> .
@prefix xsd: <http://www.w3.org/2001/XMLSchema#> .
@prefix rdfs: <http://www.w3.org/2000/01/rdf-schema#> .
@base <http://FYP-ASHS21/csonto/> .

<http://FYP-ASHS21/csonto> rdf:type owl:Ontology ;
                            owl:versionIRI <http://FYP-ASHS21/csonto/1.0> ;
                            rdfs:comment "This is the cybersecurity ontology, which represents the overall structure of the cybersecurity organisation. It allows it to monitor its current state and find out about issues by tracing it back." .

#################################################################
#    Annotation properties
#################################################################

###  http://FYP-ASHS21/csonto/implementesPolicy
:implementesPolicy rdf:type owl:AnnotationProperty ;
                   rdfs:subPropertyOf rdfs:isDefinedBy .


#################################################################
#    Object Properties
#################################################################

###  http://FYP-ASHS21/csonto#definePolicy
:definePolicy rdf:type owl:ObjectProperty ;
              rdfs:isDefinedBy "" .


###  http://FYP-ASHS21/csonto#reportTo
:reportTo rdf:type owl:ObjectProperty ,
                   owl:TransitiveProperty ;
          rdfs:domain :Asset_Management ,
                      :Assurance ,
                      :Change_Management ,
                      :Emerging_Technologies ,
                      :Governance ,
                      :Security_Operations ;
          rdfs:range :CyberSecurityScore .


###  http://purl.obolibrary.org/obo/CSONTO_cf5cef00_b075_4a8d_8d89_8700eb871011
<http://purl.obolibrary.org/obo/CSONTO_cf5cef00_b075_4a8d_8d89_8700eb871011> rdf:type owl:ObjectProperty ;
                                                                             rdfs:label "implementsPolicy"@en .


#################################################################
#    Data properties
#################################################################

###  http://FYP-ASHS21/csonto#DataPrivacy
:DataPrivacy rdf:type owl:DatatypeProperty ;
             rdfs:subPropertyOf :EmergingTechProperities ;
             rdf:type owl:FunctionalProperty ;
             rdfs:domain :Data_Protection ,
                         :Emerging_Technologies ;
             rdfs:range xsd:boolean ,
                        owl:rational .


###  http://FYP-ASHS21/csonto#Explainability
:Explainability rdf:type owl:DatatypeProperty ;
                rdfs:subPropertyOf :EmergingTechProperities ;
                rdfs:domain :Emerging_Technologies ;
                rdfs:range xsd:string .


###  http://FYP-ASHS21/csonto#Fairness
:Fairness rdf:type owl:DatatypeProperty ;
          rdfs:subPropertyOf :EmergingTechProperities ;
          rdfs:domain :Emerging_Technologies ;
          rdfs:range xsd:string .


###  http://FYP-ASHS21/csonto#Resilience
:Resilience rdf:type owl:DatatypeProperty ;
            rdfs:subPropertyOf :EmergingTechProperities ;
            rdfs:domain :Emerging_Technologies ;
            rdfs:range xsd:string .


###  http://FYP-ASHS21/csonto#Safety
:Safety rdf:type owl:DatatypeProperty ;
        rdfs:subPropertyOf :EmergingTechProperities ;
        rdfs:domain :Emerging_Technologies ;
        rdfs:range xsd:string .


###  http://FYP-ASHS21/csonto#Transparency
:Transparency rdf:type owl:DatatypeProperty ;
              rdfs:subPropertyOf :EmergingTechProperities ;
              rdfs:domain :Emerging_Technologies ;
              rdfs:range xsd:string .


###  http://FYP-ASHS21/csonto#Trustworthiness
:Trustworthiness rdf:type owl:DatatypeProperty ;
                 rdfs:subPropertyOf :EmergingTechProperities ;
                 rdfs:domain :Emerging_Technologies ;
                 rdfs:range xsd:string .


###  http://FYP-ASHS21/csonto/ASTWeight
:ASTWeight rdf:type owl:DatatypeProperty ;
           rdfs:subPropertyOf :AssetManagementProperities ,
                              :TotalScore ;
           rdf:type owl:FunctionalProperty ;
           rdfs:domain :Asset_Management ,
                       [ rdf:type owl:Restriction ;
                         owl:onProperty :ASTWeight ;
                         owl:allValuesFrom xsd:long
                       ] ,
                       [ rdf:type owl:Restriction ;
                         owl:onProperty :ASTWeight ;
                         owl:minQualifiedCardinality "737"^^xsd:nonNegativeInteger ;
                         owl:onDataRange xsd:long
                       ] .


###  http://FYP-ASHS21/csonto/ASUWeight
:ASUWeight rdf:type owl:DatatypeProperty ;
           rdfs:subPropertyOf :AssuranceProperities ,
                              :TotalScore ;
           rdfs:domain :Assurance ,
                       [ rdf:type owl:Restriction ;
                         owl:onProperty :ASUWeight ;
                         owl:allValuesFrom xsd:long
                       ] ,
                       [ rdf:type owl:Restriction ;
                         owl:onProperty :ASUWeight ;
                         owl:minQualifiedCardinality "312"^^xsd:nonNegativeInteger ;
                         owl:onDataRange xsd:long
                       ] ;
           rdfs:range xsd:long .


###  http://FYP-ASHS21/csonto/AccessControl
:AccessControl rdf:type owl:DatatypeProperty ;
               rdfs:subPropertyOf :AssetManagementProperities ;
               rdf:type owl:FunctionalProperty ;
               rdfs:domain :Asset_Management ,
                           :Infrastructure_And_Identity_And_Access_Management ;
               rdfs:range xsd:boolean ,
                          xsd:token .


###  http://FYP-ASHS21/csonto/ArchitecturalDesignOversight
:ArchitecturalDesignOversight rdf:type owl:DatatypeProperty ;
                              rdfs:subPropertyOf :EmergingTechProperities ;
                              rdfs:domain :Emerging_Technologies ;
                              rdfs:range xsd:string .


###  http://FYP-ASHS21/csonto/AssetAuthorisation
:AssetAuthorisation rdf:type owl:DatatypeProperty ;
                    rdfs:subPropertyOf :AssetManagementProperities ;
                    rdfs:domain :Asset_Management ,
                                :Infrastructure_And_Identity_And_Access_Management ;
                    rdfs:range xsd:boolean .


###  http://FYP-ASHS21/csonto/AssetManagementProperities
:AssetManagementProperities rdf:type owl:DatatypeProperty .


###  http://FYP-ASHS21/csonto/AssetTracking
:AssetTracking rdf:type owl:DatatypeProperty ;
               rdfs:subPropertyOf :AssetManagementProperities ;
               rdfs:domain :Asset_Management ;
               rdfs:range xsd:language .


###  http://FYP-ASHS21/csonto/AssuranceProperities
:AssuranceProperities rdf:type owl:DatatypeProperty .


###  http://FYP-ASHS21/csonto/AwarenessCampaignsAndFeedback
:AwarenessCampaignsAndFeedback rdf:type owl:DatatypeProperty ;
                               rdfs:subPropertyOf :AssuranceProperities ;
                               rdfs:domain :Assurance ;
                               rdfs:range xsd:string .


###  http://FYP-ASHS21/csonto/CMWeight
:CMWeight rdf:type owl:DatatypeProperty ;
          rdfs:subPropertyOf :ChangeManagementProperities ,
                             :TotalScore ;
          rdfs:domain :Change_Management ,
                      [ rdf:type owl:Restriction ;
                        owl:onProperty :CMWeight ;
                        owl:allValuesFrom xsd:long
                      ] ,
                      [ rdf:type owl:Restriction ;
                        owl:onProperty :CMWeight ;
                        owl:minQualifiedCardinality "819"^^xsd:nonNegativeInteger ;
                        owl:onDataRange xsd:long
                      ] .


###  http://FYP-ASHS21/csonto/ChangeImpactAssessment
:ChangeImpactAssessment rdf:type owl:DatatypeProperty ;
                        rdfs:subPropertyOf :ChangeManagementProperities ;
                        rdfs:domain :Change_Management ;
                        rdfs:range xsd:string .


###  http://FYP-ASHS21/csonto/ChangeManagementProperities
:ChangeManagementProperities rdf:type owl:DatatypeProperty .


###  http://FYP-ASHS21/csonto/ComplianceMonoitoring
:ComplianceMonoitoring rdf:type owl:DatatypeProperty ;
                       rdfs:subPropertyOf :AssetManagementProperities ;
                       rdfs:domain :Asset_Management ,
                                   :Compliance ;
                       rdfs:range xsd:string .


###  http://FYP-ASHS21/csonto/ContinuousDev
:ContinuousDev rdf:type owl:DatatypeProperty ;
               rdfs:subPropertyOf :EmbeddedTechSecProperities ;
               rdfs:domain :Embdded_Technologies ;
               rdfs:range xsd:language ,
                          xsd:string .


###  http://FYP-ASHS21/csonto/ContinuousMonitoring
:ContinuousMonitoring rdf:type owl:DatatypeProperty ;
                      rdfs:subPropertyOf :VulnerabilitiesManagmenetProperities ;
                      rdfs:domain :Vulnerability_And_Web_Management ;
                      rdfs:range xsd:boolean ,
                                 xsd:string .


###  http://FYP-ASHS21/csonto/ContractualFulfillmentAndInternalStandards
:ContractualFulfillmentAndInternalStandards rdf:type owl:DatatypeProperty ;
                                            rdfs:subPropertyOf :AssuranceProperities ;
                                            rdfs:domain :Assurance ;
                                            rdfs:range xsd:string .


###  http://FYP-ASHS21/csonto/CryptographicStandards
:CryptographicStandards rdf:type owl:DatatypeProperty ;
                        rdfs:subPropertyOf :DataProtectionProperities ;
                        rdfs:domain :Data_Protection ;
                        rdfs:range xsd:language ,
                                   xsd:string .


###  http://FYP-ASHS21/csonto/DataClassification
:DataClassification rdf:type owl:DatatypeProperty ;
                    rdfs:subPropertyOf :DataProtectionProperities ;
                    rdfs:domain :Data_Protection ;
                    rdfs:range xsd:string .


###  http://FYP-ASHS21/csonto/DataProtection
:DataProtection rdf:type owl:DatatypeProperty ;
                rdfs:subPropertyOf :AssetManagementProperities ;
                rdfs:domain :Asset_Management ,
                            :Data_Protection ;
                rdfs:range owl:rational .


###  http://FYP-ASHS21/csonto/DataProtectionProperities
:DataProtectionProperities rdf:type owl:DatatypeProperty ;
                           rdfs:subPropertyOf :SecOpsProprities .


###  http://FYP-ASHS21/csonto/DeviceOwnershipAndCentralizedManagement
:DeviceOwnershipAndCentralizedManagement rdf:type owl:DatatypeProperty ;
                                         rdfs:subPropertyOf :AssetManagementProperities ;
                                         rdfs:domain :Asset_Management ;
                                         rdfs:range xsd:string ,
                                                    xsd:token .


###  http://FYP-ASHS21/csonto/DisposalProcedure
:DisposalProcedure rdf:type owl:DatatypeProperty ;
                   rdfs:subPropertyOf :AssetManagementProperities ;
                   rdfs:domain :Asset_Management ;
                   rdfs:range xsd:string .


###  http://FYP-ASHS21/csonto/Documentation
:Documentation rdf:type owl:DatatypeProperty ;
               rdfs:subPropertyOf :AssetManagementProperities ;
               rdfs:domain :Asset_Management ;
               rdfs:range xsd:string .


###  http://FYP-ASHS21/csonto/ETWeight
:ETWeight rdf:type owl:DatatypeProperty ;
          rdfs:subPropertyOf :EmergingTechProperities ,
                             :TotalScore ;
          rdfs:domain :Emerging_Technologies ,
                      [ rdf:type owl:Restriction ;
                        owl:onProperty :ETWeight ;
                        owl:allValuesFrom xsd:long
                      ] ,
                      [ rdf:type owl:Restriction ;
                        owl:onProperty :ETWeight ;
                        owl:minQualifiedCardinality "658"^^xsd:nonNegativeInteger ;
                        owl:onDataRange xsd:long
                      ] .


###  http://FYP-ASHS21/csonto/EmbeddedTechSecProperities
:EmbeddedTechSecProperities rdf:type owl:DatatypeProperty ;
                            rdfs:subPropertyOf :SecOpsProprities .


###  http://FYP-ASHS21/csonto/EmergingTechProperities
:EmergingTechProperities rdf:type owl:DatatypeProperty .


###  http://FYP-ASHS21/csonto/GovWeight
:GovWeight rdf:type owl:DatatypeProperty ;
           rdfs:subPropertyOf :GovernanceProperities ,
                              :TotalScore ;
           rdfs:domain :Governance ,
                       [ rdf:type owl:Restriction ;
                         owl:onProperty :GovWeight ;
                         owl:allValuesFrom xsd:long
                       ] ,
                       [ rdf:type owl:Restriction ;
                         owl:onProperty :GovWeight ;
                         owl:minQualifiedCardinality "277"^^xsd:nonNegativeInteger ;
                         owl:onDataRange xsd:long
                       ] ;
           rdfs:range xsd:long .


###  http://FYP-ASHS21/csonto/GovernanceProperities
:GovernanceProperities rdf:type owl:DatatypeProperty .


###  http://FYP-ASHS21/csonto/HasWeight
:HasWeight rdf:type owl:DatatypeProperty .


###  http://FYP-ASHS21/csonto/IncidentResponse
:IncidentResponse rdf:type owl:DatatypeProperty ;
                  rdfs:subPropertyOf :SecOpsProprities ;
                  rdfs:domain :Security_Operations ;
                  rdfs:range rdfs:Literal ,
                             xsd:boolean ,
                             xsd:integer ,
                             xsd:string ,
                             xsd:token .


###  http://FYP-ASHS21/csonto/InformationProtectionMeasures
:InformationProtectionMeasures rdf:type owl:DatatypeProperty ;
                               rdfs:subPropertyOf :AssuranceProperities ;
                               rdfs:domain :Assurance ;
                               rdfs:range xsd:string .


###  http://FYP-ASHS21/csonto/InfraDataEncryption
:InfraDataEncryption rdf:type owl:DatatypeProperty ;
                     rdfs:subPropertyOf :InfraSecProperities ;
                     rdfs:domain :Data_Protection ,
                                 :Infrastructure_And_Identity_And_Access_Management ;
                     rdfs:range xsd:string ,
                                xsd:token .


###  http://FYP-ASHS21/csonto/InfraEndpointSecurity
:InfraEndpointSecurity rdf:type owl:DatatypeProperty ;
                       rdfs:subPropertyOf :InfraSecProperities ;
                       rdfs:domain :Infrastructure_And_Identity_And_Access_Management ;
                       rdfs:range xsd:boolean ,
                                  xsd:string ,
                                  xsd:token .


###  http://FYP-ASHS21/csonto/InfraFirewallImplementation
:InfraFirewallImplementation rdf:type owl:DatatypeProperty ;
                             rdfs:subPropertyOf :InfraSecProperities ;
                             rdfs:domain :Infrastructure_And_Identity_And_Access_Management ;
                             rdfs:range xsd:boolean ,
                                        xsd:string .


###  http://FYP-ASHS21/csonto/InfraNetworkAccessControl
:InfraNetworkAccessControl rdf:type owl:DatatypeProperty ;
                           rdfs:subPropertyOf :InfraSecProperities ;
                           rdfs:domain :Infrastructure_And_Identity_And_Access_Management ;
                           rdfs:range xsd:boolean ,
                                      xsd:string ,
                                      xsd:token .


###  http://FYP-ASHS21/csonto/InfraNetworkMonitoring
:InfraNetworkMonitoring rdf:type owl:DatatypeProperty ;
                        rdfs:subPropertyOf :InfraSecProperities ;
                        rdfs:domain :Infrastructure_And_Identity_And_Access_Management ;
                        rdfs:range xsd:dateTimeStamp ,
                                   xsd:string .


###  http://FYP-ASHS21/csonto/InfraNetworkSegmentation
:InfraNetworkSegmentation rdf:type owl:DatatypeProperty ;
                          rdfs:subPropertyOf :InfraSecProperities ;
                          rdfs:domain :Infrastructure_And_Identity_And_Access_Management ;
                          rdfs:range xsd:dateTimeStamp ,
                                     xsd:integer ,
                                     xsd:string ,
                                     xsd:token .


###  http://FYP-ASHS21/csonto/InfraSecConfiguration
:InfraSecConfiguration rdf:type owl:DatatypeProperty ;
                       rdfs:subPropertyOf :InfraSecProperities ;
                       rdfs:domain :Infrastructure_And_Identity_And_Access_Management ;
                       rdfs:range xsd:dateTimeStamp ,
                                  xsd:long ,
                                  xsd:string ,
                                  xsd:token .


###  http://FYP-ASHS21/csonto/InfraSecProperities
:InfraSecProperities rdf:type owl:DatatypeProperty ;
                     rdfs:subPropertyOf :SecOpsProprities .


###  http://FYP-ASHS21/csonto/InvnetoryManagement
:InvnetoryManagement rdf:type owl:DatatypeProperty ;
                     rdfs:subPropertyOf :AssetManagementProperities ;
                     rdfs:domain :Asset_Management ;
                     rdfs:range xsd:string .


###  http://FYP-ASHS21/csonto/LeadershipEnagement
:LeadershipEnagement rdf:type owl:DatatypeProperty ;
                     rdfs:subPropertyOf :GovernanceProperities ;
                     rdfs:domain :Governance ;
                     rdfs:range xsd:string .


###  http://FYP-ASHS21/csonto/LifeCycleManagment
:LifeCycleManagment rdf:type owl:DatatypeProperty ;
                    rdfs:subPropertyOf :AssetManagementProperities ;
                    rdfs:domain :Asset_Management ;
                    rdfs:range xsd:string .


###  http://FYP-ASHS21/csonto/MaintanenceProcedure
:MaintanenceProcedure rdf:type owl:DatatypeProperty ;
                      rdfs:subPropertyOf :AssetManagementProperities ;
                      rdfs:domain :Asset_Management ;
                      rdfs:range xsd:string .


###  http://FYP-ASHS21/csonto/NamingStandrization
:NamingStandrization rdf:type owl:DatatypeProperty ;
                     rdfs:subPropertyOf :AssetManagementProperities ;
                     rdfs:domain :Asset_Management ;
                     rdfs:range xsd:string .


###  http://FYP-ASHS21/csonto/OpsSecTraining
:OpsSecTraining rdf:type owl:DatatypeProperty ;
                rdfs:subPropertyOf :SecOpsProprities ;
                rdfs:domain :Security_Operations ;
                rdfs:range xsd:string .


###  http://FYP-ASHS21/csonto/PatchManagement
:PatchManagement rdf:type owl:DatatypeProperty ;
                 rdfs:subPropertyOf :VulnerabilitiesManagmenetProperities ;
                 rdfs:domain :Vulnerability_And_Web_Management ;
                 rdfs:range xsd:language .


###  http://FYP-ASHS21/csonto/ProactiveChangeAndSecurityIntegration
:ProactiveChangeAndSecurityIntegration rdf:type owl:DatatypeProperty ;
                                       rdfs:subPropertyOf :ChangeManagementProperities ;
                                       rdfs:domain :Change_Management ;
                                       rdfs:range xsd:string .


###  http://FYP-ASHS21/csonto/ProcurementProcedure
:ProcurementProcedure rdf:type owl:DatatypeProperty ;
                      rdfs:subPropertyOf :AssetManagementProperities ;
                      rdfs:domain :Asset_Management ;
                      rdfs:range xsd:string .


###  http://FYP-ASHS21/csonto/ProgramDevelopment
:ProgramDevelopment rdf:type owl:DatatypeProperty ;
                    rdfs:subPropertyOf :GovernanceProperities ;
                    rdfs:domain :Governance ;
                    rdfs:range xsd:string .


###  http://FYP-ASHS21/csonto/Provenance
:Provenance rdf:type owl:DatatypeProperty ;
            rdfs:subPropertyOf :AssetManagementProperities ;
            rdfs:domain :Asset_Management ;
            rdfs:range xsd:string .


###  http://FYP-ASHS21/csonto/RegulatoryAndStatutoryCompliance
:RegulatoryAndStatutoryCompliance rdf:type owl:DatatypeProperty ;
                                  rdfs:subPropertyOf :AssuranceProperities ;
                                  rdfs:domain :Assurance ;
                                  rdfs:range xsd:string .


###  http://FYP-ASHS21/csonto/ResourceAllocation
:ResourceAllocation rdf:type owl:DatatypeProperty ;
                    rdfs:subPropertyOf :SecOpsProprities ;
                    rdfs:domain :Security_Operations ;
                    rdfs:range xsd:integer ,
                               xsd:string .


###  http://FYP-ASHS21/csonto/ResourceAllocationForSecProjects
:ResourceAllocationForSecProjects rdf:type owl:DatatypeProperty ;
                                  rdfs:subPropertyOf :GovernanceProperities ;
                                  rdfs:domain :Governance ;
                                  rdfs:range xsd:string .


###  http://FYP-ASHS21/csonto/ResourceUtilizationAndPerformancePlanning
:ResourceUtilizationAndPerformancePlanning rdf:type owl:DatatypeProperty ;
                                           rdfs:subPropertyOf :AssetManagementProperities ;
                                           rdfs:domain :Asset_Management ;
                                           rdfs:range xsd:integer ,
                                                      xsd:string .


###  http://FYP-ASHS21/csonto/SecOpsCentre
:SecOpsCentre rdf:type owl:DatatypeProperty ;
              rdfs:subPropertyOf :SecOpsProprities ;
              rdfs:domain :Security_Operations ;
              rdfs:range rdfs:Literal ,
                         xsd:boolean ,
                         xsd:long ,
                         xsd:string .


###  http://FYP-ASHS21/csonto/SecOpsProprities
:SecOpsProprities rdf:type owl:DatatypeProperty .


###  http://FYP-ASHS21/csonto/SecOpsWeight
:SecOpsWeight rdf:type owl:DatatypeProperty ;
              rdfs:subPropertyOf :SecOpsProprities ,
                                 :TotalScore ;
              rdfs:domain :Security_Operations ,
                          [ rdf:type owl:Restriction ;
                            owl:onProperty :SecOpsProprities ;
                            owl:allValuesFrom xsd:long
                          ] ,
                          [ rdf:type owl:Restriction ;
                            owl:onProperty :SecOpsProprities ;
                            owl:minQualifiedCardinality "4621"^^xsd:nonNegativeInteger ;
                            owl:onDataRange xsd:long
                          ] .


###  http://FYP-ASHS21/csonto/SerivceProtocolSec
:SerivceProtocolSec rdf:type owl:DatatypeProperty ;
                    rdfs:subPropertyOf :EmbeddedTechSecProperities ;
                    rdfs:domain :Embdded_Technologies ;
                    rdfs:range xsd:long ,
                               xsd:string .


###  http://FYP-ASHS21/csonto/ServiceKeyManagement
:ServiceKeyManagement rdf:type owl:DatatypeProperty ;
                      rdfs:subPropertyOf :DataProtectionProperities ;
                      rdfs:domain :Data_Protection ;
                      rdfs:range xsd:token .


###  http://FYP-ASHS21/csonto/StackHardening
:StackHardening rdf:type owl:DatatypeProperty ;
                rdfs:subPropertyOf :EmbeddedTechSecProperities ;
                rdfs:domain :Embdded_Technologies ;
                rdfs:range xsd:string .


###  http://FYP-ASHS21/csonto/StakeholderEngagementInProjects
:StakeholderEngagementInProjects rdf:type owl:DatatypeProperty ;
                                 rdfs:subPropertyOf :GovernanceProperities ;
                                 rdfs:domain :Governance ;
                                 rdfs:range xsd:string .


###  http://FYP-ASHS21/csonto/SuccessCriteria
:SuccessCriteria rdf:type owl:DatatypeProperty ;
                 rdfs:subPropertyOf :GovernanceProperities ;
                 rdfs:domain :Governance ;
                 rdfs:range xsd:string .


###  http://FYP-ASHS21/csonto/ThreatHunting
:ThreatHunting rdf:type owl:DatatypeProperty ;
               rdfs:subPropertyOf :ThreatManagmentProperities ;
               rdfs:domain :Threat_Management ;
               rdfs:range xsd:string .


###  http://FYP-ASHS21/csonto/ThreatManagmentProperities
:ThreatManagmentProperities rdf:type owl:DatatypeProperty ;
                            rdfs:subPropertyOf :SecOpsProprities .


###  http://FYP-ASHS21/csonto/TotalScore
:TotalScore rdf:type owl:DatatypeProperty ,
                     owl:FunctionalProperty ;
            rdfs:domain :CyberSecurityScore ,
                        [ rdf:type owl:Restriction ;
                          owl:onProperty :TotalScore ;
                          owl:allValuesFrom xsd:long
                        ] ,
                        [ rdf:type owl:Restriction ;
                          owl:onProperty :TotalScore ;
                          owl:maxQualifiedCardinality "7424"^^xsd:nonNegativeInteger ;
                          owl:onDataRange xsd:long
                        ] ;
            rdfs:range xsd:long .


###  http://FYP-ASHS21/csonto/TransmissionSec
:TransmissionSec rdf:type owl:DatatypeProperty ;
                 rdfs:subPropertyOf :EmbeddedTechSecProperities ;
                 rdfs:domain :Embdded_Technologies ;
                 rdfs:range xsd:string .


###  http://FYP-ASHS21/csonto/UnifiedSecManagement
:UnifiedSecManagement rdf:type owl:DatatypeProperty ;
                      rdfs:subPropertyOf :SecOpsProprities ;
                      rdfs:domain :Security_Operations ;
                      rdfs:range xsd:string .


###  http://FYP-ASHS21/csonto/VulnerabilitiesManagmenetProperities
:VulnerabilitiesManagmenetProperities rdf:type owl:DatatypeProperty ;
                                      rdfs:subPropertyOf :SecOpsProprities .


###  http://FYP-ASHS21/csonto/VulnerabilityAssessment
:VulnerabilityAssessment rdf:type owl:DatatypeProperty ;
                         rdfs:subPropertyOf :VulnerabilitiesManagmenetProperities ;
                         rdfs:domain :Vulnerability_And_Web_Management ;
                         rdfs:range xsd:string .


###  http://FYP-ASHS21/csonto/VulnerabilityRemediation
:VulnerabilityRemediation rdf:type owl:DatatypeProperty ;
                          rdfs:subPropertyOf :VulnerabilitiesManagmenetProperities ;
                          rdfs:domain :Vulnerability_And_Web_Management ;
                          rdfs:range xsd:string .


###  http://FYP-ASHS21/csonto/ContinuousMonitoring&Analysis
<http://FYP-ASHS21/csonto/ContinuousMonitoring&Analysis> rdf:type owl:DatatypeProperty ;
                                                         rdfs:subPropertyOf :SecOpsProprities ;
                                                         rdfs:domain :Security_Operations ;
                                                         rdfs:range rdfs:Literal ,
                                                                    xsd:boolean ,
                                                                    xsd:string ,
                                                                    xsd:token .


###  http://FYP-ASHS21/csonto/ContinuousMonitoring&Detection
<http://FYP-ASHS21/csonto/ContinuousMonitoring&Detection> rdf:type owl:DatatypeProperty ;
                                                          rdfs:subPropertyOf :ThreatManagmentProperities ;
                                                          rdfs:domain :Threat_Management ;
                                                          rdfs:range xsd:string .


###  http://FYP-ASHS21/csonto/FormalChangeAuthorization&ContractualSecurity
<http://FYP-ASHS21/csonto/FormalChangeAuthorization&ContractualSecurity> rdf:type owl:DatatypeProperty ;
                                                                         rdfs:subPropertyOf :ChangeManagementProperities ;
                                                                         rdfs:domain :Change_Management ;
                                                                         rdfs:range xsd:string .


###  http://FYP-ASHS21/csonto/IncidentResponse&Planning
<http://FYP-ASHS21/csonto/IncidentResponse&Planning> rdf:type owl:DatatypeProperty ;
                                                     rdfs:subPropertyOf :ThreatManagmentProperities ;
                                                     rdfs:domain :Threat_Management ;
                                                     rdfs:range xsd:string .


###  http://FYP-ASHS21/csonto/InfraIDS&IPS
<http://FYP-ASHS21/csonto/InfraIDS&IPS> rdf:type owl:DatatypeProperty ;
                                        rdfs:subPropertyOf :InfraSecProperities ;
                                        rdfs:domain :Infrastructure_And_Identity_And_Access_Management ;
                                        rdfs:range xsd:byte ,
                                                   xsd:dateTimeStamp ,
                                                   xsd:long ,
                                                   xsd:string ,
                                                   xsd:token .


###  http://FYP-ASHS21/csonto/Mitigation&RemediationStrategies
<http://FYP-ASHS21/csonto/Mitigation&RemediationStrategies> rdf:type owl:DatatypeProperty ;
                                                            rdfs:subPropertyOf :ThreatManagmentProperities ;
                                                            rdfs:domain :Threat_Management ;
                                                            rdfs:range xsd:string .


###  http://FYP-ASHS21/csonto/PerformanceMonitoring&Reporting
<http://FYP-ASHS21/csonto/PerformanceMonitoring&Reporting> rdf:type owl:DatatypeProperty ;
                                                           rdfs:subPropertyOf :GovernanceProperities ;
                                                           rdfs:domain :Governance ;
                                                           rdfs:range xsd:string .


###  http://FYP-ASHS21/csonto/Risk&Third-partyAssessment
<http://FYP-ASHS21/csonto/Risk&Third-partyAssessment> rdf:type owl:DatatypeProperty ;
                                                      rdfs:subPropertyOf :ChangeManagementProperities ;
                                                      rdfs:domain :Change_Management ;
                                                      rdfs:range xsd:string .


###  http://FYP-ASHS21/csonto/SecureStorageAndRemoteManagement:
:SecureStorageAndRemoteManagement: rdf:type owl:DatatypeProperty ;
                                   rdfs:subPropertyOf :AssetManagementProperities ;
                                   rdfs:domain :Asset_Management ,
                                               :Infrastructure_And_Identity_And_Access_Management ;
                                   rdfs:range xsd:string ,
                                              xsd:token .


###  http://FYP-ASHS21/csonto/UnauthorizedDisclosure&ModificationPrevention
<http://FYP-ASHS21/csonto/UnauthorizedDisclosure&ModificationPrevention> rdf:type owl:DatatypeProperty ;
                                                                         rdfs:subPropertyOf :DataProtectionProperities ;
                                                                         rdfs:domain :Data_Protection ;
                                                                         rdfs:range xsd:boolean ,
                                                                                    xsd:string .


#################################################################
#    Classes
#################################################################

###  http://FYP-ASHS21/csonto#Asset_Management
:Asset_Management rdf:type owl:Class ;
                  rdfs:subClassOf :CyberSecurityScore ,
                                  [ rdf:type owl:Restriction ;
                                    owl:onProperty <http://purl.obolibrary.org/obo/CSONTO_cf5cef00_b075_4a8d_8d89_8700eb871011> ;
                                    owl:someValuesFrom :Asset_Management_Policies
                                  ] .


###  http://FYP-ASHS21/csonto#Assurance
:Assurance rdf:type owl:Class ;
           rdfs:subClassOf :CyberSecurityScore ,
                           [ rdf:type owl:Restriction ;
                             owl:onProperty <http://purl.obolibrary.org/obo/CSONTO_cf5cef00_b075_4a8d_8d89_8700eb871011> ;
                             owl:someValuesFrom :Assurance_Policies
                           ] .


###  http://FYP-ASHS21/csonto#BusinessContinuity_And_DiasterRecovery
:BusinessContinuity_And_DiasterRecovery rdf:type owl:Class ;
                                        rdfs:subClassOf :Threat_Management .


###  http://FYP-ASHS21/csonto#Capacity_And_Performance_PLanning
:Capacity_And_Performance_PLanning rdf:type owl:Class ;
                                   rdfs:subClassOf :Asset_Management .


###  http://FYP-ASHS21/csonto#Change_Management
:Change_Management rdf:type owl:Class ;
                   rdfs:subClassOf :CyberSecurityScore ,
                                   [ rdf:type owl:Restriction ;
                                     owl:onProperty <http://purl.obolibrary.org/obo/CSONTO_cf5cef00_b075_4a8d_8d89_8700eb871011> ;
                                     owl:someValuesFrom :Change_Management_Policies
                                   ] .


###  http://FYP-ASHS21/csonto#Compliance
:Compliance rdf:type owl:Class ;
            rdfs:subClassOf :Assurance ;
            owl:disjointWith :Security_Awareness_And_Training .


###  http://FYP-ASHS21/csonto#Configuration_Management
:Configuration_Management rdf:type owl:Class ;
                          rdfs:subClassOf :Asset_Management .


###  http://FYP-ASHS21/csonto#Continuous_Monitoring
:Continuous_Monitoring rdf:type owl:Class ;
                       rdfs:subClassOf :Threat_Management .


###  http://FYP-ASHS21/csonto#CyberSecurityScore
:CyberSecurityScore rdf:type owl:Class .


###  http://FYP-ASHS21/csonto#Data_Protection
:Data_Protection rdf:type owl:Class ;
                 rdfs:subClassOf :Security_Operations .


###  http://FYP-ASHS21/csonto#Embdded_Technologies
:Embdded_Technologies rdf:type owl:Class ;
                      rdfs:subClassOf :Security_Operations .


###  http://FYP-ASHS21/csonto#Emerging_Technologies
:Emerging_Technologies rdf:type owl:Class ;
                       rdfs:subClassOf :CyberSecurityScore ,
                                       [ rdf:type owl:Restriction ;
                                         owl:onProperty <http://purl.obolibrary.org/obo/CSONTO_cf5cef00_b075_4a8d_8d89_8700eb871011> ;
                                         owl:someValuesFrom :Emerging_Technologies_Policies
                                       ] .


###  http://FYP-ASHS21/csonto#Governance
:Governance rdf:type owl:Class ;
            rdfs:subClassOf :CyberSecurityScore ,
                            [ rdf:type owl:Restriction ;
                              owl:onProperty :definePolicy ;
                              owl:someValuesFrom :Asset_Management_Policies
                            ] ,
                            [ rdf:type owl:Restriction ;
                              owl:onProperty :definePolicy ;
                              owl:someValuesFrom :Assurance_Policies
                            ] ,
                            [ rdf:type owl:Restriction ;
                              owl:onProperty :definePolicy ;
                              owl:someValuesFrom :Change_Management_Policies
                            ] ,
                            [ rdf:type owl:Restriction ;
                              owl:onProperty :definePolicy ;
                              owl:someValuesFrom :Emerging_Technologies_Policies
                            ] ,
                            [ rdf:type owl:Restriction ;
                              owl:onProperty :definePolicy ;
                              owl:someValuesFrom :Governance_Policies
                            ] ,
                            [ rdf:type owl:Restriction ;
                              owl:onProperty :definePolicy ;
                              owl:someValuesFrom :Security_Operations_Policies
                            ] ,
                            [ rdf:type owl:Restriction ;
                              owl:onProperty <http://purl.obolibrary.org/obo/CSONTO_cf5cef00_b075_4a8d_8d89_8700eb871011> ;
                              owl:someValuesFrom :Governance_Policies
                            ] .


###  http://FYP-ASHS21/csonto#Incident_Response
:Incident_Response rdf:type owl:Class ;
                   rdfs:subClassOf :Threat_Management .


###  http://FYP-ASHS21/csonto#Infrastructure_And_Identity_And_Access_Management
:Infrastructure_And_Identity_And_Access_Management rdf:type owl:Class ;
                                                   rdfs:subClassOf :Security_Operations .


###  http://FYP-ASHS21/csonto#Mobile_Device_Management
:Mobile_Device_Management rdf:type owl:Class ;
                          rdfs:subClassOf :Asset_Management .


###  http://FYP-ASHS21/csonto#Risk_Management
:Risk_Management rdf:type owl:Class ;
                 rdfs:subClassOf :Change_Management .


###  http://FYP-ASHS21/csonto#Secure_Engineering_And_Architecture
:Secure_Engineering_And_Architecture rdf:type owl:Class ;
                                     rdfs:subClassOf :Change_Management .


###  http://FYP-ASHS21/csonto#Security_Awareness_And_Training
:Security_Awareness_And_Training rdf:type owl:Class ;
                                 rdfs:subClassOf :Assurance .


###  http://FYP-ASHS21/csonto#Security_Operations
:Security_Operations rdf:type owl:Class ;
                     rdfs:subClassOf :CyberSecurityScore ,
                                     [ rdf:type owl:Restriction ;
                                       owl:onProperty <http://purl.obolibrary.org/obo/CSONTO_cf5cef00_b075_4a8d_8d89_8700eb871011> ;
                                       owl:someValuesFrom :Security_Operations_Policies
                                     ] .


###  http://FYP-ASHS21/csonto#Threat_Management
:Threat_Management rdf:type owl:Class ;
                   rdfs:subClassOf :Security_Operations .


###  http://FYP-ASHS21/csonto#Vulnerability_And_Web_Management
:Vulnerability_And_Web_Management rdf:type owl:Class ;
                                  rdfs:subClassOf :Security_Operations .


###  http://FYP-ASHS21/csonto/Asset_Management_Policies
:Asset_Management_Policies rdf:type owl:Class ;
                           rdfs:subClassOf :Asset_Management .


###  http://FYP-ASHS21/csonto/Assurance_Policies
:Assurance_Policies rdf:type owl:Class ;
                    rdfs:subClassOf :Assurance .


###  http://FYP-ASHS21/csonto/Change_Management_Policies
:Change_Management_Policies rdf:type owl:Class ;
                            rdfs:subClassOf :Change_Management .


###  http://FYP-ASHS21/csonto/Emerging_Technologies_Policies
:Emerging_Technologies_Policies rdf:type owl:Class ;
                                rdfs:subClassOf :Emerging_Technologies .


###  http://FYP-ASHS21/csonto/Governance_Policies
:Governance_Policies rdf:type owl:Class ;
                     rdfs:subClassOf :Governance .


###  http://FYP-ASHS21/csonto/Security_Operations_Policies
:Security_Operations_Policies rdf:type owl:Class ;
                              rdfs:subClassOf :Security_Operations .


###  http://FYP-ASHS21/csonto/Thrid-Party-Management
:Thrid-Party-Management rdf:type owl:Class ;
                        rdfs:subClassOf :Change_Management .


###  http://FYP-ASHS21/csonto/TechnologyDevelopement&Acquisition
<http://FYP-ASHS21/csonto/TechnologyDevelopement&Acquisition> rdf:type owl:Class ;
                                                              rdfs:subClassOf :Change_Management .


#################################################################
#    Individuals
#################################################################

###  http://FYP-ASHS21/csonto/AAT-10.1-AITEVVTrustworthinessAssessment
:AAT-10.1-AITEVVTrustworthinessAssessment rdf:type owl:NamedIndividual ,
                                                   :Emerging_Technologies_Policies ;
                                          :HasWeight 10 ;
                                          rdfs:comment "Mechanisms exist to evaluate Artificial Intelligence (AI) and Autonomous Technologies (AAT) for trustworthy behavior and operation including security, anonymization and disaggregation of captured and stored data for approved purposes." .


###  http://FYP-ASHS21/csonto/AAT-10.10-AITEVVResultsEvaluation
:AAT-10.10-AITEVVResultsEvaluation rdf:type owl:NamedIndividual ,
                                            :Emerging_Technologies_Policies ;
                                   :HasWeight 10 ;
                                   rdfs:comment "Mechanisms exist to evaluate the results of Artificial Intelligence Test, Evaluation, Validation & Verification (AI TEVV) to determine the viability of the proposed Artificial Intelligence (AI) and Autonomous Technologies (AAT)." .


###  http://FYP-ASHS21/csonto/AAT-10.11-AITEVVEffectiveness
:AAT-10.11-AITEVVEffectiveness rdf:type owl:NamedIndividual ,
                                        :Emerging_Technologies_Policies ;
                               :HasWeight 5 ;
                               rdfs:comment "Mechanisms exist to evaluate the effectiveness of the processes utilized to perform Artificial Intelligence Test, Evaluation, Validation & Verification (AI TEVV)." .


###  http://FYP-ASHS21/csonto/AAT-10.12-AITEVVComparableDeploymentSettings
:AAT-10.12-AITEVVComparableDeploymentSettings rdf:type owl:NamedIndividual ,
                                                       :Emerging_Technologies_Policies ;
                                              :HasWeight 5 ;
                                              rdfs:comment "Mechanisms exist to evaluate Artificial Intelligence (AI) and Autonomous Technologies (AAT)-related performance or the assurance criteria demonstrated for conditions similar to deployment settings." .


###  http://FYP-ASHS21/csonto/AAT-10.13-AITEVVPost-DeploymentMonitoring
:AAT-10.13-AITEVVPost-DeploymentMonitoring rdf:type owl:NamedIndividual ,
                                                    :Emerging_Technologies_Policies ;
                                           :HasWeight 9 ;
                                           rdfs:comment "Mechanisms exist to proactively and continuously monitor deployed Artificial Intelligence (AI) and Autonomous Technologies (AAT)." .


###  http://FYP-ASHS21/csonto/AAT-10.2-AITEVVTools
:AAT-10.2-AITEVVTools rdf:type owl:NamedIndividual ,
                               :Emerging_Technologies_Policies ;
                      :HasWeight 7 ;
                      rdfs:comment "Mechanisms exist to document test sets, metrics and details about the tools used during Artificial Intelligence Test, Evaluation, Validation & Verification (AI TEVV) practices." .


###  http://FYP-ASHS21/csonto/AAT-10.3-AITEVVTrustworthinessDemonstration
:AAT-10.3-AITEVVTrustworthinessDemonstration rdf:type owl:NamedIndividual ,
                                                      :Emerging_Technologies_Policies ;
                                             :HasWeight 9 ;
                                             rdfs:comment "Mechanisms exist to demonstrate the Artificial Intelligence (AI) and Autonomous Technologies (AAT) to be deployed is valid, reliable and operate as intended based on approved designs." .


###  http://FYP-ASHS21/csonto/AAT-10.4-AITEVVSafetyDemonstration
:AAT-10.4-AITEVVSafetyDemonstration rdf:type owl:NamedIndividual ,
                                             :Emerging_Technologies_Policies ;
                                    :HasWeight 10 ;
                                    rdfs:comment "Mechanisms exist to demonstrate the Artificial Intelligence (AI) and Autonomous Technologies (AAT) to be deployed are safe, residual risk does not exceed the organization's risk tolerance and can fail safely, particularly if made to operate beyond its knowledge limits." .


###  http://FYP-ASHS21/csonto/AAT-10.5-AITEVVResiliencyAssessment
:AAT-10.5-AITEVVResiliencyAssessment rdf:type owl:NamedIndividual ,
                                              :Emerging_Technologies_Policies ;
                                     :HasWeight 6 ;
                                     rdfs:comment "Mechanisms exist to evaluate the security and resilience of Artificial Intelligence (AI) and Autonomous Technologies (AAT) to be deployed." .


###  http://FYP-ASHS21/csonto/AAT-10.7-AITEVVPrivacyAssessment
:AAT-10.7-AITEVVPrivacyAssessment rdf:type owl:NamedIndividual ,
                                           :Emerging_Technologies_Policies ;
                                  :HasWeight 9 ;
                                  rdfs:comment "Mechanisms exist to examine the data privacy risk of Artificial Intelligence (AI) and Autonomous Technologies (AAT) to be deployed." .


###  http://FYP-ASHS21/csonto/AAT-CLD-01-CloudServices
:AAT-CLD-01-CloudServices rdf:type owl:NamedIndividual ,
                                   :Emerging_Technologies_Policies ;
                          :HasWeight 10 ;
                          rdfs:comment "Mechanisms exist to facilitate the implementation of cloud management controls to ensure cloud instances are secure and in-line with industry practices. " .


###  http://FYP-ASHS21/csonto/AAT-CLD-01.1-CloudInfrastructureOnboarding
:AAT-CLD-01.1-CloudInfrastructureOnboarding rdf:type owl:NamedIndividual ,
                                                     :Emerging_Technologies_Policies ;
                                            :HasWeight 9 ;
                                            rdfs:comment "Mechanisms exist to ensure cloud services are designed and configured so systems, applications and processes are secured in accordance with applicable organizational standards, as well as statutory, regulatory and contractual obligations." .


###  http://FYP-ASHS21/csonto/AAT-CLD-01.2-CloudInfrastructureOffboarding
:AAT-CLD-01.2-CloudInfrastructureOffboarding rdf:type owl:NamedIndividual ,
                                                      :Emerging_Technologies_Policies ;
                                             :HasWeight 9 ;
                                             rdfs:comment "Mechanisms exist to ensure cloud services are decommissioned so that data is securely transitioned to new systems or archived in accordance with applicable organizational standards, as well as statutory, regulatory and contractual obligations." .


###  http://FYP-ASHS21/csonto/AAT-CLD-02-CloudSecurityArchitecture
:AAT-CLD-02-CloudSecurityArchitecture rdf:type owl:NamedIndividual ,
                                               :Emerging_Technologies_Policies ;
                                      :HasWeight 8 ;
                                      rdfs:comment "Mechanisms exist to ensure the cloud security architecture supports the organization's technology strategy to securely design, configure and maintain cloud employments. " .


###  http://FYP-ASHS21/csonto/AAT-CLD-03-CloudInfrastructureSecuritySubnet
:AAT-CLD-03-CloudInfrastructureSecuritySubnet rdf:type owl:NamedIndividual ,
                                                       :Emerging_Technologies_Policies ;
                                              :HasWeight 6 ;
                                              rdfs:comment "Mechanisms exist to host security-specific technologies in a dedicated subnet." .


###  http://FYP-ASHS21/csonto/AAT-CLD-05-VirtualMachineImages
:AAT-CLD-05-VirtualMachineImages rdf:type owl:NamedIndividual ,
                                          :Emerging_Technologies_Policies ;
                                 :HasWeight 8 ;
                                 rdfs:comment "Mechanisms exist to ensure the integrity of virtual machine images at all times. " .


###  http://FYP-ASHS21/csonto/AAT-CLD-06-Multi-TenantEnvironments
:AAT-CLD-06-Multi-TenantEnvironments rdf:type owl:NamedIndividual ,
                                              :Emerging_Technologies_Policies ;
                                     :HasWeight 9 ;
                                     rdfs:comment "Mechanisms exist to ensure multi-tenant owned or managed assets (physical and virtual) are designed and governed such that provider and customer (tenant) user access is appropriately segmented from other tenant users." .


###  http://FYP-ASHS21/csonto/AAT-CLD-06.1-CustomerResponsibilityMatrix-CRM-
:AAT-CLD-06.1-CustomerResponsibilityMatrix-CRM- rdf:type owl:NamedIndividual ,
                                                         :Emerging_Technologies_Policies ;
                                                :HasWeight 8 ;
                                                rdfs:comment "Mechanisms exist to formally document a Customer Responsibility Matrix (CRM), delineating assigned responsibilities for controls between the Cloud Service Provider (CSP) and its customers." .


###  http://FYP-ASHS21/csonto/AAT-CLD-06.2-Multi-TenantEventLoggingCapabilities
:AAT-CLD-06.2-Multi-TenantEventLoggingCapabilities rdf:type owl:NamedIndividual ,
                                                            :Emerging_Technologies_Policies ;
                                                   :HasWeight 8 ;
                                                   rdfs:comment "Mechanisms exist to ensure Multi-Tenant Service Providers (MTSP) facilitate security event logging capabilities for its customers that are consistent with applicable statutory, regulatory and/or contractual obligations." .


###  http://FYP-ASHS21/csonto/AAT-CLD-06.3-Multi-TenantForensicsCapabilities
:AAT-CLD-06.3-Multi-TenantForensicsCapabilities rdf:type owl:NamedIndividual ,
                                                         :Emerging_Technologies_Policies ;
                                                :HasWeight 8 ;
                                                rdfs:comment "Mechanisms exist to ensure Multi-Tenant Service Providers (MTSP) facilitate prompt forensic investigations in the event of a suspected or confirmed security incident." .


###  http://FYP-ASHS21/csonto/AAT-CLD-06.4-Multi-TenantIncidentResponseCapabilities
:AAT-CLD-06.4-Multi-TenantIncidentResponseCapabilities rdf:type owl:NamedIndividual ,
                                                                :Emerging_Technologies_Policies ;
                                                       :HasWeight 8 ;
                                                       rdfs:comment "Mechanisms exist to ensure Multi-Tenant Service Providers (MTSP) facilitate prompt response to suspected or confirmed security incidents and vulnerabilities, including timely notification to affected customers." .


###  http://FYP-ASHS21/csonto/AAT-CLD-08-StandardizedVirtualizationFormats
:AAT-CLD-08-StandardizedVirtualizationFormats rdf:type owl:NamedIndividual ,
                                                       :Emerging_Technologies_Policies ;
                                              :HasWeight 4 ;
                                              rdfs:comment "Mechanisms exist to ensure interoperability by requiring cloud providers to use industry-recognized formats and provide documentation of custom changes for review." .


###  http://FYP-ASHS21/csonto/AAT-CLD-09-GeolocationRequirementsforProcessing-StorageandServiceLocations
:AAT-CLD-09-GeolocationRequirementsforProcessing-StorageandServiceLocations rdf:type owl:NamedIndividual ,
                                                                                     :Emerging_Technologies_Policies ;
                                                                            :HasWeight 10 ;
                                                                            rdfs:comment "Mechanisms exist to control the location of cloud processing/storage based on business requirements that includes statutory, regulatory and contractual obligations. " .


###  http://FYP-ASHS21/csonto/AAT-CLD-10-SensitiveDataInPublicCloudProviders
:AAT-CLD-10-SensitiveDataInPublicCloudProviders rdf:type owl:NamedIndividual ,
                                                         :Emerging_Technologies_Policies ;
                                                :HasWeight 6 ;
                                                rdfs:comment "Mechanisms exist to limit and manage the storage of sensitive/regulated data in public cloud providers. " .


###  http://FYP-ASHS21/csonto/AAT-CLD-11-CloudAccessPoint-CAP-
:AAT-CLD-11-CloudAccessPoint-CAP- rdf:type owl:NamedIndividual ,
                                           :Emerging_Technologies_Policies ;
                                  :HasWeight 7 ;
                                  rdfs:comment "Mechanisms exist to utilize Cloud Access Points (CAPs) to provide boundary protection and monitoring functions that both provide access to the cloud and protect the organization from the cloud." .


###  http://FYP-ASHS21/csonto/AAT-CLD-12-SideChannelAttackPrevention
:AAT-CLD-12-SideChannelAttackPrevention rdf:type owl:NamedIndividual ,
                                                 :Emerging_Technologies_Policies ;
                                        :HasWeight 3 ;
                                        rdfs:comment "Mechanisms exist to prevent \"side channel attacks\" when using a Content Delivery Network (CDN) by restricting access to the origin server's IP address to the CDN and an authorized management network." .


###  http://FYP-ASHS21/csonto/AST-01-AssetGovernance
:AST-01-AssetGovernance rdf:type owl:NamedIndividual ,
                                 :Asset_Management_Policies ;
                        :HasWeight 10 ;
                        rdfs:comment "Mechanisms exist to facilitate an IT Asset Management (ITAM) program to implement and manage asset management controls." .


###  http://FYP-ASHS21/csonto/AST-01.1-Asset-ServiceDependencies
:AST-01.1-Asset-ServiceDependencies rdf:type owl:NamedIndividual ,
                                             :Asset_Management_Policies ;
                                    :HasWeight 5 ;
                                    rdfs:comment "Mechanisms exist to identify and assess the security of technology assets that support more than one critical business function. " .


###  http://FYP-ASHS21/csonto/AST-01.3-StandardizedNamingConvention
:AST-01.3-StandardizedNamingConvention rdf:type owl:NamedIndividual ,
                                                :Asset_Management_Policies ;
                                       :HasWeight 5 ;
                                       rdfs:comment "Mechanisms exist to implement a scalable, standardized naming convention for systems, applications and services that avoids asset naming conflicts." .


###  http://FYP-ASHS21/csonto/AST-02-AssetInventories
:AST-02-AssetInventories rdf:type owl:NamedIndividual ,
                                  :Asset_Management_Policies ;
                         :HasWeight 10 ;
                         rdfs:comment """Mechanisms exist to perform inventories of technology assets that:
  Accurately reflects the current systems, applications and services in use; 
  Identifies authorized software products, including business justification details;
  Is at the level of granularity deemed necessary for tracking and reporting;
  Includes organization-defined information deemed necessary to achieve effective property accountability; and
  Is available for review and audit by designated organizational personnel.""" .


###  http://FYP-ASHS21/csonto/AST-02.1-UpdatesDuringInstallations-Removals
:AST-02.1-UpdatesDuringInstallations-Removals rdf:type owl:NamedIndividual ,
                                                       :Asset_Management_Policies ;
                                              :HasWeight 7 ;
                                              rdfs:comment "Mechanisms exist to update asset inventories as part of component installations, removals and asset upgrades. " .


###  http://FYP-ASHS21/csonto/AST-02.10-AutomatedLocationTracking
:AST-02.10-AutomatedLocationTracking rdf:type owl:NamedIndividual ,
                                              :Asset_Management_Policies ;
                                     :HasWeight 5 ;
                                     rdfs:comment "Mechanisms exist to track the geographic location of system components." .


###  http://FYP-ASHS21/csonto/AST-02.11-ComponentAssignment
:AST-02.11-ComponentAssignment rdf:type owl:NamedIndividual ,
                                        :Asset_Management_Policies ;
                               :HasWeight 3 ;
                               rdfs:comment "Mechanisms exist to bind components to a specific system." .


###  http://FYP-ASHS21/csonto/AST-02.2-AutomatedUnauthorizedComponentDetection
:AST-02.2-AutomatedUnauthorizedComponentDetection rdf:type owl:NamedIndividual ,
                                                           :Asset_Management_Policies ;
                                                  :HasWeight 3 ;
                                                  rdfs:comment "Automated mechanisms exist to detect and alert upon the detection of unauthorized hardware, software and firmware components." .


###  http://FYP-ASHS21/csonto/AST-02.3-ComponentDuplicationAvoidance
:AST-02.3-ComponentDuplicationAvoidance rdf:type owl:NamedIndividual ,
                                                 :Asset_Management_Policies ;
                                        :HasWeight 2 ;
                                        rdfs:comment "Mechanisms exist to establish and maintain an authoritative source and repository to provide a trusted source and accountability for approved and implemented system components that prevents assets from being duplicated in other asset inventories." .


###  http://FYP-ASHS21/csonto/AST-02.4-ApprovedBaselineDeviations
:AST-02.4-ApprovedBaselineDeviations rdf:type owl:NamedIndividual ,
                                              :Asset_Management_Policies ;
                                     :HasWeight 8 ;
                                     rdfs:comment "Mechanisms exist to document and govern instances of approved deviations from established baseline configurations. " .


###  http://FYP-ASHS21/csonto/AST-02.5-NetworkAccessControl-NAC-
:AST-02.5-NetworkAccessControl-NAC- rdf:type owl:NamedIndividual ,
                                             :Asset_Management_Policies ;
                                    :HasWeight 4 ;
                                    rdfs:comment "Automated mechanisms exist to employ Network Access Control (NAC), or a similar technology, that is capable of detecting unauthorized devices and disable network access to those unauthorized devices." .


###  http://FYP-ASHS21/csonto/AST-02.6-DynamicHostConfigurationProtocol-DHCP-ServerLogging
:AST-02.6-DynamicHostConfigurationProtocol-DHCP-ServerLogging rdf:type owl:NamedIndividual ,
                                                                       :Asset_Management_Policies ;
                                                              :HasWeight 3 ;
                                                              rdfs:comment "Mechanisms exist to enable Dynamic Host Configuration Protocol (DHCP) server logging to improve asset inventories and assist in detecting unknown systems. " .


###  http://FYP-ASHS21/csonto/AST-02.7-SoftwareLicensingRestrictions
:AST-02.7-SoftwareLicensingRestrictions rdf:type owl:NamedIndividual ,
                                                 :Asset_Management_Policies ;
                                        :HasWeight 8 ;
                                        rdfs:comment """Mechanisms exist to protect Intellectual Property (IP) rights with software licensing restrictions.
""" .


###  http://FYP-ASHS21/csonto/AST-02.8-DataActionMapping
:AST-02.8-DataActionMapping rdf:type owl:NamedIndividual ,
                                     :Asset_Management_Policies ;
                            :HasWeight 9 ;
                            rdfs:comment "Mechanisms exist to create and maintain a map of technology assets where sensitive/regulated data is stored, transmitted or processed." .


###  http://FYP-ASHS21/csonto/AST-02.9-ConfigurationManagementDatabase-CMDB-
:AST-02.9-ConfigurationManagementDatabase-CMDB- rdf:type owl:NamedIndividual ,
                                                         :Asset_Management_Policies ;
                                                :HasWeight 5 ;
                                                rdfs:comment "Mechanisms exist to implement and manage a Configuration Management Database (CMDB), or similar technology, to monitor and govern technology asset-specific information." .


###  http://FYP-ASHS21/csonto/AST-03-AssetOwnershipAssignment
:AST-03-AssetOwnershipAssignment rdf:type owl:NamedIndividual ,
                                          :Asset_Management_Policies ;
                                 :HasWeight 8 ;
                                 rdfs:comment "Mechanisms exist to ensure asset ownership responsibilities are assigned, tracked and managed at a team, individual, or responsible organization level to establish a common understanding of requirements for asset protection." .


###  http://FYP-ASHS21/csonto/AST-03.1-AccountabilityInformation
:AST-03.1-AccountabilityInformation rdf:type owl:NamedIndividual ,
                                             :Asset_Management_Policies ;
                                    :HasWeight 5 ;
                                    rdfs:comment "Mechanisms exist to include capturing the name, position and/or role of individuals responsible/accountable for administering assets as part of the technology asset inventory process." .


###  http://FYP-ASHS21/csonto/AST-03.2-Provenance
:AST-03.2-Provenance rdf:type owl:NamedIndividual ,
                              :Asset_Management_Policies ;
                     :HasWeight 8 ;
                     rdfs:comment "Mechanisms exist to track the origin, development, ownership, location and changes to systems, system components and associated data." .


###  http://FYP-ASHS21/csonto/AST-04.1-AssetScopeClassification
:AST-04.1-AssetScopeClassification rdf:type owl:NamedIndividual ,
                                            :Asset_Management_Policies ;
                                   :HasWeight 8 ;
                                   rdfs:comment "Mechanisms exist to determine cybersecurity & data privacy control applicability by identifying, assigning and documenting the appropriate asset scope categorization for all systems, applications, services and personnel (internal and third-parties)." .


###  http://FYP-ASHS21/csonto/AST-04.2-ControlApplicabilityBoundaryGraphicalRepresentation
:AST-04.2-ControlApplicabilityBoundaryGraphicalRepresentation rdf:type owl:NamedIndividual ,
                                                                       :Asset_Management_Policies ;
                                                              :HasWeight 6 ;
                                                              rdfs:comment "Mechanisms exist to ensure control applicability is appropriately-determined for systems, applications, services and third parties by graphically representing applicable boundaries." .


###  http://FYP-ASHS21/csonto/AST-04.3-Compliance-SpecificAssetIdentification
:AST-04.3-Compliance-SpecificAssetIdentification rdf:type owl:NamedIndividual ,
                                                          :Asset_Management_Policies ;
                                                 :HasWeight 6 ;
                                                 rdfs:comment "Mechanisms exist to create and maintain a current inventory of systems, applications and services that are in scope for statutory, regulatory and/or contractual compliance obligations that provides sufficient detail to determine control applicability, based on asset scope categorization." .


###  http://FYP-ASHS21/csonto/AST-05.1-ManagementApprovalForExternalMediaTransfer
:AST-05.1-ManagementApprovalForExternalMediaTransfer rdf:type owl:NamedIndividual ,
                                                              :Asset_Management_Policies ;
                                                     :HasWeight 8 ;
                                                     rdfs:comment "Mechanisms exist to obtain management approval for any sensitive / regulated media that is transferred outside of the organization's facilities." .


###  http://FYP-ASHS21/csonto/AST-06-UnattendedEnd-UserEquipment
:AST-06-UnattendedEnd-UserEquipment rdf:type owl:NamedIndividual ,
                                             :Asset_Management_Policies ;
                                    :HasWeight 9 ;
                                    rdfs:comment "Mechanisms exist to implement enhanced protection measures for unattended systems to protect against tampering and unauthorized access." .


###  http://FYP-ASHS21/csonto/AST-06.1-AssetStorageInAutomobiles
:AST-06.1-AssetStorageInAutomobiles rdf:type owl:NamedIndividual ,
                                             :Asset_Management_Policies ;
                                    :HasWeight 7 ;
                                    rdfs:comment "Mechanisms exist to educate users on the need to physically secure laptops and other mobile devices out of site when traveling, preferably in the trunk of a vehicle." .


###  http://FYP-ASHS21/csonto/AST-08-TamperDetection
:AST-08-TamperDetection rdf:type owl:NamedIndividual ,
                                 :Asset_Management_Policies ;
                        :HasWeight 9 ;
                        rdfs:comment "Mechanisms exist to periodically inspect systems and system components for Indicators of Compromise (IoC)." .


###  http://FYP-ASHS21/csonto/AST-09-SecureDisposal-DestructionorRe-UseofEquipment
:AST-09-SecureDisposal-DestructionorRe-UseofEquipment rdf:type owl:NamedIndividual ,
                                                               :Asset_Management_Policies ;
                                                      :HasWeight 10 ;
                                                      rdfs:comment "Mechanisms exist to securely dispose of, destroy or repurpose system components using organization-defined techniques and methods to prevent information being recovered from these components." .


###  http://FYP-ASHS21/csonto/AST-10-ReturnofAssets
:AST-10-ReturnofAssets rdf:type owl:NamedIndividual ,
                                :Asset_Management_Policies ;
                       :HasWeight 8 ;
                       rdfs:comment "Mechanisms exist to ensure that employees and third-party users return all organizational assets in their possession upon termination of employment, contract or agreement." .


###  http://FYP-ASHS21/csonto/AST-11-RemovalofAssets
:AST-11-RemovalofAssets rdf:type owl:NamedIndividual ,
                                 :Asset_Management_Policies ;
                        :HasWeight 8 ;
                        rdfs:comment "Mechanisms exist to authorize, control and track technology assets entering and exiting organizational facilities. " .


###  http://FYP-ASHS21/csonto/AST-12-UseofPersonalDevices
:AST-12-UseofPersonalDevices rdf:type owl:NamedIndividual ,
                                      :Asset_Management_Policies ;
                             :HasWeight 10 ;
                             rdfs:comment "Mechanisms exist to restrict the possession and usage of personally-owned technology devices within organization-controlled facilities." .


###  http://FYP-ASHS21/csonto/AST-13-UseofThird-PartyDevices
:AST-13-UseofThird-PartyDevices rdf:type owl:NamedIndividual ,
                                         :Asset_Management_Policies ;
                                :HasWeight 9 ;
                                rdfs:comment "Mechanisms exist to reduce the risk associated with third-party assets that are attached to the network from harming organizational assets or exfiltrating organizational data." .


###  http://FYP-ASHS21/csonto/AST-14-UsageParameters
:AST-14-UsageParameters rdf:type owl:NamedIndividual ,
                                 :Asset_Management_Policies ;
                        :HasWeight 7 ;
                        rdfs:comment """Mechanisms exist to monitor and enforce usage parameters that limit the potential damage caused from the unauthorized or unintentional alteration of system parameters. 
""" .


###  http://FYP-ASHS21/csonto/AST-14.2-InfraredCommunications
:AST-14.2-InfraredCommunications rdf:type owl:NamedIndividual ,
                                          :Asset_Management_Policies ;
                                 :HasWeight 5 ;
                                 rdfs:comment "Mechanisms exist to prevent line of sight and reflected infrared (IR) communications use in an unsecured space." .


###  http://FYP-ASHS21/csonto/AST-15-TamperProtection
:AST-15-TamperProtection rdf:type owl:NamedIndividual ,
                                  :Asset_Management_Policies ;
                         :HasWeight 6 ;
                         rdfs:comment "Mechanisms exist to verify logical configuration settings and the physical integrity of critical technology assets throughout their lifecycle." .


###  http://FYP-ASHS21/csonto/AST-16-BringYourOwnDevice-BYOD-Usage
:AST-16-BringYourOwnDevice-BYOD-Usage rdf:type owl:NamedIndividual ,
                                               :Asset_Management_Policies ;
                                      :HasWeight 10 ;
                                      rdfs:comment "Mechanisms exist to implement and govern a Bring Your Own Device (BYOD) program to reduce risk associated with personally-owned devices in the workplace." .


###  http://FYP-ASHS21/csonto/AST-18-RootsofTrustProtection
:AST-18-RootsofTrustProtection rdf:type owl:NamedIndividual ,
                                        :Asset_Management_Policies ;
                               :HasWeight 4 ;
                               rdfs:comment "Mechanisms exist to provision and protect the confidentiality, integrity and authenticity of product supplier keys and data that can be used as a roots of trust basis for integrity verification." .


###  http://FYP-ASHS21/csonto/AST-19-TelecommunicationsEquipment
:AST-19-TelecommunicationsEquipment rdf:type owl:NamedIndividual ,
                                             :Asset_Management_Policies ;
                                    :HasWeight 9 ;
                                    rdfs:comment "Mechanisms exist to establish usage restrictions and implementation guidance for telecommunication equipment to prevent potential damage or unauthorized modification and to prevent potential eavesdropping." .


###  http://FYP-ASHS21/csonto/AST-20-VideoTeleconference-VTC-Security
:AST-20-VideoTeleconference-VTC-Security rdf:type owl:NamedIndividual ,
                                                  :Asset_Management_Policies ;
                                         :HasWeight 8 ;
                                         rdfs:comment "Mechanisms exist to implement secure Video Teleconference (VTC) capabilities on endpoint devices and in designated conference rooms, to prevent potential eavesdropping." .


###  http://FYP-ASHS21/csonto/AST-21-VoiceOverInternetProtocol-VoIP-Security
:AST-21-VoiceOverInternetProtocol-VoIP-Security rdf:type owl:NamedIndividual ,
                                                         :Asset_Management_Policies ;
                                                :HasWeight 8 ;
                                                rdfs:comment "Mechanisms exist to implement secure Internet Protocol Telephony (IPT) that logically or physically separates Voice Over Internet Protocol (VoIP) traffic from data networks." .


###  http://FYP-ASHS21/csonto/AST-23-Multi-FunctionDevices-MFD-
:AST-23-Multi-FunctionDevices-MFD- rdf:type owl:NamedIndividual ,
                                            :Asset_Management_Policies ;
                                   :HasWeight 8 ;
                                   rdfs:comment "Mechanisms exist to securely configure Multi-Function Devices (MFD) according to industry-recognized secure practices for the type of device." .


###  http://FYP-ASHS21/csonto/AST-24-Travel-OnlyDevices
:AST-24-Travel-OnlyDevices rdf:type owl:NamedIndividual ,
                                    :Asset_Management_Policies ;
                           :HasWeight 8 ;
                           rdfs:comment "Mechanisms exist to issue personnel travelling overseas with temporary, loaner or \"travel-only\" end user technology (e.g., laptops and mobile devices) when travelling to authoritarian countries with a higher-than average risk for Intellectual Property (IP) theft or espionage against individuals and private companies." .


###  http://FYP-ASHS21/csonto/AST-25-Re-ImagingDevicesAfterTravel
:AST-25-Re-ImagingDevicesAfterTravel rdf:type owl:NamedIndividual ,
                                              :Asset_Management_Policies ;
                                     :HasWeight 8 ;
                                     rdfs:comment "Mechanisms exist to re-image end user technology (e.g., laptops and mobile devices) when returning from overseas travel to an authoritarian country with a higher-than average risk for Intellectual Property (IP) theft or espionage against individuals and private companies." .


###  http://FYP-ASHS21/csonto/AST-26-SystemAdministrativeProcesses
:AST-26-SystemAdministrativeProcesses rdf:type owl:NamedIndividual ,
                                               :Asset_Management_Policies ;
                                      :HasWeight 9 ;
                                      rdfs:comment "Mechanisms exist to develop, implement and govern system administration processes, with corresponding Standardized Operating Procedures (SOP), for operating and maintaining systems, applications and services." .


###  http://FYP-ASHS21/csonto/AST-27-JumpServer
:AST-27-JumpServer rdf:type owl:NamedIndividual ,
                            :Asset_Management_Policies ;
                   :HasWeight 7 ;
                   rdfs:comment "Mechanisms exist to conduct remote system administrative functions via a \"jump box\" or \"jump server\" that is located in a separate network zone to user workstations." .


###  http://FYP-ASHS21/csonto/AST-28-DatabaseAdministrativeProcesses
:AST-28-DatabaseAdministrativeProcesses rdf:type owl:NamedIndividual ,
                                                 :Asset_Management_Policies ;
                                        :HasWeight 9 ;
                                        rdfs:comment "Mechanisms exist to develop, implement and govern database management processes, with corresponding Standardized Operating Procedures (SOP), for operating and maintaining databases." .


###  http://FYP-ASHS21/csonto/AST-28.1-DatabaseManagementSystem-DBMS-
:AST-28.1-DatabaseManagementSystem-DBMS- rdf:type owl:NamedIndividual ,
                                                  :Asset_Management_Policies ;
                                         :HasWeight 6 ;
                                         rdfs:comment "Mechanisms exist to implement and maintain Database Management Systems (DBMSs), where applicable." .


###  http://FYP-ASHS21/csonto/AST-29-RadioFrequencyIdentification-RFID-Security
:AST-29-RadioFrequencyIdentification-RFID-Security rdf:type owl:NamedIndividual ,
                                                            :Asset_Management_Policies ;
                                                   :HasWeight 3 ;
                                                   rdfs:comment "Mechanisms exist to securely govern Radio Frequency Identification (RFID) deployments to ensure RFID is used safely and securely to protect the confidentiality and integrity of data and prevent the compromise of secure spaces." .


###  http://FYP-ASHS21/csonto/AST-29.1-ContactlessAccessControlSystems
:AST-29.1-ContactlessAccessControlSystems rdf:type owl:NamedIndividual ,
                                                   :Asset_Management_Policies ;
                                          :HasWeight 3 ;
                                          rdfs:comment "Mechanisms exist to securely configure contactless access control systems incorporating contactless RFID or smart cards to protect the confidentiality and integrity of data and prevent the compromise of secure spaces." .


###  http://FYP-ASHS21/csonto/AST-30-Decommissioning
:AST-30-Decommissioning rdf:type owl:NamedIndividual ,
                                 :Asset_Management_Policies ;
                        :HasWeight 4 ;
                        rdfs:comment "Mechanisms exist to ensure systems, applications and services are properly decommissioned so that data is properly transitioned to new systems or archived in accordance with applicable organizational standards, as well as statutory, regulatory and contractual obligations." .


###  http://FYP-ASHS21/csonto/AST-31-AssetCategorization
:AST-31-AssetCategorization rdf:type owl:NamedIndividual ,
                                     :Asset_Management_Policies ;
                            :HasWeight 9 ;
                            rdfs:comment "Mechanisms exist to categorize technology assets." .


###  http://FYP-ASHS21/csonto/AST-31.1-CategorizeArtificialIntelligence-AI--RelatedTechnologies
:AST-31.1-CategorizeArtificialIntelligence-AI--RelatedTechnologies rdf:type owl:NamedIndividual ,
                                                                            :Asset_Management_Policies ;
                                                                   :HasWeight 9 ;
                                                                   rdfs:comment "Mechanisms exist to categorize Artificial Intelligence (AI) and Autonomous Technologies (AAT)." .


###  http://FYP-ASHS21/csonto/AST-CAP-02-ResourcePriority
:AST-CAP-02-ResourcePriority rdf:type owl:NamedIndividual ,
                                      :Asset_Management_Policies ;
                             :HasWeight 8 ;
                             rdfs:comment "Mechanisms exist to control resource utilization of systems that are susceptible to Denial of Service (DoS) attacks to limit and prioritize the use of resources." .


###  http://FYP-ASHS21/csonto/AST-CAP-03-CapacityPlanning
:AST-CAP-03-CapacityPlanning rdf:type owl:NamedIndividual ,
                                      :Asset_Management_Policies ;
                             :HasWeight 8 ;
                             rdfs:comment "Mechanisms exist to conduct capacity planning so that necessary capacity for information processing, telecommunications and environmental support will exist during contingency operations. " .


###  http://FYP-ASHS21/csonto/AST-CAP-04-PerformanceMonitoring
:AST-CAP-04-PerformanceMonitoring rdf:type owl:NamedIndividual ,
                                           :Asset_Management_Policies ;
                                  :HasWeight 7 ;
                                  rdfs:comment "Automated mechanisms exist to centrally-monitor and alert on the operating state and health status of critical systems, applications and services." .


###  http://FYP-ASHS21/csonto/AST-CFG-01-ConfigurationManagementProgram
:AST-CFG-01-ConfigurationManagementProgram rdf:type owl:NamedIndividual ,
                                                    :Asset_Management_Policies ;
                                           :HasWeight 9 ;
                                           rdfs:comment "Mechanisms exist to facilitate the implementation of configuration management controls." .


###  http://FYP-ASHS21/csonto/AST-CFG-01.1-AssignmentofResponsibility
:AST-CFG-01.1-AssignmentofResponsibility rdf:type owl:NamedIndividual ,
                                                  :Asset_Management_Policies ;
                                         :HasWeight 5 ;
                                         rdfs:comment "Mechanisms exist to implement a segregation of duties for configuration management that prevents developers from performing production configuration management duties." .


###  http://FYP-ASHS21/csonto/AST-CFG-02-SystemHardeningThroughBaselineConfigurations
:AST-CFG-02-SystemHardeningThroughBaselineConfigurations rdf:type owl:NamedIndividual ,
                                                                  :Asset_Management_Policies ;
                                                         :HasWeight 10 ;
                                                         rdfs:comment "Mechanisms exist to develop, document and maintain secure baseline configurations for technology platforms that are consistent with industry-accepted system hardening standards. " .


###  http://FYP-ASHS21/csonto/AST-CFG-02.3-RetentionOfPreviousConfigurations
:AST-CFG-02.3-RetentionOfPreviousConfigurations rdf:type owl:NamedIndividual ,
                                                         :Asset_Management_Policies ;
                                                :HasWeight 3 ;
                                                rdfs:comment "Mechanisms exist to retain previous versions of baseline configuration to support roll back. " .


###  http://FYP-ASHS21/csonto/AST-CFG-02.5-ConfigureSystems-ComponentsorServicesforHigh-RiskAreas
:AST-CFG-02.5-ConfigureSystems-ComponentsorServicesforHigh-RiskAreas rdf:type owl:NamedIndividual ,
                                                                              :Asset_Management_Policies ;
                                                                     :HasWeight 8 ;
                                                                     rdfs:comment "Mechanisms exist to configure systems utilized in high-risk areas with more restrictive baseline configurations." .


###  http://FYP-ASHS21/csonto/AST-CFG-02.6-NetworkDeviceConfigurationFileSynchronization
:AST-CFG-02.6-NetworkDeviceConfigurationFileSynchronization rdf:type owl:NamedIndividual ,
                                                                     :Asset_Management_Policies ;
                                                            :HasWeight 7 ;
                                                            rdfs:comment "Mechanisms exist to configure network devices to synchronize startup and running configuration files. " .


###  http://FYP-ASHS21/csonto/AST-CFG-02.7-ApprovedConfigurationDeviations
:AST-CFG-02.7-ApprovedConfigurationDeviations rdf:type owl:NamedIndividual ,
                                                       :Asset_Management_Policies ;
                                              :HasWeight 9 ;
                                              rdfs:comment "Mechanisms exist to document, assess risk and approve or deny deviations to standardized configurations." .


###  http://FYP-ASHS21/csonto/AST-CFG-02.8-RespondToUnauthorizedChanges
:AST-CFG-02.8-RespondToUnauthorizedChanges rdf:type owl:NamedIndividual ,
                                                    :Asset_Management_Policies ;
                                           :HasWeight 9 ;
                                           rdfs:comment "Mechanisms exist to respond to unauthorized changes to configuration settings as security incidents. " .


###  http://FYP-ASHS21/csonto/AST-CFG-02.9-BaselineTailoring
:AST-CFG-02.9-BaselineTailoring rdf:type owl:NamedIndividual ,
                                         :Asset_Management_Policies ;
                                :HasWeight 9 ;
                                rdfs:comment """Mechanisms exist to allow baseline controls to be specialized or customized by applying a defined set of tailoring actions that are specific to:
  Mission / business functions;
  Operational environment;
  Specific threats or vulnerabilities; or
  Other conditions or situations that could affect mission / business success.""" .


###  http://FYP-ASHS21/csonto/AST-CFG-03-LeastFunctionality
:AST-CFG-03-LeastFunctionality rdf:type owl:NamedIndividual ,
                                        :Asset_Management_Policies ;
                               :HasWeight 10 ;
                               rdfs:comment "Mechanisms exist to configure systems to provide only essential capabilities by specifically prohibiting or restricting the use of ports, protocols, and/or services. " .


###  http://FYP-ASHS21/csonto/AST-CFG-03.1-PeriodicReview
:AST-CFG-03.1-PeriodicReview rdf:type owl:NamedIndividual ,
                                      :Asset_Management_Policies ;
                             :HasWeight 8 ;
                             rdfs:comment "Mechanisms exist to periodically review system configurations to identify and disable unnecessary and/or non-secure functions, ports, protocols and services." .


###  http://FYP-ASHS21/csonto/AST-CFG-03.2-PreventUnauthorizedSoftwareExecution
:AST-CFG-03.2-PreventUnauthorizedSoftwareExecution rdf:type owl:NamedIndividual ,
                                                            :Asset_Management_Policies ;
                                                   :HasWeight 7 ;
                                                   rdfs:comment "Mechanisms exist to configure systems to prevent the execution of unauthorized software programs. " .


###  http://FYP-ASHS21/csonto/AST-CFG-03.3-UnauthorizedorAuthorizedSoftware-BlacklistingorWhitelisting-
:AST-CFG-03.3-UnauthorizedorAuthorizedSoftware-BlacklistingorWhitelisting- rdf:type owl:NamedIndividual ,
                                                                                    :Asset_Management_Policies ;
                                                                           :HasWeight 5 ;
                                                                           rdfs:comment "Mechanisms exist to whitelist or blacklist applications in an order to limit what is authorized to execute on systems." .


###  http://FYP-ASHS21/csonto/AST-CFG-03.4-SplitTunneling
:AST-CFG-03.4-SplitTunneling rdf:type owl:NamedIndividual ,
                                      :Asset_Management_Policies ;
                             :HasWeight 8 ;
                             rdfs:comment "Mechanisms exist to prevent systems from creating split tunneling connections or similar techniques that could be used to exfiltrate data." .


###  http://FYP-ASHS21/csonto/AST-CFG-04-SoftwareUsageRestrictions
:AST-CFG-04-SoftwareUsageRestrictions rdf:type owl:NamedIndividual ,
                                               :Asset_Management_Policies ;
                                      :HasWeight 9 ;
                                      rdfs:comment "Mechanisms exist to enforce software usage restrictions to comply with applicable contract agreements and copyright laws." .


###  http://FYP-ASHS21/csonto/AST-CFG-04.1-OpenSourceSoftware
:AST-CFG-04.1-OpenSourceSoftware rdf:type owl:NamedIndividual ,
                                          :Asset_Management_Policies ;
                                 :HasWeight 9 ;
                                 rdfs:comment "Mechanisms exist to establish parameters for the secure use of open source software. " .


###  http://FYP-ASHS21/csonto/AST-CFG-05-User-InstalledSoftware
:AST-CFG-05-User-InstalledSoftware rdf:type owl:NamedIndividual ,
                                            :Asset_Management_Policies ;
                                   :HasWeight 10 ;
                                   rdfs:comment "Mechanisms exist to restrict the ability of non-privileged users to install unauthorized software." .


###  http://FYP-ASHS21/csonto/AST-CFG-05.1-UnauthorizedInstallationAlerts
:AST-CFG-05.1-UnauthorizedInstallationAlerts rdf:type owl:NamedIndividual ,
                                                      :Asset_Management_Policies ;
                                             :HasWeight 8 ;
                                             rdfs:comment "Mechanisms exist to configure systems to generate an alert when the unauthorized installation of software is detected. " .


###  http://FYP-ASHS21/csonto/AST-CFG-05.2-RestrictRolesPermittedToInstallSoftware
:AST-CFG-05.2-RestrictRolesPermittedToInstallSoftware rdf:type owl:NamedIndividual ,
                                                               :Asset_Management_Policies ;
                                                      :HasWeight 9 ;
                                                      rdfs:comment "Mechanisms exist to configure systems to prevent the installation of software, unless the action is performed by a privileged user or service." .


###  http://FYP-ASHS21/csonto/AST-CFG-06-ConfigurationEnforcement
:AST-CFG-06-ConfigurationEnforcement rdf:type owl:NamedIndividual ,
                                              :Asset_Management_Policies ;
                                     :HasWeight 7 ;
                                     rdfs:comment "Automated mechanisms exist to monitor, enforce and report on configurations for endpoint devices." .


###  http://FYP-ASHS21/csonto/AST-CFG-07-Zero-TouchProvisioning-ZTP-
:AST-CFG-07-Zero-TouchProvisioning-ZTP- rdf:type owl:NamedIndividual ,
                                                 :Asset_Management_Policies ;
                                        :HasWeight 8 ;
                                        rdfs:comment "Mechanisms exist to implement Zero-Touch Provisioning (ZTP), or similar technology, to automatically and securely configure devices upon being added to a network." .


###  http://FYP-ASHS21/csonto/AST-CFG-08-Sensitive-RegulatedDataAccessEnforcement
:AST-CFG-08-Sensitive-RegulatedDataAccessEnforcement rdf:type owl:NamedIndividual ,
                                                              :Asset_Management_Policies ;
                                                     :HasWeight 7 ;
                                                     rdfs:comment "Mechanisms exist to configure systems, applications and processes to restrict access to sensitive/regulated data." .


###  http://FYP-ASHS21/csonto/AST-CFG-08.1-Sensitive-RegulatedDataActions
:AST-CFG-08.1-Sensitive-RegulatedDataActions rdf:type owl:NamedIndividual ,
                                                      :Asset_Management_Policies ;
                                             :HasWeight 7 ;
                                             rdfs:comment "Automated mechanisms exist to generate event logs whenever sensitive/regulated data is collected, created, updated, deleted and/or archived." .


###  http://FYP-ASHS21/csonto/AST-MDM-01-CentralizedManagementOfMobileDevices
:AST-MDM-01-CentralizedManagementOfMobileDevices rdf:type owl:NamedIndividual ,
                                                          :Asset_Management_Policies ;
                                                 :HasWeight 10 ;
                                                 rdfs:comment "Mechanisms exist to develop, govern & update procedures to facilitate the implementation of mobile device management controls." .


###  http://FYP-ASHS21/csonto/AST-MDM-02-AccessControlForMobileDevices
:AST-MDM-02-AccessControlForMobileDevices rdf:type owl:NamedIndividual ,
                                                   :Asset_Management_Policies ;
                                          :HasWeight 9 ;
                                          rdfs:comment "Mechanisms exist to enforce access control requirements for the connection of mobile devices to organizational systems. " .


###  http://FYP-ASHS21/csonto/AST-MDM-04-MobileDeviceTampering
:AST-MDM-04-MobileDeviceTampering rdf:type owl:NamedIndividual ,
                                           :Asset_Management_Policies ;
                                  :HasWeight 9 ;
                                  rdfs:comment "Mechanisms exist to protect mobile devices from tampering through inspecting devices returning from locations that the organization deems to be of significant risk, prior to the device being connected to the organizations network." .


###  http://FYP-ASHS21/csonto/AST-MDM-05-RemotePurging
:AST-MDM-05-RemotePurging rdf:type owl:NamedIndividual ,
                                   :Asset_Management_Policies ;
                          :HasWeight 9 ;
                          rdfs:comment "Mechanisms exist to remotely purge selected information from mobile devices. " .


###  http://FYP-ASHS21/csonto/AST-MDM-06-Personally-OwnedMobileDevices
:AST-MDM-06-Personally-OwnedMobileDevices rdf:type owl:NamedIndividual ,
                                                   :Asset_Management_Policies ;
                                          :HasWeight 8 ;
                                          rdfs:comment "Mechanisms exist to restrict the connection of personally-owned, mobile devices to organizational systems and networks. " .


###  http://FYP-ASHS21/csonto/AST-MDM-07-Organization-OwnedMobileDevices
:AST-MDM-07-Organization-OwnedMobileDevices rdf:type owl:NamedIndividual ,
                                                     :Asset_Management_Policies ;
                                            :HasWeight 8 ;
                                            rdfs:comment "Mechanisms exist to prohibit the installation of non-approved applications or approved applications not obtained through the organization-approved application store." .


###  http://FYP-ASHS21/csonto/AST-MDM-08-MobileDeviceDataRetentionLimitations
:AST-MDM-08-MobileDeviceDataRetentionLimitations rdf:type owl:NamedIndividual ,
                                                          :Asset_Management_Policies ;
                                                 :HasWeight 7 ;
                                                 rdfs:comment "Mechanisms exist to limit data retention on mobile devices to the smallest usable dataset and timeframe." .


###  http://FYP-ASHS21/csonto/AST-MDM-09-MobileDeviceGeofencing
:AST-MDM-09-MobileDeviceGeofencing rdf:type owl:NamedIndividual ,
                                            :Asset_Management_Policies ;
                                   :HasWeight 7 ;
                                   rdfs:comment "Mechanisms exist to restrict the functionality of mobile devices based on geographic location." .


###  http://FYP-ASHS21/csonto/AST-MDM-10-SeparateMobileDeviceProfiles
:AST-MDM-10-SeparateMobileDeviceProfiles rdf:type owl:NamedIndividual ,
                                                  :Asset_Management_Policies ;
                                         :HasWeight 7 ;
                                         rdfs:comment "Mechanisms exist to enforce a separate device workspace on applicable mobile devices to separate work-related and personal-related applications and data. " .


###  http://FYP-ASHS21/csonto/AST-MDM-11-RestrictingAccessToAuthorizedDevices
:AST-MDM-11-RestrictingAccessToAuthorizedDevices rdf:type owl:NamedIndividual ,
                                                          :Asset_Management_Policies ;
                                                 :HasWeight 8 ;
                                                 rdfs:comment "Mechanisms exist to restrict the connectivity of unauthorized mobile devices from communicating with systems, applications and services." .


###  http://FYP-ASHS21/csonto/CHG-CHG-01-ChangeManagementProgram
:CHG-CHG-01-ChangeManagementProgram rdf:type owl:NamedIndividual ,
                                             :Change_Management_Policies ;
                                    :HasWeight 10 ;
                                    rdfs:comment "Mechanisms exist to facilitate the implementation of a change management program." .


###  http://FYP-ASHS21/csonto/CHG-CHG-02-ConfigurationChangeControl
:CHG-CHG-02-ConfigurationChangeControl rdf:type owl:NamedIndividual ,
                                                :Change_Management_Policies ;
                                       :HasWeight 8 ;
                                       rdfs:comment "Mechanisms exist to govern the technical configuration change control processes." .


###  http://FYP-ASHS21/csonto/CHG-CHG-02.1-ProhibitionOfChanges
:CHG-CHG-02.1-ProhibitionOfChanges rdf:type owl:NamedIndividual ,
                                            :Change_Management_Policies ;
                                   :HasWeight 10 ;
                                   rdfs:comment "Mechanisms exist to prohibit unauthorized changes, unless organization-approved change requests are received." .


###  http://FYP-ASHS21/csonto/CHG-CHG-02.4-AutomatedSecurityResponse
:CHG-CHG-02.4-AutomatedSecurityResponse rdf:type owl:NamedIndividual ,
                                                 :Change_Management_Policies ;
                                        :HasWeight 5 ;
                                        rdfs:comment "Automated mechanisms exist to implement remediation actions upon the detection of unauthorized baseline configurations change(s)." .


###  http://FYP-ASHS21/csonto/CHG-CHG-02.5-CryptographicManagement
:CHG-CHG-02.5-CryptographicManagement rdf:type owl:NamedIndividual ,
                                               :Change_Management_Policies ;
                                      :HasWeight 5 ;
                                      rdfs:comment "Mechanisms exist to govern assets involved in providing cryptographic protections according to the organization's configuration management processes. " .


###  http://FYP-ASHS21/csonto/CHG-CHG-03-SecurityImpactAnalysisforChanges
:CHG-CHG-03-SecurityImpactAnalysisforChanges rdf:type owl:NamedIndividual ,
                                                      :Change_Management_Policies ;
                                             :HasWeight 9 ;
                                             rdfs:comment "Mechanisms exist to analyze proposed changes for potential security impacts, prior to the implementation of the change." .


###  http://FYP-ASHS21/csonto/CHG-CHG-04-AccessRestrictionForChange
:CHG-CHG-04-AccessRestrictionForChange rdf:type owl:NamedIndividual ,
                                                :Change_Management_Policies ;
                                       :HasWeight 8 ;
                                       rdfs:comment "Mechanisms exist to enforce configuration restrictions in an effort to restrict the ability of users to conduct unauthorized changes." .


###  http://FYP-ASHS21/csonto/CHG-CHG-04.1-AutomatedAccessEnforcement-Auditing
:CHG-CHG-04.1-AutomatedAccessEnforcement-Auditing rdf:type owl:NamedIndividual ,
                                                           :Change_Management_Policies ;
                                                  :HasWeight 3 ;
                                                  rdfs:comment "Mechanisms exist to perform after-the-fact reviews of configuration change logs to discover any unauthorized changes." .


###  http://FYP-ASHS21/csonto/CHG-CHG-04.2-SignedComponents
:CHG-CHG-04.2-SignedComponents rdf:type owl:NamedIndividual ,
                                        :Change_Management_Policies ;
                               :HasWeight 3 ;
                               rdfs:comment "Mechanisms exist to prevent the installation of software and firmware components without verification that the component has been digitally signed using an organization-approved certificate authority." .


###  http://FYP-ASHS21/csonto/CHG-CHG-04.3-DualAuthorizationforChange
:CHG-CHG-04.3-DualAuthorizationforChange rdf:type owl:NamedIndividual ,
                                                  :Change_Management_Policies ;
                                         :HasWeight 6 ;
                                         rdfs:comment "Mechanisms exist to enforce a two-person rule for implementing changes to critical assets." .


###  http://FYP-ASHS21/csonto/CHG-CHG-04.4-LimitProduction-OperationalPrivileges-IncompatibleRoles-
:CHG-CHG-04.4-LimitProduction-OperationalPrivileges-IncompatibleRoles- rdf:type owl:NamedIndividual ,
                                                                                :Change_Management_Policies ;
                                                                       :HasWeight 6 ;
                                                                       rdfs:comment "Mechanisms exist to limit operational privileges for implementing changes." .


###  http://FYP-ASHS21/csonto/CHG-CHG-04.5-LibraryPrivileges
:CHG-CHG-04.5-LibraryPrivileges rdf:type owl:NamedIndividual ,
                                         :Change_Management_Policies ;
                                :HasWeight 8 ;
                                rdfs:comment "Mechanisms exist to restrict software library privileges to those individuals with a pertinent business need for access. " .


###  http://FYP-ASHS21/csonto/CHG-CHG-05-StakeholderNotificationofChanges
:CHG-CHG-05-StakeholderNotificationofChanges rdf:type owl:NamedIndividual ,
                                                      :Change_Management_Policies ;
                                             :HasWeight 9 ;
                                             rdfs:comment "Mechanisms exist to ensure stakeholders are made aware of and understand the impact of proposed changes. " .


###  http://FYP-ASHS21/csonto/CHG-CHG-06-CybersecurityFunctionalityVerification
:CHG-CHG-06-CybersecurityFunctionalityVerification rdf:type owl:NamedIndividual ,
                                                            :Change_Management_Policies ;
                                                   :HasWeight 9 ;
                                                   rdfs:comment "Mechanisms exist to verify the functionality of cybersecurity controls when anomalies are discovered." .


###  http://FYP-ASHS21/csonto/CHG-CHG-06.1-ReportVerificationResults
:CHG-CHG-06.1-ReportVerificationResults rdf:type owl:NamedIndividual ,
                                                 :Change_Management_Policies ;
                                        :HasWeight 5 ;
                                        rdfs:comment "Mechanisms exist to report the results of cybersecurity & data privacy function verification to appropriate organizational management." .


###  http://FYP-ASHS21/csonto/CHG-RSK-01-RiskManagementProgram
:CHG-RSK-01-RiskManagementProgram rdf:type owl:NamedIndividual ,
                                           :Change_Management_Policies ;
                                  :HasWeight 10 ;
                                  rdfs:comment "Mechanisms exist to facilitate the implementation of risk management controls." .


###  http://FYP-ASHS21/csonto/CHG-RSK-01.1-RiskFraming
:CHG-RSK-01.1-RiskFraming rdf:type owl:NamedIndividual ,
                                   :Change_Management_Policies ;
                          :HasWeight 9 ;
                          rdfs:comment """Mechanisms exist to identify:
  Assumptions affecting risk assessments, risk response and risk monitoring;
  Constraints affecting risk assessments, risk response and risk monitoring;
  The organizational risk tolerance; and
  Priorities and trade-offs considered by the organization for managing risk.""" .


###  http://FYP-ASHS21/csonto/CHG-RSK-01.2-RiskManagementResourcing
:CHG-RSK-01.2-RiskManagementResourcing rdf:type owl:NamedIndividual ,
                                                :Change_Management_Policies ;
                                       :HasWeight 8 ;
                                       rdfs:comment "Mechanisms exist to reduce the magnitude or likelihood of potential impacts by resourcing the capability required to manage technology-related risks." .


###  http://FYP-ASHS21/csonto/CHG-RSK-01.3-RiskTolerance
:CHG-RSK-01.3-RiskTolerance rdf:type owl:NamedIndividual ,
                                     :Change_Management_Policies ;
                            :HasWeight 9 ;
                            rdfs:comment "Mechanisms exist to define organizational risk tolerance, the specified range of acceptable results." .


###  http://FYP-ASHS21/csonto/CHG-RSK-01.4-RiskThreshold
:CHG-RSK-01.4-RiskThreshold rdf:type owl:NamedIndividual ,
                                     :Change_Management_Policies ;
                            :HasWeight 9 ;
                            rdfs:comment "Mechanisms exist to define organizational risk threshold, the level of risk exposure above which risks are addressed and below which risks may be accepted." .


###  http://FYP-ASHS21/csonto/CHG-RSK-01.5-RiskAppetite
:CHG-RSK-01.5-RiskAppetite rdf:type owl:NamedIndividual ,
                                    :Change_Management_Policies ;
                           :HasWeight 9 ;
                           rdfs:comment "Mechanisms exist to define organizational risk appetite, the degree of uncertainty the organization is willing to accept in anticipation of a reward." .


###  http://FYP-ASHS21/csonto/CHG-RSK-02-Risk-BasedSecurityCategorization
:CHG-RSK-02-Risk-BasedSecurityCategorization rdf:type owl:NamedIndividual ,
                                                      :Change_Management_Policies ;
                                             :HasWeight 9 ;
                                             rdfs:comment """Mechanisms exist to categorize systems and data in accordance with applicable local, state and Federal laws that:
  Document the security categorization results (including supporting rationale) in the security plan for systems; and
  Ensure the security categorization decision is reviewed and approved by the asset owner.""" .


###  http://FYP-ASHS21/csonto/CHG-RSK-02.1-Impact-LevelPrioritization
:CHG-RSK-02.1-Impact-LevelPrioritization rdf:type owl:NamedIndividual ,
                                                  :Change_Management_Policies ;
                                         :HasWeight 9 ;
                                         rdfs:comment "Mechanisms exist to prioritize the impact level for systems, applications and/or services to prevent potential disruptions." .


###  http://FYP-ASHS21/csonto/CHG-RSK-03-RiskIdentification
:CHG-RSK-03-RiskIdentification rdf:type owl:NamedIndividual ,
                                        :Change_Management_Policies ;
                               :HasWeight 9 ;
                               rdfs:comment "Mechanisms exist to identify and document risks, both internal and external. " .


###  http://FYP-ASHS21/csonto/CHG-RSK-03.1-RiskCatalog
:CHG-RSK-03.1-RiskCatalog rdf:type owl:NamedIndividual ,
                                   :Change_Management_Policies ;
                          :HasWeight 5 ;
                          rdfs:comment "Mechanisms exist to develop and keep current a catalog of applicable risks associated with the organization's business operations and technologies in use." .


###  http://FYP-ASHS21/csonto/CHG-RSK-04-RiskAssessment
:CHG-RSK-04-RiskAssessment rdf:type owl:NamedIndividual ,
                                    :Change_Management_Policies ;
                           :HasWeight 10 ;
                           rdfs:comment "Mechanisms exist to conduct recurring assessments of risk that includes the likelihood and magnitude of harm, from unauthorized access, use, disclosure, disruption, modification or destruction of the organization's systems and data." .


###  http://FYP-ASHS21/csonto/CHG-RSK-04.1-RiskRegister
:CHG-RSK-04.1-RiskRegister rdf:type owl:NamedIndividual ,
                                    :Change_Management_Policies ;
                           :HasWeight 10 ;
                           rdfs:comment "Mechanisms exist to maintain a risk register that facilitates monitoring and reporting of risks." .


###  http://FYP-ASHS21/csonto/CHG-RSK-05-RiskRanking
:CHG-RSK-05-RiskRanking rdf:type owl:NamedIndividual ,
                                 :Change_Management_Policies ;
                        :HasWeight 9 ;
                        rdfs:comment "Mechanisms exist to identify and assign a risk ranking to newly discovered security vulnerabilities that is based on industry-recognized practices. " .


###  http://FYP-ASHS21/csonto/CHG-RSK-06-RiskRemediation
:CHG-RSK-06-RiskRemediation rdf:type owl:NamedIndividual ,
                                     :Change_Management_Policies ;
                            :HasWeight 10 ;
                            rdfs:comment "Mechanisms exist to remediate risks to an acceptable level. " .


###  http://FYP-ASHS21/csonto/CHG-RSK-06.1-RiskResponse
:CHG-RSK-06.1-RiskResponse rdf:type owl:NamedIndividual ,
                                    :Change_Management_Policies ;
                           :HasWeight 9 ;
                           rdfs:comment "Mechanisms exist to respond to findings from cybersecurity & data privacy assessments, incidents and audits to ensure proper remediation has been performed." .


###  http://FYP-ASHS21/csonto/CHG-RSK-06.2-CompensatingCountermeasures
:CHG-RSK-06.2-CompensatingCountermeasures rdf:type owl:NamedIndividual ,
                                                   :Change_Management_Policies ;
                                          :HasWeight 9 ;
                                          rdfs:comment "Mechanisms exist to identify and implement compensating countermeasures to reduce risk and exposure to threats." .


###  http://FYP-ASHS21/csonto/CHG-RSK-07-RiskAssessmentUpdate
:CHG-RSK-07-RiskAssessmentUpdate rdf:type owl:NamedIndividual ,
                                          :Change_Management_Policies ;
                                 :HasWeight 9 ;
                                 rdfs:comment "Mechanisms exist to routinely update risk assessments and react accordingly upon identifying new security vulnerabilities, including using outside sources for security vulnerability information. " .


###  http://FYP-ASHS21/csonto/CHG-RSK-08-BusinessImpactAnalysis-BIA-
:CHG-RSK-08-BusinessImpactAnalysis-BIA- rdf:type owl:NamedIndividual ,
                                                 :Change_Management_Policies ;
                                        :HasWeight 8 ;
                                        rdfs:comment "Mechanisms exist to conduct a Business Impact Analysis (BIA) to identify and assess cybersecurity and data protection risks." .


###  http://FYP-ASHS21/csonto/CHG-RSK-09-SupplyChainRiskManagement-SCRM-Plan
:CHG-RSK-09-SupplyChainRiskManagement-SCRM-Plan rdf:type owl:NamedIndividual ,
                                                         :Change_Management_Policies ;
                                                :HasWeight 10 ;
                                                rdfs:comment "Mechanisms exist to develop a plan for Supply Chain Risk Management (SCRM) associated with the development, acquisition, maintenance and disposal of systems, system components and services, including documenting selected mitigating actions and monitoring performance against those plans." .


###  http://FYP-ASHS21/csonto/CHG-RSK-09.1-SupplyChainRiskAssessment
:CHG-RSK-09.1-SupplyChainRiskAssessment rdf:type owl:NamedIndividual ,
                                                 :Change_Management_Policies ;
                                        :HasWeight 9 ;
                                        rdfs:comment "Mechanisms exist to periodically assess supply chain risks associated with systems, system components and services." .


###  http://FYP-ASHS21/csonto/CHG-RSK-10-DataProtectionImpactAssessment-DPIA-
:CHG-RSK-10-DataProtectionImpactAssessment-DPIA- rdf:type owl:NamedIndividual ,
                                                          :Change_Management_Policies ;
                                                 :HasWeight 9 ;
                                                 rdfs:comment "Mechanisms exist to conduct a Data Protection Impact Assessment (DPIA) on systems, applications and services that store, process and/or transmit Personal Data (PD) to identify and remediate reasonably-expected risks." .


###  http://FYP-ASHS21/csonto/CHG-RSK-11-RiskMonitoring
:CHG-RSK-11-RiskMonitoring rdf:type owl:NamedIndividual ,
                                    :Change_Management_Policies ;
                           :HasWeight 9 ;
                           rdfs:comment "Mechanisms exist to ensure risk monitoring as an integral part of the continuous monitoring strategy that includes monitoring the effectiveness of cybersecurity & data privacy controls, compliance and change management." .


###  http://FYP-ASHS21/csonto/CHG-RSK-12-RiskCulture
:CHG-RSK-12-RiskCulture rdf:type owl:NamedIndividual ,
                                 :Change_Management_Policies ;
                        :HasWeight 4 ;
                        rdfs:comment "Mechanisms exist to ensure teams are committed to a culture that considers and communicates technology-related risk." .


###  http://FYP-ASHS21/csonto/CHG-SEA-01-SecureEngineeringPrinciples
:CHG-SEA-01-SecureEngineeringPrinciples rdf:type owl:NamedIndividual ,
                                                 :Change_Management_Policies ;
                                        :HasWeight 10 ;
                                        rdfs:comment "Mechanisms exist to facilitate the implementation of industry-recognized cybersecurity & data privacy practices in the specification, design, development, implementation and modification of systems and services." .


###  http://FYP-ASHS21/csonto/CHG-SEA-01.2-AchievingResilienceRequirements
:CHG-SEA-01.2-AchievingResilienceRequirements rdf:type owl:NamedIndividual ,
                                                       :Change_Management_Policies ;
                                              :HasWeight 4 ;
                                              rdfs:comment "Mechanisms exist to achieve resilience requirements in normal and adverse situations." .


###  http://FYP-ASHS21/csonto/CHG-SEA-02-AlignmentWithEnterpriseArchitecture
:CHG-SEA-02-AlignmentWithEnterpriseArchitecture rdf:type owl:NamedIndividual ,
                                                         :Change_Management_Policies ;
                                                :HasWeight 9 ;
                                                rdfs:comment "Mechanisms exist to develop an enterprise architecture, aligned with industry-recognized leading practices, with consideration for cybersecurity & data privacy principles that addresses risk to organizational operations, assets, individuals, other organizations. " .


###  http://FYP-ASHS21/csonto/CHG-SEA-02.1-StandardizedTerminology
:CHG-SEA-02.1-StandardizedTerminology rdf:type owl:NamedIndividual ,
                                               :Change_Management_Policies ;
                                      :HasWeight 3 ;
                                      rdfs:comment "Mechanisms exist to standardize technology and process terminology to reduce confusion amongst groups and departments. " .


###  http://FYP-ASHS21/csonto/CHG-SEA-02.2-OutsourcingNon-EssentialFunctionsorServices
:CHG-SEA-02.2-OutsourcingNon-EssentialFunctionsorServices rdf:type owl:NamedIndividual ,
                                                                   :Change_Management_Policies ;
                                                          :HasWeight 3 ;
                                                          rdfs:comment "Mechanisms exist to identify non-essential functions or services that are capable of being outsourced to external service providers and align with the organization's enterprise architecture and security standards." .


###  http://FYP-ASHS21/csonto/CHG-SEA-02.3-TechnicalDebtReviews
:CHG-SEA-02.3-TechnicalDebtReviews rdf:type owl:NamedIndividual ,
                                            :Change_Management_Policies ;
                                   :HasWeight 9 ;
                                   rdfs:comment "Mechanisms exist to conduct ongoing technical debt reviews of hardware and software technologies to remediate outdated and/or unsupported technologies." .


###  http://FYP-ASHS21/csonto/CHG-SEA-03-Defense-In-Depth-DiD-Architecture
:CHG-SEA-03-Defense-In-Depth-DiD-Architecture rdf:type owl:NamedIndividual ,
                                                       :Change_Management_Policies ;
                                              :HasWeight 10 ;
                                              rdfs:comment "Mechanisms exist to implement security functions as a layered structure minimizing interactions between layers of the design and avoiding any dependence by lower layers on the functionality or correctness of higher layers. " .


###  http://FYP-ASHS21/csonto/CHG-SEA-03.1-SystemPartitioning
:CHG-SEA-03.1-SystemPartitioning rdf:type owl:NamedIndividual ,
                                          :Change_Management_Policies ;
                                 :HasWeight 8 ;
                                 rdfs:comment "Mechanisms exist to partition systems so that partitions reside in separate physical domains or environments. " .


###  http://FYP-ASHS21/csonto/CHG-SEA-03.2-ApplicationPartitioning
:CHG-SEA-03.2-ApplicationPartitioning rdf:type owl:NamedIndividual ,
                                               :Change_Management_Policies ;
                                      :HasWeight 8 ;
                                      rdfs:comment "Mechanisms exist to separate user functionality from system management functionality. " .


###  http://FYP-ASHS21/csonto/CHG-SEA-04-ProcessIsolation
:CHG-SEA-04-ProcessIsolation rdf:type owl:NamedIndividual ,
                                      :Change_Management_Policies ;
                             :HasWeight 7 ;
                             rdfs:comment "Mechanisms exist to implement a separate execution domain for each executing process. " .


###  http://FYP-ASHS21/csonto/CHG-SEA-04.1-SecurityFunctionIsolation
:CHG-SEA-04.1-SecurityFunctionIsolation rdf:type owl:NamedIndividual ,
                                                 :Change_Management_Policies ;
                                        :HasWeight 7 ;
                                        rdfs:comment "Mechanisms exist to isolate security functions from non-security functions. " .


###  http://FYP-ASHS21/csonto/CHG-SEA-04.2-HardwareSeparation
:CHG-SEA-04.2-HardwareSeparation rdf:type owl:NamedIndividual ,
                                          :Change_Management_Policies ;
                                 :HasWeight 7 ;
                                 rdfs:comment "Mechanisms exist to implement underlying hardware separation mechanisms to facilitate process separation. " .


###  http://FYP-ASHS21/csonto/CHG-SEA-04.3-ThreadSeparation
:CHG-SEA-04.3-ThreadSeparation rdf:type owl:NamedIndividual ,
                                        :Change_Management_Policies ;
                               :HasWeight 7 ;
                               rdfs:comment "Mechanisms exist to maintain a separate execution domain for each thread in multi-threaded processing. " .


###  http://FYP-ASHS21/csonto/CHG-SEA-05-InformationInSharedResources
:CHG-SEA-05-InformationInSharedResources rdf:type owl:NamedIndividual ,
                                                  :Change_Management_Policies ;
                                         :HasWeight 8 ;
                                         rdfs:comment "Mechanisms exist to prevent unauthorized and unintended information transfer via shared system resources. " .


###  http://FYP-ASHS21/csonto/CHG-SEA-06-PreventProgramExecution
:CHG-SEA-06-PreventProgramExecution rdf:type owl:NamedIndividual ,
                                             :Change_Management_Policies ;
                                    :HasWeight 8 ;
                                    rdfs:comment "Automated mechanisms exist to prevent the execution of unauthorized software programs. " .


###  http://FYP-ASHS21/csonto/CHG-SEA-07-PredictableFailureAnalysis
:CHG-SEA-07-PredictableFailureAnalysis rdf:type owl:NamedIndividual ,
                                                :Change_Management_Policies ;
                                       :HasWeight 5 ;
                                       rdfs:comment "Mechanisms exist to determine the Mean Time to Failure (MTTF) for system components in specific environments of operation." .


###  http://FYP-ASHS21/csonto/CHG-SEA-07.1-TechnologyLifecycleManagement
:CHG-SEA-07.1-TechnologyLifecycleManagement rdf:type owl:NamedIndividual ,
                                                     :Change_Management_Policies ;
                                            :HasWeight 7 ;
                                            rdfs:comment "Mechanisms exist to manage the usable lifecycles of technology assets. " .


###  http://FYP-ASHS21/csonto/CHG-SEA-07.2-FailSecure
:CHG-SEA-07.2-FailSecure rdf:type owl:NamedIndividual ,
                                  :Change_Management_Policies ;
                         :HasWeight 8 ;
                         rdfs:comment "Mechanisms exist to enable systems to fail to an organization-defined known-state for types of failures, preserving system state information in failure. " .


###  http://FYP-ASHS21/csonto/CHG-SEA-07.3-FailSafe
:CHG-SEA-07.3-FailSafe rdf:type owl:NamedIndividual ,
                                :Change_Management_Policies ;
                       :HasWeight 8 ;
                       rdfs:comment "Mechanisms exist to implement fail-safe procedures when failure conditions occur. " .


###  http://FYP-ASHS21/csonto/CHG-SEA-08-Non-Persistence
:CHG-SEA-08-Non-Persistence rdf:type owl:NamedIndividual ,
                                     :Change_Management_Policies ;
                            :HasWeight 9 ;
                            rdfs:comment "Mechanisms exist to implement non-persistent system components and services that are initiated in a known state and terminated upon the end of the session of use or periodically at an organization-defined frequency. " .


###  http://FYP-ASHS21/csonto/CHG-SEA-08.1-RefreshfromTrustedSources
:CHG-SEA-08.1-RefreshfromTrustedSources rdf:type owl:NamedIndividual ,
                                                 :Change_Management_Policies ;
                                        :HasWeight 5 ;
                                        rdfs:comment "Mechanisms exist to ensure that software and data needed for information system component and service refreshes are obtained from trusted sources." .


###  http://FYP-ASHS21/csonto/CHG-SEA-09-InformationOutputFiltering
:CHG-SEA-09-InformationOutputFiltering rdf:type owl:NamedIndividual ,
                                                :Change_Management_Policies ;
                                       :HasWeight 8 ;
                                       rdfs:comment "Mechanisms exist to validate information output from software programs and/or applications to ensure that the information is consistent with the expected content. " .


###  http://FYP-ASHS21/csonto/CHG-SEA-09.1-LimitPersonalData-PD-Dissemination
:CHG-SEA-09.1-LimitPersonalData-PD-Dissemination rdf:type owl:NamedIndividual ,
                                                          :Change_Management_Policies ;
                                                 :HasWeight 8 ;
                                                 rdfs:comment "Mechanisms exist to limit the dissemination of Personal Data (PD) to organization-defined elements identified in the Data Protection Impact Assessment (DPIA) and consistent with authorized purposes." .


###  http://FYP-ASHS21/csonto/CHG-SEA-10-MemoryProtection
:CHG-SEA-10-MemoryProtection rdf:type owl:NamedIndividual ,
                                      :Change_Management_Policies ;
                             :HasWeight 8 ;
                             rdfs:comment "Mechanisms exist to implement security safeguards to protect system memory from unauthorized code execution. " .


###  http://FYP-ASHS21/csonto/CHG-SEA-11-Honeypots
:CHG-SEA-11-Honeypots rdf:type owl:NamedIndividual ,
                               :Change_Management_Policies ;
                      :HasWeight 3 ;
                      rdfs:comment "Mechanisms exist to utilize honeypots that are specifically designed to be the target of malicious attacks for the purpose of detecting, deflecting and analyzing such attacks. " .


###  http://FYP-ASHS21/csonto/CHG-SEA-12-Honeyclients
:CHG-SEA-12-Honeyclients rdf:type owl:NamedIndividual ,
                                  :Change_Management_Policies ;
                         :HasWeight 3 ;
                         rdfs:comment "Mechanisms exist to utilize honeyclients that proactively seek to identify malicious websites and/or web-based malicious code. " .


###  http://FYP-ASHS21/csonto/CHG-SEA-13-Heterogeneity
:CHG-SEA-13-Heterogeneity rdf:type owl:NamedIndividual ,
                                   :Change_Management_Policies ;
                          :HasWeight 3 ;
                          rdfs:comment "Mechanisms exist to utilize a diverse set of technologies for system components to reduce the impact of technical vulnerabilities from the same Original Equipment Manufacturer (OEM). " .


###  http://FYP-ASHS21/csonto/CHG-SEA-13.1-VirtualizationTechniques
:CHG-SEA-13.1-VirtualizationTechniques rdf:type owl:NamedIndividual ,
                                                :Change_Management_Policies ;
                                       :HasWeight 6 ;
                                       rdfs:comment "Mechanisms exist to utilize virtualization techniques to support the employment of a diversity of operating systems and applications." .


###  http://FYP-ASHS21/csonto/CHG-SEA-14.1-Randomness
:CHG-SEA-14.1-Randomness rdf:type owl:NamedIndividual ,
                                  :Change_Management_Policies ;
                         :HasWeight 5 ;
                         rdfs:comment "Automated mechanisms exist to introduce randomness into organizational operations and assets." .


###  http://FYP-ASHS21/csonto/CHG-SEA-16-Non-ModifiableExecutablePrograms
:CHG-SEA-16-Non-ModifiableExecutablePrograms rdf:type owl:NamedIndividual ,
                                                      :Change_Management_Policies ;
                                             :HasWeight 1 ;
                                             rdfs:comment "Mechanisms exist to utilize non-modifiable executable programs that load and execute the operating environment and applications from hardware-enforced, read-only media." .


###  http://FYP-ASHS21/csonto/CHG-SEA-17-SecureLog-OnProcedures
:CHG-SEA-17-SecureLog-OnProcedures rdf:type owl:NamedIndividual ,
                                            :Change_Management_Policies ;
                                   :HasWeight 8 ;
                                   rdfs:comment "Mechanisms exist to utilize a trusted communications path between the user and the security functions of the system." .


###  http://FYP-ASHS21/csonto/CHG-SEA-18-SystemUseNotification-LogonBanner-
:CHG-SEA-18-SystemUseNotification-LogonBanner- rdf:type owl:NamedIndividual ,
                                                        :Change_Management_Policies ;
                                               :HasWeight 9 ;
                                               rdfs:comment "Mechanisms exist to utilize system use notification / logon banners that display an approved system use notification message or banner before granting access to the system that provides cybersecurity & data privacy notices." .


###  http://FYP-ASHS21/csonto/CHG-SEA-18.1-StandardizedMicrosoftWindowsBanner
:CHG-SEA-18.1-StandardizedMicrosoftWindowsBanner rdf:type owl:NamedIndividual ,
                                                          :Change_Management_Policies ;
                                                 :HasWeight 9 ;
                                                 rdfs:comment "Mechanisms exist to configure Microsoft Windows-based systems to display an approved logon banner before granting access to the system that provides cybersecurity & data privacy notices." .


###  http://FYP-ASHS21/csonto/CHG-SEA-18.2-TruncatedBanner
:CHG-SEA-18.2-TruncatedBanner rdf:type owl:NamedIndividual ,
                                       :Change_Management_Policies ;
                              :HasWeight 9 ;
                              rdfs:comment "Mechanisms exist to utilize a truncated system use notification / logon banner on systems not capable of displaying a logon banner from a centralized source, such as Active Directory." .


###  http://FYP-ASHS21/csonto/CHG-SEA-19-PreviousLogonNotification
:CHG-SEA-19-PreviousLogonNotification rdf:type owl:NamedIndividual ,
                                               :Change_Management_Policies ;
                                      :HasWeight 3 ;
                                      rdfs:comment "Mechanisms exist to configure systems that process, store or transmit sensitive/regulated data to notify the user, upon successful logon, of the number of unsuccessful logon attempts since the last successful logon." .


###  http://FYP-ASHS21/csonto/CHG-SEA-20-ClockSynchronization
:CHG-SEA-20-ClockSynchronization rdf:type owl:NamedIndividual ,
                                          :Change_Management_Policies ;
                                 :HasWeight 9 ;
                                 rdfs:comment "Mechanisms exist to utilize time-synchronization technology to synchronize all critical system clocks. " .


###  http://FYP-ASHS21/csonto/CHG-TDA-01.1-ProductManagement
:CHG-TDA-01.1-ProductManagement rdf:type owl:NamedIndividual ,
                                         :Change_Management_Policies ;
                                :HasWeight 10 ;
                                rdfs:comment "Mechanisms exist to design and implement product management processes to update products, including systems, software and services, to improve functionality and correct security deficiencies." .


###  http://FYP-ASHS21/csonto/CHG-TDA-01.2-IntegrityMechanismsforSoftware-FirmwareUpdates
:CHG-TDA-01.2-IntegrityMechanismsforSoftware-FirmwareUpdates rdf:type owl:NamedIndividual ,
                                                                      :Change_Management_Policies ;
                                                             :HasWeight 5 ;
                                                             rdfs:comment "Mechanisms exist to utilize integrity validation mechanisms for security updates." .


###  http://FYP-ASHS21/csonto/CHG-TDA-01.3-MalwareTestingPriortoRelease
:CHG-TDA-01.3-MalwareTestingPriortoRelease rdf:type owl:NamedIndividual ,
                                                    :Change_Management_Policies ;
                                           :HasWeight 9 ;
                                           rdfs:comment "Mechanisms exist to utilize at least one (1) malware detection tool to identify if any known malware exists in the final binaries of the product or security update." .


###  http://FYP-ASHS21/csonto/CHG-TDA-02-MinimumViableProduct-MVP-SecurityRequirements
:CHG-TDA-02-MinimumViableProduct-MVP-SecurityRequirements rdf:type owl:NamedIndividual ,
                                                                   :Change_Management_Policies ;
                                                          :HasWeight 9 ;
                                                          rdfs:comment "Mechanisms exist to ensure risk-based technical and functional specifications are established to define a Minimum Viable Product (MVP)." .


###  http://FYP-ASHS21/csonto/CHG-TDA-02.2-InformationAssuranceEnabledProducts
:CHG-TDA-02.2-InformationAssuranceEnabledProducts rdf:type owl:NamedIndividual ,
                                                           :Change_Management_Policies ;
                                                  :HasWeight 2 ;
                                                  rdfs:comment "Mechanisms exist to limit the use of commercially-provided Information Assurance (IA) and IA-enabled IT products to those products that have been successfully evaluated against a National Information Assurance partnership (NIAP)-approved Protection Profile or the cryptographic module is FIPS-validated or NSA-approved." .


###  http://FYP-ASHS21/csonto/CHG-TDA-02.4-Pre-EstablishedSecureConfigurations
:CHG-TDA-02.4-Pre-EstablishedSecureConfigurations rdf:type owl:NamedIndividual ,
                                                           :Change_Management_Policies ;
                                                  :HasWeight 8 ;
                                                  rdfs:comment """Mechanisms exist to ensure vendors / manufacturers:
  Deliver the system, component, or service with a pre-established, secure configuration implemented; and
  Use the pre-established, secure configuration as the default for any subsequent system, component, or service reinstallation or upgrade.""" .


###  http://FYP-ASHS21/csonto/CHG-TDA-03-CommercialOff-The-Shelf-COTS-SecuritySolutions
:CHG-TDA-03-CommercialOff-The-Shelf-COTS-SecuritySolutions rdf:type owl:NamedIndividual ,
                                                                    :Change_Management_Policies ;
                                                           :HasWeight 5 ;
                                                           rdfs:comment "Mechanisms exist to utilize only Commercial Off-the-Shelf (COTS) security products. " .


###  http://FYP-ASHS21/csonto/CHG-TDA-03.1-SupplierDiversity
:CHG-TDA-03.1-SupplierDiversity rdf:type owl:NamedIndividual ,
                                         :Change_Management_Policies ;
                                :HasWeight 3 ;
                                rdfs:comment "Mechanisms exist to obtain cybersecurity & data privacy technologies from different suppliers to minimize supply chain risk." .


###  http://FYP-ASHS21/csonto/CHG-TDA-04-DocumentationRequirements
:CHG-TDA-04-DocumentationRequirements rdf:type owl:NamedIndividual ,
                                               :Change_Management_Policies ;
                                      :HasWeight 8 ;
                                      rdfs:comment """Mechanisms exist to obtain, protect and distribute administrator documentation for systems that describe:
  Secure configuration, installation and operation of the system;
  Effective use and maintenance of security features/functions; and
  Known vulnerabilities regarding configuration and use of administrative (e.g., privileged) functions.""" .


###  http://FYP-ASHS21/csonto/CHG-TDA-04.1-FunctionalProperties
:CHG-TDA-04.1-FunctionalProperties rdf:type owl:NamedIndividual ,
                                            :Change_Management_Policies ;
                                   :HasWeight 8 ;
                                   rdfs:comment "Mechanisms exist to require vendors/contractors to provide information describing the functional properties of the security controls to be utilized within systems, system components or services in sufficient detail to permit analysis and testing of the controls. " .


###  http://FYP-ASHS21/csonto/CHG-TDA-04.2-SoftwareBillofMaterials-SBOM-
:CHG-TDA-04.2-SoftwareBillofMaterials-SBOM- rdf:type owl:NamedIndividual ,
                                                     :Change_Management_Policies ;
                                            :HasWeight 9 ;
                                            rdfs:comment "Mechanisms exist to require a Software Bill of Materials (SBOM) for systems, applications and services that lists software packages in use, including versions and applicable licenses." .


###  http://FYP-ASHS21/csonto/CHG-TDA-06-SecureCoding
:CHG-TDA-06-SecureCoding rdf:type owl:NamedIndividual ,
                                  :Change_Management_Policies ;
                         :HasWeight 10 ;
                         rdfs:comment "Mechanisms exist to develop applications based on secure coding principles. " .


###  http://FYP-ASHS21/csonto/CHG-TDA-06.1-CriticalityAnalysis
:CHG-TDA-06.1-CriticalityAnalysis rdf:type owl:NamedIndividual ,
                                           :Change_Management_Policies ;
                                  :HasWeight 9 ;
                                  rdfs:comment "Mechanisms exist to require the developer of the system, system component or service to perform a criticality analysis at organization-defined decision points in the Secure Development Life Cycle (SDLC)." .


###  http://FYP-ASHS21/csonto/CHG-TDA-06.2-ThreatModeling
:CHG-TDA-06.2-ThreatModeling rdf:type owl:NamedIndividual ,
                                      :Change_Management_Policies ;
                             :HasWeight 7 ;
                             rdfs:comment "Mechanisms exist to perform threat modelling and other secure design techniques, to ensure that threats to software and solutions are identified and accounted for." .


###  http://FYP-ASHS21/csonto/CHG-TDA-06.3-SoftwareAssuranceMaturityModel-SAMM-
:CHG-TDA-06.3-SoftwareAssuranceMaturityModel-SAMM- rdf:type owl:NamedIndividual ,
                                                            :Change_Management_Policies ;
                                                   :HasWeight 9 ;
                                                   rdfs:comment "Mechanisms exist to utilize a Software Assurance Maturity Model (SAMM) to govern a secure development lifecycle for the development of systems, applications and services." .


###  http://FYP-ASHS21/csonto/CHG-TDA-06.4-SupportingToolchain
:CHG-TDA-06.4-SupportingToolchain rdf:type owl:NamedIndividual ,
                                           :Change_Management_Policies ;
                                  :HasWeight 6 ;
                                  rdfs:comment "Automated mechanisms exist to improve the accuracy, consistency and comprehensiveness of secure practices throughout the asset's lifecycle." .


###  http://FYP-ASHS21/csonto/CHG-TDA-06.5-SoftwareDesignReview
:CHG-TDA-06.5-SoftwareDesignReview rdf:type owl:NamedIndividual ,
                                            :Change_Management_Policies ;
                                   :HasWeight 10 ;
                                   rdfs:comment "Mechanisms exist to have an independent review of the software design to confirm that all cybersecurity & data privacy requirements are met and that any identified risks are satisfactorily addressed." .


###  http://FYP-ASHS21/csonto/CHG-TDA-07-SecureDevelopmentEnvironments
:CHG-TDA-07-SecureDevelopmentEnvironments rdf:type owl:NamedIndividual ,
                                                   :Change_Management_Policies ;
                                          :HasWeight 9 ;
                                          rdfs:comment "Mechanisms exist to maintain a segmented development network to ensure a secure development environment. " .


###  http://FYP-ASHS21/csonto/CHG-TDA-08-SeparationofDevelopment-TestingandOperationalEnvironments
:CHG-TDA-08-SeparationofDevelopment-TestingandOperationalEnvironments rdf:type owl:NamedIndividual ,
                                                                               :Change_Management_Policies ;
                                                                      :HasWeight 10 ;
                                                                      rdfs:comment "Mechanisms exist to manage separate development, testing and operational environments to reduce the risks of unauthorized access or changes to the operational environment and to ensure no impact to production systems." .


###  http://FYP-ASHS21/csonto/CHG-TDA-08.1-SecureMigrationPractices
:CHG-TDA-08.1-SecureMigrationPractices rdf:type owl:NamedIndividual ,
                                                :Change_Management_Policies ;
                                       :HasWeight 8 ;
                                       rdfs:comment "Mechanisms exist to ensure secure migration practices purge systems, applications and services of test/development/staging data and accounts before it is migrated into a production environment." .


###  http://FYP-ASHS21/csonto/CHG-TDA-09.1-ContinuousMonitoringPlan
:CHG-TDA-09.1-ContinuousMonitoringPlan rdf:type owl:NamedIndividual ,
                                                :Change_Management_Policies ;
                                       :HasWeight 9 ;
                                       rdfs:comment "Mechanisms exist to require the developers of systems, system components or services to produce a plan for the continuous monitoring of cybersecurity & data privacy control effectiveness. " .


###  http://FYP-ASHS21/csonto/CHG-TDA-09.2-StaticCodeAnalysis
:CHG-TDA-09.2-StaticCodeAnalysis rdf:type owl:NamedIndividual ,
                                          :Change_Management_Policies ;
                                 :HasWeight 9 ;
                                 rdfs:comment "Mechanisms exist to require the developers of systems, system components or services to employ static code analysis tools to identify and remediate common flaws and document the results of the analysis. " .


###  http://FYP-ASHS21/csonto/CHG-TDA-09.3-DynamicCodeAnalysis
:CHG-TDA-09.3-DynamicCodeAnalysis rdf:type owl:NamedIndividual ,
                                           :Change_Management_Policies ;
                                  :HasWeight 9 ;
                                  rdfs:comment "Mechanisms exist to require the developers of systems, system components or services to employ dynamic code analysis tools to identify and remediate common flaws and document the results of the analysis. " .


###  http://FYP-ASHS21/csonto/CHG-TDA-09.4-MalformedInputTesting
:CHG-TDA-09.4-MalformedInputTesting rdf:type owl:NamedIndividual ,
                                             :Change_Management_Policies ;
                                    :HasWeight 7 ;
                                    rdfs:comment "Mechanisms exist to utilize testing methods to ensure systems, services and products continue to operate as intended when subject to invalid or unexpected inputs on its interfaces." .


###  http://FYP-ASHS21/csonto/CHG-TDA-09.5-ApplicationPenetrationTesting
:CHG-TDA-09.5-ApplicationPenetrationTesting rdf:type owl:NamedIndividual ,
                                                     :Change_Management_Policies ;
                                            :HasWeight 9 ;
                                            rdfs:comment "Mechanisms exist to perform application-level penetration testing of custom-made applications and services." .


###  http://FYP-ASHS21/csonto/CHG-TDA-09.6-SecureSettingsByDefault
:CHG-TDA-09.6-SecureSettingsByDefault rdf:type owl:NamedIndividual ,
                                               :Change_Management_Policies ;
                                      :HasWeight 9 ;
                                      rdfs:comment "Mechanisms exist to implement secure configuration settings by default to reduce the likelihood of software being deployed with weak security settings that would put the asset at a greater risk of compromise." .


###  http://FYP-ASHS21/csonto/CHG-TDA-09.7-ManualCodeReview
:CHG-TDA-09.7-ManualCodeReview rdf:type owl:NamedIndividual ,
                                        :Change_Management_Policies ;
                               :HasWeight 5 ;
                               rdfs:comment "Mechanisms exist to require the developers of systems, system components or services to employ a manual code review process to identify and remediate unique flaws that require knowledge of the applications requirements and design." .


###  http://FYP-ASHS21/csonto/CHG-TDA-10-UseofLiveData
:CHG-TDA-10-UseofLiveData rdf:type owl:NamedIndividual ,
                                   :Change_Management_Policies ;
                          :HasWeight 9 ;
                          rdfs:comment "Mechanisms exist to approve, document and control the use of live data in development and test environments." .


###  http://FYP-ASHS21/csonto/CHG-TDA-10.1-TestDataIntegrity
:CHG-TDA-10.1-TestDataIntegrity rdf:type owl:NamedIndividual ,
                                         :Change_Management_Policies ;
                                :HasWeight 8 ;
                                rdfs:comment "Mechanisms exist to ensure the integrity of test data through existing cybersecurity & data privacy controls." .


###  http://FYP-ASHS21/csonto/CHG-TDA-11-ProductTamperingandCounterfeiting-PTC-
:CHG-TDA-11-ProductTamperingandCounterfeiting-PTC- rdf:type owl:NamedIndividual ,
                                                            :Change_Management_Policies ;
                                                   :HasWeight 9 ;
                                                   rdfs:comment "Mechanisms exist to maintain awareness of component authenticity by developing and implementing Product Tampering and Counterfeiting (PTC) practices that include the means to detect and prevent counterfeit components." .


###  http://FYP-ASHS21/csonto/CHG-TDA-11.1-Anti-CounterfeitTraining
:CHG-TDA-11.1-Anti-CounterfeitTraining rdf:type owl:NamedIndividual ,
                                                :Change_Management_Policies ;
                                       :HasWeight 6 ;
                                       rdfs:comment "Mechanisms exist to train personnel to detect counterfeit system components, including hardware, software and firmware. " .


###  http://FYP-ASHS21/csonto/CHG-TDA-11.2-ComponentDisposal
:CHG-TDA-11.2-ComponentDisposal rdf:type owl:NamedIndividual ,
                                         :Change_Management_Policies ;
                                :HasWeight 9 ;
                                rdfs:comment """[deprecated - incorporated into AST-09]
Mechanisms exist to dispose of system components using organization-defined techniques and methods to prevent such components from entering the gray market. """ .


###  http://FYP-ASHS21/csonto/CHG-TDA-12-CustomizedDevelopmentofCriticalComponents
:CHG-TDA-12-CustomizedDevelopmentofCriticalComponents rdf:type owl:NamedIndividual ,
                                                               :Change_Management_Policies ;
                                                      :HasWeight 8 ;
                                                      rdfs:comment "Mechanisms exist to custom-develop critical system components, when Commercial Off The Shelf (COTS) solutions are unavailable." .


###  http://FYP-ASHS21/csonto/CHG-TDA-13-DeveloperScreening
:CHG-TDA-13-DeveloperScreening rdf:type owl:NamedIndividual ,
                                        :Change_Management_Policies ;
                               :HasWeight 9 ;
                               rdfs:comment "Mechanisms exist to ensure that the developers of systems, applications and/or services have the requisite skillset and appropriate access authorizations." .


###  http://FYP-ASHS21/csonto/CHG-TDA-14-DeveloperConfigurationManagement
:CHG-TDA-14-DeveloperConfigurationManagement rdf:type owl:NamedIndividual ,
                                                      :Change_Management_Policies ;
                                             :HasWeight 9 ;
                                             rdfs:comment "Mechanisms exist to require system developers and integrators to perform configuration management during system design, development, implementation and operation." .


###  http://FYP-ASHS21/csonto/CHG-TDA-14.1-Software-FirmwareIntegrityVerification
:CHG-TDA-14.1-Software-FirmwareIntegrityVerification rdf:type owl:NamedIndividual ,
                                                              :Change_Management_Policies ;
                                                     :HasWeight 8 ;
                                                     rdfs:comment "Mechanisms exist to require developer of systems, system components or services to enable integrity verification of software and firmware components. " .


###  http://FYP-ASHS21/csonto/CHG-TDA-14.2-HardwareIntegrityVerification
:CHG-TDA-14.2-HardwareIntegrityVerification rdf:type owl:NamedIndividual ,
                                                     :Change_Management_Policies ;
                                            :HasWeight 5 ;
                                            rdfs:comment "Mechanisms exist to require developer of systems, system components or services to enable integrity verification of hardware components." .


###  http://FYP-ASHS21/csonto/CHG-TDA-16-Developer-ProvidedTraining
:CHG-TDA-16-Developer-ProvidedTraining rdf:type owl:NamedIndividual ,
                                                :Change_Management_Policies ;
                                       :HasWeight 9 ;
                                       rdfs:comment "Mechanisms exist to require the developers of systems, system components or services to provide training on the correct use and operation of the system, system component or service." .


###  http://FYP-ASHS21/csonto/CHG-TDA-17-UnsupportedSystems
:CHG-TDA-17-UnsupportedSystems rdf:type owl:NamedIndividual ,
                                        :Change_Management_Policies ;
                               :HasWeight 10 ;
                               rdfs:comment """Mechanisms exist to prevent unsupported systems by:
  Replacing systems when support for the components is no longer available from the developer, vendor or manufacturer; and
  Requiring justification and documented approval for the continued use of unsupported system components required to satisfy mission/business needs.""" .


###  http://FYP-ASHS21/csonto/CHG-TDA-17.1-AlternateSourcesforContinuedSupport
:CHG-TDA-17.1-AlternateSourcesforContinuedSupport rdf:type owl:NamedIndividual ,
                                                           :Change_Management_Policies ;
                                                  :HasWeight 8 ;
                                                  rdfs:comment "Mechanisms exist to provide in-house support or contract external providers for support with unsupported system components. " .


###  http://FYP-ASHS21/csonto/CHG-TDA-18-InputDataValidation
:CHG-TDA-18-InputDataValidation rdf:type owl:NamedIndividual ,
                                         :Change_Management_Policies ;
                                :HasWeight 9 ;
                                rdfs:comment "Mechanisms exist to check the validity of information inputs. " .


###  http://FYP-ASHS21/csonto/CHG-TDA-19-ErrorHandling
:CHG-TDA-19-ErrorHandling rdf:type owl:NamedIndividual ,
                                   :Change_Management_Policies ;
                          :HasWeight 9 ;
                          rdfs:comment """Mechanisms exist to handle error conditions by: 
  Identifying potentially security-relevant error conditions;
  Generating error messages that provide information necessary for corrective actions without revealing sensitive or potentially harmful information in error logs and administrative messages that could be exploited; and
  Revealing error messages only to authorized personnel.""" .


###  http://FYP-ASHS21/csonto/CHG-TDA-20-AccesstoProgramSourceCode
:CHG-TDA-20-AccesstoProgramSourceCode rdf:type owl:NamedIndividual ,
                                               :Change_Management_Policies ;
                                      :HasWeight 9 ;
                                      rdfs:comment "Mechanisms exist to limit privileges to change software resident within software libraries. " .


###  http://FYP-ASHS21/csonto/CHG-TDA-20.1-SoftwareReleaseIntegrityVerification
:CHG-TDA-20.1-SoftwareReleaseIntegrityVerification rdf:type owl:NamedIndividual ,
                                                            :Change_Management_Policies ;
                                                   :HasWeight 6 ;
                                                   rdfs:comment "Mechanisms exist to publish integrity verification information for software releases." .


###  http://FYP-ASHS21/csonto/CHG-TDA-20.2-ArchivingSoftwareReleases
:CHG-TDA-20.2-ArchivingSoftwareReleases rdf:type owl:NamedIndividual ,
                                                 :Change_Management_Policies ;
                                        :HasWeight 8 ;
                                        rdfs:comment "Mechanisms exist to archive software releases and all of their components (e.g., code, package files, third-party libraries, documentation) to maintain integrity verification information." .


###  http://FYP-ASHS21/csonto/CHG-TDA-20.3-SoftwareEscrow
:CHG-TDA-20.3-SoftwareEscrow rdf:type owl:NamedIndividual ,
                                      :Change_Management_Policies ;
                             :HasWeight 7 ;
                             rdfs:comment "Mechanisms exist to escrow source code and supporting documentation to ensure software availability in the event the software provider goes out of business or is unable to provide support. " .


###  http://FYP-ASHS21/csonto/CHG-TPM-01-Third-PartyManagement
:CHG-TPM-01-Third-PartyManagement rdf:type owl:NamedIndividual ,
                                           :Change_Management_Policies ;
                                  :HasWeight 10 ;
                                  rdfs:comment "Mechanisms exist to facilitate the implementation of third-party management controls." .


###  http://FYP-ASHS21/csonto/CHG-TPM-01.1-Third-PartyInventories
:CHG-TPM-01.1-Third-PartyInventories rdf:type owl:NamedIndividual ,
                                              :Change_Management_Policies ;
                                     :HasWeight 8 ;
                                     rdfs:comment "Mechanisms exist to maintain a current, accurate and complete list of External Service Providers (ESPs) that can potentially impact the Confidentiality, Integrity, Availability and/or Safety (CIAS) of the organization's systems, applications, services and data." .


###  http://FYP-ASHS21/csonto/CHG-TPM-02-Third-PartyCriticalityAssessments
:CHG-TPM-02-Third-PartyCriticalityAssessments rdf:type owl:NamedIndividual ,
                                                       :Change_Management_Policies ;
                                              :HasWeight 9 ;
                                              rdfs:comment "Mechanisms exist to identify, prioritize and assess suppliers and partners of critical systems, components and services using a supply chain risk assessment process relative to their importance in supporting the delivery of high-value services." .


###  http://FYP-ASHS21/csonto/CHG-TPM-03-SupplyChainProtection
:CHG-TPM-03-SupplyChainProtection rdf:type owl:NamedIndividual ,
                                           :Change_Management_Policies ;
                                  :HasWeight 9 ;
                                  rdfs:comment "Mechanisms exist to evaluate security risks associated with the services and product supply chain. " .


###  http://FYP-ASHS21/csonto/CHG-TPM-03.2-LimitPotentialHarm
:CHG-TPM-03.2-LimitPotentialHarm rdf:type owl:NamedIndividual ,
                                          :Change_Management_Policies ;
                                 :HasWeight 9 ;
                                 rdfs:comment "Mechanisms exist to utilize security safeguards to limit harm from potential adversaries who identify and target the organization's supply chain. " .


###  http://FYP-ASHS21/csonto/CHG-TPM-03.3-ProcessesToAddressWeaknessesorDeficiencies
:CHG-TPM-03.3-ProcessesToAddressWeaknessesorDeficiencies rdf:type owl:NamedIndividual ,
                                                                  :Change_Management_Policies ;
                                                         :HasWeight 9 ;
                                                         rdfs:comment "Mechanisms exist to address identified weaknesses or deficiencies in the security of the supply chain " .


###  http://FYP-ASHS21/csonto/CHG-TPM-04-Third-PartyServices
:CHG-TPM-04-Third-PartyServices rdf:type owl:NamedIndividual ,
                                         :Change_Management_Policies ;
                                :HasWeight 10 ;
                                rdfs:comment "Mechanisms exist to mitigate the risks associated with third-party access to the organizations systems and data." .


###  http://FYP-ASHS21/csonto/CHG-TPM-04.3-ConflictofInterests
:CHG-TPM-04.3-ConflictofInterests rdf:type owl:NamedIndividual ,
                                           :Change_Management_Policies ;
                                  :HasWeight 8 ;
                                  rdfs:comment "Mechanisms exist to ensure that the interests of external service providers are consistent with and reflect organizational interests." .


###  http://FYP-ASHS21/csonto/CHG-TPM-04.4-Third-PartyProcessing-StorageandServiceLocations
:CHG-TPM-04.4-Third-PartyProcessing-StorageandServiceLocations rdf:type owl:NamedIndividual ,
                                                                        :Change_Management_Policies ;
                                                               :HasWeight 10 ;
                                                               rdfs:comment "Mechanisms exist to restrict the location of information processing/storage based on business requirements. " .


###  http://FYP-ASHS21/csonto/CHG-TPM-05-Third-PartyContractRequirements
:CHG-TPM-05-Third-PartyContractRequirements rdf:type owl:NamedIndividual ,
                                                     :Change_Management_Policies ;
                                            :HasWeight 10 ;
                                            rdfs:comment "Mechanisms exist to identify, regularly review and document third-party confidentiality, Non-Disclosure Agreements (NDAs) and other contracts that reflect the organizations needs to protect systems and data." .


###  http://FYP-ASHS21/csonto/CHG-TPM-05.1-SecurityCompromiseNotificationAgreements
:CHG-TPM-05.1-SecurityCompromiseNotificationAgreements rdf:type owl:NamedIndividual ,
                                                                :Change_Management_Policies ;
                                                       :HasWeight 9 ;
                                                       rdfs:comment "Mechanisms exist to compel External Service Providers (ESPs) to provide notification of actual or potential compromises in the supply chain that can potentially affect or have adversely affected systems, applications and/or services that the organization utilizes." .


###  http://FYP-ASHS21/csonto/CHG-TPM-05.2-ContractFlow-DownRequirements
:CHG-TPM-05.2-ContractFlow-DownRequirements rdf:type owl:NamedIndividual ,
                                                     :Change_Management_Policies ;
                                            :HasWeight 9 ;
                                            rdfs:comment "Mechanisms exist to ensure cybersecurity & data privacy requirements are included in contracts that flow-down to applicable sub-contractors and suppliers." .


###  http://FYP-ASHS21/csonto/CHG-TPM-05.3-Third-PartyAuthenticationPractices
:CHG-TPM-05.3-Third-PartyAuthenticationPractices rdf:type owl:NamedIndividual ,
                                                          :Change_Management_Policies ;
                                                 :HasWeight 8 ;
                                                 rdfs:comment "Mechanisms exist to ensure External Service Providers (ESPs) use unique authentication factors for each of its customers." .


###  http://FYP-ASHS21/csonto/CHG-TPM-05.5-Third-PartyScopeReview
:CHG-TPM-05.5-Third-PartyScopeReview rdf:type owl:NamedIndividual ,
                                              :Change_Management_Policies ;
                                     :HasWeight 10 ;
                                     rdfs:comment "Mechanisms exist to perform recurring validation of the Responsible, Accountable, Supportive, Consulted & Informed (RASCI) matrix, or similar documentation, to ensure cybersecurity & data privacy control assignments accurately reflect current business practices, compliance obligations, technologies and stakeholders. " .


###  http://FYP-ASHS21/csonto/CHG-TPM-05.6-First-PartyDeclaration-1PD-
:CHG-TPM-05.6-First-PartyDeclaration-1PD- rdf:type owl:NamedIndividual ,
                                                   :Change_Management_Policies ;
                                          :HasWeight 7 ;
                                          rdfs:comment "Mechanisms exist to obtain a First-Party Declaration (1PD) from applicable External Service Providers (ESPs) that provides assurance of compliance with specified statutory, regulatory and contractual obligations for cybersecurity & data privacy controls, including any flow-down requirements to subcontractors. " .


###  http://FYP-ASHS21/csonto/CHG-TPM-05.7-BreakClauses
:CHG-TPM-05.7-BreakClauses rdf:type owl:NamedIndividual ,
                                    :Change_Management_Policies ;
                           :HasWeight 9 ;
                           rdfs:comment "Mechanisms exist to include \"break clauses\" within contracts for failure to meet contract criteria for cybersecurity and/or data privacy controls." .


###  http://FYP-ASHS21/csonto/CHG-TPM-06-Third-PartyPersonnelSecurity
:CHG-TPM-06-Third-PartyPersonnelSecurity rdf:type owl:NamedIndividual ,
                                                  :Change_Management_Policies ;
                                         :HasWeight 9 ;
                                         rdfs:comment "Mechanisms exist to control personnel security requirements including security roles and responsibilities for third-party providers." .


###  http://FYP-ASHS21/csonto/CHG-TPM-07-MonitoringforThird-PartyInformationDisclosure
:CHG-TPM-07-MonitoringforThird-PartyInformationDisclosure rdf:type owl:NamedIndividual ,
                                                                   :Change_Management_Policies ;
                                                          :HasWeight 8 ;
                                                          rdfs:comment "Mechanisms exist to monitor for evidence of unauthorized exfiltration or disclosure of organizational information. " .


###  http://FYP-ASHS21/csonto/CHG-TPM-08-ReviewofThird-PartyServices
:CHG-TPM-08-ReviewofThird-PartyServices rdf:type owl:NamedIndividual ,
                                                 :Change_Management_Policies ;
                                        :HasWeight 9 ;
                                        rdfs:comment "Mechanisms exist to monitor, regularly review and audit External Service Providers (ESPs) for compliance with established contractual requirements for cybersecurity & data privacy controls. " .


###  http://FYP-ASHS21/csonto/CHG-TPM-09-Third-PartyDeficiencyRemediation
:CHG-TPM-09-Third-PartyDeficiencyRemediation rdf:type owl:NamedIndividual ,
                                                      :Change_Management_Policies ;
                                             :HasWeight 9 ;
                                             rdfs:comment "Mechanisms exist to address weaknesses or deficiencies in supply chain elements identified during independent or organizational assessments of such elements. " .


###  http://FYP-ASHS21/csonto/CHG-TPM-10-ManagingChangesToThird-PartyServices
:CHG-TPM-10-ManagingChangesToThird-PartyServices rdf:type owl:NamedIndividual ,
                                                          :Change_Management_Policies ;
                                                 :HasWeight 8 ;
                                                 rdfs:comment "Mechanisms exist to control changes to services by suppliers, taking into account the criticality of business information, systems and processes that are in scope by the third-party." .


###  http://FYP-ASHS21/csonto/GOV-01.2-StatusReportingToGoverningBody
:GOV-01.2-StatusReportingToGoverningBody rdf:type owl:NamedIndividual ,
                                                  :Governance_Policies ;
                                         :HasWeight 5 ;
                                         rdfs:comment "Mechanisms exist to provide governance oversight reporting and recommendations to those entrusted to make executive decisions about matters considered material to the organizations cybersecurity & data protection program." .


###  http://FYP-ASHS21/csonto/GOV-02.1-ExceptionManagement
:GOV-02.1-ExceptionManagement rdf:type owl:NamedIndividual ,
                                       :Governance_Policies ;
                              :HasWeight 8 ;
                              rdfs:comment "Mechanisms exist to prohibit exceptions to standards, except when the exception has been formally assessed for risk impact, approved and recorded." .


###  http://FYP-ASHS21/csonto/GOV-04.1-StakeholderAccountabilityStructure
:GOV-04.1-StakeholderAccountabilityStructure rdf:type owl:NamedIndividual ,
                                                      :Governance_Policies ;
                                             :HasWeight 8 ;
                                             rdfs:comment "Mechanisms exist to enforce an accountability structure so that appropriate teams and individuals are empowered, responsible and trained for mapping, measuring and managing data and technology-related risks." .


###  http://FYP-ASHS21/csonto/GOV-04.2-AuthoritativeChainofCommand
:GOV-04.2-AuthoritativeChainofCommand rdf:type owl:NamedIndividual ,
                                               :Governance_Policies ;
                                      :HasWeight 7 ;
                                      rdfs:comment "Mechanisms exist to establish an authoritative chain of command with clear lines of communication to remove ambiguity from individuals and teams related to managing data and technology-related risks." .


###  http://FYP-ASHS21/csonto/GOV-05-MeasuresofPerformance
:GOV-05-MeasuresofPerformance rdf:type owl:NamedIndividual ,
                                       :Governance_Policies ;
                              :HasWeight 6 ;
                              rdfs:comment "Mechanisms exist to develop, report and monitor cybersecurity & data privacy program measures of performance." .


###  http://FYP-ASHS21/csonto/GOV-05.1-KeyPerformanceIndicators-KPIs-
:GOV-05.1-KeyPerformanceIndicators-KPIs- rdf:type owl:NamedIndividual ,
                                                  :Governance_Policies ;
                                         :HasWeight 6 ;
                                         rdfs:comment "Mechanisms exist to develop, report and monitor Key Performance Indicators (KPIs) to assist organizational management in performance monitoring and trend analysis of the cybersecurity & data privacy program." .


###  http://FYP-ASHS21/csonto/GOV-05.2-KeyRiskIndicators-KRIs-
:GOV-05.2-KeyRiskIndicators-KRIs- rdf:type owl:NamedIndividual ,
                                           :Governance_Policies ;
                                  :HasWeight 6 ;
                                  rdfs:comment "Mechanisms exist to develop, report and monitor Key Risk Indicators (KRIs) to assist senior management in performance monitoring and trend analysis of the cybersecurity & data privacy program." .


###  http://FYP-ASHS21/csonto/GOV-06-ContactsWithAuthorities
:GOV-06-ContactsWithAuthorities rdf:type owl:NamedIndividual ,
                                         :Governance_Policies ;
                                :HasWeight 5 ;
                                rdfs:comment "Mechanisms exist to identify and document appropriate contacts with relevant law enforcement and regulatory bodies." .


###  http://FYP-ASHS21/csonto/GOV-09-DefineControlObjectives
:GOV-09-DefineControlObjectives rdf:type owl:NamedIndividual ,
                                         :Governance_Policies ;
                                :HasWeight 5 ;
                                rdfs:comment "Mechanisms exist to establish control objectives as the basis for the selection, implementation and management of the organizations internal control system." .


###  http://FYP-ASHS21/csonto/GOV-10-DataGovernance
:GOV-10-DataGovernance rdf:type owl:NamedIndividual ,
                                :Governance_Policies ;
                       :HasWeight 9 ;
                       rdfs:comment "Mechanisms exist to facilitate data governance to oversee the organization's policies, standards and procedures so that sensitive/regulated data is effectively managed and maintained in accordance with applicable statutory, regulatory and contractual obligations." .


###  http://FYP-ASHS21/csonto/GOV-11-PurposeValidation
:GOV-11-PurposeValidation rdf:type owl:NamedIndividual ,
                                   :Governance_Policies ;
                          :HasWeight 5 ;
                          rdfs:comment "Mechanisms exist to monitor mission/business-critical services or functions to ensure those resources are being used consistent with their intended purpose." .


###  http://FYP-ASHS21/csonto/GOV-12-ForcedTechnologyTransfer-FTT-
:GOV-12-ForcedTechnologyTransfer-FTT- rdf:type owl:NamedIndividual ,
                                               :Governance_Policies ;
                                      :HasWeight 10 ;
                                      rdfs:comment "Mechanisms exist to avoid and/or constrain the forced exfiltration of sensitive / regulated information (e.g., Intellectual Property (IP)) to the host government for purposes of market access or market management practices." .


###  http://FYP-ASHS21/csonto/GOV-13-State-SponsoredEspionage
:GOV-13-State-SponsoredEspionage rdf:type owl:NamedIndividual ,
                                          :Governance_Policies ;
                                 :HasWeight 10 ;
                                 rdfs:comment "Mechanisms exist to constrain the host government's ability to leverage the organization's technology assets for economic or political espionage and/or cyberwarfare activities. " .


###  http://FYP-ASHS21/csonto/GOV-14-BusinessAsUsual-BAU-SecurePractices
:GOV-14-BusinessAsUsual-BAU-SecurePractices rdf:type owl:NamedIndividual ,
                                                     :Governance_Policies ;
                                            :HasWeight 6 ;
                                            rdfs:comment "Mechanisms exist to incorporate cybersecurity & data privacy principles into Business As Usual (BAU) practices through executive leadership involvement." .


###  http://FYP-ASHS21/csonto/GOV-15.1-SelectControls
:GOV-15.1-SelectControls rdf:type owl:NamedIndividual ,
                                  :Governance_Policies ;
                         :HasWeight 8 ;
                         rdfs:comment "Mechanisms exist to compel data and/or process owners to select required cybersecurity & data privacy controls for each system, application and/or service under their control." .


###  http://FYP-ASHS21/csonto/GOV-15.2-ImplementControls
:GOV-15.2-ImplementControls rdf:type owl:NamedIndividual ,
                                     :Governance_Policies ;
                            :HasWeight 9 ;
                            rdfs:comment "Mechanisms exist to compel data and/or process owners to implement required cybersecurity & data privacy controls for each system, application and/or service under their control." .


###  http://FYP-ASHS21/csonto/GOV-15.3-AssessControls
:GOV-15.3-AssessControls rdf:type owl:NamedIndividual ,
                                  :Governance_Policies ;
                         :HasWeight 8 ;
                         rdfs:comment "Mechanisms exist to compel data and/or process owners to assess if required cybersecurity & data privacy controls for each system, application and/or service under their control are implemented correctly and are operating as intended." .


###  http://FYP-ASHS21/csonto/GOV-15.5-MonitorControls
:GOV-15.5-MonitorControls rdf:type owl:NamedIndividual ,
                                   :Governance_Policies ;
                          :HasWeight 8 ;
                          rdfs:comment "Mechanisms exist to compel data and/or process owners to monitor systems, applications and/or services under their control on an ongoing basis for applicable threats and risks, as well as to ensure cybersecurity & data privacy controls are operating as intended." .


###  http://FYP-ASHS21/csonto/GOV-PRM-01.2-TargetedCapabilityMaturityLevels
:GOV-PRM-01.2-TargetedCapabilityMaturityLevels rdf:type owl:NamedIndividual ,
                                                        :Governance_Policies ;
                                               :HasWeight 5 ;
                                               rdfs:comment "Mechanisms exist to define and identify targeted capability maturity levels." .


###  http://FYP-ASHS21/csonto/GOV-PRM-03-AllocationofResources
:GOV-PRM-03-AllocationofResources rdf:type owl:NamedIndividual ,
                                           :Governance_Policies ;
                                  :HasWeight 8 ;
                                  rdfs:comment "Mechanisms exist to identify and allocate resources for management, operational, technical and data privacy requirements within business process planning for projects / initiatives." .


###  http://FYP-ASHS21/csonto/GOV-PRM-06-BusinessProcessDefinition
:GOV-PRM-06-BusinessProcessDefinition rdf:type owl:NamedIndividual ,
                                               :Governance_Policies ;
                                      :HasWeight 7 ;
                                      rdfs:comment """Mechanisms exist to define business processes with consideration for cybersecurity & data privacy that determines: 
  The resulting risk to organizational operations, assets, individuals and other organizations; and
  Information protection needs arising from the defined business processes and revises the processes as necessary, until an achievable set of protection needs is obtained.""" .


###  http://FYP-ASHS21/csonto/GOV-PRM-07-SecureDevelopmentLifeCycle-SDLC-Management
:GOV-PRM-07-SecureDevelopmentLifeCycle-SDLC-Management rdf:type owl:NamedIndividual ,
                                                                :Governance_Policies ;
                                                       :HasWeight 10 ;
                                                       rdfs:comment "Mechanisms exist to ensure changes to systems within the Secure Development Life Cycle (SDLC) are controlled through formal change control procedures. " .


###  http://FYP-ASHS21/csonto/GOV-PRM-08-ManageOrganizationalKnowledge
:GOV-PRM-08-ManageOrganizationalKnowledge rdf:type owl:NamedIndividual ,
                                                   :Governance_Policies ;
                                          :HasWeight 5 ;
                                          rdfs:comment "Mechanisms exist to manage the organizational knowledge of the cybersecurity & data privacy staff." .


###  http://FYP-ASHS21/csonto/IAO-01-InformationAssurance-IA-Operations
:IAO-01-InformationAssurance-IA-Operations rdf:type owl:NamedIndividual ,
                                                    :Assurance_Policies ;
                                           :HasWeight 10 ;
                                           rdfs:comment "Mechanisms exist to facilitate the implementation of cybersecurity & data privacy assessment and authorization controls. " .


###  http://FYP-ASHS21/csonto/IAO-01.1-AssessmentBoundaries
:IAO-01.1-AssessmentBoundaries rdf:type owl:NamedIndividual ,
                                        :Assurance_Policies ;
                               :HasWeight 9 ;
                               rdfs:comment "Mechanisms exist to establish the scope of assessments by defining the assessment boundary, according to people, processes and technology that directly or indirectly impact the confidentiality, integrity, availability and safety of the data and systems under review." .


###  http://FYP-ASHS21/csonto/IAO-02-Assessments
:IAO-02-Assessments rdf:type owl:NamedIndividual ,
                             :Assurance_Policies ;
                    :HasWeight 10 ;
                    rdfs:comment "Mechanisms exist to formally assess the cybersecurity & data privacy controls in systems, applications and services through Information Assurance Program (IAP) activities to determine the extent to which the controls are implemented correctly, operating as intended and producing the desired outcome with respect to meeting expected requirements." .


###  http://FYP-ASHS21/csonto/IAO-02.1-AssessorIndependence
:IAO-02.1-AssessorIndependence rdf:type owl:NamedIndividual ,
                                        :Assurance_Policies ;
                               :HasWeight 9 ;
                               rdfs:comment "Mechanisms exist to ensure assessors or assessment teams have the appropriate independence to conduct cybersecurity & data privacy control assessments. " .


###  http://FYP-ASHS21/csonto/IAO-02.2-SpecializedAssessments
:IAO-02.2-SpecializedAssessments rdf:type owl:NamedIndividual ,
                                          :Assurance_Policies ;
                                 :HasWeight 9 ;
                                 rdfs:comment """Mechanisms exist to conduct specialized assessments for: 
  Statutory, regulatory and contractual compliance obligations;
  Monitoring capabilities; 
  Mobile devices;
  Databases;
  Application security;
  Embedded technologies (e.g., IoT, OT, etc.);
  Vulnerability management; 
  Malicious code; 
  Insider threats and
  Performance/load testing. """ .


###  http://FYP-ASHS21/csonto/IAO-02.3-Third-PartyAssessments
:IAO-02.3-Third-PartyAssessments rdf:type owl:NamedIndividual ,
                                          :Assurance_Policies ;
                                 :HasWeight 9 ;
                                 rdfs:comment "Mechanisms exist to accept and respond to the results of external assessments that are performed by impartial, external organizations. " .


###  http://FYP-ASHS21/csonto/IAO-02.4-SecurityAssessmentReport-SAR-
:IAO-02.4-SecurityAssessmentReport-SAR- rdf:type owl:NamedIndividual ,
                                                 :Assurance_Policies ;
                                        :HasWeight 7 ;
                                        rdfs:comment "Mechanisms exist to produce a Security Assessment Report (SAR) at the conclusion of a security assessment to certify the results of the assessment and assist with any remediation actions." .


###  http://FYP-ASHS21/csonto/IAO-03.1-Plan-CoordinatewithOtherOrganizationalEntities
:IAO-03.1-Plan-CoordinatewithOtherOrganizationalEntities rdf:type owl:NamedIndividual ,
                                                                  :Assurance_Policies ;
                                                         :HasWeight 5 ;
                                                         rdfs:comment "Mechanisms exist to plan and coordinate Information Assurance Program (IAP) activities with affected stakeholders before conducting such activities in order to reduce the potential impact on operations. " .


###  http://FYP-ASHS21/csonto/IAO-03.2-AdequateSecurityforSensitive-RegulatedDataInSupportofContracts
:IAO-03.2-AdequateSecurityforSensitive-RegulatedDataInSupportofContracts rdf:type owl:NamedIndividual ,
                                                                                  :Assurance_Policies ;
                                                                         :HasWeight 7 ;
                                                                         rdfs:comment "Mechanisms exist to protect sensitive / regulated data that is collected, developed, received, transmitted, used or stored in support of the performance of a contract. " .


###  http://FYP-ASHS21/csonto/IAO-06-TechnicalVerification
:IAO-06-TechnicalVerification rdf:type owl:NamedIndividual ,
                                       :Assurance_Policies ;
                              :HasWeight 8 ;
                              rdfs:comment "Mechanisms exist to perform Information Assurance Program (IAP) activities to evaluate the design, implementation and effectiveness of technical cybersecurity & data privacy controls." .


###  http://FYP-ASHS21/csonto/IAO-07-SecurityAuthorization
:IAO-07-SecurityAuthorization rdf:type owl:NamedIndividual ,
                                       :Assurance_Policies ;
                              :HasWeight 10 ;
                              rdfs:comment "Mechanisms exist to ensure systems, projects and services are officially authorized prior to \"go live\" in a production environment." .


###  http://FYP-ASHS21/csonto/IAO-CPL-01.1-Non-ComplianceOversight
:IAO-CPL-01.1-Non-ComplianceOversight rdf:type owl:NamedIndividual ,
                                               :Assurance_Policies ;
                                      :HasWeight 9 ;
                                      rdfs:comment "Mechanisms exist to document and review instances of non-compliance with statutory, regulatory and/or contractual obligations to develop appropriate risk mitigation actions." .


###  http://FYP-ASHS21/csonto/IAO-CPL-01.2-ComplianceScope
:IAO-CPL-01.2-ComplianceScope rdf:type owl:NamedIndividual ,
                                       :Assurance_Policies ;
                              :HasWeight 10 ;
                              rdfs:comment "Mechanisms exist to document and validate the scope of cybersecurity & data privacy controls that are determined to meet statutory, regulatory and/or contractual compliance obligations." .


###  http://FYP-ASHS21/csonto/IAO-CPL-02.1-InternalAuditFunction
:IAO-CPL-02.1-InternalAuditFunction rdf:type owl:NamedIndividual ,
                                             :Assurance_Policies ;
                                    :HasWeight 5 ;
                                    rdfs:comment "Mechanisms exist to implement an internal audit function that is capable of providing senior organization management with insights into the appropriateness of the organization's technology and information governance processes." .


###  http://FYP-ASHS21/csonto/IAO-CPL-03.1-IndependentAssessors
:IAO-CPL-03.1-IndependentAssessors rdf:type owl:NamedIndividual ,
                                            :Assurance_Policies ;
                                   :HasWeight 6 ;
                                   rdfs:comment "Mechanisms exist to utilize independent assessors to evaluate cybersecurity & data privacy controls at planned intervals or when the system, service or project undergoes significant changes." .


###  http://FYP-ASHS21/csonto/IAO-CPL-04-AuditActivities
:IAO-CPL-04-AuditActivities rdf:type owl:NamedIndividual ,
                                     :Assurance_Policies ;
                            :HasWeight 5 ;
                            rdfs:comment "Mechanisms exist to thoughtfully plan audits by including input from operational risk and compliance partners to minimize the impact of audit-related activities on business operations." .


###  http://FYP-ASHS21/csonto/IAO-CPL-05-LegalAssessmentofInvestigativeInquires
:IAO-CPL-05-LegalAssessmentofInvestigativeInquires rdf:type owl:NamedIndividual ,
                                                            :Assurance_Policies ;
                                                   :HasWeight 2 ;
                                                   rdfs:comment "Mechanisms exist to determine whether a government agency has an applicable and valid legal basis to request data from the organization and what further steps need to be taken, if necessary." .


###  http://FYP-ASHS21/csonto/IAO-CPL-05.1-InvestigationRequestNotifications
:IAO-CPL-05.1-InvestigationRequestNotifications rdf:type owl:NamedIndividual ,
                                                         :Assurance_Policies ;
                                                :HasWeight 2 ;
                                                rdfs:comment "Mechanisms exist to notify customers about investigation request notifications, unless the applicable legal basis for a government agency's action prohibits notification (e.g., potential criminal prosecution)." .


###  http://FYP-ASHS21/csonto/IAO-CPL-05.2-InvestigationAccessRestrictions
:IAO-CPL-05.2-InvestigationAccessRestrictions rdf:type owl:NamedIndividual ,
                                                       :Assurance_Policies ;
                                              :HasWeight 2 ;
                                              rdfs:comment "Mechanisms exist to support official investigations by provisioning government investigators with \"least privileges\" and \"least functionality\" to ensure that government investigators only have access to the data and systems needed to perform the investigation." .


###  http://FYP-ASHS21/csonto/IAO-CPL-06-GovernmentSurveillance
:IAO-CPL-06-GovernmentSurveillance rdf:type owl:NamedIndividual ,
                                            :Assurance_Policies ;
                                   :HasWeight 10 ;
                                   rdfs:comment "Mechanisms exist to constrain the host government from having unrestricted and non-monitored access to the organization's systems, applications and services that could potentially violate other applicable statutory, regulatory and/or contractual obligations." .


###  http://FYP-ASHS21/csonto/IAO-SAT-02.1-SimulatedCyberAttackScenarioTraining
:IAO-SAT-02.1-SimulatedCyberAttackScenarioTraining rdf:type owl:NamedIndividual ,
                                                            :Assurance_Policies ;
                                                   :HasWeight 3 ;
                                                   rdfs:comment "Mechanisms exist to include simulated actual cyber-attacks through practical exercises that are aligned with current threat scenarios." .


###  http://FYP-ASHS21/csonto/IAO-SAT-03.1-PracticalExercises
:IAO-SAT-03.1-PracticalExercises rdf:type owl:NamedIndividual ,
                                          :Assurance_Policies ;
                                 :HasWeight 3 ;
                                 rdfs:comment "Mechanisms exist to include practical exercises in cybersecurity & data privacy training that reinforce training objectives." .


###  http://FYP-ASHS21/csonto/IAO-SAT-03.5-PrivilegedUsers
:IAO-SAT-03.5-PrivilegedUsers rdf:type owl:NamedIndividual ,
                                       :Assurance_Policies ;
                              :HasWeight 9 ;
                              rdfs:comment "Mechanisms exist to provide specific training for privileged users to ensure privileged users understand their unique roles and responsibilities " .


###  http://FYP-ASHS21/csonto/IAO-SAT-03.6-CyberThreatEnvironment
:IAO-SAT-03.6-CyberThreatEnvironment rdf:type owl:NamedIndividual ,
                                              :Assurance_Policies ;
                                     :HasWeight 8 ;
                                     rdfs:comment "Mechanisms exist to provide role-based cybersecurity & data privacy awareness training that is specific to the cyber threats that the user might encounter the user's specific day-to-day business operations." .


###  http://FYP-ASHS21/csonto/IAO-SAT-03.8-ContinuingProfessionalEducation-CPE--DevOpsPersonnel
:IAO-SAT-03.8-ContinuingProfessionalEducation-CPE--DevOpsPersonnel rdf:type owl:NamedIndividual ,
                                                                            :Assurance_Policies ;
                                                                   :HasWeight 8 ;
                                                                   rdfs:comment "Mechanisms exist to ensure application development and operations (DevOps) personnel receive Continuing Professional Education (CPE) training on Secure Software Development Practices (SSDP) to appropriately address evolving threats." .


###  http://FYP-ASHS21/csonto/OPS-BCD-01-BusinessContinuityManagementSystem-BCMS-
:OPS-BCD-01-BusinessContinuityManagementSystem-BCMS- rdf:type owl:NamedIndividual ,
                                                              :Security_Operations_Policies ;
                                                     :HasWeight 10 ;
                                                     rdfs:comment "Mechanisms exist to facilitate the implementation of contingency planning controls to help ensure resilient assets and services (e.g., Continuity of Operations Plan (COOP) or Business Continuity & Disaster Recovery (BC/DR) playbooks)." .


###  http://FYP-ASHS21/csonto/OPS-BCD-01.1-CoordinatewithRelatedPlans
:OPS-BCD-01.1-CoordinatewithRelatedPlans rdf:type owl:NamedIndividual ,
                                                  :Security_Operations_Policies ;
                                         :HasWeight 5 ;
                                         rdfs:comment "Mechanisms exist to coordinate contingency plan development with internal and external elements responsible for related plans. " .


###  http://FYP-ASHS21/csonto/OPS-BCD-01.2-CoordinateWithExternalServiceProviders
:OPS-BCD-01.2-CoordinateWithExternalServiceProviders rdf:type owl:NamedIndividual ,
                                                              :Security_Operations_Policies ;
                                                     :HasWeight 5 ;
                                                     rdfs:comment "Mechanisms exist to coordinate internal contingency plans with the contingency plans of external service providers to ensure that contingency requirements can be satisfied." .


###  http://FYP-ASHS21/csonto/OPS-BCD-01.3-TransfertoAlternateProcessing-StorageSite
:OPS-BCD-01.3-TransfertoAlternateProcessing-StorageSite rdf:type owl:NamedIndividual ,
                                                                 :Security_Operations_Policies ;
                                                        :HasWeight 5 ;
                                                        rdfs:comment "Mechanisms exist to redeploy personnel to other roles during a disruptive event or in the execution of a continuity plan." .


###  http://FYP-ASHS21/csonto/OPS-BCD-01.4-RecoveryTime-PointObjectives-RTO-RPO-
:OPS-BCD-01.4-RecoveryTime-PointObjectives-RTO-RPO- rdf:type owl:NamedIndividual ,
                                                             :Security_Operations_Policies ;
                                                    :HasWeight 5 ;
                                                    rdfs:comment "Mechanisms exist to facilitate recovery operations in accordance with Recovery Time Objectives (RTOs) and Recovery Point Objectives (RPOs)." .


###  http://FYP-ASHS21/csonto/OPS-BCD-02-IdentifyCriticalAssets
:OPS-BCD-02-IdentifyCriticalAssets rdf:type owl:NamedIndividual ,
                                            :Security_Operations_Policies ;
                                   :HasWeight 9 ;
                                   rdfs:comment "Mechanisms exist to identify and document the critical systems, applications and services that support essential missions and business functions." .


###  http://FYP-ASHS21/csonto/OPS-BCD-02.4-DataStorageLocationReviews
:OPS-BCD-02.4-DataStorageLocationReviews rdf:type owl:NamedIndividual ,
                                                  :Security_Operations_Policies ;
                                         :HasWeight 8 ;
                                         rdfs:comment "Mechanisms exist to perform periodic security reviews of storage locations that contain sensitive / regulated data." .


###  http://FYP-ASHS21/csonto/OPS-BCD-03-ContingencyTraining
:OPS-BCD-03-ContingencyTraining rdf:type owl:NamedIndividual ,
                                         :Security_Operations_Policies ;
                                :HasWeight 5 ;
                                rdfs:comment "Mechanisms exist to adequately train contingency personnel and applicable stakeholders in their contingency roles and responsibilities. " .


###  http://FYP-ASHS21/csonto/OPS-BCD-03.1-SimulatedEvents
:OPS-BCD-03.1-SimulatedEvents rdf:type owl:NamedIndividual ,
                                       :Security_Operations_Policies ;
                              :HasWeight 3 ;
                              rdfs:comment "Mechanisms exist to incorporate simulated events into contingency training to facilitate effective response by personnel in crisis situations." .


###  http://FYP-ASHS21/csonto/OPS-BCD-03.2-AutomatedTrainingEnvironments
:OPS-BCD-03.2-AutomatedTrainingEnvironments rdf:type owl:NamedIndividual ,
                                                     :Security_Operations_Policies ;
                                            :HasWeight 1 ;
                                            rdfs:comment "Automated mechanisms exist to provide a more thorough and realistic contingency training environment." .


###  http://FYP-ASHS21/csonto/OPS-BCD-04.1-CoordinatedTestingwithRelatedPlans
:OPS-BCD-04.1-CoordinatedTestingwithRelatedPlans rdf:type owl:NamedIndividual ,
                                                          :Security_Operations_Policies ;
                                                 :HasWeight 3 ;
                                                 rdfs:comment "Mechanisms exist to coordinate contingency plan testing with internal and external elements responsible for related plans. " .


###  http://FYP-ASHS21/csonto/OPS-BCD-07-AlternativeSecurityMeasures
:OPS-BCD-07-AlternativeSecurityMeasures rdf:type owl:NamedIndividual ,
                                                 :Security_Operations_Policies ;
                                        :HasWeight 9 ;
                                        rdfs:comment "Mechanisms exist to implement alternative or compensating controls to satisfy security functions when the primary means of implementing the security function is unavailable or compromised. " .


###  http://FYP-ASHS21/csonto/OPS-BCD-08-AlternateStorageSite
:OPS-BCD-08-AlternateStorageSite rdf:type owl:NamedIndividual ,
                                          :Security_Operations_Policies ;
                                 :HasWeight 9 ;
                                 rdfs:comment "Mechanisms exist to establish an alternate storage site that includes both the assets and necessary agreements to permit the storage and recovery of system backup information. " .


###  http://FYP-ASHS21/csonto/OPS-BCD-08.1-SeparationfromPrimarySite
:OPS-BCD-08.1-SeparationfromPrimarySite rdf:type owl:NamedIndividual ,
                                                 :Security_Operations_Policies ;
                                        :HasWeight 7 ;
                                        rdfs:comment "Mechanisms exist to separate the alternate storage site from the primary storage site to reduce susceptibility to similar threats." .


###  http://FYP-ASHS21/csonto/OPS-BCD-08.2-Accessibility
:OPS-BCD-08.2-Accessibility rdf:type owl:NamedIndividual ,
                                     :Security_Operations_Policies ;
                            :HasWeight 5 ;
                            rdfs:comment "Mechanisms exist to identify and mitigate potential accessibility problems to the alternate storage site in the event of an area-wide disruption or disaster." .


###  http://FYP-ASHS21/csonto/OPS-BCD-09-AlternateProcessingSite
:OPS-BCD-09-AlternateProcessingSite rdf:type owl:NamedIndividual ,
                                             :Security_Operations_Policies ;
                                    :HasWeight 9 ;
                                    rdfs:comment "Mechanisms exist to establish an alternate processing site that provides security measures equivalent to that of the primary site." .


###  http://FYP-ASHS21/csonto/OPS-BCD-09.1-SeparationfromPrimarySite
:OPS-BCD-09.1-SeparationfromPrimarySite rdf:type owl:NamedIndividual ,
                                                 :Security_Operations_Policies ;
                                        :HasWeight 7 ;
                                        rdfs:comment "Mechanisms exist to separate the alternate processing site from the primary processing site to reduce susceptibility to similar threats." .


###  http://FYP-ASHS21/csonto/OPS-BCD-09.2-Accessibility
:OPS-BCD-09.2-Accessibility rdf:type owl:NamedIndividual ,
                                     :Security_Operations_Policies ;
                            :HasWeight 5 ;
                            rdfs:comment "Mechanisms exist to identify and mitigate potential accessibility problems to the alternate processing site and possible mitigation actions, in the event of an area-wide disruption or disaster." .


###  http://FYP-ASHS21/csonto/OPS-BCD-09.3-AlternateSitePriorityofService
:OPS-BCD-09.3-AlternateSitePriorityofService rdf:type owl:NamedIndividual ,
                                                      :Security_Operations_Policies ;
                                             :HasWeight 6 ;
                                             rdfs:comment "Mechanisms exist to address priority-of-service provisions in alternate processing and storage sites that support availability requirements, including Recovery Time Objectives (RTOs). " .


###  http://FYP-ASHS21/csonto/OPS-BCD-09.4-PreparationforUse
:OPS-BCD-09.4-PreparationforUse rdf:type owl:NamedIndividual ,
                                         :Security_Operations_Policies ;
                                :HasWeight 5 ;
                                rdfs:comment "Mechanisms exist to prepare the alternate processing alternate to support essential missions and business functions so that the alternate site is capable of being used as the primary site." .


###  http://FYP-ASHS21/csonto/OPS-BCD-09.5-InabilitytoReturntoPrimarySite
:OPS-BCD-09.5-InabilitytoReturntoPrimarySite rdf:type owl:NamedIndividual ,
                                                      :Security_Operations_Policies ;
                                             :HasWeight 5 ;
                                             rdfs:comment "Mechanisms exist to plan and prepare for both natural and manmade circumstances that preclude returning to the primary processing site." .


###  http://FYP-ASHS21/csonto/OPS-BCD-10-TelecommunicationsServicesAvailability
:OPS-BCD-10-TelecommunicationsServicesAvailability rdf:type owl:NamedIndividual ,
                                                            :Security_Operations_Policies ;
                                                   :HasWeight 6 ;
                                                   rdfs:comment "Mechanisms exist to reduce the likelihood of a single point of failure with primary telecommunications services." .


###  http://FYP-ASHS21/csonto/OPS-BCD-10.1-TelecommunicationsPriorityofServiceProvisions
:OPS-BCD-10.1-TelecommunicationsPriorityofServiceProvisions rdf:type owl:NamedIndividual ,
                                                                     :Security_Operations_Policies ;
                                                            :HasWeight 6 ;
                                                            rdfs:comment "Mechanisms exist to formalize primary and alternate telecommunications service agreements contain priority-of-service provisions that support availability requirements, including Recovery Time Objectives (RTOs). " .


###  http://FYP-ASHS21/csonto/OPS-BCD-10.2-SeparationofPrimary-AlternateProviders
:OPS-BCD-10.2-SeparationofPrimary-AlternateProviders rdf:type owl:NamedIndividual ,
                                                              :Security_Operations_Policies ;
                                                     :HasWeight 5 ;
                                                     rdfs:comment "Mechanisms exist to obtain alternate telecommunications services from providers that are separated from primary service providers to reduce susceptibility to the same threats. " .


###  http://FYP-ASHS21/csonto/OPS-BCD-10.3-ProviderContinencyPlan
:OPS-BCD-10.3-ProviderContinencyPlan rdf:type owl:NamedIndividual ,
                                              :Security_Operations_Policies ;
                                     :HasWeight 5 ;
                                     rdfs:comment "Mechanisms exist to contractually-require external service providers to have contingency plans that meet organizational contingency requirements." .


###  http://FYP-ASHS21/csonto/OPS-BCD-10.4-AlternateCommunicationsPaths
:OPS-BCD-10.4-AlternateCommunicationsPaths rdf:type owl:NamedIndividual ,
                                                    :Security_Operations_Policies ;
                                           :HasWeight 5 ;
                                           rdfs:comment "Mechanisms exist to maintain command and control capabilities via alternate communications channels and designating alternative decision makers if primary decision makers are unavailable." .


###  http://FYP-ASHS21/csonto/OPS-BCD-11-DataBackups
:OPS-BCD-11-DataBackups rdf:type owl:NamedIndividual ,
                                 :Security_Operations_Policies ;
                        :HasWeight 10 ;
                        rdfs:comment "Mechanisms exist to create recurring backups of data, software and/or system images, as well as verify the integrity of these backups, to ensure the availability of the data to satisfying Recovery Time Objectives (RTOs) and Recovery Point Objectives (RPOs)." .


###  http://FYP-ASHS21/csonto/OPS-BCD-11.10-BackupModificationand-orDestruction
:OPS-BCD-11.10-BackupModificationand-orDestruction rdf:type owl:NamedIndividual ,
                                                            :Security_Operations_Policies ;
                                                   :HasWeight 9 ;
                                                   rdfs:comment "Mechanisms exist to restrict access to modify and/or delete backups to privileged users with assigned data backup and recovery operations roles." .


###  http://FYP-ASHS21/csonto/OPS-BCD-11.2-SeparateStorageforCriticalInformation
:OPS-BCD-11.2-SeparateStorageforCriticalInformation rdf:type owl:NamedIndividual ,
                                                             :Security_Operations_Policies ;
                                                    :HasWeight 8 ;
                                                    rdfs:comment "Mechanisms exist to store backup copies of critical software and other security-related information in a separate facility or in a fire-rated container that is not collocated with the system being backed up." .


###  http://FYP-ASHS21/csonto/OPS-BCD-11.3-InformationSystemImaging
:OPS-BCD-11.3-InformationSystemImaging rdf:type owl:NamedIndividual ,
                                                :Security_Operations_Policies ;
                                       :HasWeight 8 ;
                                       rdfs:comment "Mechanisms exist to reimage assets from configuration-controlled and integrity-protected images that represent a secure, operational state." .


###  http://FYP-ASHS21/csonto/OPS-BCD-11.4-CryptographicProtection
:OPS-BCD-11.4-CryptographicProtection rdf:type owl:NamedIndividual ,
                                               :Security_Operations_Policies ;
                                      :HasWeight 9 ;
                                      rdfs:comment "Cryptographic mechanisms exist to prevent the unauthorized disclosure and/or modification of backup information." .


###  http://FYP-ASHS21/csonto/OPS-BCD-11.5-TestRestorationUsingSampling
:OPS-BCD-11.5-TestRestorationUsingSampling rdf:type owl:NamedIndividual ,
                                                    :Security_Operations_Policies ;
                                           :HasWeight 5 ;
                                           rdfs:comment "Mechanisms exist to utilize sampling of available backups to test recovery capabilities as part of business continuity plan testing. " .


###  http://FYP-ASHS21/csonto/OPS-BCD-11.6-TransfertoAlternateStorageSite
:OPS-BCD-11.6-TransfertoAlternateStorageSite rdf:type owl:NamedIndividual ,
                                                      :Security_Operations_Policies ;
                                             :HasWeight 5 ;
                                             rdfs:comment "Mechanisms exist to transfer backup data to the alternate storage site at a rate that is capable of meeting both Recovery Time Objectives (RTOs) and Recovery Point Objectives (RPOs)." .


###  http://FYP-ASHS21/csonto/OPS-BCD-11.7-RedundantSecondarySystem
:OPS-BCD-11.7-RedundantSecondarySystem rdf:type owl:NamedIndividual ,
                                                :Security_Operations_Policies ;
                                       :HasWeight 5 ;
                                       rdfs:comment "Mechanisms exist to maintain a failover system, that is not collocated with the primary system, application and/or service, which can be activated with little-to-no loss of information or disruption to operations." .


###  http://FYP-ASHS21/csonto/OPS-BCD-11.8-DualAuthorizationForBackupMediaDestruction
:OPS-BCD-11.8-DualAuthorizationForBackupMediaDestruction rdf:type owl:NamedIndividual ,
                                                                  :Security_Operations_Policies ;
                                                         :HasWeight 5 ;
                                                         rdfs:comment "Mechanisms exist to implement and enforce dual authorization for the deletion or destruction of sensitive backup media and data." .


###  http://FYP-ASHS21/csonto/OPS-BCD-11.9-BackupAccess
:OPS-BCD-11.9-BackupAccess rdf:type owl:NamedIndividual ,
                                    :Security_Operations_Policies ;
                           :HasWeight 9 ;
                           rdfs:comment "Mechanisms exist to restrict access to backups to privileged users with assigned roles for data backup and recovery operations." .


###  http://FYP-ASHS21/csonto/OPS-BCD-12.1-TransactionRecovery
:OPS-BCD-12.1-TransactionRecovery rdf:type owl:NamedIndividual ,
                                           :Security_Operations_Policies ;
                                  :HasWeight 9 ;
                                  rdfs:comment "Mechanisms exist to utilize specialized backup mechanisms that will allow transaction recovery for transaction-based applications and services in accordance with Recovery Point Objectives (RPOs)." .


###  http://FYP-ASHS21/csonto/OPS-BCD-12.2-FailoverCapability
:OPS-BCD-12.2-FailoverCapability rdf:type owl:NamedIndividual ,
                                          :Security_Operations_Policies ;
                                 :HasWeight 8 ;
                                 rdfs:comment "Mechanisms exist to implement real-time or near-real-time failover capability to maintain availability of critical systems, applications and/or services." .


###  http://FYP-ASHS21/csonto/OPS-BCD-12.3-ElectronicDiscovery-eDiscovery-
:OPS-BCD-12.3-ElectronicDiscovery-eDiscovery- rdf:type owl:NamedIndividual ,
                                                       :Security_Operations_Policies ;
                                              :HasWeight 8 ;
                                              rdfs:comment "Mechanisms exist to utilize electronic discovery (eDiscovery) that covers current and archived communication transactions." .


###  http://FYP-ASHS21/csonto/OPS-BCD-12.4-RestoreWithinTimePeriod
:OPS-BCD-12.4-RestoreWithinTimePeriod rdf:type owl:NamedIndividual ,
                                               :Security_Operations_Policies ;
                                      :HasWeight 5 ;
                                      rdfs:comment "Mechanisms exist to restore systems, applications and/or services within organization-defined restoration time-periods from configuration-controlled and integrity-protected information; representing a known, operational state for the asset. " .


###  http://FYP-ASHS21/csonto/OPS-BCD-14-IsolatedRecoveryEnvironment
:OPS-BCD-14-IsolatedRecoveryEnvironment rdf:type owl:NamedIndividual ,
                                                 :Security_Operations_Policies ;
                                        :HasWeight 5 ;
                                        rdfs:comment "Mechanisms exist to utilize an isolated, non-production environment to perform data backup and recovery operations through offline, cloud or off-site capabilities." .


###  http://FYP-ASHS21/csonto/OPS-BCD-15-ReserveHardware
:OPS-BCD-15-ReserveHardware rdf:type owl:NamedIndividual ,
                                     :Security_Operations_Policies ;
                            :HasWeight 7 ;
                            rdfs:comment "Mechanisms exist to purchase and maintain a sufficient reserve of spare hardware to ensure essential missions and business functions can be maintained in the event of a supply chain disruption." .


###  http://FYP-ASHS21/csonto/OPS-CRY-01-UseofCryptographicControls
:OPS-CRY-01-UseofCryptographicControls rdf:type owl:NamedIndividual ,
                                                :Security_Operations_Policies ;
                                       :HasWeight 10 ;
                                       rdfs:comment "Mechanisms exist to facilitate the implementation of cryptographic protections controls using known public standards and trusted cryptographic technologies." .


###  http://FYP-ASHS21/csonto/OPS-CRY-01.1-AlternatePhysicalProtection
:OPS-CRY-01.1-AlternatePhysicalProtection rdf:type owl:NamedIndividual ,
                                                   :Security_Operations_Policies ;
                                          :HasWeight 5 ;
                                          rdfs:comment "Cryptographic mechanisms exist to prevent unauthorized disclosure of information as an alternative to physical safeguards. " .


###  http://FYP-ASHS21/csonto/OPS-CRY-01.2-Export-ControlledTechnology
:OPS-CRY-01.2-Export-ControlledTechnology rdf:type owl:NamedIndividual ,
                                                   :Security_Operations_Policies ;
                                          :HasWeight 5 ;
                                          rdfs:comment "Mechanisms exist to address the exporting of cryptographic technologies in compliance with relevant statutory and regulatory requirements." .


###  http://FYP-ASHS21/csonto/OPS-CRY-01.3-Pre-PostTransmissionHandling
:OPS-CRY-01.3-Pre-PostTransmissionHandling rdf:type owl:NamedIndividual ,
                                                    :Security_Operations_Policies ;
                                           :HasWeight 5 ;
                                           rdfs:comment "Cryptographic mechanisms exist to ensure the confidentiality and integrity of information during preparation for transmission and during reception." .


###  http://FYP-ASHS21/csonto/OPS-CRY-01.4-Conceal-RandomizeCommunications
:OPS-CRY-01.4-Conceal-RandomizeCommunications rdf:type owl:NamedIndividual ,
                                                       :Security_Operations_Policies ;
                                              :HasWeight 5 ;
                                              rdfs:comment "Cryptographic mechanisms exist to conceal or randomize communication patterns." .


###  http://FYP-ASHS21/csonto/OPS-CRY-01.5-CryptographicCipherSuitesandProtocolsInventory
:OPS-CRY-01.5-CryptographicCipherSuitesandProtocolsInventory rdf:type owl:NamedIndividual ,
                                                                      :Security_Operations_Policies ;
                                                             :HasWeight 9 ;
                                                             rdfs:comment "Mechanisms exist to identify, document and review deployed cryptographic cipher suites and protocols to proactively respond to industry trends regarding the continued viability of utilized cryptographic cipher suites and protocols." .


###  http://FYP-ASHS21/csonto/OPS-CRY-02-CryptographicModuleAuthentication
:OPS-CRY-02-CryptographicModuleAuthentication rdf:type owl:NamedIndividual ,
                                                       :Security_Operations_Policies ;
                                              :HasWeight 8 ;
                                              rdfs:comment "Automated mechanisms exist to enable systems to authenticate to a cryptographic module." .


###  http://FYP-ASHS21/csonto/OPS-CRY-03-TransmissionConfidentiality
:OPS-CRY-03-TransmissionConfidentiality rdf:type owl:NamedIndividual ,
                                                 :Security_Operations_Policies ;
                                        :HasWeight 10 ;
                                        rdfs:comment "Cryptographic mechanisms exist to protect the confidentiality of data being transmitted. " .


###  http://FYP-ASHS21/csonto/OPS-CRY-04-TransmissionIntegrity
:OPS-CRY-04-TransmissionIntegrity rdf:type owl:NamedIndividual ,
                                           :Security_Operations_Policies ;
                                  :HasWeight 10 ;
                                  rdfs:comment "Cryptographic mechanisms exist to protect the integrity of data being transmitted. " .


###  http://FYP-ASHS21/csonto/OPS-CRY-05-EncryptingDataAtRest
:OPS-CRY-05-EncryptingDataAtRest rdf:type owl:NamedIndividual ,
                                          :Security_Operations_Policies ;
                                 :HasWeight 10 ;
                                 rdfs:comment "Cryptographic mechanisms exist to prevent unauthorized disclosure of data at rest. " .


###  http://FYP-ASHS21/csonto/OPS-CRY-05.1-StorageMedia
:OPS-CRY-05.1-StorageMedia rdf:type owl:NamedIndividual ,
                                    :Security_Operations_Policies ;
                           :HasWeight 8 ;
                           rdfs:comment "Cryptographic mechanisms exist to protect the confidentiality and integrity of sensitive/regulated data residing on storage media." .


###  http://FYP-ASHS21/csonto/OPS-CRY-05.2-OfflineStorage
:OPS-CRY-05.2-OfflineStorage rdf:type owl:NamedIndividual ,
                                      :Security_Operations_Policies ;
                             :HasWeight 5 ;
                             rdfs:comment "Mechanisms exist to remove unused data from online storage and archive it off-line in a secure location until it can be disposed of according to data retention requirements." .


###  http://FYP-ASHS21/csonto/OPS-CRY-05.3-DatabaseEncryption
:OPS-CRY-05.3-DatabaseEncryption rdf:type owl:NamedIndividual ,
                                          :Security_Operations_Policies ;
                                 :HasWeight 8 ;
                                 rdfs:comment "Mechanisms exist to ensure that database servers utilize encryption to protect the confidentiality of the data within the databases." .


###  http://FYP-ASHS21/csonto/OPS-CRY-06-Non-ConsoleAdministrativeAccess
:OPS-CRY-06-Non-ConsoleAdministrativeAccess rdf:type owl:NamedIndividual ,
                                                     :Security_Operations_Policies ;
                                            :HasWeight 9 ;
                                            rdfs:comment "Cryptographic mechanisms exist to protect the confidentiality and integrity of non-console administrative access." .


###  http://FYP-ASHS21/csonto/OPS-CRY-08-PublicKeyInfrastructure-PKI-
:OPS-CRY-08-PublicKeyInfrastructure-PKI- rdf:type owl:NamedIndividual ,
                                                  :Security_Operations_Policies ;
                                         :HasWeight 9 ;
                                         rdfs:comment "Mechanisms exist to securely implement an internal Public Key Infrastructure (PKI) infrastructure or obtain PKI services from a reputable PKI service provider. " .


###  http://FYP-ASHS21/csonto/OPS-CRY-08.1-Availability
:OPS-CRY-08.1-Availability rdf:type owl:NamedIndividual ,
                                    :Security_Operations_Policies ;
                           :HasWeight 9 ;
                           rdfs:comment "Resiliency mechanisms exist to ensure the availability of data in the event of the loss of cryptographic keys." .


###  http://FYP-ASHS21/csonto/OPS-CRY-09-CryptographicKeyManagement
:OPS-CRY-09-CryptographicKeyManagement rdf:type owl:NamedIndividual ,
                                                :Security_Operations_Policies ;
                                       :HasWeight 10 ;
                                       rdfs:comment "Mechanisms exist to facilitate cryptographic key management controls to protect the confidentiality, integrity and availability of keys." .


###  http://FYP-ASHS21/csonto/OPS-CRY-09.1-SymmetricKeys
:OPS-CRY-09.1-SymmetricKeys rdf:type owl:NamedIndividual ,
                                     :Security_Operations_Policies ;
                            :HasWeight 9 ;
                            rdfs:comment "Mechanisms exist to facilitate the production and management of symmetric cryptographic keys using Federal Information Processing Standards (FIPS)-compliant key management technology and processes. " .


###  http://FYP-ASHS21/csonto/OPS-CRY-09.2-AsymmetricKeys
:OPS-CRY-09.2-AsymmetricKeys rdf:type owl:NamedIndividual ,
                                      :Security_Operations_Policies ;
                             :HasWeight 9 ;
                             rdfs:comment "Mechanisms exist to facilitate the production and management of asymmetric cryptographic keys using Federal Information Processing Standards (FIPS)-compliant key management technology and processes that protect the users private key. " .


###  http://FYP-ASHS21/csonto/OPS-CRY-09.3-CryptographicKeyLossorChange
:OPS-CRY-09.3-CryptographicKeyLossorChange rdf:type owl:NamedIndividual ,
                                                    :Security_Operations_Policies ;
                                           :HasWeight 8 ;
                                           rdfs:comment "Mechanisms exist to ensure the availability of information in the event of the loss of cryptographic keys by individual users. " .


###  http://FYP-ASHS21/csonto/OPS-CRY-09.5-AssignedOwners
:OPS-CRY-09.5-AssignedOwners rdf:type owl:NamedIndividual ,
                                      :Security_Operations_Policies ;
                             :HasWeight 8 ;
                             rdfs:comment "Mechanisms exist to ensure cryptographic keys are bound to individual identities. " .


###  http://FYP-ASHS21/csonto/OPS-CRY-09.6-Third-PartyCryptographicKeys
:OPS-CRY-09.6-Third-PartyCryptographicKeys rdf:type owl:NamedIndividual ,
                                                    :Security_Operations_Policies ;
                                           :HasWeight 7 ;
                                           rdfs:comment "Mechanisms exist to ensure customers are provided with appropriate key management guidance whenever cryptographic keys are shared." .


###  http://FYP-ASHS21/csonto/OPS-CRY-09.7-ExternalSystemCryptographicKeyControl
:OPS-CRY-09.7-ExternalSystemCryptographicKeyControl rdf:type owl:NamedIndividual ,
                                                             :Security_Operations_Policies ;
                                                    :HasWeight 5 ;
                                                    rdfs:comment "Mechanisms exist to maintain control of cryptographic keys for encrypted material stored or transmitted through an external system." .


###  http://FYP-ASHS21/csonto/OPS-CRY-11-CertificateAuthorities
:OPS-CRY-11-CertificateAuthorities rdf:type owl:NamedIndividual ,
                                            :Security_Operations_Policies ;
                                   :HasWeight 8 ;
                                   rdfs:comment "Automated mechanisms exist to enable the use of organization-defined Certificate Authorities (CAs) to facilitate the establishment of protected sessions." .


###  http://FYP-ASHS21/csonto/OPS-DCH-01-DataProtection
:OPS-DCH-01-DataProtection rdf:type owl:NamedIndividual ,
                                    :Security_Operations_Policies ;
                           :HasWeight 10 ;
                           rdfs:comment "Mechanisms exist to facilitate the implementation of data protection controls. " .


###  http://FYP-ASHS21/csonto/OPS-DCH-01.1-DataStewardship
:OPS-DCH-01.1-DataStewardship rdf:type owl:NamedIndividual ,
                                       :Security_Operations_Policies ;
                              :HasWeight 10 ;
                              rdfs:comment "Mechanisms exist to ensure data stewardship is assigned, documented and communicated. " .


###  http://FYP-ASHS21/csonto/OPS-DCH-01.2-Sensitive-RegulatedDataProtection
:OPS-DCH-01.2-Sensitive-RegulatedDataProtection rdf:type owl:NamedIndividual ,
                                                         :Security_Operations_Policies ;
                                                :HasWeight 9 ;
                                                rdfs:comment "Mechanisms exist to protect sensitive/regulated data wherever it is stored." .


###  http://FYP-ASHS21/csonto/OPS-DCH-01.3-Sensitive-RegulatedMediaRecords
:OPS-DCH-01.3-Sensitive-RegulatedMediaRecords rdf:type owl:NamedIndividual ,
                                                       :Security_Operations_Policies ;
                                              :HasWeight 6 ;
                                              rdfs:comment "Mechanisms exist to ensure media records for sensitive/regulated data contain sufficient information to determine the potential impact in the event of a data loss incident." .


###  http://FYP-ASHS21/csonto/OPS-DCH-02.1-HighestClassificationLevel
:OPS-DCH-02.1-HighestClassificationLevel rdf:type owl:NamedIndividual ,
                                                  :Security_Operations_Policies ;
                                         :HasWeight 8 ;
                                         rdfs:comment "Mechanisms exist to ensure that systems, applications and services are classified according to the highest level of data sensitivity that is stored, transmitted and/or processed." .


###  http://FYP-ASHS21/csonto/OPS-DCH-03-MediaAccess
:OPS-DCH-03-MediaAccess rdf:type owl:NamedIndividual ,
                                 :Security_Operations_Policies ;
                        :HasWeight 8 ;
                        rdfs:comment "Mechanisms exist to control and restrict access to digital and non-digital media to authorized individuals. " .


###  http://FYP-ASHS21/csonto/OPS-DCH-03.1-DisclosureofInformation
:OPS-DCH-03.1-DisclosureofInformation rdf:type owl:NamedIndividual ,
                                               :Security_Operations_Policies ;
                                      :HasWeight 10 ;
                                      rdfs:comment "Mechanisms exist to restrict the disclosure of sensitive / regulated data to authorized parties with a need to know." .


###  http://FYP-ASHS21/csonto/OPS-DCH-03.2-MaskingDisplayedData
:OPS-DCH-03.2-MaskingDisplayedData rdf:type owl:NamedIndividual ,
                                            :Security_Operations_Policies ;
                                   :HasWeight 7 ;
                                   rdfs:comment "Mechanisms exist to apply data masking to sensitive/regulated information that is displayed or printed. " .


###  http://FYP-ASHS21/csonto/OPS-DCH-03.3-ControlledRelease
:OPS-DCH-03.3-ControlledRelease rdf:type owl:NamedIndividual ,
                                         :Security_Operations_Policies ;
                                :HasWeight 4 ;
                                rdfs:comment "Automated mechanisms exist to validate cybersecurity & data privacy attributes prior to releasing information to external systems." .


###  http://FYP-ASHS21/csonto/OPS-DCH-04-MediaMarking
:OPS-DCH-04-MediaMarking rdf:type owl:NamedIndividual ,
                                  :Security_Operations_Policies ;
                         :HasWeight 7 ;
                         rdfs:comment "Mechanisms exist to mark media in accordance with data protection requirements so that personnel are alerted to distribution limitations, handling caveats and applicable security requirements. " .


###  http://FYP-ASHS21/csonto/OPS-DCH-04.1-AutomatedMarking
:OPS-DCH-04.1-AutomatedMarking rdf:type owl:NamedIndividual ,
                                        :Security_Operations_Policies ;
                               :HasWeight 2 ;
                               rdfs:comment "Automated mechanisms exist to mark physical media and digital files to indicate the distribution limitations, handling requirements and applicable security markings (if any) of the information to aid Data Loss Prevention (DLP) technologies. " .


###  http://FYP-ASHS21/csonto/OPS-DCH-05.1-DynamicAttributeAssociation
:OPS-DCH-05.1-DynamicAttributeAssociation rdf:type owl:NamedIndividual ,
                                                   :Security_Operations_Policies ;
                                          :HasWeight 2 ;
                                          rdfs:comment "Mechanisms exist to dynamically associate cybersecurity & data privacy attributes with individuals and objects as information is created, combined, or transformed, in accordance with organization-defined cybersecurity and data privacy policies." .


###  http://FYP-ASHS21/csonto/OPS-DCH-05.10-AttributeConfigurationByAuthorizedIndividuals
:OPS-DCH-05.10-AttributeConfigurationByAuthorizedIndividuals rdf:type owl:NamedIndividual ,
                                                                      :Security_Operations_Policies ;
                                                             :HasWeight 8 ;
                                                             rdfs:comment "Mechanisms exist to provide authorized individuals the capability to define or change the type and value of cybersecurity & data privacy attributes available for association with subjects and objects." .


###  http://FYP-ASHS21/csonto/OPS-DCH-05.11-AuditChanges
:OPS-DCH-05.11-AuditChanges rdf:type owl:NamedIndividual ,
                                     :Security_Operations_Policies ;
                            :HasWeight 7 ;
                            rdfs:comment "Mechanisms exist to audit changes to cybersecurity & data privacy attributes and responds to events in accordance with incident response procedures." .


###  http://FYP-ASHS21/csonto/OPS-DCH-05.2-AttributeValueChangesByAuthorizedIndividuals
:OPS-DCH-05.2-AttributeValueChangesByAuthorizedIndividuals rdf:type owl:NamedIndividual ,
                                                                    :Security_Operations_Policies ;
                                                           :HasWeight 8 ;
                                                           rdfs:comment "Mechanisms exist to provide authorized individuals (or processes acting on behalf of individuals) the capability to define or change the value of associated cybersecurity & data privacy attributes." .


###  http://FYP-ASHS21/csonto/OPS-DCH-05.3-MaintenanceofAttributeAssociationsBySystem
:OPS-DCH-05.3-MaintenanceofAttributeAssociationsBySystem rdf:type owl:NamedIndividual ,
                                                                  :Security_Operations_Policies ;
                                                         :HasWeight 2 ;
                                                         rdfs:comment "Mechanisms exist to maintain the association and integrity of cybersecurity & data privacy attributes to individuals and objects." .


###  http://FYP-ASHS21/csonto/OPS-DCH-05.4-AssociationofAttributesByAuthorizedIndividuals
:OPS-DCH-05.4-AssociationofAttributesByAuthorizedIndividuals rdf:type owl:NamedIndividual ,
                                                                      :Security_Operations_Policies ;
                                                             :HasWeight 2 ;
                                                             rdfs:comment "Mechanisms exist to provide the capability to associate cybersecurity & data privacy attributes with individuals and objects by authorized individuals (or processes acting on behalf of individuals)." .


###  http://FYP-ASHS21/csonto/OPS-DCH-05.5-AttributeDisplaysforOutputDevices
:OPS-DCH-05.5-AttributeDisplaysforOutputDevices rdf:type owl:NamedIndividual ,
                                                         :Security_Operations_Policies ;
                                                :HasWeight 8 ;
                                                rdfs:comment "Mechanisms exist to display cybersecurity & data privacy attributes in human-readable form on each object that the system transmits to output devices to identify special dissemination, handling or distribution instructions using human-readable, standard naming conventions." .


###  http://FYP-ASHS21/csonto/OPS-DCH-05.6-DataSubjectAttributeAssociations
:OPS-DCH-05.6-DataSubjectAttributeAssociations rdf:type owl:NamedIndividual ,
                                                        :Security_Operations_Policies ;
                                               :HasWeight 2 ;
                                               rdfs:comment "Mechanisms exist to require personnel to associate and maintain the association of cybersecurity & data privacy attributes with individuals and objects in accordance with cybersecurity and data privacy policies." .


###  http://FYP-ASHS21/csonto/OPS-DCH-05.7-ConsistentAttributeInterpretation
:OPS-DCH-05.7-ConsistentAttributeInterpretation rdf:type owl:NamedIndividual ,
                                                         :Security_Operations_Policies ;
                                                :HasWeight 2 ;
                                                rdfs:comment "Mechanisms exist to provide a consistent, organizationally agreed upon interpretation of cybersecurity & data privacy attributes employed in access enforcement and flow enforcement decisions between distributed system components." .


###  http://FYP-ASHS21/csonto/OPS-DCH-05.9-AttributeReassignment
:OPS-DCH-05.9-AttributeReassignment rdf:type owl:NamedIndividual ,
                                             :Security_Operations_Policies ;
                                    :HasWeight 7 ;
                                    rdfs:comment "Mechanisms exist to reclassify data as required, due to changing business/technical requirements." .


###  http://FYP-ASHS21/csonto/OPS-DCH-06-MediaStorage
:OPS-DCH-06-MediaStorage rdf:type owl:NamedIndividual ,
                                  :Security_Operations_Policies ;
                         :HasWeight 8 ;
                         rdfs:comment """Mechanisms exist to: 
  Physically control and securely store digital and non-digital media within controlled areas using organization-defined security measures; and
  Protect system media until the media are destroyed or sanitized using approved equipment, techniques and procedures.""" .


###  http://FYP-ASHS21/csonto/OPS-DCH-06.1-PhysicallySecureAllMedia
:OPS-DCH-06.1-PhysicallySecureAllMedia rdf:type owl:NamedIndividual ,
                                                :Security_Operations_Policies ;
                                       :HasWeight 9 ;
                                       rdfs:comment "Mechanisms exist to physically secure all media that contains sensitive information." .


###  http://FYP-ASHS21/csonto/OPS-DCH-06.2-SensitiveDataInventories
:OPS-DCH-06.2-SensitiveDataInventories rdf:type owl:NamedIndividual ,
                                                :Security_Operations_Policies ;
                                       :HasWeight 9 ;
                                       rdfs:comment "Mechanisms exist to maintain inventory logs of all sensitive media and conduct sensitive media inventories at least annually. " .


###  http://FYP-ASHS21/csonto/OPS-DCH-06.3-PeriodicScansforSensitiveData
:OPS-DCH-06.3-PeriodicScansforSensitiveData rdf:type owl:NamedIndividual ,
                                                     :Security_Operations_Policies ;
                                            :HasWeight 7 ;
                                            rdfs:comment "Mechanisms exist to periodically scan unstructured data sources for sensitive/regulated data or data requiring special protection measures by statutory, regulatory or contractual obligations. " .


###  http://FYP-ASHS21/csonto/OPS-DCH-06.4-MakingSensitiveDataUnreadableInStorage
:OPS-DCH-06.4-MakingSensitiveDataUnreadableInStorage rdf:type owl:NamedIndividual ,
                                                              :Security_Operations_Policies ;
                                                     :HasWeight 9 ;
                                                     rdfs:comment "Mechanisms exist to ensure sensitive/regulated data is rendered human unreadable anywhere sensitive/regulated data is stored. " .


###  http://FYP-ASHS21/csonto/OPS-DCH-06.5-StoringAuthenticationData
:OPS-DCH-06.5-StoringAuthenticationData rdf:type owl:NamedIndividual ,
                                                 :Security_Operations_Policies ;
                                        :HasWeight 5 ;
                                        rdfs:comment "Mechanisms exist to prohibit the storage of sensitive transaction authentication data after authorization. " .


###  http://FYP-ASHS21/csonto/OPS-DCH-07-MediaTransportation
:OPS-DCH-07-MediaTransportation rdf:type owl:NamedIndividual ,
                                         :Security_Operations_Policies ;
                                :HasWeight 9 ;
                                rdfs:comment "Mechanisms exist to protect and control digital and non-digital media during transport outside of controlled areas using appropriate security measures." .


###  http://FYP-ASHS21/csonto/OPS-DCH-07.1-Custodians
:OPS-DCH-07.1-Custodians rdf:type owl:NamedIndividual ,
                                  :Security_Operations_Policies ;
                         :HasWeight 9 ;
                         rdfs:comment "Mechanisms exist to identify custodians throughout the transport of digital or non-digital media. " .


###  http://FYP-ASHS21/csonto/OPS-DCH-07.2-EncryptingDataInStorageMedia
:OPS-DCH-07.2-EncryptingDataInStorageMedia rdf:type owl:NamedIndividual ,
                                                    :Security_Operations_Policies ;
                                           :HasWeight 5 ;
                                           rdfs:comment "Cryptographic mechanisms exist to protect the confidentiality and integrity of information stored on digital media during transport outside of controlled areas." .


###  http://FYP-ASHS21/csonto/OPS-DCH-08-PhysicalMediaDisposal
:OPS-DCH-08-PhysicalMediaDisposal rdf:type owl:NamedIndividual ,
                                           :Security_Operations_Policies ;
                                  :HasWeight 10 ;
                                  rdfs:comment "Mechanisms exist to securely dispose of media when it is no longer required, using formal procedures. " .


###  http://FYP-ASHS21/csonto/OPS-DCH-09-DigitalMediaSanitization
:OPS-DCH-09-DigitalMediaSanitization rdf:type owl:NamedIndividual ,
                                              :Security_Operations_Policies ;
                                     :HasWeight 10 ;
                                     rdfs:comment "Mechanisms exist to sanitize digital media with the strength and integrity commensurate with the classification or sensitivity of the information prior to disposal, release out of organizational control or release for reuse." .


###  http://FYP-ASHS21/csonto/OPS-DCH-09.1-MediaSanitizationDocumentation
:OPS-DCH-09.1-MediaSanitizationDocumentation rdf:type owl:NamedIndividual ,
                                                      :Security_Operations_Policies ;
                                             :HasWeight 7 ;
                                             rdfs:comment "Mechanisms exist to supervise, track, document and verify media sanitization and disposal actions. " .


###  http://FYP-ASHS21/csonto/OPS-DCH-09.2-EquipmentTesting
:OPS-DCH-09.2-EquipmentTesting rdf:type owl:NamedIndividual ,
                                        :Security_Operations_Policies ;
                               :HasWeight 5 ;
                               rdfs:comment "Mechanisms exist to test sanitization equipment and procedures to verify that the intended result is achieved. " .


###  http://FYP-ASHS21/csonto/OPS-DCH-09.3-SanitizationofPersonalData-PD-
:OPS-DCH-09.3-SanitizationofPersonalData-PD- rdf:type owl:NamedIndividual ,
                                                      :Security_Operations_Policies ;
                                             :HasWeight 9 ;
                                             rdfs:comment "Mechanisms exist to facilitate the sanitization of Personal Data (PD)." .


###  http://FYP-ASHS21/csonto/OPS-DCH-09.4-FirstTimeUseSanitization
:OPS-DCH-09.4-FirstTimeUseSanitization rdf:type owl:NamedIndividual ,
                                                :Security_Operations_Policies ;
                                       :HasWeight 5 ;
                                       rdfs:comment "Mechanisms exist to apply nondestructive sanitization techniques to portable storage devices prior to first use." .


###  http://FYP-ASHS21/csonto/OPS-DCH-09.5-DualAuthorizationforSensitiveDataDestruction
:OPS-DCH-09.5-DualAuthorizationforSensitiveDataDestruction rdf:type owl:NamedIndividual ,
                                                                    :Security_Operations_Policies ;
                                                           :HasWeight 5 ;
                                                           rdfs:comment "Mechanisms exist to enforce dual authorization for the destruction, disposal or sanitization of digital media that contains sensitive / regulated data." .


###  http://FYP-ASHS21/csonto/OPS-DCH-10-MediaUse
:OPS-DCH-10-MediaUse rdf:type owl:NamedIndividual ,
                              :Security_Operations_Policies ;
                     :HasWeight 8 ;
                     rdfs:comment "Mechanisms exist to restrict the use of types of digital media on systems or system components. " .


###  http://FYP-ASHS21/csonto/OPS-DCH-10.1-LimitationsonUse
:OPS-DCH-10.1-LimitationsonUse rdf:type owl:NamedIndividual ,
                                        :Security_Operations_Policies ;
                               :HasWeight 10 ;
                               rdfs:comment "Mechanisms exist to restrict the use and distribution of sensitive / regulated data. " .


###  http://FYP-ASHS21/csonto/OPS-DCH-10.2-ProhibitUseWithoutOwner
:OPS-DCH-10.2-ProhibitUseWithoutOwner rdf:type owl:NamedIndividual ,
                                               :Security_Operations_Policies ;
                                      :HasWeight 5 ;
                                      rdfs:comment "Mechanisms exist to prohibit the use of portable storage devices in organizational information systems when such devices have no identifiable owner." .


###  http://FYP-ASHS21/csonto/OPS-DCH-11-DataReclassification
:OPS-DCH-11-DataReclassification rdf:type owl:NamedIndividual ,
                                          :Security_Operations_Policies ;
                                 :HasWeight 8 ;
                                 rdfs:comment "Mechanisms exist to reclassify data, including associated systems, applications and services, commensurate with the security category and/or classification level of the information." .


###  http://FYP-ASHS21/csonto/OPS-DCH-12-RemovableMediaSecurity
:OPS-DCH-12-RemovableMediaSecurity rdf:type owl:NamedIndividual ,
                                            :Security_Operations_Policies ;
                                   :HasWeight 10 ;
                                   rdfs:comment "Mechanisms exist to restrict removable media in accordance with data handling and acceptable usage parameters." .


###  http://FYP-ASHS21/csonto/OPS-DCH-13-UseofExternalInformationSystems
:OPS-DCH-13-UseofExternalInformationSystems rdf:type owl:NamedIndividual ,
                                                     :Security_Operations_Policies ;
                                            :HasWeight 9 ;
                                            rdfs:comment "Mechanisms exist to govern how external parties, systems and services are used to securely store, process and transmit data. " .


###  http://FYP-ASHS21/csonto/OPS-DCH-13.1-LimitsofAuthorizedUse
:OPS-DCH-13.1-LimitsofAuthorizedUse rdf:type owl:NamedIndividual ,
                                             :Security_Operations_Policies ;
                                    :HasWeight 8 ;
                                    rdfs:comment """Mechanisms exist to prohibit external parties, systems and services from storing, processing and transmitting data unless authorized individuals first: 
  Verifying the implementation of required security controls; or
  Retaining a processing agreement with the entity hosting the external systems or service.""" .


###  http://FYP-ASHS21/csonto/OPS-DCH-13.2-PortableStorageDevices
:OPS-DCH-13.2-PortableStorageDevices rdf:type owl:NamedIndividual ,
                                              :Security_Operations_Policies ;
                                     :HasWeight 9 ;
                                     rdfs:comment "Mechanisms exist to restrict or prohibit the use of portable storage devices by users on external systems. " .


###  http://FYP-ASHS21/csonto/OPS-DCH-13.3-ProtectingSensitiveDataonExternalSystems
:OPS-DCH-13.3-ProtectingSensitiveDataonExternalSystems rdf:type owl:NamedIndividual ,
                                                                :Security_Operations_Policies ;
                                                       :HasWeight 10 ;
                                                       rdfs:comment "Mechanisms exist to ensure that the requirements for the protection of sensitive information processed, stored or transmitted on external systems, are implemented in accordance with applicable statutory, regulatory and contractual obligations." .


###  http://FYP-ASHS21/csonto/OPS-DCH-13.4-Non-OrganizationallyOwnedSystems-Components-Devices
:OPS-DCH-13.4-Non-OrganizationallyOwnedSystems-Components-Devices rdf:type owl:NamedIndividual ,
                                                                           :Security_Operations_Policies ;
                                                                  :HasWeight 5 ;
                                                                  rdfs:comment "Mechanisms exist to restrict the use of non-organizationally owned information systems, system components or devices to process, store or transmit organizational information." .


###  http://FYP-ASHS21/csonto/OPS-DCH-14-InformationSharing
:OPS-DCH-14-InformationSharing rdf:type owl:NamedIndividual ,
                                        :Security_Operations_Policies ;
                               :HasWeight 9 ;
                               rdfs:comment "Mechanisms exist to utilize a process to assist users in making information sharing decisions to ensure data is appropriately protected." .


###  http://FYP-ASHS21/csonto/OPS-DCH-14.2-TransferAuthorizations
:OPS-DCH-14.2-TransferAuthorizations rdf:type owl:NamedIndividual ,
                                              :Security_Operations_Policies ;
                                     :HasWeight 8 ;
                                     rdfs:comment "Mechanisms exist to verify that individuals or systems transferring data between interconnecting systems have the requisite authorizations (e.g., write permissions or privileges) prior to transferring said data." .


###  http://FYP-ASHS21/csonto/OPS-DCH-14.3-DataAccessMapping
:OPS-DCH-14.3-DataAccessMapping rdf:type owl:NamedIndividual ,
                                         :Security_Operations_Policies ;
                                :HasWeight 9 ;
                                rdfs:comment "Mechanisms exist to develop a data-specific Access Control List (ACL) or Data Information Sharing Agreement (DISA) to determine the personnel with whom sensitive/regulated data is shared." .


###  http://FYP-ASHS21/csonto/OPS-DCH-15-PubliclyAccessibleContent
:OPS-DCH-15-PubliclyAccessibleContent rdf:type owl:NamedIndividual ,
                                               :Security_Operations_Policies ;
                                      :HasWeight 10 ;
                                      rdfs:comment "Mechanisms exist to control publicly-accessible content." .


###  http://FYP-ASHS21/csonto/OPS-DCH-16-DataMiningProtection
:OPS-DCH-16-DataMiningProtection rdf:type owl:NamedIndividual ,
                                          :Security_Operations_Policies ;
                                 :HasWeight 7 ;
                                 rdfs:comment "Mechanisms exist to protect data storage objects against unauthorized data mining and data harvesting techniques. " .


###  http://FYP-ASHS21/csonto/OPS-DCH-17-Ad-HocTransfers
:OPS-DCH-17-Ad-HocTransfers rdf:type owl:NamedIndividual ,
                                     :Security_Operations_Policies ;
                            :HasWeight 8 ;
                            rdfs:comment "Mechanisms exist to secure ad-hoc exchanges of large digital files with internal or external parties." .


###  http://FYP-ASHS21/csonto/OPS-DCH-18.1-MinimizePersonalData-PD-
:OPS-DCH-18.1-MinimizePersonalData-PD- rdf:type owl:NamedIndividual ,
                                                :Security_Operations_Policies ;
                                       :HasWeight 8 ;
                                       rdfs:comment "Mechanisms exist to limit Personal Data (PD) being processed in the information lifecycle to elements identified in the Data Protection Impact Assessment (DPIA)." .


###  http://FYP-ASHS21/csonto/OPS-DCH-18.3-TemporaryFilesContainingPersonalData-PD-
:OPS-DCH-18.3-TemporaryFilesContainingPersonalData-PD- rdf:type owl:NamedIndividual ,
                                                                :Security_Operations_Policies ;
                                                       :HasWeight 5 ;
                                                       rdfs:comment "Mechanisms exist to perform periodic checks of temporary files for the existence of Personal Data (PD)." .


###  http://FYP-ASHS21/csonto/OPS-DCH-19-GeographicLocationofData
:OPS-DCH-19-GeographicLocationofData rdf:type owl:NamedIndividual ,
                                              :Security_Operations_Policies ;
                                     :HasWeight 9 ;
                                     rdfs:comment "Mechanisms exist to inventory, document and maintain data flows for data that is resident (permanently or temporarily) within a service's geographically distributed applications (physical and virtual), infrastructure, systems components and/or shared with other third-parties." .


###  http://FYP-ASHS21/csonto/OPS-DCH-20-ArchivedDataSets
:OPS-DCH-20-ArchivedDataSets rdf:type owl:NamedIndividual ,
                                      :Security_Operations_Policies ;
                             :HasWeight 8 ;
                             rdfs:comment "Mechanisms exist to protect archived data in accordance with applicable statutory, regulatory and contractual obligations. " .


###  http://FYP-ASHS21/csonto/OPS-DCH-21-InformationDisposal
:OPS-DCH-21-InformationDisposal rdf:type owl:NamedIndividual ,
                                         :Security_Operations_Policies ;
                                :HasWeight 10 ;
                                rdfs:comment "Mechanisms exist to securely dispose of, destroy or erase information." .


###  http://FYP-ASHS21/csonto/OPS-DCH-22-DataQualityOperations
:OPS-DCH-22-DataQualityOperations rdf:type owl:NamedIndividual ,
                                           :Security_Operations_Policies ;
                                  :HasWeight 5 ;
                                  rdfs:comment "Mechanisms exist to check for the accuracy, relevance, timeliness, impact, completeness and de-identification of information across the information lifecycle." .


###  http://FYP-ASHS21/csonto/OPS-DCH-22.2-DataTags
:OPS-DCH-22.2-DataTags rdf:type owl:NamedIndividual ,
                                :Security_Operations_Policies ;
                       :HasWeight 3 ;
                       rdfs:comment "Mechanisms exist to utilize data tags to automate tracking of sensitive/regulated data across the information lifecycle." .


###  http://FYP-ASHS21/csonto/OPS-DCH-22.3-PrimarySourcePersonalData-PD-Collection
:OPS-DCH-22.3-PrimarySourcePersonalData-PD-Collection rdf:type owl:NamedIndividual ,
                                                               :Security_Operations_Policies ;
                                                      :HasWeight 8 ;
                                                      rdfs:comment "Mechanisms exist to collect Personal Data (PD) directly from the individual. " .


###  http://FYP-ASHS21/csonto/OPS-DCH-23-De-Identification-Anonymization-
:OPS-DCH-23-De-Identification-Anonymization- rdf:type owl:NamedIndividual ,
                                                      :Security_Operations_Policies ;
                                             :HasWeight 8 ;
                                             rdfs:comment "Mechanisms exist to anonymize data by removing Personal Data (PD) from datasets." .


###  http://FYP-ASHS21/csonto/OPS-DCH-23.1-De-IdentifyDatasetUponCollection
:OPS-DCH-23.1-De-IdentifyDatasetUponCollection rdf:type owl:NamedIndividual ,
                                                        :Security_Operations_Policies ;
                                               :HasWeight 8 ;
                                               rdfs:comment "Mechanisms exist to de-identify the dataset upon collection by not collecting Personal Data (PD)." .


###  http://FYP-ASHS21/csonto/OPS-DCH-23.2-Archiving
:OPS-DCH-23.2-Archiving rdf:type owl:NamedIndividual ,
                                 :Security_Operations_Policies ;
                        :HasWeight 8 ;
                        rdfs:comment "Mechanisms exist to refrain from archiving Personal Data (PD) elements if those elements in a dataset will not be needed after the dataset is archived." .


###  http://FYP-ASHS21/csonto/OPS-DCH-23.3-Release
:OPS-DCH-23.3-Release rdf:type owl:NamedIndividual ,
                               :Security_Operations_Policies ;
                      :HasWeight 8 ;
                      rdfs:comment "Mechanisms exist to remove Personal Data (PD) elements from a dataset prior to its release if those elements in the dataset do not need to be part of the data release." .


###  http://FYP-ASHS21/csonto/OPS-DCH-23.4-Removal-Masking-Encryption-HashingorReplacementofDirectIdentifiers
:OPS-DCH-23.4-Removal-Masking-Encryption-HashingorReplacementofDirectIdentifiers rdf:type owl:NamedIndividual ,
                                                                                          :Security_Operations_Policies ;
                                                                                 :HasWeight 8 ;
                                                                                 rdfs:comment "Mechanisms exist to remove, mask, encrypt, hash or replace direct identifiers in a dataset." .


###  http://FYP-ASHS21/csonto/OPS-DCH-23.5-StatisticalDisclosureControl
:OPS-DCH-23.5-StatisticalDisclosureControl rdf:type owl:NamedIndividual ,
                                                    :Security_Operations_Policies ;
                                           :HasWeight 1 ;
                                           rdfs:comment "Mechanisms exist to manipulate numerical data, contingency tables and statistical findings so that no person or organization is identifiable in the results of the analysis." .


###  http://FYP-ASHS21/csonto/OPS-DCH-23.6-DifferentialDataPrivacy
:OPS-DCH-23.6-DifferentialDataPrivacy rdf:type owl:NamedIndividual ,
                                               :Security_Operations_Policies ;
                                      :HasWeight 1 ;
                                      rdfs:comment "Mechanisms exist to prevent disclosure of Personal Data (PD) by adding non-deterministic noise to the results of mathematical operations before the results are reported." .


###  http://FYP-ASHS21/csonto/OPS-DCH-23.7-AutomatedDe-IdentificationofSensitiveData
:OPS-DCH-23.7-AutomatedDe-IdentificationofSensitiveData rdf:type owl:NamedIndividual ,
                                                                 :Security_Operations_Policies ;
                                                        :HasWeight 1 ;
                                                        rdfs:comment "Mechanisms exist to perform de-identification of sensitive/regulated data, using validated algorithms and software to implement the algorithms." .


###  http://FYP-ASHS21/csonto/OPS-DCH-23.8-MotivatedIntruder
:OPS-DCH-23.8-MotivatedIntruder rdf:type owl:NamedIndividual ,
                                         :Security_Operations_Policies ;
                                :HasWeight 3 ;
                                rdfs:comment "Mechanisms exist to perform a motivated intruder test on the de-identified dataset to determine if the identified data remains or if the de-identified data can be re-identified." .


###  http://FYP-ASHS21/csonto/OPS-DCH-23.9-CodeNames
:OPS-DCH-23.9-CodeNames rdf:type owl:NamedIndividual ,
                                 :Security_Operations_Policies ;
                        :HasWeight 1 ;
                        rdfs:comment "Mechanisms exist to use aliases to name assets, which are mission-critical and/or contain highly-sensitive/regulated data, are unique and not readily associated with a product, project or type of data." .


###  http://FYP-ASHS21/csonto/OPS-DCH-24-InformationLocation
:OPS-DCH-24-InformationLocation rdf:type owl:NamedIndividual ,
                                         :Security_Operations_Policies ;
                                :HasWeight 10 ;
                                rdfs:comment "Mechanisms exist to identify and document the location of information and the specific system components on which the information resides." .


###  http://FYP-ASHS21/csonto/OPS-DCH-24.1-AutomatedToolstoSupportInformationLocation
:OPS-DCH-24.1-AutomatedToolstoSupportInformationLocation rdf:type owl:NamedIndividual ,
                                                                  :Security_Operations_Policies ;
                                                         :HasWeight 6 ;
                                                         rdfs:comment "Automated mechanisms exist to identify by data classification type to ensure adequate cybersecurity & data privacy controls are in place to protect organizational information and individual data privacy." .


###  http://FYP-ASHS21/csonto/OPS-DCH-25-TransferofSensitiveand-orRegulatedData
:OPS-DCH-25-TransferofSensitiveand-orRegulatedData rdf:type owl:NamedIndividual ,
                                                            :Security_Operations_Policies ;
                                                   :HasWeight 10 ;
                                                   rdfs:comment "Mechanisms exist to restrict and govern the transfer of sensitive and/or regulated data to third-countries or international organizations." .


###  http://FYP-ASHS21/csonto/OPS-DCH-25.1-TransferActivityLimits
:OPS-DCH-25.1-TransferActivityLimits rdf:type owl:NamedIndividual ,
                                              :Security_Operations_Policies ;
                                     :HasWeight 7 ;
                                     rdfs:comment "Mechanisms exist to establish organization-defined \"normal business activities\" to identify anomalous transaction activities that can reduce the opportunity for sending (outbound) and/or receiving (inbound) fraudulent actions." .


###  http://FYP-ASHS21/csonto/OPS-DCH-26-DataLocalization
:OPS-DCH-26-DataLocalization rdf:type owl:NamedIndividual ,
                                      :Security_Operations_Policies ;
                             :HasWeight 10 ;
                             rdfs:comment "Mechanisms exist to constrain the impact of \"digital sovereignty laws,\" that require localized data within the host country, where data and processes may be subjected to arbitrary enforcement actions that potentially violate other applicable statutory, regulatory and/or contractual obligations." .


###  http://FYP-ASHS21/csonto/OPS-EMB-01-EmbeddedTechnologySecurityProgram
:OPS-EMB-01-EmbeddedTechnologySecurityProgram rdf:type owl:NamedIndividual ,
                                                       :Security_Operations_Policies ;
                                              :HasWeight 10 ;
                                              rdfs:comment "Mechanisms exist to facilitate the implementation of embedded technology controls. " .


###  http://FYP-ASHS21/csonto/OPS-EMB-02-InternetofThings-IOT-
:OPS-EMB-02-InternetofThings-IOT- rdf:type owl:NamedIndividual ,
                                           :Security_Operations_Policies ;
                                  :HasWeight 9 ;
                                  rdfs:comment "Mechanisms exist to proactively manage the cybersecurity & data privacy risks associated with Internet of Things (IoT)." .


###  http://FYP-ASHS21/csonto/OPS-EMB-03-OperationalTechnology-OT-
:OPS-EMB-03-OperationalTechnology-OT- rdf:type owl:NamedIndividual ,
                                               :Security_Operations_Policies ;
                                      :HasWeight 9 ;
                                      rdfs:comment "Mechanisms exist to proactively manage the cybersecurity & data privacy risks associated with Operational Technology (OT)." .


###  http://FYP-ASHS21/csonto/OPS-EMB-04-InterfaceSecurity
:OPS-EMB-04-InterfaceSecurity rdf:type owl:NamedIndividual ,
                                       :Security_Operations_Policies ;
                              :HasWeight 4 ;
                              rdfs:comment "Mechanisms exist to protect embedded devices against unauthorized use of the physical factory diagnostic and test interface(s)." .


###  http://FYP-ASHS21/csonto/OPS-EMB-05-EmbeddedTechnologyConfigurationMonitoring
:OPS-EMB-05-EmbeddedTechnologyConfigurationMonitoring rdf:type owl:NamedIndividual ,
                                                               :Security_Operations_Policies ;
                                                      :HasWeight 6 ;
                                                      rdfs:comment "Mechanisms exist to generate log entries on embedded devices when configuration changes or attempts to access interfaces are detected." .


###  http://FYP-ASHS21/csonto/OPS-EMB-06-PreventAlterations
:OPS-EMB-06-PreventAlterations rdf:type owl:NamedIndividual ,
                                        :Security_Operations_Policies ;
                               :HasWeight 6 ;
                               rdfs:comment "Mechanisms exist to protect embedded devices by preventing the unauthorized installation and execution of software." .


###  http://FYP-ASHS21/csonto/OPS-EMB-07-EmbeddedTechnologyMaintenance
:OPS-EMB-07-EmbeddedTechnologyMaintenance rdf:type owl:NamedIndividual ,
                                                   :Security_Operations_Policies ;
                                          :HasWeight 6 ;
                                          rdfs:comment "Mechanisms exist to securely update software and upgrade functionality on embedded devices." .


###  http://FYP-ASHS21/csonto/OPS-EMB-08-ResilienceToOutages
:OPS-EMB-08-ResilienceToOutages rdf:type owl:NamedIndividual ,
                                         :Security_Operations_Policies ;
                                :HasWeight 2 ;
                                rdfs:comment "Mechanisms exist to configure embedded technology to be resilient to data network and power outages." .


###  http://FYP-ASHS21/csonto/OPS-EMB-09-PowerLevelMonitoring
:OPS-EMB-09-PowerLevelMonitoring rdf:type owl:NamedIndividual ,
                                          :Security_Operations_Policies ;
                                 :HasWeight 4 ;
                                 rdfs:comment "Automated mechanisms exist to monitor the power levels of embedded technologies for decreased or excessive power usage, including battery drainage, to investigate for device tampering." .


###  http://FYP-ASHS21/csonto/OPS-EMB-10-EmbeddedTechnologyReviews
:OPS-EMB-10-EmbeddedTechnologyReviews rdf:type owl:NamedIndividual ,
                                               :Security_Operations_Policies ;
                                      :HasWeight 8 ;
                                      rdfs:comment "Mechanisms exist to perform evaluations of deployed embedded technologies as needed, or at least on an annual basis, to ensure that necessary updates to mitigate the risks associated with legacy embedded technologies are identified and implemented." .


###  http://FYP-ASHS21/csonto/OPS-EMB-11-MessageQueuingTelemetryTransport-MQTT-Security
:OPS-EMB-11-MessageQueuingTelemetryTransport-MQTT-Security rdf:type owl:NamedIndividual ,
                                                                    :Security_Operations_Policies ;
                                                           :HasWeight 7 ;
                                                           rdfs:comment "Mechanisms exist to enforce the security of Message Queuing Telemetry Transport (MQTT) traffic." .


###  http://FYP-ASHS21/csonto/OPS-EMB-12-RestrictCommunications
:OPS-EMB-12-RestrictCommunications rdf:type owl:NamedIndividual ,
                                            :Security_Operations_Policies ;
                                   :HasWeight 8 ;
                                   rdfs:comment "Mechanisms exist to require embedded technologies to initiate all communications and drop new, incoming communications." .


###  http://FYP-ASHS21/csonto/OPS-EMB-13-AuthorizedCommunications
:OPS-EMB-13-AuthorizedCommunications rdf:type owl:NamedIndividual ,
                                              :Security_Operations_Policies ;
                                     :HasWeight 8 ;
                                     rdfs:comment "Mechanisms exist to restrict embedded technologies to communicate only with authorized peers and service endpoints." .


###  http://FYP-ASHS21/csonto/OPS-EMB-14-OperatingEnvironmentCertification
:OPS-EMB-14-OperatingEnvironmentCertification rdf:type owl:NamedIndividual ,
                                                       :Security_Operations_Policies ;
                                              :HasWeight 9 ;
                                              rdfs:comment "Mechanisms exist to determine if embedded technologies are certified for secure use in the proposed operating environment." .


###  http://FYP-ASHS21/csonto/OPS-EMB-15-SafetyAssessment
:OPS-EMB-15-SafetyAssessment rdf:type owl:NamedIndividual ,
                                      :Security_Operations_Policies ;
                             :HasWeight 9 ;
                             rdfs:comment "Mechanisms exist to evaluate the safety aspects of embedded technologies via a fault tree analysis, or similar method, to determine possible consequences of misuse, misconfiguration and/or failure." .


###  http://FYP-ASHS21/csonto/OPS-EMB-16-Certificate-BasedAuthentication
:OPS-EMB-16-Certificate-BasedAuthentication rdf:type owl:NamedIndividual ,
                                                     :Security_Operations_Policies ;
                                            :HasWeight 5 ;
                                            rdfs:comment "Mechanisms exist to enforce certificate-based authentication for embedded technologies (e.g., IoT, OT, etc.) and their supporting services." .


###  http://FYP-ASHS21/csonto/OPS-EMB-17-Chip-To-CloudSecurity
:OPS-EMB-17-Chip-To-CloudSecurity rdf:type owl:NamedIndividual ,
                                           :Security_Operations_Policies ;
                                  :HasWeight 6 ;
                                  rdfs:comment "Mechanisms exist to implement embedded technologies that utilize pre-provisioned cloud trust anchors to support secure bootstrap and Zero Touch Provisioning (ZTP)." .


###  http://FYP-ASHS21/csonto/OPS-EMB-18-Real-TimeOperatingSystem-RTOS-Security
:OPS-EMB-18-Real-TimeOperatingSystem-RTOS-Security rdf:type owl:NamedIndividual ,
                                                            :Security_Operations_Policies ;
                                                   :HasWeight 5 ;
                                                   rdfs:comment "Mechanisms exist to ensure embedded technologies utilize a securely configured Real-Time Operating System (RTOS)." .


###  http://FYP-ASHS21/csonto/OPS-EMB-19-SafeOperations
:OPS-EMB-19-SafeOperations rdf:type owl:NamedIndividual ,
                                    :Security_Operations_Policies ;
                           :HasWeight 9 ;
                           rdfs:comment "Mechanisms exist to continuously validate autonomous systems that trigger an automatic state change when safe operation is no longer assured." .


###  http://FYP-ASHS21/csonto/OPS-END-01-EndpointSecurity
:OPS-END-01-EndpointSecurity rdf:type owl:NamedIndividual ,
                                      :Security_Operations_Policies ;
                             :HasWeight 10 ;
                             rdfs:comment "Mechanisms exist to facilitate the implementation of endpoint security controls." .


###  http://FYP-ASHS21/csonto/OPS-END-02-EndpointProtectionMeasures
:OPS-END-02-EndpointProtectionMeasures rdf:type owl:NamedIndividual ,
                                                :Security_Operations_Policies ;
                                       :HasWeight 9 ;
                                       rdfs:comment "Mechanisms exist to protect the confidentiality, integrity, availability and safety of endpoint devices." .


###  http://FYP-ASHS21/csonto/OPS-END-03-ProhibitInstallationWithoutPrivilegedStatus
:OPS-END-03-ProhibitInstallationWithoutPrivilegedStatus rdf:type owl:NamedIndividual ,
                                                                 :Security_Operations_Policies ;
                                                        :HasWeight 9 ;
                                                        rdfs:comment "Automated mechanisms exist to prohibit software installations without explicitly assigned privileged status. " .


###  http://FYP-ASHS21/csonto/OPS-END-03.1-SoftwareInstallationAlerts
:OPS-END-03.1-SoftwareInstallationAlerts rdf:type owl:NamedIndividual ,
                                                  :Security_Operations_Policies ;
                                         :HasWeight 8 ;
                                         rdfs:comment "Mechanisms exist to generate an alert when new software is detected. " .


###  http://FYP-ASHS21/csonto/OPS-END-03.2-GoverningAccessRestrictionforChange
:OPS-END-03.2-GoverningAccessRestrictionforChange rdf:type owl:NamedIndividual ,
                                                           :Security_Operations_Policies ;
                                                  :HasWeight 8 ;
                                                  rdfs:comment "Mechanisms exist to define, document, approve and enforce access restrictions associated with changes to systems." .


###  http://FYP-ASHS21/csonto/OPS-END-04-MaliciousCodeProtection-Anti-Malware-
:OPS-END-04-MaliciousCodeProtection-Anti-Malware- rdf:type owl:NamedIndividual ,
                                                           :Security_Operations_Policies ;
                                                  :HasWeight 10 ;
                                                  rdfs:comment "Mechanisms exist to utilize antimalware technologies to detect and eradicate malicious code." .


###  http://FYP-ASHS21/csonto/OPS-END-04.1-AutomaticAntimalwareSignatureUpdates
:OPS-END-04.1-AutomaticAntimalwareSignatureUpdates rdf:type owl:NamedIndividual ,
                                                            :Security_Operations_Policies ;
                                                   :HasWeight 9 ;
                                                   rdfs:comment "Mechanisms exist to automatically update antimalware technologies, including signature definitions. " .


###  http://FYP-ASHS21/csonto/OPS-END-04.2-DocumentedProtectionMeasures
:OPS-END-04.2-DocumentedProtectionMeasures rdf:type owl:NamedIndividual ,
                                                    :Security_Operations_Policies ;
                                           :HasWeight 3 ;
                                           rdfs:comment "Mechanisms exist to document antimalware technologies." .


###  http://FYP-ASHS21/csonto/OPS-END-04.3-CentralizedManagementofAntimalwareTechnologies
:OPS-END-04.3-CentralizedManagementofAntimalwareTechnologies rdf:type owl:NamedIndividual ,
                                                                      :Security_Operations_Policies ;
                                                             :HasWeight 8 ;
                                                             rdfs:comment "Mechanisms exist to centrally-manage antimalware technologies." .


###  http://FYP-ASHS21/csonto/OPS-END-04.4-Heuristic-Nonsignature-BasedDetection
:OPS-END-04.4-Heuristic-Nonsignature-BasedDetection rdf:type owl:NamedIndividual ,
                                                             :Security_Operations_Policies ;
                                                    :HasWeight 8 ;
                                                    rdfs:comment "Mechanisms exist to utilize heuristic / nonsignature-based antimalware detection capabilities." .


###  http://FYP-ASHS21/csonto/OPS-END-04.5-MalwareProtectionMechanismTesting
:OPS-END-04.5-MalwareProtectionMechanismTesting rdf:type owl:NamedIndividual ,
                                                         :Security_Operations_Policies ;
                                                :HasWeight 5 ;
                                                rdfs:comment "Mechanisms exist to test antimalware technologies by introducing a known benign, non-spreading test case into the system and subsequently verifying that both detection of the test case and associated incident reporting occurs. " .


###  http://FYP-ASHS21/csonto/OPS-END-04.6-EvolvingMalwareThreats
:OPS-END-04.6-EvolvingMalwareThreats rdf:type owl:NamedIndividual ,
                                              :Security_Operations_Policies ;
                                     :HasWeight 3 ;
                                     rdfs:comment "Mechanisms exist to perform periodic evaluations evolving malware threats to assess systems that are generally not considered to be commonly affected by malicious software. " .


###  http://FYP-ASHS21/csonto/OPS-END-04.7-AlwaysOnProtection
:OPS-END-04.7-AlwaysOnProtection rdf:type owl:NamedIndividual ,
                                          :Security_Operations_Policies ;
                                 :HasWeight 9 ;
                                 rdfs:comment "Mechanisms exist to ensure that anti-malware technologies are continuously running in real-time and cannot be disabled or altered by non-privileged users, unless specifically authorized by management on a case-by-case basis for a limited time period. " .


###  http://FYP-ASHS21/csonto/OPS-END-05-SoftwareFirewall
:OPS-END-05-SoftwareFirewall rdf:type owl:NamedIndividual ,
                                      :Security_Operations_Policies ;
                             :HasWeight 9 ;
                             rdfs:comment "Mechanisms exist to utilize host-based firewall software, or a similar technology, on all information systems, where technically feasible." .


###  http://FYP-ASHS21/csonto/OPS-END-06-EndpointFileIntegrityMonitoring-FIM-
:OPS-END-06-EndpointFileIntegrityMonitoring-FIM- rdf:type owl:NamedIndividual ,
                                                          :Security_Operations_Policies ;
                                                 :HasWeight 8 ;
                                                 rdfs:comment "Mechanisms exist to utilize File Integrity Monitor (FIM) technology to detect and report unauthorized changes to system files and configurations." .


###  http://FYP-ASHS21/csonto/OPS-END-06.1-IntegrityChecks
:OPS-END-06.1-IntegrityChecks rdf:type owl:NamedIndividual ,
                                       :Security_Operations_Policies ;
                              :HasWeight 6 ;
                              rdfs:comment "Mechanisms exist to validate configurations through integrity checking of software and firmware." .


###  http://FYP-ASHS21/csonto/OPS-END-06.3-AutomatedNotificationsofIntegrityViolations
:OPS-END-06.3-AutomatedNotificationsofIntegrityViolations rdf:type owl:NamedIndividual ,
                                                                   :Security_Operations_Policies ;
                                                          :HasWeight 5 ;
                                                          rdfs:comment "Automated mechanisms exist to alert incident response personnel upon discovering discrepancies during integrity verification. " .


###  http://FYP-ASHS21/csonto/OPS-END-06.4-AutomatedResponsetoIntegrityViolations
:OPS-END-06.4-AutomatedResponsetoIntegrityViolations rdf:type owl:NamedIndividual ,
                                                              :Security_Operations_Policies ;
                                                     :HasWeight 5 ;
                                                     rdfs:comment "Automated mechanisms exist to implement remediation actions when integrity violations are discovered. " .


###  http://FYP-ASHS21/csonto/OPS-END-06.5-BootProcessIntegrity
:OPS-END-06.5-BootProcessIntegrity rdf:type owl:NamedIndividual ,
                                            :Security_Operations_Policies ;
                                   :HasWeight 5 ;
                                   rdfs:comment "Automated mechanisms exist to verify the integrity of the boot process of information systems." .


###  http://FYP-ASHS21/csonto/OPS-END-06.6-ProtectionofBootFirmware
:OPS-END-06.6-ProtectionofBootFirmware rdf:type owl:NamedIndividual ,
                                                :Security_Operations_Policies ;
                                       :HasWeight 5 ;
                                       rdfs:comment "Automated mechanisms exist to protect the integrity of boot firmware in information systems." .


###  http://FYP-ASHS21/csonto/OPS-END-06.7-BinaryorMachine-ExecutableCode
:OPS-END-06.7-BinaryorMachine-ExecutableCode rdf:type owl:NamedIndividual ,
                                                      :Security_Operations_Policies ;
                                             :HasWeight 5 ;
                                             rdfs:comment "Mechanisms exist to prohibit the use of binary or machine-executable code from sources with limited or no warranty and without access to source code." .


###  http://FYP-ASHS21/csonto/OPS-END-07-HostIntrusionDetectionandPreventionSystems-HIDS-HIPS-
:OPS-END-07-HostIntrusionDetectionandPreventionSystems-HIDS-HIPS- rdf:type owl:NamedIndividual ,
                                                                           :Security_Operations_Policies ;
                                                                  :HasWeight 9 ;
                                                                  rdfs:comment "Mechanisms exist to utilize Host-based Intrusion Detection / Prevention Systems (HIDS / HIPS) on sensitive systems." .


###  http://FYP-ASHS21/csonto/OPS-END-08.1-CentralManagement
:OPS-END-08.1-CentralManagement rdf:type owl:NamedIndividual ,
                                         :Security_Operations_Policies ;
                                :HasWeight 5 ;
                                rdfs:comment "Mechanisms exist to centrally-manage anti-phishing and spam protection technologies." .


###  http://FYP-ASHS21/csonto/OPS-END-08.2-AutomaticSpamandPhishingProtectionUpdates
:OPS-END-08.2-AutomaticSpamandPhishingProtectionUpdates rdf:type owl:NamedIndividual ,
                                                                 :Security_Operations_Policies ;
                                                        :HasWeight 8 ;
                                                        rdfs:comment "Mechanisms exist to automatically update anti-phishing and spam protection technologies when new releases are available in accordance with configuration and change management practices." .


###  http://FYP-ASHS21/csonto/OPS-END-09-TrustedPath
:OPS-END-09-TrustedPath rdf:type owl:NamedIndividual ,
                                 :Security_Operations_Policies ;
                        :HasWeight 9 ;
                        rdfs:comment "Mechanisms exist to establish a trusted communications path between the user and the security functions of the operating system." .


###  http://FYP-ASHS21/csonto/OPS-END-10-MobileCode
:OPS-END-10-MobileCode rdf:type owl:NamedIndividual ,
                                :Security_Operations_Policies ;
                       :HasWeight 4 ;
                       rdfs:comment "Mechanisms exist to address mobile code / operating system-independent applications. " .


###  http://FYP-ASHS21/csonto/OPS-END-11-ThinNodes
:OPS-END-11-ThinNodes rdf:type owl:NamedIndividual ,
                               :Security_Operations_Policies ;
                      :HasWeight 4 ;
                      rdfs:comment "Mechanisms exist to configure thin nodes to have minimal functionality and information storage. " .


###  http://FYP-ASHS21/csonto/OPS-END-13-SensorCapability
:OPS-END-13-SensorCapability rdf:type owl:NamedIndividual ,
                                      :Security_Operations_Policies ;
                             :HasWeight 7 ;
                             rdfs:comment """Mechanisms exist to configure embedded sensors on systems to: 
  Prohibit the remote activation of sensing capabilities; and
  Provide an explicit indication of sensor use to users.""" .


###  http://FYP-ASHS21/csonto/OPS-END-13.1-AuthorizedUse
:OPS-END-13.1-AuthorizedUse rdf:type owl:NamedIndividual ,
                                     :Security_Operations_Policies ;
                            :HasWeight 8 ;
                            rdfs:comment "Mechanisms exist to utilize organization-defined measures so that data or information collected by sensors is only used for authorized purposes." .


###  http://FYP-ASHS21/csonto/OPS-END-13.2-NoticeofCollection
:OPS-END-13.2-NoticeofCollection rdf:type owl:NamedIndividual ,
                                          :Security_Operations_Policies ;
                                 :HasWeight 6 ;
                                 rdfs:comment "Mechanisms exist to notify individuals that Personal Data (PD) is collected by sensors." .


###  http://FYP-ASHS21/csonto/OPS-END-13.3-CollectionMinimization
:OPS-END-13.3-CollectionMinimization rdf:type owl:NamedIndividual ,
                                              :Security_Operations_Policies ;
                                     :HasWeight 8 ;
                                     rdfs:comment "Mechanisms exist to utilize sensors that are configured to minimize the collection of information about individuals." .


###  http://FYP-ASHS21/csonto/OPS-END-13.4-SensorDeliveryVerification
:OPS-END-13.4-SensorDeliveryVerification rdf:type owl:NamedIndividual ,
                                                  :Security_Operations_Policies ;
                                         :HasWeight 4 ;
                                         rdfs:comment "Mechanisms exist to verify embedded technology sensors are configured so that data collected by the sensor(s) is only reported to authorized individuals or roles." .


###  http://FYP-ASHS21/csonto/OPS-END-14-CollaborativeComputingDevices
:OPS-END-14-CollaborativeComputingDevices rdf:type owl:NamedIndividual ,
                                                   :Security_Operations_Policies ;
                                          :HasWeight 9 ;
                                          rdfs:comment """Mechanisms exist to unplug or prohibit the remote activation of collaborative computing devices with the following exceptions: 
  Networked whiteboards; 
  Video teleconference cameras; and 
  Teleconference microphones. """ .


###  http://FYP-ASHS21/csonto/OPS-END-14.1-Disabling-RemovalInSecureWorkAreas
:OPS-END-14.1-Disabling-RemovalInSecureWorkAreas rdf:type owl:NamedIndividual ,
                                                          :Security_Operations_Policies ;
                                                 :HasWeight 5 ;
                                                 rdfs:comment "Mechanisms exist to disable or remove collaborative computing devices from critical information systems and secure work areas." .


###  http://FYP-ASHS21/csonto/OPS-END-14.2-ExplicitlyIndicateCurrentParticipants
:OPS-END-14.2-ExplicitlyIndicateCurrentParticipants rdf:type owl:NamedIndividual ,
                                                             :Security_Operations_Policies ;
                                                    :HasWeight 5 ;
                                                    rdfs:comment "Automated mechanisms exist to provide an explicit indication of current participants in online meetings and teleconferences." .


###  http://FYP-ASHS21/csonto/OPS-END-15-HypervisorAccess
:OPS-END-15-HypervisorAccess rdf:type owl:NamedIndividual ,
                                      :Security_Operations_Policies ;
                             :HasWeight 9 ;
                             rdfs:comment "Mechanisms exist to restrict access to hypervisor management functions or administrative consoles for systems hosting virtualized systems." .


###  http://FYP-ASHS21/csonto/OPS-END-16-RestrictAccessToSecurityFunctions
:OPS-END-16-RestrictAccessToSecurityFunctions rdf:type owl:NamedIndividual ,
                                                       :Security_Operations_Policies ;
                                              :HasWeight 7 ;
                                              rdfs:comment "Mechanisms exist to ensure security functions are restricted to authorized individuals and enforce least privilege control requirements for necessary job functions." .


###  http://FYP-ASHS21/csonto/OPS-END-16.1-Host-BasedSecurityFunctionIsolation
:OPS-END-16.1-Host-BasedSecurityFunctionIsolation rdf:type owl:NamedIndividual ,
                                                           :Security_Operations_Policies ;
                                                  :HasWeight 7 ;
                                                  rdfs:comment "Mechanisms exist to implement underlying software separation mechanisms to facilitate security function isolation. " .


###  http://FYP-ASHS21/csonto/OPS-IAC-01.1-RetainAccessRecords
:OPS-IAC-01.1-RetainAccessRecords rdf:type owl:NamedIndividual ,
                                           :Security_Operations_Policies ;
                                  :HasWeight 3 ;
                                  rdfs:comment "Mechanisms exist to retain a record of personnel accountability to ensure there is a record of all access granted to an individual (system and application-wise), who provided the authorization, when the authorization was granted and when the access was last reviewed." .


###  http://FYP-ASHS21/csonto/OPS-IAC-02.1-GroupAuthentication
:OPS-IAC-02.1-GroupAuthentication rdf:type owl:NamedIndividual ,
                                           :Security_Operations_Policies ;
                                  :HasWeight 7 ;
                                  rdfs:comment "Mechanisms exist to require individuals to be authenticated with an individual authenticator when a group authenticator is utilized. " .


###  http://FYP-ASHS21/csonto/OPS-IAC-02.2-NetworkAccesstoPrivilegedAccounts-ReplayResistant
:OPS-IAC-02.2-NetworkAccesstoPrivilegedAccounts-ReplayResistant rdf:type owl:NamedIndividual ,
                                                                         :Security_Operations_Policies ;
                                                                :HasWeight 9 ;
                                                                rdfs:comment "Automated mechanisms exist to employ replay-resistant network access authentication." .


###  http://FYP-ASHS21/csonto/OPS-IAC-02.3-AcceptanceofPIVCredentials
:OPS-IAC-02.3-AcceptanceofPIVCredentials rdf:type owl:NamedIndividual ,
                                                  :Security_Operations_Policies ;
                                         :HasWeight 2 ;
                                         rdfs:comment "Mechanisms exist to accept and electronically verify organizational Personal Identity Verification (PIV) credentials. " .


###  http://FYP-ASHS21/csonto/OPS-IAC-02.4-Out-of-BandAuthentication-OOBA-
:OPS-IAC-02.4-Out-of-BandAuthentication-OOBA- rdf:type owl:NamedIndividual ,
                                                       :Security_Operations_Policies ;
                                              :HasWeight 5 ;
                                              rdfs:comment "Mechanisms exist to implement Out-of-Band Authentication (OOBA) under specific conditions. " .


###  http://FYP-ASHS21/csonto/OPS-IAC-03.1-AcceptanceofPIVCredentialsfromOtherOrganizations
:OPS-IAC-03.1-AcceptanceofPIVCredentialsfromOtherOrganizations rdf:type owl:NamedIndividual ,
                                                                        :Security_Operations_Policies ;
                                                               :HasWeight 2 ;
                                                               rdfs:comment "Mechanisms exist to accept and electronically verify Personal Identity Verification (PIV) credentials from third-parties." .


###  http://FYP-ASHS21/csonto/OPS-IAC-03.2-AcceptanceofThird-PartyCredentials
:OPS-IAC-03.2-AcceptanceofThird-PartyCredentials rdf:type owl:NamedIndividual ,
                                                          :Security_Operations_Policies ;
                                                 :HasWeight 2 ;
                                                 rdfs:comment "Automated mechanisms exist to accept Federal Identity, Credential and Access Management (FICAM)-approved third-party credentials. " .


###  http://FYP-ASHS21/csonto/OPS-IAC-03.3-UseofFICAM-IssuedProfiles
:OPS-IAC-03.3-UseofFICAM-IssuedProfiles rdf:type owl:NamedIndividual ,
                                                 :Security_Operations_Policies ;
                                        :HasWeight 2 ;
                                        rdfs:comment "Mechanisms exist to conform systems to Federal Identity, Credential and Access Management (FICAM)-issued profiles. " .


###  http://FYP-ASHS21/csonto/OPS-IAC-03.4-Disassociability
:OPS-IAC-03.4-Disassociability rdf:type owl:NamedIndividual ,
                                        :Security_Operations_Policies ;
                               :HasWeight 2 ;
                               rdfs:comment "Mechanisms exist to disassociate user attributes or credential assertion relationships among individuals, credential service providers and relying parties." .


###  http://FYP-ASHS21/csonto/OPS-IAC-03.5-AcceptanceofExternalAuthenticators
:OPS-IAC-03.5-AcceptanceofExternalAuthenticators rdf:type owl:NamedIndividual ,
                                                          :Security_Operations_Policies ;
                                                 :HasWeight 4 ;
                                                 rdfs:comment "Mechanisms exist to restrict the use of external authenticators to those that are National Institute of Standards and Technology (NIST)-compliant and maintain a list of accepted external authenticators." .


###  http://FYP-ASHS21/csonto/OPS-IAC-04.1-DeviceAttestation
:OPS-IAC-04.1-DeviceAttestation rdf:type owl:NamedIndividual ,
                                         :Security_Operations_Policies ;
                                :HasWeight 5 ;
                                rdfs:comment "Mechanisms exist to ensure device identification and authentication is accurate by centrally-managing the joining of systems to the domain as part of the initial asset configuration management process." .


###  http://FYP-ASHS21/csonto/OPS-IAC-05.2-PrivilegedAccessbyNon-OrganizationalUsers
:OPS-IAC-05.2-PrivilegedAccessbyNon-OrganizationalUsers rdf:type owl:NamedIndividual ,
                                                                 :Security_Operations_Policies ;
                                                        :HasWeight 9 ;
                                                        rdfs:comment "Mechanisms exist to prohibit privileged access by non-organizational users." .


###  http://FYP-ASHS21/csonto/OPS-IAC-06-Multi-FactorAuthentication-MFA-
:OPS-IAC-06-Multi-FactorAuthentication-MFA- rdf:type owl:NamedIndividual ,
                                                     :Security_Operations_Policies ;
                                            :HasWeight 9 ;
                                            rdfs:comment """Automated mechanisms exist to enforce Multi-Factor Authentication (MFA) for:
  Remote network access; 
  Third-party systems, applications and/or services; and/ or
  Non-console access to critical systems or systems that store, transmit and/or process sensitive/regulated data.""" .


###  http://FYP-ASHS21/csonto/OPS-IAC-06.1-NetworkAccesstoPrivilegedAccounts
:OPS-IAC-06.1-NetworkAccesstoPrivilegedAccounts rdf:type owl:NamedIndividual ,
                                                         :Security_Operations_Policies ;
                                                :HasWeight 9 ;
                                                rdfs:comment "Mechanisms exist to utilize Multi-Factor Authentication (MFA) to authenticate network access for privileged accounts. " .


###  http://FYP-ASHS21/csonto/OPS-IAC-06.2-NetworkAccesstoNon-PrivilegedAccounts
:OPS-IAC-06.2-NetworkAccesstoNon-PrivilegedAccounts rdf:type owl:NamedIndividual ,
                                                             :Security_Operations_Policies ;
                                                    :HasWeight 7 ;
                                                    rdfs:comment "Mechanisms exist to utilize Multi-Factor Authentication (MFA) to authenticate network access for non-privileged accounts. " .


###  http://FYP-ASHS21/csonto/OPS-IAC-06.3-LocalAccesstoPrivilegedAccounts
:OPS-IAC-06.3-LocalAccesstoPrivilegedAccounts rdf:type owl:NamedIndividual ,
                                                       :Security_Operations_Policies ;
                                              :HasWeight 5 ;
                                              rdfs:comment "Mechanisms exist to utilize Multi-Factor Authentication (MFA) to authenticate local access for privileged accounts. " .


###  http://FYP-ASHS21/csonto/OPS-IAC-06.4-Out-of-BandMulti-FactorAuthentication
:OPS-IAC-06.4-Out-of-BandMulti-FactorAuthentication rdf:type owl:NamedIndividual ,
                                                             :Security_Operations_Policies ;
                                                    :HasWeight 5 ;
                                                    rdfs:comment "Mechanisms exist to implement Multi-Factor Authentication (MFA) for remote access to privileged and non-privileged accounts such that one of the factors is securely provided by a device separate from the system gaining access. " .


###  http://FYP-ASHS21/csonto/OPS-IAC-07.2-TerminationofEmployment
:OPS-IAC-07.2-TerminationofEmployment rdf:type owl:NamedIndividual ,
                                               :Security_Operations_Policies ;
                                      :HasWeight 10 ;
                                      rdfs:comment "Mechanisms exist to revoke user access rights in a timely manner, upon termination of employment or contract." .


###  http://FYP-ASHS21/csonto/OPS-IAC-08-Role-BasedAccessControl-RBAC-
:OPS-IAC-08-Role-BasedAccessControl-RBAC- rdf:type owl:NamedIndividual ,
                                                   :Security_Operations_Policies ;
                                          :HasWeight 9 ;
                                          rdfs:comment "Mechanisms exist to enforce a Role-Based Access Control (RBAC) policy over users and resources that applies need-to-know and fine-grained access control for sensitive/regulated data access." .


###  http://FYP-ASHS21/csonto/OPS-IAC-09-IdentifierManagement-UserNames-
:OPS-IAC-09-IdentifierManagement-UserNames- rdf:type owl:NamedIndividual ,
                                                     :Security_Operations_Policies ;
                                            :HasWeight 9 ;
                                            rdfs:comment "Mechanisms exist to govern naming standards for usernames and systems." .


###  http://FYP-ASHS21/csonto/OPS-IAC-09.1-UserIdentity-ID-Management
:OPS-IAC-09.1-UserIdentity-ID-Management rdf:type owl:NamedIndividual ,
                                                  :Security_Operations_Policies ;
                                         :HasWeight 9 ;
                                         rdfs:comment "Mechanisms exist to ensure proper user identification management for non-consumer users and administrators. " .


###  http://FYP-ASHS21/csonto/OPS-IAC-09.2-IdentityUserStatus
:OPS-IAC-09.2-IdentityUserStatus rdf:type owl:NamedIndividual ,
                                          :Security_Operations_Policies ;
                                 :HasWeight 7 ;
                                 rdfs:comment "Mechanisms exist to identify contractors and other third-party users through unique username characteristics. " .


###  http://FYP-ASHS21/csonto/OPS-IAC-09.3-DynamicManagement
:OPS-IAC-09.3-DynamicManagement rdf:type owl:NamedIndividual ,
                                         :Security_Operations_Policies ;
                                :HasWeight 5 ;
                                rdfs:comment "Mechanisms exist to dynamically manage usernames and system identifiers. " .


###  http://FYP-ASHS21/csonto/OPS-IAC-09.4-Cross-OrganizationManagement
:OPS-IAC-09.4-Cross-OrganizationManagement rdf:type owl:NamedIndividual ,
                                                    :Security_Operations_Policies ;
                                           :HasWeight 5 ;
                                           rdfs:comment "Mechanisms exist to coordinate username identifiers with external organizations for cross-organization management of identifiers. " .


###  http://FYP-ASHS21/csonto/OPS-IAC-09.5-PrivilegedAccountIdentifiers
:OPS-IAC-09.5-PrivilegedAccountIdentifiers rdf:type owl:NamedIndividual ,
                                                    :Security_Operations_Policies ;
                                           :HasWeight 9 ;
                                           rdfs:comment "Mechanisms exist to uniquely manage privileged accounts to identify the account as a privileged user or service." .


###  http://FYP-ASHS21/csonto/OPS-IAC-09.6-PairwisePseudonymousIdentifiers-PPID-
:OPS-IAC-09.6-PairwisePseudonymousIdentifiers-PPID- rdf:type owl:NamedIndividual ,
                                                             :Security_Operations_Policies ;
                                                    :HasWeight 1 ;
                                                    rdfs:comment "Mechanisms exist to generate pairwise pseudonymous identifiers with no identifying information about a data subject to discourage activity tracking and profiling of the data subject." .


###  http://FYP-ASHS21/csonto/OPS-IAC-10-AuthenticatorManagement
:OPS-IAC-10-AuthenticatorManagement rdf:type owl:NamedIndividual ,
                                             :Security_Operations_Policies ;
                                    :HasWeight 10 ;
                                    rdfs:comment "Mechanisms exist to securely manage authenticators for users and devices." .


###  http://FYP-ASHS21/csonto/OPS-IAC-10.1-Password-BasedAuthentication
:OPS-IAC-10.1-Password-BasedAuthentication rdf:type owl:NamedIndividual ,
                                                    :Security_Operations_Policies ;
                                           :HasWeight 9 ;
                                           rdfs:comment "Mechanisms exist to enforce complexity, length and lifespan considerations to ensure strong criteria for password-based authentication." .


###  http://FYP-ASHS21/csonto/OPS-IAC-10.10-ExpirationofCachedAuthenticators
:OPS-IAC-10.10-ExpirationofCachedAuthenticators rdf:type owl:NamedIndividual ,
                                                         :Security_Operations_Policies ;
                                                :HasWeight 5 ;
                                                rdfs:comment "Automated mechanisms exist to prohibit the use of cached authenticators after organization-defined time period." .


###  http://FYP-ASHS21/csonto/OPS-IAC-10.11-PasswordManagers
:OPS-IAC-10.11-PasswordManagers rdf:type owl:NamedIndividual ,
                                         :Security_Operations_Policies ;
                                :HasWeight 8 ;
                                rdfs:comment "Mechanisms exist to protect and store passwords via a password manager tool." .


###  http://FYP-ASHS21/csonto/OPS-IAC-10.12-BiometricAuthentication
:OPS-IAC-10.12-BiometricAuthentication rdf:type owl:NamedIndividual ,
                                                :Security_Operations_Policies ;
                                       :HasWeight 5 ;
                                       rdfs:comment "Mechanisms exist to ensure biometric-based authentication satisfies organization-defined biometric quality requirements for false positives and false negatives." .


###  http://FYP-ASHS21/csonto/OPS-IAC-10.2-PKI-BasedAuthentication
:OPS-IAC-10.2-PKI-BasedAuthentication rdf:type owl:NamedIndividual ,
                                               :Security_Operations_Policies ;
                                      :HasWeight 9 ;
                                      rdfs:comment "Automated mechanisms exist to validate certificates by constructing and verifying a certification path to an accepted trust anchor including checking certificate status information for PKI-based authentication." .


###  http://FYP-ASHS21/csonto/OPS-IAC-10.3-In-PersonorTrustedThird-PartyRegistration
:OPS-IAC-10.3-In-PersonorTrustedThird-PartyRegistration rdf:type owl:NamedIndividual ,
                                                                 :Security_Operations_Policies ;
                                                        :HasWeight 9 ;
                                                        rdfs:comment "Mechanisms exist to conduct in-person or trusted third-party identify verification before user accounts for third-parties are created." .


###  http://FYP-ASHS21/csonto/OPS-IAC-10.4-AutomatedSupportForPasswordStrength
:OPS-IAC-10.4-AutomatedSupportForPasswordStrength rdf:type owl:NamedIndividual ,
                                                           :Security_Operations_Policies ;
                                                  :HasWeight 5 ;
                                                  rdfs:comment "Automated mechanisms exist to determine if password authenticators are sufficiently strong enough to satisfy organization-defined password length and complexity requirements. " .


###  http://FYP-ASHS21/csonto/OPS-IAC-10.5-ProtectionofAuthenticators
:OPS-IAC-10.5-ProtectionofAuthenticators rdf:type owl:NamedIndividual ,
                                                  :Security_Operations_Policies ;
                                         :HasWeight 10 ;
                                         rdfs:comment "Mechanisms exist to protect authenticators commensurate with the sensitivity of the information to which use of the authenticator permits access. " .


###  http://FYP-ASHS21/csonto/OPS-IAC-10.6-NoEmbeddedUnencryptedStaticAuthenticators
:OPS-IAC-10.6-NoEmbeddedUnencryptedStaticAuthenticators rdf:type owl:NamedIndividual ,
                                                                 :Security_Operations_Policies ;
                                                        :HasWeight 10 ;
                                                        rdfs:comment "Mechanisms exist to ensure that unencrypted, static authenticators are not embedded in applications, scripts or stored on function keys. " .


###  http://FYP-ASHS21/csonto/OPS-IAC-10.7-HardwareToken-BasedAuthentication
:OPS-IAC-10.7-HardwareToken-BasedAuthentication rdf:type owl:NamedIndividual ,
                                                         :Security_Operations_Policies ;
                                                :HasWeight 9 ;
                                                rdfs:comment "Automated mechanisms exist to ensure organization-defined token quality requirements are satisfied for hardware token-based authentication." .


###  http://FYP-ASHS21/csonto/OPS-IAC-10.8-Vendor-SuppliedDefaults
:OPS-IAC-10.8-Vendor-SuppliedDefaults rdf:type owl:NamedIndividual ,
                                               :Security_Operations_Policies ;
                                      :HasWeight 10 ;
                                      rdfs:comment "Mechanisms exist to ensure vendor-supplied defaults are changed as part of the installation process." .


###  http://FYP-ASHS21/csonto/OPS-IAC-10.9-MultipleInformationSystemAccounts
:OPS-IAC-10.9-MultipleInformationSystemAccounts rdf:type owl:NamedIndividual ,
                                                         :Security_Operations_Policies ;
                                                :HasWeight 5 ;
                                                rdfs:comment "Mechanisms exist to implement security safeguards to manage the risk of compromise due to individuals having accounts on multiple information systems." .


###  http://FYP-ASHS21/csonto/OPS-IAC-11-AuthenticatorFeedback
:OPS-IAC-11-AuthenticatorFeedback rdf:type owl:NamedIndividual ,
                                           :Security_Operations_Policies ;
                                  :HasWeight 6 ;
                                  rdfs:comment "Mechanisms exist to obscure the feedback of authentication information during the authentication process to protect the information from possible exploitation/use by unauthorized individuals. " .


###  http://FYP-ASHS21/csonto/OPS-IAC-12-CryptographicModuleAuthentication
:OPS-IAC-12-CryptographicModuleAuthentication rdf:type owl:NamedIndividual ,
                                                       :Security_Operations_Policies ;
                                              :HasWeight 8 ;
                                              rdfs:comment "Mechanisms exist to ensure cryptographic modules adhere to applicable statutory, regulatory and contractual requirements for security strength." .


###  http://FYP-ASHS21/csonto/OPS-IAC-12.1-HardwareSecurityModules-HSM-
:OPS-IAC-12.1-HardwareSecurityModules-HSM- rdf:type owl:NamedIndividual ,
                                                    :Security_Operations_Policies ;
                                           :HasWeight 3 ;
                                           rdfs:comment "Automated mechanisms exist to utilize Hardware Security Modules (HSM) to protect authenticators on which the component relies. " .


###  http://FYP-ASHS21/csonto/OPS-IAC-13.1-SingleSign-On-SSO-
:OPS-IAC-13.1-SingleSign-On-SSO- rdf:type owl:NamedIndividual ,
                                          :Security_Operations_Policies ;
                                 :HasWeight 5 ;
                                 rdfs:comment "Mechanisms exist to provide a Single Sign-On (SSO) capability to the organization's systems and services." .


###  http://FYP-ASHS21/csonto/OPS-IAC-13.2-FederatedCredentialManagement
:OPS-IAC-13.2-FederatedCredentialManagement rdf:type owl:NamedIndividual ,
                                                     :Security_Operations_Policies ;
                                            :HasWeight 4 ;
                                            rdfs:comment "Mechanisms exist to federate credentials to allow cross-organization authentication of individuals and devices." .


###  http://FYP-ASHS21/csonto/OPS-IAC-14-Re-Authentication
:OPS-IAC-14-Re-Authentication rdf:type owl:NamedIndividual ,
                                       :Security_Operations_Policies ;
                              :HasWeight 8 ;
                              rdfs:comment "Mechanisms exist to force users and devices to re-authenticate according to organization-defined circumstances that necessitate re-authentication. " .


###  http://FYP-ASHS21/csonto/OPS-IAC-15-AccountManagement
:OPS-IAC-15-AccountManagement rdf:type owl:NamedIndividual ,
                                       :Security_Operations_Policies ;
                              :HasWeight 10 ;
                              rdfs:comment "Mechanisms exist to proactively govern account management of individual, group, system, service, application, guest and temporary accounts." .


###  http://FYP-ASHS21/csonto/OPS-IAC-15.1-AutomatedSystemAccountManagement
:OPS-IAC-15.1-AutomatedSystemAccountManagement rdf:type owl:NamedIndividual ,
                                                        :Security_Operations_Policies ;
                                               :HasWeight 5 ;
                                               rdfs:comment "Automated mechanisms exist to support the management of system accounts. " .


###  http://FYP-ASHS21/csonto/OPS-IAC-15.2-RemovalofTemporary-EmergencyAccounts
:OPS-IAC-15.2-RemovalofTemporary-EmergencyAccounts rdf:type owl:NamedIndividual ,
                                                            :Security_Operations_Policies ;
                                                   :HasWeight 9 ;
                                                   rdfs:comment "Automated mechanisms exist to disable or remove temporary and emergency accounts after an organization-defined time period for each type of account. " .


###  http://FYP-ASHS21/csonto/OPS-IAC-15.3-DisableInactiveAccounts
:OPS-IAC-15.3-DisableInactiveAccounts rdf:type owl:NamedIndividual ,
                                               :Security_Operations_Policies ;
                                      :HasWeight 10 ;
                                      rdfs:comment "Automated mechanisms exist to disable inactive accounts after an organization-defined time period. " .


###  http://FYP-ASHS21/csonto/OPS-IAC-15.4-AutomatedAuditActions
:OPS-IAC-15.4-AutomatedAuditActions rdf:type owl:NamedIndividual ,
                                             :Security_Operations_Policies ;
                                    :HasWeight 5 ;
                                    rdfs:comment "Automated mechanisms exist to audit account creation, modification, enabling, disabling and removal actions and notify organization-defined personnel or roles. " .


###  http://FYP-ASHS21/csonto/OPS-IAC-15.5-RestrictionsonSharedGroups-Accounts
:OPS-IAC-15.5-RestrictionsonSharedGroups-Accounts rdf:type owl:NamedIndividual ,
                                                           :Security_Operations_Policies ;
                                                  :HasWeight 10 ;
                                                  rdfs:comment "Mechanisms exist to authorize the use of shared/group accounts only under certain organization-defined conditions." .


###  http://FYP-ASHS21/csonto/OPS-IAC-15.6-AccountDisablingforHighRiskIndividuals
:OPS-IAC-15.6-AccountDisablingforHighRiskIndividuals rdf:type owl:NamedIndividual ,
                                                              :Security_Operations_Policies ;
                                                     :HasWeight 10 ;
                                                     rdfs:comment "Mechanisms exist to disable accounts immediately upon notification for users posing a significant risk to the organization." .


###  http://FYP-ASHS21/csonto/OPS-IAC-15.7-SystemAccounts
:OPS-IAC-15.7-SystemAccounts rdf:type owl:NamedIndividual ,
                                      :Security_Operations_Policies ;
                             :HasWeight 10 ;
                             rdfs:comment "Mechanisms exist to review all system accounts and disable any account that cannot be associated with a business process and owner. " .


###  http://FYP-ASHS21/csonto/OPS-IAC-15.8-UsageConditions
:OPS-IAC-15.8-UsageConditions rdf:type owl:NamedIndividual ,
                                       :Security_Operations_Policies ;
                              :HasWeight 5 ;
                              rdfs:comment "Automated mechanisms exist to enforce usage conditions for users and/or roles." .


###  http://FYP-ASHS21/csonto/OPS-IAC-15.9-EmergencyAccounts
:OPS-IAC-15.9-EmergencyAccounts rdf:type owl:NamedIndividual ,
                                         :Security_Operations_Policies ;
                                :HasWeight 5 ;
                                rdfs:comment "Mechanisms exist to establish and control \"emergency access only\" accounts." .


###  http://FYP-ASHS21/csonto/OPS-IAC-16-PrivilegedAccountManagement-PAM-
:OPS-IAC-16-PrivilegedAccountManagement-PAM- rdf:type owl:NamedIndividual ,
                                                      :Security_Operations_Policies ;
                                             :HasWeight 10 ;
                                             rdfs:comment "Mechanisms exist to restrict and control privileged access rights for users and services." .


###  http://FYP-ASHS21/csonto/OPS-IAC-16.1-PrivilegedAccountInventories
:OPS-IAC-16.1-PrivilegedAccountInventories rdf:type owl:NamedIndividual ,
                                                    :Security_Operations_Policies ;
                                           :HasWeight 10 ;
                                           rdfs:comment "Mechanisms exist to inventory all privileged accounts and validate that each person with elevated privileges is authorized by the appropriate level of organizational management. " .


###  http://FYP-ASHS21/csonto/OPS-IAC-16.2-PrivilegedAccountSeparation
:OPS-IAC-16.2-PrivilegedAccountSeparation rdf:type owl:NamedIndividual ,
                                                   :Security_Operations_Policies ;
                                          :HasWeight 4 ;
                                          rdfs:comment "Mechanisms exist to separate privileged accounts between infrastructure environments to reduce the risk of a compromise in one infrastructure environment from laterally affecting other infrastructure environments." .


###  http://FYP-ASHS21/csonto/OPS-IAC-17-PeriodicReviewofAccountPrivileges
:OPS-IAC-17-PeriodicReviewofAccountPrivileges rdf:type owl:NamedIndividual ,
                                                       :Security_Operations_Policies ;
                                              :HasWeight 10 ;
                                              rdfs:comment "Mechanisms exist to periodically-review the privileges assigned to individuals and service accounts to validate the need for such privileges and reassign or remove unnecessary privileges, as necessary." .


###  http://FYP-ASHS21/csonto/OPS-IAC-18-UserResponsibilitiesforAccountManagement
:OPS-IAC-18-UserResponsibilitiesforAccountManagement rdf:type owl:NamedIndividual ,
                                                              :Security_Operations_Policies ;
                                                     :HasWeight 10 ;
                                                     rdfs:comment "Mechanisms exist to compel users to follow accepted practices in the use of authentication mechanisms (e.g., passwords, passphrases, physical or logical security tokens, smart cards, certificates, etc.). " .


###  http://FYP-ASHS21/csonto/OPS-IAC-19-CredentialSharing
:OPS-IAC-19-CredentialSharing rdf:type owl:NamedIndividual ,
                                       :Security_Operations_Policies ;
                              :HasWeight 10 ;
                              rdfs:comment "Mechanisms exist to prevent the sharing of generic IDs, passwords or other generic authentication methods." .


###  http://FYP-ASHS21/csonto/OPS-IAC-20-AccessEnforcement
:OPS-IAC-20-AccessEnforcement rdf:type owl:NamedIndividual ,
                                       :Security_Operations_Policies ;
                              :HasWeight 10 ;
                              rdfs:comment "Mechanisms exist to enforce Logical Access Control (LAC) permissions that conform to the principle of \"least privilege.\"" .


###  http://FYP-ASHS21/csonto/OPS-IAC-20.1-AccessToSensitiveData
:OPS-IAC-20.1-AccessToSensitiveData rdf:type owl:NamedIndividual ,
                                             :Security_Operations_Policies ;
                                    :HasWeight 10 ;
                                    rdfs:comment "Mechanisms exist to limit access to sensitive/regulated data to only those individuals whose job requires such access. " .


###  http://FYP-ASHS21/csonto/OPS-IAC-20.2-DatabaseAccess
:OPS-IAC-20.2-DatabaseAccess rdf:type owl:NamedIndividual ,
                                      :Security_Operations_Policies ;
                             :HasWeight 10 ;
                             rdfs:comment "Mechanisms exist to restrict access to databases containing sensitive/regulated data to only necessary services or those individuals whose job requires such access. " .


###  http://FYP-ASHS21/csonto/OPS-IAC-20.3-UseofPrivilegedUtilityPrograms
:OPS-IAC-20.3-UseofPrivilegedUtilityPrograms rdf:type owl:NamedIndividual ,
                                                      :Security_Operations_Policies ;
                                             :HasWeight 9 ;
                                             rdfs:comment "Mechanisms exist to restrict and tightly control utility programs that are capable of overriding system and application controls." .


###  http://FYP-ASHS21/csonto/OPS-IAC-20.4-DedicatedAdministrativeMachines
:OPS-IAC-20.4-DedicatedAdministrativeMachines rdf:type owl:NamedIndividual ,
                                                       :Security_Operations_Policies ;
                                              :HasWeight 8 ;
                                              rdfs:comment "Mechanisms exist to restrict executing administrative tasks or tasks requiring elevated access to a dedicated machine." .


###  http://FYP-ASHS21/csonto/OPS-IAC-20.5-DualAuthorizationforPrivilegedCommands
:OPS-IAC-20.5-DualAuthorizationforPrivilegedCommands rdf:type owl:NamedIndividual ,
                                                              :Security_Operations_Policies ;
                                                     :HasWeight 5 ;
                                                     rdfs:comment "Automated mechanisms exist to enforce dual authorization for privileged commands." .


###  http://FYP-ASHS21/csonto/OPS-IAC-20.6-RevocationofAccessAuthorizations
:OPS-IAC-20.6-RevocationofAccessAuthorizations rdf:type owl:NamedIndividual ,
                                                        :Security_Operations_Policies ;
                                               :HasWeight 9 ;
                                               rdfs:comment "Mechanisms exist to revoke logical and physical access authorizations." .


###  http://FYP-ASHS21/csonto/OPS-IAC-21-LeastPrivilege
:OPS-IAC-21-LeastPrivilege rdf:type owl:NamedIndividual ,
                                    :Security_Operations_Policies ;
                           :HasWeight 10 ;
                           rdfs:comment "Mechanisms exist to utilize the concept of least privilege, allowing only authorized access to processes necessary to accomplish assigned tasks in accordance with organizational business functions. " .


###  http://FYP-ASHS21/csonto/OPS-IAC-21.1-AuthorizeAccesstoSecurityFunctions
:OPS-IAC-21.1-AuthorizeAccesstoSecurityFunctions rdf:type owl:NamedIndividual ,
                                                          :Security_Operations_Policies ;
                                                 :HasWeight 9 ;
                                                 rdfs:comment "Mechanisms exist to limit access to security functions to explicitly-authorized privileged users." .


###  http://FYP-ASHS21/csonto/OPS-IAC-21.2-Non-PrivilegedAccessforNon-SecurityFunctions
:OPS-IAC-21.2-Non-PrivilegedAccessforNon-SecurityFunctions rdf:type owl:NamedIndividual ,
                                                                    :Security_Operations_Policies ;
                                                           :HasWeight 9 ;
                                                           rdfs:comment """Mechanisms exist to prohibit privileged users from using privileged accounts, while performing non-security functions. 
""" .


###  http://FYP-ASHS21/csonto/OPS-IAC-21.3-PrivilegedAccounts
:OPS-IAC-21.3-PrivilegedAccounts rdf:type owl:NamedIndividual ,
                                          :Security_Operations_Policies ;
                                 :HasWeight 10 ;
                                 rdfs:comment "Mechanisms exist to restrict the assignment of privileged accounts to organization-defined personnel or roles without management approval." .


###  http://FYP-ASHS21/csonto/OPS-IAC-21.4-AuditingUseofPrivilegedFunctions
:OPS-IAC-21.4-AuditingUseofPrivilegedFunctions rdf:type owl:NamedIndividual ,
                                                        :Security_Operations_Policies ;
                                               :HasWeight 9 ;
                                               rdfs:comment "Mechanisms exist to audit the execution of privileged functions. " .


###  http://FYP-ASHS21/csonto/OPS-IAC-21.5-ProhibitNon-PrivilegedUsersfromExecutingPrivilegedFunctions
:OPS-IAC-21.5-ProhibitNon-PrivilegedUsersfromExecutingPrivilegedFunctions rdf:type owl:NamedIndividual ,
                                                                                   :Security_Operations_Policies ;
                                                                          :HasWeight 9 ;
                                                                          rdfs:comment "Mechanisms exist to prevent non-privileged users from executing privileged functions to include disabling, circumventing or altering implemented security safeguards / countermeasures. " .


###  http://FYP-ASHS21/csonto/OPS-IAC-21.6-NetworkAccesstoPrivilegedCommands
:OPS-IAC-21.6-NetworkAccesstoPrivilegedCommands rdf:type owl:NamedIndividual ,
                                                         :Security_Operations_Policies ;
                                                :HasWeight 5 ;
                                                rdfs:comment "Mechanisms exist to authorize remote access to perform privileged commands on critical systems or where sensitive/regulated data is stored, transmitted and/or processed only for compelling operational needs." .


###  http://FYP-ASHS21/csonto/OPS-IAC-21.7-PrivilegeLevelsforCodeExecution
:OPS-IAC-21.7-PrivilegeLevelsforCodeExecution rdf:type owl:NamedIndividual ,
                                                       :Security_Operations_Policies ;
                                              :HasWeight 5 ;
                                              rdfs:comment "Automated mechanisms exist to prevent applications from executing at higher privilege levels than the user's privileges. " .


###  http://FYP-ASHS21/csonto/OPS-IAC-22-AccountLockout
:OPS-IAC-22-AccountLockout rdf:type owl:NamedIndividual ,
                                    :Security_Operations_Policies ;
                           :HasWeight 9 ;
                           rdfs:comment "Mechanisms exist to enforce a limit for consecutive invalid login attempts by a user during an organization-defined time period and automatically locks the account when the maximum number of unsuccessful attempts is exceeded." .


###  http://FYP-ASHS21/csonto/OPS-IAC-23-ConcurrentSessionControl
:OPS-IAC-23-ConcurrentSessionControl rdf:type owl:NamedIndividual ,
                                              :Security_Operations_Policies ;
                                     :HasWeight 6 ;
                                     rdfs:comment "Mechanisms exist to limit the number of concurrent sessions for each system account. " .


###  http://FYP-ASHS21/csonto/OPS-IAC-24-SessionLock
:OPS-IAC-24-SessionLock rdf:type owl:NamedIndividual ,
                                 :Security_Operations_Policies ;
                        :HasWeight 9 ;
                        rdfs:comment "Mechanisms exist to initiate a session lock after an organization-defined time period of inactivity, or upon receiving a request from a user and retain the session lock until the user reestablishes access using established identification and authentication methods." .


###  http://FYP-ASHS21/csonto/OPS-IAC-24.1-Pattern-HidingDisplays
:OPS-IAC-24.1-Pattern-HidingDisplays rdf:type owl:NamedIndividual ,
                                              :Security_Operations_Policies ;
                                     :HasWeight 9 ;
                                     rdfs:comment "Mechanisms exist to implement pattern-hiding displays to conceal information previously visible on the display during the session lock. " .


###  http://FYP-ASHS21/csonto/OPS-IAC-25-SessionTermination
:OPS-IAC-25-SessionTermination rdf:type owl:NamedIndividual ,
                                        :Security_Operations_Policies ;
                               :HasWeight 9 ;
                               rdfs:comment "Automated mechanisms exist to log out users, both locally on the network and for remote sessions, at the end of the session or after an organization-defined period of inactivity. " .


###  http://FYP-ASHS21/csonto/OPS-IAC-25.1-User-InitiatedLogouts-MessageDisplays
:OPS-IAC-25.1-User-InitiatedLogouts-MessageDisplays rdf:type owl:NamedIndividual ,
                                                             :Security_Operations_Policies ;
                                                    :HasWeight 5 ;
                                                    rdfs:comment "Mechanisms exist to provide a logout capability and display an explicit logout message to users indicating the reliable termination of the session. " .


###  http://FYP-ASHS21/csonto/OPS-IAC-26-PermittedActionsWithoutIdentificationorAuthorization
:OPS-IAC-26-PermittedActionsWithoutIdentificationorAuthorization rdf:type owl:NamedIndividual ,
                                                                          :Security_Operations_Policies ;
                                                                 :HasWeight 8 ;
                                                                 rdfs:comment "Mechanisms exist to identify and document the supporting rationale for specific user actions that can be performed on a system without identification or authentication." .


###  http://FYP-ASHS21/csonto/OPS-IAC-27-ReferenceMonitor
:OPS-IAC-27-ReferenceMonitor rdf:type owl:NamedIndividual ,
                                      :Security_Operations_Policies ;
                             :HasWeight 1 ;
                             rdfs:comment "Mechanisms exist to implement a reference monitor that is tamperproof, always-invoked, small enough to be subject to analysis / testing and the completeness of which can be assured." .


###  http://FYP-ASHS21/csonto/OPS-IAC-28-IdentityProofing-IdentityVerification-
:OPS-IAC-28-IdentityProofing-IdentityVerification- rdf:type owl:NamedIndividual ,
                                                            :Security_Operations_Policies ;
                                                   :HasWeight 10 ;
                                                   rdfs:comment "Mechanisms exist to verify the identity of a user before modifying any permissions or authentication factor." .


###  http://FYP-ASHS21/csonto/OPS-IAC-28.1-ManagementApprovalForNeworChangedAccounts
:OPS-IAC-28.1-ManagementApprovalForNeworChangedAccounts rdf:type owl:NamedIndividual ,
                                                                 :Security_Operations_Policies ;
                                                        :HasWeight 10 ;
                                                        rdfs:comment "Mechanisms exist to ensure management approvals are required for new accounts or changes in permissions to existing accounts." .


###  http://FYP-ASHS21/csonto/OPS-IAC-28.2-IdentityEvidence
:OPS-IAC-28.2-IdentityEvidence rdf:type owl:NamedIndividual ,
                                        :Security_Operations_Policies ;
                               :HasWeight 5 ;
                               rdfs:comment "Mechanisms exist to require evidence of individual identification to be presented to the registration authority." .


###  http://FYP-ASHS21/csonto/OPS-IAC-28.5-AddressConfirmation
:OPS-IAC-28.5-AddressConfirmation rdf:type owl:NamedIndividual ,
                                           :Security_Operations_Policies ;
                                  :HasWeight 1 ;
                                  rdfs:comment "Mechanisms exist to require that a notice of proofing be delivered through an out-of-band channel to verify the user's address (physical or digital)." .


###  http://FYP-ASHS21/csonto/OPS-IAC-29-Attribute-BasedAccessControl-ABAC-
:OPS-IAC-29-Attribute-BasedAccessControl-ABAC- rdf:type owl:NamedIndividual ,
                                                        :Security_Operations_Policies ;
                                               :HasWeight 5 ;
                                               rdfs:comment "Mechanisms exist to enforce Attribute-Based Access Control (ABAC) for policy-driven, dynamic authorizations that supports the secure sharing of information." .


###  http://FYP-ASHS21/csonto/OPS-IRO-01-IncidentResponseOperations
:OPS-IRO-01-IncidentResponseOperations rdf:type owl:NamedIndividual ,
                                                :Security_Operations_Policies ;
                                       :HasWeight 9 ;
                                       rdfs:comment "Mechanisms exist to implement and govern processes and documentation to facilitate an organization-wide response capability for cybersecurity & data privacy-related incidents." .


###  http://FYP-ASHS21/csonto/OPS-IRO-02-IncidentHandling
:OPS-IRO-02-IncidentHandling rdf:type owl:NamedIndividual ,
                                      :Security_Operations_Policies ;
                             :HasWeight 10 ;
                             rdfs:comment "Mechanisms exist to cover the preparation, automated detection or intake of incident reporting, analysis, containment, eradication and recovery." .


###  http://FYP-ASHS21/csonto/OPS-IRO-02.1-AutomatedIncidentHandlingProcesses
:OPS-IRO-02.1-AutomatedIncidentHandlingProcesses rdf:type owl:NamedIndividual ,
                                                          :Security_Operations_Policies ;
                                                 :HasWeight 1 ;
                                                 rdfs:comment "Automated mechanisms exist to support the incident handling process. " .


###  http://FYP-ASHS21/csonto/OPS-IRO-02.2-InsiderThreatResponseCapability
:OPS-IRO-02.2-InsiderThreatResponseCapability rdf:type owl:NamedIndividual ,
                                                       :Security_Operations_Policies ;
                                              :HasWeight 5 ;
                                              rdfs:comment "Mechanisms exist to implement and govern an insider threat program. " .


###  http://FYP-ASHS21/csonto/OPS-IRO-02.3-DynamicReconfiguration
:OPS-IRO-02.3-DynamicReconfiguration rdf:type owl:NamedIndividual ,
                                              :Security_Operations_Policies ;
                                     :HasWeight 5 ;
                                     rdfs:comment "Automated mechanisms exist to dynamically reconfigure information system components as part of the incident response capability. " .


###  http://FYP-ASHS21/csonto/OPS-IRO-02.5-CorrelationwithExternalOrganizations
:OPS-IRO-02.5-CorrelationwithExternalOrganizations rdf:type owl:NamedIndividual ,
                                                            :Security_Operations_Policies ;
                                                   :HasWeight 5 ;
                                                   rdfs:comment "Mechanisms exist to coordinate with approved third-parties to achieve a cross-organization perspective on incident awareness and more effective incident responses. " .


###  http://FYP-ASHS21/csonto/OPS-IRO-02.6-AutomaticDisablingofSystem
:OPS-IRO-02.6-AutomaticDisablingofSystem rdf:type owl:NamedIndividual ,
                                                  :Security_Operations_Policies ;
                                         :HasWeight 6 ;
                                         rdfs:comment "Mechanisms exist to automatically disable systems, upon detection of a possible incident that meets organizational criteria, which allows for forensic analysis to be performed." .


###  http://FYP-ASHS21/csonto/OPS-IRO-03-IndicatorsofCompromise-IOC-
:OPS-IRO-03-IndicatorsofCompromise-IOC- rdf:type owl:NamedIndividual ,
                                                 :Security_Operations_Policies ;
                                        :HasWeight 8 ;
                                        rdfs:comment "Mechanisms exist to define specific Indicators of Compromise (IOC) to identify the signs of potential cybersecurity events." .


###  http://FYP-ASHS21/csonto/OPS-IRO-04-IncidentResponsePlan-IRP-
:OPS-IRO-04-IncidentResponsePlan-IRP- rdf:type owl:NamedIndividual ,
                                               :Security_Operations_Policies ;
                                      :HasWeight 9 ;
                                      rdfs:comment "Mechanisms exist to maintain and make available a current and viable Incident Response Plan (IRP) to all stakeholders." .


###  http://FYP-ASHS21/csonto/OPS-IRO-04.1-DataBreach
:OPS-IRO-04.1-DataBreach rdf:type owl:NamedIndividual ,
                                  :Security_Operations_Policies ;
                         :HasWeight 8 ;
                         rdfs:comment "Mechanisms exist to address data breaches, or other incidents involving the unauthorized disclosure of sensitive or regulated data, according to applicable laws, regulations and contractual obligations. " .


###  http://FYP-ASHS21/csonto/OPS-IRO-04.2-IRPUpdate
:OPS-IRO-04.2-IRPUpdate rdf:type owl:NamedIndividual ,
                                 :Security_Operations_Policies ;
                        :HasWeight 8 ;
                        rdfs:comment "Mechanisms exist to regularly review and modify incident response practices to incorporate lessons learned, business process changes and industry developments, as necessary." .


###  http://FYP-ASHS21/csonto/OPS-IRO-04.3-ContinuousIncidentResponseImprovements
:OPS-IRO-04.3-ContinuousIncidentResponseImprovements rdf:type owl:NamedIndividual ,
                                                              :Security_Operations_Policies ;
                                                     :HasWeight 3 ;
                                                     rdfs:comment """Mechanisms exist to use qualitative and quantitative data from incident response testing to: 
Determine the effectiveness of incident response processes;
Continuously improve incident response processes; and
Provide incident response measures and metrics that are accurate, consistent, and in a reproducible format.""" .


###  http://FYP-ASHS21/csonto/OPS-IRO-05-IncidentResponseTraining
:OPS-IRO-05-IncidentResponseTraining rdf:type owl:NamedIndividual ,
                                              :Security_Operations_Policies ;
                                     :HasWeight 9 ;
                                     rdfs:comment "Mechanisms exist to train personnel in their incident response roles and responsibilities." .


###  http://FYP-ASHS21/csonto/OPS-IRO-05.1-SimulatedIncidents
:OPS-IRO-05.1-SimulatedIncidents rdf:type owl:NamedIndividual ,
                                          :Security_Operations_Policies ;
                                 :HasWeight 5 ;
                                 rdfs:comment "Mechanisms exist to incorporate simulated events into incident response training to facilitate effective response by personnel in crisis situations." .


###  http://FYP-ASHS21/csonto/OPS-IRO-05.2-AutomatedIncidentResponseTrainingEnvironments
:OPS-IRO-05.2-AutomatedIncidentResponseTrainingEnvironments rdf:type owl:NamedIndividual ,
                                                                     :Security_Operations_Policies ;
                                                            :HasWeight 5 ;
                                                            rdfs:comment "Automated mechanisms exist to provide a more thorough and realistic incident response training environment." .


###  http://FYP-ASHS21/csonto/OPS-IRO-06-IncidentResponseTesting
:OPS-IRO-06-IncidentResponseTesting rdf:type owl:NamedIndividual ,
                                             :Security_Operations_Policies ;
                                    :HasWeight 9 ;
                                    rdfs:comment "Mechanisms exist to formally test incident response capabilities through realistic exercises to determine the operational effectiveness of those capabilities." .


###  http://FYP-ASHS21/csonto/OPS-IRO-06.1-CoordinationwithRelatedPlans
:OPS-IRO-06.1-CoordinationwithRelatedPlans rdf:type owl:NamedIndividual ,
                                                    :Security_Operations_Policies ;
                                           :HasWeight 7 ;
                                           rdfs:comment "Mechanisms exist to coordinate incident response testing with organizational elements responsible for related plans. " .


###  http://FYP-ASHS21/csonto/OPS-IRO-07-IntegratedSecurityIncidentResponseTeam-ISIRT-
:OPS-IRO-07-IntegratedSecurityIncidentResponseTeam-ISIRT- rdf:type owl:NamedIndividual ,
                                                                   :Security_Operations_Policies ;
                                                          :HasWeight 9 ;
                                                          rdfs:comment "Mechanisms exist to establish an integrated team of cybersecurity, IT and business function representatives that are capable of addressing cybersecurity & data privacy incident response operations." .


###  http://FYP-ASHS21/csonto/OPS-IRO-09-SituationalAwarenessForIncidents
:OPS-IRO-09-SituationalAwarenessForIncidents rdf:type owl:NamedIndividual ,
                                                      :Security_Operations_Policies ;
                                             :HasWeight 8 ;
                                             rdfs:comment "Mechanisms exist to document, monitor and report the status of cybersecurity & data privacy incidents to internal stakeholders all the way through the resolution of the incident." .


###  http://FYP-ASHS21/csonto/OPS-IRO-10-IncidentStakeholderReporting
:OPS-IRO-10-IncidentStakeholderReporting rdf:type owl:NamedIndividual ,
                                                  :Security_Operations_Policies ;
                                         :HasWeight 9 ;
                                         rdfs:comment """Mechanisms exist to timely-report incidents to applicable:
  Internal stakeholders; 
  Affected clients & third-parties; and
  Regulatory authorities.""" .


###  http://FYP-ASHS21/csonto/OPS-IRO-10.1-AutomatedReporting
:OPS-IRO-10.1-AutomatedReporting rdf:type owl:NamedIndividual ,
                                          :Security_Operations_Policies ;
                                 :HasWeight 9 ;
                                 rdfs:comment "Automated mechanisms exist to assist in the reporting of cybersecurity & data privacy incidents." .


###  http://FYP-ASHS21/csonto/OPS-IRO-10.2-CyberIncidentReportingforSensitiveData
:OPS-IRO-10.2-CyberIncidentReportingforSensitiveData rdf:type owl:NamedIndividual ,
                                                              :Security_Operations_Policies ;
                                                     :HasWeight 9 ;
                                                     rdfs:comment "Mechanisms exist to report sensitive/regulated data incidents in a timely manner." .


###  http://FYP-ASHS21/csonto/OPS-IRO-10.3-VulnerabilitiesRelatedToIncidents
:OPS-IRO-10.3-VulnerabilitiesRelatedToIncidents rdf:type owl:NamedIndividual ,
                                                         :Security_Operations_Policies ;
                                                :HasWeight 8 ;
                                                rdfs:comment "Mechanisms exist to report system vulnerabilities associated with reported cybersecurity & data privacy incidents to organization-defined personnel or roles." .


###  http://FYP-ASHS21/csonto/OPS-IRO-10.4-SupplyChainCoordination
:OPS-IRO-10.4-SupplyChainCoordination rdf:type owl:NamedIndividual ,
                                               :Security_Operations_Policies ;
                                      :HasWeight 7 ;
                                      rdfs:comment "Mechanisms exist to provide cybersecurity & data privacy incident information to the provider of the product or service and other organizations involved in the supply chain for systems or system components related to the incident." .


###  http://FYP-ASHS21/csonto/OPS-IRO-11-IncidentReportingAssistance
:OPS-IRO-11-IncidentReportingAssistance rdf:type owl:NamedIndividual ,
                                                 :Security_Operations_Policies ;
                                        :HasWeight 5 ;
                                        rdfs:comment "Mechanisms exist to provide incident response advice and assistance to users of systems for the handling and reporting of actual and potential cybersecurity & data privacy incidents. " .


###  http://FYP-ASHS21/csonto/OPS-IRO-11.1-AutomationSupportofAvailabilityofInformation-Support
:OPS-IRO-11.1-AutomationSupportofAvailabilityofInformation-Support rdf:type owl:NamedIndividual ,
                                                                            :Security_Operations_Policies ;
                                                                   :HasWeight 1 ;
                                                                   rdfs:comment "Automated mechanisms exist to increase the availability of incident response-related information and support. " .


###  http://FYP-ASHS21/csonto/OPS-IRO-11.2-CoordinationWithExternalProviders
:OPS-IRO-11.2-CoordinationWithExternalProviders rdf:type owl:NamedIndividual ,
                                                         :Security_Operations_Policies ;
                                                :HasWeight 5 ;
                                                rdfs:comment "Mechanisms exist to establish a direct, cooperative relationship between the organization's incident response capability and external service providers." .


###  http://FYP-ASHS21/csonto/OPS-IRO-12-InformationSpillageResponse
:OPS-IRO-12-InformationSpillageResponse rdf:type owl:NamedIndividual ,
                                                 :Security_Operations_Policies ;
                                        :HasWeight 8 ;
                                        rdfs:comment "Mechanisms exist to respond to sensitive information spills." .


###  http://FYP-ASHS21/csonto/OPS-IRO-12.1-ResponsiblePersonnel
:OPS-IRO-12.1-ResponsiblePersonnel rdf:type owl:NamedIndividual ,
                                            :Security_Operations_Policies ;
                                   :HasWeight 8 ;
                                   rdfs:comment "Mechanisms exist to formally assign personnel or roles with responsibility for responding to sensitive information spills. " .


###  http://FYP-ASHS21/csonto/OPS-IRO-12.2-Training
:OPS-IRO-12.2-Training rdf:type owl:NamedIndividual ,
                                :Security_Operations_Policies ;
                       :HasWeight 8 ;
                       rdfs:comment "Mechanisms exist to ensure incident response training material provides coverage for sensitive information spillage response." .


###  http://FYP-ASHS21/csonto/OPS-IRO-12.3-Post-SpillOperations
:OPS-IRO-12.3-Post-SpillOperations rdf:type owl:NamedIndividual ,
                                            :Security_Operations_Policies ;
                                   :HasWeight 8 ;
                                   rdfs:comment "Mechanisms exist to ensure that organizational personnel impacted by sensitive information spills can continue to carry out assigned tasks while contaminated systems are undergoing corrective actions. " .


###  http://FYP-ASHS21/csonto/OPS-IRO-12.4-ExposuretoUnauthorizedPersonnel
:OPS-IRO-12.4-ExposuretoUnauthorizedPersonnel rdf:type owl:NamedIndividual ,
                                                       :Security_Operations_Policies ;
                                              :HasWeight 8 ;
                                              rdfs:comment "Mechanisms exist to address security safeguards for personnel exposed to sensitive information that is not within their assigned access authorizations. " .


###  http://FYP-ASHS21/csonto/OPS-IRO-15-DetonationChambers-Sandboxes-
:OPS-IRO-15-DetonationChambers-Sandboxes- rdf:type owl:NamedIndividual ,
                                                   :Security_Operations_Policies ;
                                          :HasWeight 5 ;
                                          rdfs:comment "Mechanisms exist to utilize a detonation chamber capability to detect and/or block potentially-malicious files and email attachments." .


###  http://FYP-ASHS21/csonto/OPS-MON-01-ContinuousMonitoring
:OPS-MON-01-ContinuousMonitoring rdf:type owl:NamedIndividual ,
                                          :Security_Operations_Policies ;
                                 :HasWeight 10 ;
                                 rdfs:comment "Mechanisms exist to facilitate the implementation of enterprise-wide monitoring controls." .


###  http://FYP-ASHS21/csonto/OPS-MON-01.10-DeactivatedAccountActivity
:OPS-MON-01.10-DeactivatedAccountActivity rdf:type owl:NamedIndividual ,
                                                   :Security_Operations_Policies ;
                                          :HasWeight 9 ;
                                          rdfs:comment "Mechanisms exist to monitor deactivated accounts for attempted usage." .


###  http://FYP-ASHS21/csonto/OPS-MON-01.11-AutomatedResponsetoSuspiciousEvents
:OPS-MON-01.11-AutomatedResponsetoSuspiciousEvents rdf:type owl:NamedIndividual ,
                                                            :Security_Operations_Policies ;
                                                   :HasWeight 5 ;
                                                   rdfs:comment "Mechanisms exist to automatically implement pre-determined corrective actions in response to detected events that have security incident implications." .


###  http://FYP-ASHS21/csonto/OPS-MON-01.12-AutomatedAlerts
:OPS-MON-01.12-AutomatedAlerts rdf:type owl:NamedIndividual ,
                                        :Security_Operations_Policies ;
                               :HasWeight 5 ;
                               rdfs:comment "Mechanisms exist to automatically alert incident response personnel to inappropriate or anomalous activities that have potential security incident implications." .


###  http://FYP-ASHS21/csonto/OPS-MON-01.13-AlertThresholdTuning
:OPS-MON-01.13-AlertThresholdTuning rdf:type owl:NamedIndividual ,
                                             :Security_Operations_Policies ;
                                    :HasWeight 5 ;
                                    rdfs:comment "Mechanisms exist to \"tune\" event monitoring technologies through analyzing communications traffic/event patterns and developing profiles representing common traffic patterns and/or events." .


###  http://FYP-ASHS21/csonto/OPS-MON-01.14-IndividualsPosingGreaterRisk
:OPS-MON-01.14-IndividualsPosingGreaterRisk rdf:type owl:NamedIndividual ,
                                                     :Security_Operations_Policies ;
                                            :HasWeight 5 ;
                                            rdfs:comment "Mechanisms exist to implement enhanced activity monitoring for individuals who have been identified as posing an increased level of risk. " .


###  http://FYP-ASHS21/csonto/OPS-MON-01.15-PrivilegedUserOversight
:OPS-MON-01.15-PrivilegedUserOversight rdf:type owl:NamedIndividual ,
                                                :Security_Operations_Policies ;
                                       :HasWeight 5 ;
                                       rdfs:comment "Mechanisms exist to implement enhanced activity monitoring for privileged users." .


###  http://FYP-ASHS21/csonto/OPS-MON-01.16-AnalyzeandPrioritizeMonitoringRequirements
:OPS-MON-01.16-AnalyzeandPrioritizeMonitoringRequirements rdf:type owl:NamedIndividual ,
                                                                   :Security_Operations_Policies ;
                                                          :HasWeight 5 ;
                                                          rdfs:comment "Mechanisms exist to assess the organization's needs for monitoring and prioritize the monitoring of assets, based on asset criticality and the sensitivity of the data it stores, transmits and processes." .


###  http://FYP-ASHS21/csonto/OPS-MON-01.17-Real-TimeSessionMonitoring
:OPS-MON-01.17-Real-TimeSessionMonitoring rdf:type owl:NamedIndividual ,
                                                   :Security_Operations_Policies ;
                                          :HasWeight 4 ;
                                          rdfs:comment "Mechanisms exist to enable authorized personnel the ability to remotely view and hear content related to an established user session in real time, in accordance with organizational standards, as well as statutory, regulatory and contractual obligations." .


###  http://FYP-ASHS21/csonto/OPS-MON-01.2-AutomatedToolsforReal-TimeAnalysis
:OPS-MON-01.2-AutomatedToolsforReal-TimeAnalysis rdf:type owl:NamedIndividual ,
                                                          :Security_Operations_Policies ;
                                                 :HasWeight 9 ;
                                                 rdfs:comment "Mechanisms exist to utilize a Security Incident Event Manager (SIEM), or similar automated tool, to support near real-time analysis and incident escalation. " .


###  http://FYP-ASHS21/csonto/OPS-MON-01.4-SystemGeneratedAlerts
:OPS-MON-01.4-SystemGeneratedAlerts rdf:type owl:NamedIndividual ,
                                             :Security_Operations_Policies ;
                                    :HasWeight 7 ;
                                    rdfs:comment "Mechanisms exist to monitor, correlate and respond to alerts from physical, cybersecurity, data privacy and supply chain activities to achieve integrated situational awareness. " .


###  http://FYP-ASHS21/csonto/OPS-MON-01.5-WirelessIntrusionDetectionSystem-WIDS-
:OPS-MON-01.5-WirelessIntrusionDetectionSystem-WIDS- rdf:type owl:NamedIndividual ,
                                                              :Security_Operations_Policies ;
                                                     :HasWeight 5 ;
                                                     rdfs:comment "Mechanisms exist to utilize Wireless Intrusion Detection / Protection Systems (WIDS / WIPS) to identify rogue wireless devices and to detect attack attempts via wireless networks. " .


###  http://FYP-ASHS21/csonto/OPS-MON-01.6-Host-BasedDevices
:OPS-MON-01.6-Host-BasedDevices rdf:type owl:NamedIndividual ,
                                         :Security_Operations_Policies ;
                                :HasWeight 8 ;
                                rdfs:comment "Mechanisms exist to utilize Host-based Intrusion Detection / Prevention Systems (HIDS / HIPS) to actively alert on or block unwanted activities and send logs to a Security Incident Event Manager (SIEM), or similar automated tool, to maintain situational awareness." .


###  http://FYP-ASHS21/csonto/OPS-MON-01.7-FileIntegrityMonitoring-FIM-
:OPS-MON-01.7-FileIntegrityMonitoring-FIM- rdf:type owl:NamedIndividual ,
                                                    :Security_Operations_Policies ;
                                           :HasWeight 9 ;
                                           rdfs:comment "Mechanisms exist to utilize a File Integrity Monitor (FIM), or similar change-detection technology, on critical assets to generate alerts for unauthorized modifications. " .


###  http://FYP-ASHS21/csonto/OPS-MON-01.9-ProxyLogging
:OPS-MON-01.9-ProxyLogging rdf:type owl:NamedIndividual ,
                                    :Security_Operations_Policies ;
                           :HasWeight 8 ;
                           rdfs:comment "Mechanisms exist to log all Internet-bound requests, in order to identify prohibited activities and assist incident handlers with identifying potentially compromised systems. " .


###  http://FYP-ASHS21/csonto/OPS-MON-02-CentralizedCollectionofSecurityEventLogs
:OPS-MON-02-CentralizedCollectionofSecurityEventLogs rdf:type owl:NamedIndividual ,
                                                              :Security_Operations_Policies ;
                                                     :HasWeight 10 ;
                                                     rdfs:comment "Mechanisms exist to utilize a Security Incident Event Manager (SIEM) or similar automated tool, to support the centralized collection of security-related event logs." .


###  http://FYP-ASHS21/csonto/OPS-MON-02.1-CorrelateMonitoringInformation
:OPS-MON-02.1-CorrelateMonitoringInformation rdf:type owl:NamedIndividual ,
                                                      :Security_Operations_Policies ;
                                             :HasWeight 9 ;
                                             rdfs:comment "Automated mechanisms exist to correlate both technical and non-technical information from across the enterprise by a Security Incident Event Manager (SIEM) or similar automated tool, to enhance organization-wide situational awareness." .


###  http://FYP-ASHS21/csonto/OPS-MON-02.4-CorrelationwithPhysicalMonitoring
:OPS-MON-02.4-CorrelationwithPhysicalMonitoring rdf:type owl:NamedIndividual ,
                                                         :Security_Operations_Policies ;
                                                :HasWeight 5 ;
                                                rdfs:comment "Automated mechanisms exist to correlate information from audit records with information obtained from monitoring physical access to further enhance the ability to identify suspicious, inappropriate, unusual or malevolent activity. " .


###  http://FYP-ASHS21/csonto/OPS-MON-02.5-PermittedActions
:OPS-MON-02.5-PermittedActions rdf:type owl:NamedIndividual ,
                                        :Security_Operations_Policies ;
                               :HasWeight 5 ;
                               rdfs:comment "Mechanisms exist to specify the permitted actions for both users and systems associated with the review, analysis and reporting of audit information. " .


###  http://FYP-ASHS21/csonto/OPS-MON-02.6-AuditLevelAdjustments
:OPS-MON-02.6-AuditLevelAdjustments rdf:type owl:NamedIndividual ,
                                             :Security_Operations_Policies ;
                                    :HasWeight 5 ;
                                    rdfs:comment "Mechanisms exist to adjust the level of audit review, analysis and reporting based on evolving threat information from law enforcement, industry associations or other credible sources of threat intelligence. " .


###  http://FYP-ASHS21/csonto/OPS-MON-02.7-System-Wide-Time-CorrelatedAuditTrail
:OPS-MON-02.7-System-Wide-Time-CorrelatedAuditTrail rdf:type owl:NamedIndividual ,
                                                             :Security_Operations_Policies ;
                                                    :HasWeight 5 ;
                                                    rdfs:comment "Automated mechanisms exist to compile audit records into an organization-wide audit trail that is time-correlated." .


###  http://FYP-ASHS21/csonto/OPS-MON-02.8-ChangesbyAuthorizedIndividuals
:OPS-MON-02.8-ChangesbyAuthorizedIndividuals rdf:type owl:NamedIndividual ,
                                                      :Security_Operations_Policies ;
                                             :HasWeight 5 ;
                                             rdfs:comment "Mechanisms exist to provide privileged users or roles the capability to change the auditing to be performed on specified information system components, based on specific event criteria within specified time thresholds. " .


###  http://FYP-ASHS21/csonto/OPS-MON-03-ContentofEventLogs
:OPS-MON-03-ContentofEventLogs rdf:type owl:NamedIndividual ,
                                        :Security_Operations_Policies ;
                               :HasWeight 10 ;
                               rdfs:comment """Mechanisms exist to configure systems to produce audit records that contain sufficient information to, at a minimum:
  Establish what type of event occurred;
  When (date and time) the event occurred;
  Where the event occurred;
  The source of the event;
  The outcome (success or failure) of the event; and 
  The identity of any user/subject associated with the event. """ .


###  http://FYP-ASHS21/csonto/OPS-MON-03.1-SensitiveAuditInformation
:OPS-MON-03.1-SensitiveAuditInformation rdf:type owl:NamedIndividual ,
                                                 :Security_Operations_Policies ;
                                        :HasWeight 8 ;
                                        rdfs:comment "Mechanisms exist to protect sensitive/regulated data contained in log files. " .


###  http://FYP-ASHS21/csonto/OPS-MON-03.2-AuditTrails
:OPS-MON-03.2-AuditTrails rdf:type owl:NamedIndividual ,
                                   :Security_Operations_Policies ;
                          :HasWeight 10 ;
                          rdfs:comment "Mechanisms exist to link system access to individual users or service accounts." .


###  http://FYP-ASHS21/csonto/OPS-MON-03.3-PrivilegedFunctionsLogging
:OPS-MON-03.3-PrivilegedFunctionsLogging rdf:type owl:NamedIndividual ,
                                                  :Security_Operations_Policies ;
                                         :HasWeight 8 ;
                                         rdfs:comment "Mechanisms exist to log and review the actions of users and/or services with elevated privileges." .


###  http://FYP-ASHS21/csonto/OPS-MON-03.4-VerbosityLoggingforBoundaryDevices
:OPS-MON-03.4-VerbosityLoggingforBoundaryDevices rdf:type owl:NamedIndividual ,
                                                          :Security_Operations_Policies ;
                                                 :HasWeight 5 ;
                                                 rdfs:comment "Mechanisms exist to verbosely log all traffic (both allowed and blocked) arriving at network boundary devices, including firewalls, Intrusion Detection / Prevention Systems (IDS/IPS) and inbound and outbound proxies." .


###  http://FYP-ASHS21/csonto/OPS-MON-03.5-LimitPersonalData-PD-InAuditRecords
:OPS-MON-03.5-LimitPersonalData-PD-InAuditRecords rdf:type owl:NamedIndividual ,
                                                           :Security_Operations_Policies ;
                                                  :HasWeight 8 ;
                                                  rdfs:comment "Mechanisms exist to limit Personal Data (PD) contained in audit records to the elements identified in the data privacy risk assessment." .


###  http://FYP-ASHS21/csonto/OPS-MON-03.6-CentralizedManagementofPlannedAuditRecordContent
:OPS-MON-03.6-CentralizedManagementofPlannedAuditRecordContent rdf:type owl:NamedIndividual ,
                                                                        :Security_Operations_Policies ;
                                                               :HasWeight 5 ;
                                                               rdfs:comment "Mechanisms exist to centrally manage and configure the content required to be captured in audit records generated by organization-defined information system components. " .


###  http://FYP-ASHS21/csonto/OPS-MON-03.7-DatabaseLogging
:OPS-MON-03.7-DatabaseLogging rdf:type owl:NamedIndividual ,
                                       :Security_Operations_Policies ;
                              :HasWeight 8 ;
                              rdfs:comment "Mechanisms exist to ensure databases produce audit records that contain sufficient information to monitor database activities." .


###  http://FYP-ASHS21/csonto/OPS-MON-04-EventLogStorageCapacity
:OPS-MON-04-EventLogStorageCapacity rdf:type owl:NamedIndividual ,
                                             :Security_Operations_Policies ;
                                    :HasWeight 8 ;
                                    rdfs:comment "Mechanisms exist to allocate and proactively manage sufficient event log storage capacity to reduce the likelihood of such capacity being exceeded. " .


###  http://FYP-ASHS21/csonto/OPS-MON-05-ResponseToEventLogProcessingFailures
:OPS-MON-05-ResponseToEventLogProcessingFailures rdf:type owl:NamedIndividual ,
                                                          :Security_Operations_Policies ;
                                                 :HasWeight 8 ;
                                                 rdfs:comment "Mechanisms exist to alert appropriate personnel in the event of a log processing failure and take actions to remedy the disruption." .


###  http://FYP-ASHS21/csonto/OPS-MON-05.1-Real-TimeAlertsofEventLoggingFailure
:OPS-MON-05.1-Real-TimeAlertsofEventLoggingFailure rdf:type owl:NamedIndividual ,
                                                            :Security_Operations_Policies ;
                                                   :HasWeight 6 ;
                                                   rdfs:comment "Mechanisms exist to provide 24x7x365 near real-time alerting capability when an event log processing failure occurs. " .


###  http://FYP-ASHS21/csonto/OPS-MON-05.2-EventLogStorageCapacityAlerting
:OPS-MON-05.2-EventLogStorageCapacityAlerting rdf:type owl:NamedIndividual ,
                                                       :Security_Operations_Policies ;
                                              :HasWeight 5 ;
                                              rdfs:comment "Automated mechanisms exist to alert appropriate personnel when the allocated volume reaches an organization-defined percentage of maximum event log storage capacity." .


###  http://FYP-ASHS21/csonto/OPS-MON-06-MonitoringReporting
:OPS-MON-06-MonitoringReporting rdf:type owl:NamedIndividual ,
                                         :Security_Operations_Policies ;
                                :HasWeight 7 ;
                                rdfs:comment "Mechanisms exist to provide an event log report generation capability to aid in detecting and assessing anomalous activities. " .


###  http://FYP-ASHS21/csonto/OPS-MON-06.1-QueryParameterAuditsofPersonalData-PD-
:OPS-MON-06.1-QueryParameterAuditsofPersonalData-PD- rdf:type owl:NamedIndividual ,
                                                              :Security_Operations_Policies ;
                                                     :HasWeight 3 ;
                                                     rdfs:comment "Mechanisms exist to provide and implement the capability for auditing the parameters of user query events for data sets containing Personal Data (PD)." .


###  http://FYP-ASHS21/csonto/OPS-MON-06.2-TrendAnalysisReporting
:OPS-MON-06.2-TrendAnalysisReporting rdf:type owl:NamedIndividual ,
                                              :Security_Operations_Policies ;
                                     :HasWeight 5 ;
                                     rdfs:comment "Mechanisms exist to employ trend analyses to determine if security control implementations, the frequency of continuous monitoring activities, and/or the types of activities used in the continuous monitoring process need to be modified based on empirical data." .


###  http://FYP-ASHS21/csonto/OPS-MON-07-TimeStamps
:OPS-MON-07-TimeStamps rdf:type owl:NamedIndividual ,
                                :Security_Operations_Policies ;
                       :HasWeight 10 ;
                       rdfs:comment "Mechanisms exist to configure systems to use an authoritative time source to generate time stamps for event logs. " .


###  http://FYP-ASHS21/csonto/OPS-MON-07.1-SynchronizationWithAuthoritativeTimeSource
:OPS-MON-07.1-SynchronizationWithAuthoritativeTimeSource rdf:type owl:NamedIndividual ,
                                                                  :Security_Operations_Policies ;
                                                         :HasWeight 8 ;
                                                         rdfs:comment "Mechanisms exist to synchronize internal system clocks with an authoritative time source. " .


###  http://FYP-ASHS21/csonto/OPS-MON-08-ProtectionofEventLogs
:OPS-MON-08-ProtectionofEventLogs rdf:type owl:NamedIndividual ,
                                           :Security_Operations_Policies ;
                                  :HasWeight 10 ;
                                  rdfs:comment "Mechanisms exist to protect event logs and audit tools from unauthorized access, modification and deletion." .


###  http://FYP-ASHS21/csonto/OPS-MON-08.1-EventLogBackuponSeparatePhysicalSystems-Components
:OPS-MON-08.1-EventLogBackuponSeparatePhysicalSystems-Components rdf:type owl:NamedIndividual ,
                                                                          :Security_Operations_Policies ;
                                                                 :HasWeight 5 ;
                                                                 rdfs:comment "Mechanisms exist to back up event logs onto a physically different system or system component than the Security Incident Event Manager (SIEM) or similar automated tool." .


###  http://FYP-ASHS21/csonto/OPS-MON-08.2-AccessbySubsetofPrivilegedUsers
:OPS-MON-08.2-AccessbySubsetofPrivilegedUsers rdf:type owl:NamedIndividual ,
                                                       :Security_Operations_Policies ;
                                              :HasWeight 8 ;
                                              rdfs:comment "Mechanisms exist to restrict access to the management of event logs to privileged users with a specific business need." .


###  http://FYP-ASHS21/csonto/OPS-MON-08.3-CryptographicProtectionofEventLogInformation
:OPS-MON-08.3-CryptographicProtectionofEventLogInformation rdf:type owl:NamedIndividual ,
                                                                    :Security_Operations_Policies ;
                                                           :HasWeight 5 ;
                                                           rdfs:comment "Cryptographic mechanisms exist to protect the integrity of event logs and audit tools. " .


###  http://FYP-ASHS21/csonto/OPS-MON-08.4-DualAuthorizationforEventLogMovement
:OPS-MON-08.4-DualAuthorizationforEventLogMovement rdf:type owl:NamedIndividual ,
                                                            :Security_Operations_Policies ;
                                                   :HasWeight 5 ;
                                                   rdfs:comment "Automated mechanisms exist to enforce dual authorization for the movement or deletion of event logs." .


###  http://FYP-ASHS21/csonto/OPS-MON-09-Non-Repudiation
:OPS-MON-09-Non-Repudiation rdf:type owl:NamedIndividual ,
                                     :Security_Operations_Policies ;
                            :HasWeight 8 ;
                            rdfs:comment "Mechanisms exist to utilize a non-repudiation capability to protect against an individual falsely denying having performed a particular action. " .


###  http://FYP-ASHS21/csonto/OPS-MON-09.1-IdentityBinding
:OPS-MON-09.1-IdentityBinding rdf:type owl:NamedIndividual ,
                                       :Security_Operations_Policies ;
                              :HasWeight 4 ;
                              rdfs:comment "Mechanisms exist to bind the identity of the information producer to the information generated." .


###  http://FYP-ASHS21/csonto/OPS-MON-10-EventLogRetention
:OPS-MON-10-EventLogRetention rdf:type owl:NamedIndividual ,
                                       :Security_Operations_Policies ;
                              :HasWeight 10 ;
                              rdfs:comment "Mechanisms exist to retain event logs for a time period consistent with records retention requirements to provide support for after-the-fact investigations of security incidents and to meet statutory, regulatory and contractual retention requirements. " .


###  http://FYP-ASHS21/csonto/OPS-MON-11-MonitoringForInformationDisclosure
:OPS-MON-11-MonitoringForInformationDisclosure rdf:type owl:NamedIndividual ,
                                                        :Security_Operations_Policies ;
                                               :HasWeight 8 ;
                                               rdfs:comment "Mechanisms exist to monitor for evidence of unauthorized exfiltration or disclosure of non-public information. " .


###  http://FYP-ASHS21/csonto/OPS-MON-11.1-AnalyzeTrafficforCovertExfiltration
:OPS-MON-11.1-AnalyzeTrafficforCovertExfiltration rdf:type owl:NamedIndividual ,
                                                           :Security_Operations_Policies ;
                                                  :HasWeight 5 ;
                                                  rdfs:comment "Automated mechanisms exist to analyze network traffic to detect covert data exfiltration." .


###  http://FYP-ASHS21/csonto/OPS-MON-11.2-UnauthorizedNetworkServices
:OPS-MON-11.2-UnauthorizedNetworkServices rdf:type owl:NamedIndividual ,
                                                   :Security_Operations_Policies ;
                                          :HasWeight 5 ;
                                          rdfs:comment "Automated mechanisms exist to detect unauthorized network services and alert incident response personnel. " .


###  http://FYP-ASHS21/csonto/OPS-MON-11.3-MonitoringforIndicatorsofCompromise-IOC-
:OPS-MON-11.3-MonitoringforIndicatorsofCompromise-IOC- rdf:type owl:NamedIndividual ,
                                                                :Security_Operations_Policies ;
                                                       :HasWeight 5 ;
                                                       rdfs:comment "Automated mechanisms exist to identify and alert on Indicators of Compromise (IoC). " .


###  http://FYP-ASHS21/csonto/OPS-MON-12-SessionAudit
:OPS-MON-12-SessionAudit rdf:type owl:NamedIndividual ,
                                  :Security_Operations_Policies ;
                         :HasWeight 7 ;
                         rdfs:comment """Mechanisms exist to provide session audit capabilities that can: 
  Capture and log all content related to a user session; and
  Remotely view all content related to an established user session in real time.""" .


###  http://FYP-ASHS21/csonto/OPS-MON-13-AlternateEventLoggingCapability
:OPS-MON-13-AlternateEventLoggingCapability rdf:type owl:NamedIndividual ,
                                                     :Security_Operations_Policies ;
                                            :HasWeight 3 ;
                                            rdfs:comment "Mechanisms exist to provide an alternate event logging capability in the event of a failure in primary audit capability." .


###  http://FYP-ASHS21/csonto/OPS-MON-14-Cross-OrganizationalMonitoring
:OPS-MON-14-Cross-OrganizationalMonitoring rdf:type owl:NamedIndividual ,
                                                    :Security_Operations_Policies ;
                                           :HasWeight 3 ;
                                           rdfs:comment "Mechanisms exist to coordinate sanitized event logs among external organizations to identify anomalous events when event logs are shared across organizational boundaries, without giving away sensitive or critical business data." .


###  http://FYP-ASHS21/csonto/OPS-MON-14.1-SharingofEventLogs
:OPS-MON-14.1-SharingofEventLogs rdf:type owl:NamedIndividual ,
                                          :Security_Operations_Policies ;
                                 :HasWeight 5 ;
                                 rdfs:comment "Mechanisms exist to share event logs with third-party organizations based on specific cross-organizational sharing agreements." .


###  http://FYP-ASHS21/csonto/OPS-MON-15-CovertChannelAnalysis
:OPS-MON-15-CovertChannelAnalysis rdf:type owl:NamedIndividual ,
                                           :Security_Operations_Policies ;
                                  :HasWeight 3 ;
                                  rdfs:comment "Mechanisms exist to conduct covert channel analysis to identify aspects of communications that are potential avenues for covert channels." .


###  http://FYP-ASHS21/csonto/OPS-MON-16-AnomalousBehavior
:OPS-MON-16-AnomalousBehavior rdf:type owl:NamedIndividual ,
                                       :Security_Operations_Policies ;
                              :HasWeight 10 ;
                              rdfs:comment "Mechanisms exist to detect and respond to anomalous behavior that could indicate account compromise or other malicious activities." .


###  http://FYP-ASHS21/csonto/OPS-MON-16.1-InsiderThreats
:OPS-MON-16.1-InsiderThreats rdf:type owl:NamedIndividual ,
                                      :Security_Operations_Policies ;
                             :HasWeight 8 ;
                             rdfs:comment "Mechanisms exist to monitor internal personnel activity for potential security incidents." .


###  http://FYP-ASHS21/csonto/OPS-MON-16.2-Third-PartyThreats
:OPS-MON-16.2-Third-PartyThreats rdf:type owl:NamedIndividual ,
                                          :Security_Operations_Policies ;
                                 :HasWeight 8 ;
                                 rdfs:comment "Mechanisms exist to monitor third-party personnel activity for potential security incidents." .


###  http://FYP-ASHS21/csonto/OPS-MON-16.3-UnauthorizedActivities
:OPS-MON-16.3-UnauthorizedActivities rdf:type owl:NamedIndividual ,
                                              :Security_Operations_Policies ;
                                     :HasWeight 8 ;
                                     rdfs:comment "Mechanisms exist to monitor for unauthorized activities, accounts, connections, devices and software." .


###  http://FYP-ASHS21/csonto/OPS-MON-16.4-AccountCreationandModificationLogging
:OPS-MON-16.4-AccountCreationandModificationLogging rdf:type owl:NamedIndividual ,
                                                             :Security_Operations_Policies ;
                                                    :HasWeight 7 ;
                                                    rdfs:comment "Automated mechanisms exist to generate event logs for permissions changes to privileged accounts and/or groups." .


###  http://FYP-ASHS21/csonto/OPS-NET-01-NetworkSecurityControls-NSC-
:OPS-NET-01-NetworkSecurityControls-NSC- rdf:type owl:NamedIndividual ,
                                                  :Security_Operations_Policies ;
                                         :HasWeight 10 ;
                                         rdfs:comment "Mechanisms exist to develop, govern & update procedures to facilitate the implementation of Network Security Controls (NSC)." .


###  http://FYP-ASHS21/csonto/OPS-NET-01.1-ZeroTrustArchitecture-ZTA-
:OPS-NET-01.1-ZeroTrustArchitecture-ZTA- rdf:type owl:NamedIndividual ,
                                                  :Security_Operations_Policies ;
                                         :HasWeight 8 ;
                                         rdfs:comment "Mechanisms exist to treat all users and devices as potential threats and prevent access to data and resources until the users can be properly authenticated and their access authorized." .


###  http://FYP-ASHS21/csonto/OPS-NET-02-LayeredNetworkDefenses
:OPS-NET-02-LayeredNetworkDefenses rdf:type owl:NamedIndividual ,
                                            :Security_Operations_Policies ;
                                   :HasWeight 9 ;
                                   rdfs:comment "Mechanisms exist to implement security functions as a layered structure that minimizes interactions between layers of the design and avoids any dependence by lower layers on the functionality or correctness of higher layers. " .


###  http://FYP-ASHS21/csonto/OPS-NET-02.1-DenialofService-DoS-Protection
:OPS-NET-02.1-DenialofService-DoS-Protection rdf:type owl:NamedIndividual ,
                                                      :Security_Operations_Policies ;
                                             :HasWeight 9 ;
                                             rdfs:comment "Automated mechanisms exist to protect against or limit the effects of denial of service attacks. " .


###  http://FYP-ASHS21/csonto/OPS-NET-02.2-GuestNetworks
:OPS-NET-02.2-GuestNetworks rdf:type owl:NamedIndividual ,
                                     :Security_Operations_Policies ;
                            :HasWeight 6 ;
                            rdfs:comment "Mechanisms exist to implement and manage a secure guest network. " .


###  http://FYP-ASHS21/csonto/OPS-NET-02.3-CrossDomainSolution-CDS-
:OPS-NET-02.3-CrossDomainSolution-CDS- rdf:type owl:NamedIndividual ,
                                                :Security_Operations_Policies ;
                                       :HasWeight 6 ;
                                       rdfs:comment "Mechanisms exist to implement a Cross Domain Solution (CDS) to mitigate the specific security risks of accessing or transferring information between security domains." .


###  http://FYP-ASHS21/csonto/OPS-NET-03-BoundaryProtection
:OPS-NET-03-BoundaryProtection rdf:type owl:NamedIndividual ,
                                        :Security_Operations_Policies ;
                               :HasWeight 10 ;
                               rdfs:comment "Mechanisms exist to monitor and control communications at the external network boundary and at key internal boundaries within the network." .


###  http://FYP-ASHS21/csonto/OPS-NET-03.1-LimitNetworkConnections
:OPS-NET-03.1-LimitNetworkConnections rdf:type owl:NamedIndividual ,
                                               :Security_Operations_Policies ;
                                      :HasWeight 9 ;
                                      rdfs:comment "Mechanisms exist to limit the number of concurrent external network connections to its systems. " .


###  http://FYP-ASHS21/csonto/OPS-NET-03.2-ExternalTelecommunicationsServices
:OPS-NET-03.2-ExternalTelecommunicationsServices rdf:type owl:NamedIndividual ,
                                                          :Security_Operations_Policies ;
                                                 :HasWeight 7 ;
                                                 rdfs:comment "Mechanisms exist to maintain a managed interface for each external telecommunication service that protects the confidentiality and integrity of the information being transmitted across each interface." .


###  http://FYP-ASHS21/csonto/OPS-NET-03.3-PreventDiscoveryofInternalInformation
:OPS-NET-03.3-PreventDiscoveryofInternalInformation rdf:type owl:NamedIndividual ,
                                                             :Security_Operations_Policies ;
                                                    :HasWeight 7 ;
                                                    rdfs:comment "Mechanisms exist to prevent the public disclosure of internal network information. " .


###  http://FYP-ASHS21/csonto/OPS-NET-03.4-PersonalData-PD-
:OPS-NET-03.4-PersonalData-PD- rdf:type owl:NamedIndividual ,
                                        :Security_Operations_Policies ;
                               :HasWeight 7 ;
                               rdfs:comment "Mechanisms exist to apply network-based processing rules to data elements of Personal Data (PD)." .


###  http://FYP-ASHS21/csonto/OPS-NET-03.5-PreventUnauthorizedExfiltration
:OPS-NET-03.5-PreventUnauthorizedExfiltration rdf:type owl:NamedIndividual ,
                                                       :Security_Operations_Policies ;
                                              :HasWeight 5 ;
                                              rdfs:comment "Automated mechanisms exist to prevent the unauthorized exfiltration of sensitive/regulated data across managed interfaces. " .


###  http://FYP-ASHS21/csonto/OPS-NET-03.7-IsolationofInformationSystemComponents
:OPS-NET-03.7-IsolationofInformationSystemComponents rdf:type owl:NamedIndividual ,
                                                              :Security_Operations_Policies ;
                                                     :HasWeight 5 ;
                                                     rdfs:comment "Mechanisms exist to employ boundary protections to isolate systems, services and processes that support critical missions and/or business functions. " .


###  http://FYP-ASHS21/csonto/OPS-NET-03.8-SeparateSubnetforConnectingtoDifferentSecurityDomains
:OPS-NET-03.8-SeparateSubnetforConnectingtoDifferentSecurityDomains rdf:type owl:NamedIndividual ,
                                                                             :Security_Operations_Policies ;
                                                                    :HasWeight 5 ;
                                                                    rdfs:comment "Mechanisms exist to implement separate network addresses (e.g., different subnets) to connect to systems in different security domains." .


###  http://FYP-ASHS21/csonto/OPS-NET-04.10-DetectionofUnsanctionedInformation
:OPS-NET-04.10-DetectionofUnsanctionedInformation rdf:type owl:NamedIndividual ,
                                                           :Security_Operations_Policies ;
                                                  :HasWeight 5 ;
                                                  rdfs:comment "Automated mechanisms exist to implement security policy filters requiring fully enumerated formats that restrict data structure and content, when transferring information between different security domains." .


###  http://FYP-ASHS21/csonto/OPS-NET-04.11-ApprovedSolutions
:OPS-NET-04.11-ApprovedSolutions rdf:type owl:NamedIndividual ,
                                          :Security_Operations_Policies ;
                                 :HasWeight 5 ;
                                 rdfs:comment "Automated mechanisms exist to examine information for the presence of unsanctioned information and prohibits the transfer of such information, when transferring information between different security domains." .


###  http://FYP-ASHS21/csonto/OPS-NET-04.12-CrossDomainAuthentication
:OPS-NET-04.12-CrossDomainAuthentication rdf:type owl:NamedIndividual ,
                                                  :Security_Operations_Policies ;
                                         :HasWeight 5 ;
                                         rdfs:comment "Automated mechanisms exist to uniquely identify and authenticate source and destination points for information transfer." .


###  http://FYP-ASHS21/csonto/OPS-NET-04.13-MetadataValidation
:OPS-NET-04.13-MetadataValidation rdf:type owl:NamedIndividual ,
                                           :Security_Operations_Policies ;
                                  :HasWeight 2 ;
                                  rdfs:comment "Automated mechanisms exist to apply cybersecurity and/or data privacy filters on metadata." .


###  http://FYP-ASHS21/csonto/OPS-NET-04.2-ObjectSecurityAttributes
:OPS-NET-04.2-ObjectSecurityAttributes rdf:type owl:NamedIndividual ,
                                                :Security_Operations_Policies ;
                                       :HasWeight 5 ;
                                       rdfs:comment "Mechanisms exist to associate security attributes with information, source and destination objects to enforce defined information flow control configurations as a basis for flow control decisions. " .


###  http://FYP-ASHS21/csonto/OPS-NET-04.3-ContentCheckforEncryptedData
:OPS-NET-04.3-ContentCheckforEncryptedData rdf:type owl:NamedIndividual ,
                                                    :Security_Operations_Policies ;
                                           :HasWeight 4 ;
                                           rdfs:comment "Mechanisms exist to prevent encrypted data from bypassing content-checking mechanisms. " .


###  http://FYP-ASHS21/csonto/OPS-NET-04.4-EmbeddedDataTypes
:OPS-NET-04.4-EmbeddedDataTypes rdf:type owl:NamedIndividual ,
                                         :Security_Operations_Policies ;
                                :HasWeight 2 ;
                                rdfs:comment "Mechanisms exist to enforce limitations on embedding data within other data types. " .


###  http://FYP-ASHS21/csonto/OPS-NET-04.5-Metadata
:OPS-NET-04.5-Metadata rdf:type owl:NamedIndividual ,
                                :Security_Operations_Policies ;
                       :HasWeight 2 ;
                       rdfs:comment "Mechanisms exist to enforce information flow controls based on metadata. " .


###  http://FYP-ASHS21/csonto/OPS-NET-04.6-HumanReviews
:OPS-NET-04.6-HumanReviews rdf:type owl:NamedIndividual ,
                                    :Security_Operations_Policies ;
                           :HasWeight 9 ;
                           rdfs:comment "Mechanisms exist to enforce the use of human reviews for Access Control Lists (ACLs) and similar rulesets on a routine basis. " .


###  http://FYP-ASHS21/csonto/OPS-NET-04.7-SecurityPolicyFilters
:OPS-NET-04.7-SecurityPolicyFilters rdf:type owl:NamedIndividual ,
                                             :Security_Operations_Policies ;
                                    :HasWeight 5 ;
                                    rdfs:comment "Automated mechanisms exist to enforce information flow control using security policy filters as a basis for flow control decisions." .


###  http://FYP-ASHS21/csonto/OPS-NET-04.8-DataTypeIdentifiers
:OPS-NET-04.8-DataTypeIdentifiers rdf:type owl:NamedIndividual ,
                                           :Security_Operations_Policies ;
                                  :HasWeight 5 ;
                                  rdfs:comment "Automated mechanisms exist to utilize data type identifiers to validate data essential for information flow decisions when transferring information between different security domains." .


###  http://FYP-ASHS21/csonto/OPS-NET-04.9-DecompositionIntoPolicy-RelatedSubcomponents
:OPS-NET-04.9-DecompositionIntoPolicy-RelatedSubcomponents rdf:type owl:NamedIndividual ,
                                                                    :Security_Operations_Policies ;
                                                           :HasWeight 5 ;
                                                           rdfs:comment "Automated mechanisms exist to decompose information into policy-relevant subcomponents for submission to policy enforcement mechanisms, when transferring information between different security domains." .


###  http://FYP-ASHS21/csonto/OPS-NET-05-SystemInterconnections
:OPS-NET-05-SystemInterconnections rdf:type owl:NamedIndividual ,
                                            :Security_Operations_Policies ;
                                   :HasWeight 9 ;
                                   rdfs:comment "Mechanisms exist to authorize connections from systems to other systems using Interconnection Security Agreements (ISAs) that document, for each interconnection, the interface characteristics, cybersecurity & data privacy requirements and the nature of the information communicated." .


###  http://FYP-ASHS21/csonto/OPS-NET-05.1-ExternalSystemConnections
:OPS-NET-05.1-ExternalSystemConnections rdf:type owl:NamedIndividual ,
                                                 :Security_Operations_Policies ;
                                        :HasWeight 8 ;
                                        rdfs:comment "Mechanisms exist to prohibit the direct connection of a sensitive system to an external network without the use of an organization-defined boundary protection device. " .


###  http://FYP-ASHS21/csonto/OPS-NET-05.2-InternalSystemConnections
:OPS-NET-05.2-InternalSystemConnections rdf:type owl:NamedIndividual ,
                                                 :Security_Operations_Policies ;
                                        :HasWeight 7 ;
                                        rdfs:comment "Mechanisms exist to control internal system connections through authorizing internal connections of systems and documenting, for each internal connection, the interface characteristics, security requirements and the nature of the information communicated." .


###  http://FYP-ASHS21/csonto/OPS-NET-06-NetworkSegmentation
:OPS-NET-06-NetworkSegmentation rdf:type owl:NamedIndividual ,
                                         :Security_Operations_Policies ;
                                :HasWeight 10 ;
                                rdfs:comment "Mechanisms exist to ensure network architecture utilizes network segmentation to isolate systems, applications and services that protections from other network resources." .


###  http://FYP-ASHS21/csonto/OPS-NET-06.1-SecurityManagementSubnets
:OPS-NET-06.1-SecurityManagementSubnets rdf:type owl:NamedIndividual ,
                                                 :Security_Operations_Policies ;
                                        :HasWeight 9 ;
                                        rdfs:comment "Mechanisms exist to implement security management subnets to isolate security tools and support components from other internal system components by implementing separate subnetworks with managed interfaces to other components of the system. " .


###  http://FYP-ASHS21/csonto/OPS-NET-06.2-VirtualLocalAreaNetwork-VLAN-Separation
:OPS-NET-06.2-VirtualLocalAreaNetwork-VLAN-Separation rdf:type owl:NamedIndividual ,
                                                               :Security_Operations_Policies ;
                                                      :HasWeight 9 ;
                                                      rdfs:comment "Mechanisms exist to enable Virtual Local Area Networks (VLANs) to limit the ability of devices on a network to directly communicate with other devices on the subnet and limit an attacker's ability to laterally move to compromise neighboring systems. " .


###  http://FYP-ASHS21/csonto/OPS-NET-06.3-Sensitive-RegulatedDataEnclave-SecureZone-
:OPS-NET-06.3-Sensitive-RegulatedDataEnclave-SecureZone- rdf:type owl:NamedIndividual ,
                                                                  :Security_Operations_Policies ;
                                                         :HasWeight 10 ;
                                                         rdfs:comment "Mechanisms exist to implement segmentation controls to restrict inbound and outbound connectivity for sensitive / regulated data enclaves (secure zones). " .


###  http://FYP-ASHS21/csonto/OPS-NET-06.4-SegregationFromEnterpriseServices
:OPS-NET-06.4-SegregationFromEnterpriseServices rdf:type owl:NamedIndividual ,
                                                         :Security_Operations_Policies ;
                                                :HasWeight 4 ;
                                                rdfs:comment "Mechanisms exist to isolate sensitive / regulated data enclaves (secure zones) from corporate-provided IT resources by providing enclave-specific IT services (e.g., directory services, DNS, NTP, ITAM, antimalware, patch management, etc.) to those isolated network segments." .


###  http://FYP-ASHS21/csonto/OPS-NET-06.5-DirectInternetAccessRestrictions
:OPS-NET-06.5-DirectInternetAccessRestrictions rdf:type owl:NamedIndividual ,
                                                        :Security_Operations_Policies ;
                                               :HasWeight 6 ;
                                               rdfs:comment "Mechanisms exist to prohibit, or strictly-control, Internet access from sensitive / regulated data enclaves (secure zones)." .


###  http://FYP-ASHS21/csonto/OPS-NET-07-RemoteSessionTermination
:OPS-NET-07-RemoteSessionTermination rdf:type owl:NamedIndividual ,
                                              :Security_Operations_Policies ;
                                     :HasWeight 8 ;
                                     rdfs:comment "Mechanisms exist to terminate remote sessions at the end of the session or after an organization-defined time period of inactivity. " .


###  http://FYP-ASHS21/csonto/OPS-NET-08-NetworkIntrusionDetection-PreventionSystems-NIDS-NIPS-
:OPS-NET-08-NetworkIntrusionDetection-PreventionSystems-NIDS-NIPS- rdf:type owl:NamedIndividual ,
                                                                            :Security_Operations_Policies ;
                                                                   :HasWeight 9 ;
                                                                   rdfs:comment "Mechanisms exist to employ Network Intrusion Detection / Prevention Systems (NIDS/NIPS) to detect and/or prevent intrusions into the network. " .


###  http://FYP-ASHS21/csonto/OPS-NET-08.1-DMZNetworks
:OPS-NET-08.1-DMZNetworks rdf:type owl:NamedIndividual ,
                                   :Security_Operations_Policies ;
                          :HasWeight 8 ;
                          rdfs:comment "Mechanisms exist to monitor De-Militarized Zone (DMZ) network segments to separate untrusted networks from trusted networks." .


###  http://FYP-ASHS21/csonto/OPS-NET-08.2-WirelessIntrusionDetection-PreventionSystems-WIDS-WIPS-
:OPS-NET-08.2-WirelessIntrusionDetection-PreventionSystems-WIDS-WIPS- rdf:type owl:NamedIndividual ,
                                                                               :Security_Operations_Policies ;
                                                                      :HasWeight 8 ;
                                                                      rdfs:comment "Mechanisms exist to monitor wireless network segments to implement Wireless Intrusion Detection / Prevention Systems (WIDS/WIPS) technologies." .


###  http://FYP-ASHS21/csonto/OPS-NET-09-SessionIntegrity
:OPS-NET-09-SessionIntegrity rdf:type owl:NamedIndividual ,
                                      :Security_Operations_Policies ;
                             :HasWeight 8 ;
                             rdfs:comment "Mechanisms exist to protect the authenticity and integrity of communications sessions. " .


###  http://FYP-ASHS21/csonto/OPS-NET-09.1-InvalidateSessionIdentifiersatLogout
:OPS-NET-09.1-InvalidateSessionIdentifiersatLogout rdf:type owl:NamedIndividual ,
                                                            :Security_Operations_Policies ;
                                                   :HasWeight 5 ;
                                                   rdfs:comment "Automated mechanisms exist to invalidate session identifiers upon user logout or other session termination. " .


###  http://FYP-ASHS21/csonto/OPS-NET-09.2-UniqueSystem-GeneratedSessionIdentifiers
:OPS-NET-09.2-UniqueSystem-GeneratedSessionIdentifiers rdf:type owl:NamedIndividual ,
                                                                :Security_Operations_Policies ;
                                                       :HasWeight 3 ;
                                                       rdfs:comment "Automated mechanisms exist to generate and recognize unique session identifiers for each session." .


###  http://FYP-ASHS21/csonto/OPS-NET-10-DomainNameService-DNS-Resolution
:OPS-NET-10-DomainNameService-DNS-Resolution rdf:type owl:NamedIndividual ,
                                                      :Security_Operations_Policies ;
                                             :HasWeight 10 ;
                                             rdfs:comment "Mechanisms exist to ensure Domain Name Service (DNS) resolution is designed, implemented and managed to protect the security of name / address resolution." .


###  http://FYP-ASHS21/csonto/OPS-NET-10.2-SecureName-AddressResolutionService-RecursiveorCachingResolver-
:OPS-NET-10.2-SecureName-AddressResolutionService-RecursiveorCachingResolver- rdf:type owl:NamedIndividual ,
                                                                                       :Security_Operations_Policies ;
                                                                              :HasWeight 9 ;
                                                                              rdfs:comment "Mechanisms exist to perform data origin authentication and data integrity verification on the Domain Name Service (DNS) resolution responses received from authoritative sources when requested by client systems. " .


###  http://FYP-ASHS21/csonto/OPS-NET-10.3-SenderPolicyFramework-SPF-
:OPS-NET-10.3-SenderPolicyFramework-SPF- rdf:type owl:NamedIndividual ,
                                                  :Security_Operations_Policies ;
                                         :HasWeight 8 ;
                                         rdfs:comment "Mechanisms exist to validate the legitimacy of email communications through configuring a Domain Naming Service (DNS) Sender Policy Framework (SPF) record to specify the IP addresses and/or hostnames that are authorized to send email from the specified domain." .


###  http://FYP-ASHS21/csonto/OPS-NET-10.4-DomainRegistrarSecurity
:OPS-NET-10.4-DomainRegistrarSecurity rdf:type owl:NamedIndividual ,
                                               :Security_Operations_Policies ;
                                      :HasWeight 9 ;
                                      rdfs:comment "Mechanisms exist to lock the domain name registrar to prevent a denial of service caused by unauthorized deletion, transfer or other unauthorized modification of a domains registration details." .


###  http://FYP-ASHS21/csonto/OPS-NET-11-Out-of-BandChannels
:OPS-NET-11-Out-of-BandChannels rdf:type owl:NamedIndividual ,
                                         :Security_Operations_Policies ;
                                :HasWeight 9 ;
                                rdfs:comment "Mechanisms exist to utilize out-of-band channels for the electronic transmission of information and/or the physical shipment of system components or devices to authorized individuals. " .


###  http://FYP-ASHS21/csonto/OPS-NET-12-SafeguardingDataOverOpenNetworks
:OPS-NET-12-SafeguardingDataOverOpenNetworks rdf:type owl:NamedIndividual ,
                                                      :Security_Operations_Policies ;
                                             :HasWeight 8 ;
                                             rdfs:comment "Cryptographic mechanisms exist to implement strong cryptography and security protocols to safeguard sensitive/regulated data during transmission over open, public networks. " .


###  http://FYP-ASHS21/csonto/OPS-NET-12.1-WirelessLinkProtection
:OPS-NET-12.1-WirelessLinkProtection rdf:type owl:NamedIndividual ,
                                              :Security_Operations_Policies ;
                                     :HasWeight 8 ;
                                     rdfs:comment "Mechanisms exist to protect external and internal wireless links from signal parameter attacks through monitoring for unauthorized wireless connections, including scanning for unauthorized wireless access points and taking appropriate action, if an unauthorized connection is discovered." .


###  http://FYP-ASHS21/csonto/OPS-NET-12.2-End-UserMessagingTechnologies
:OPS-NET-12.2-End-UserMessagingTechnologies rdf:type owl:NamedIndividual ,
                                                     :Security_Operations_Policies ;
                                            :HasWeight 9 ;
                                            rdfs:comment "Mechanisms exist to prohibit the transmission of unprotected sensitive/regulated data by end-user messaging technologies. " .


###  http://FYP-ASHS21/csonto/OPS-NET-13-ElectronicMessaging
:OPS-NET-13-ElectronicMessaging rdf:type owl:NamedIndividual ,
                                         :Security_Operations_Policies ;
                                :HasWeight 10 ;
                                rdfs:comment "Mechanisms exist to protect the confidentiality, integrity and availability of electronic messaging communications." .


###  http://FYP-ASHS21/csonto/OPS-NET-14-RemoteAccess
:OPS-NET-14-RemoteAccess rdf:type owl:NamedIndividual ,
                                  :Security_Operations_Policies ;
                         :HasWeight 10 ;
                         rdfs:comment "Mechanisms exist to define, control and review organization-approved, secure remote access methods." .


###  http://FYP-ASHS21/csonto/OPS-NET-14.2-ProtectionofConfidentiality-IntegrityUsingEncryption
:OPS-NET-14.2-ProtectionofConfidentiality-IntegrityUsingEncryption rdf:type owl:NamedIndividual ,
                                                                            :Security_Operations_Policies ;
                                                                   :HasWeight 9 ;
                                                                   rdfs:comment "Cryptographic mechanisms exist to protect the confidentiality and integrity of remote access sessions (e.g., VPN). " .


###  http://FYP-ASHS21/csonto/OPS-NET-14.3-ManagedAccessControlPoints
:OPS-NET-14.3-ManagedAccessControlPoints rdf:type owl:NamedIndividual ,
                                                  :Security_Operations_Policies ;
                                         :HasWeight 9 ;
                                         rdfs:comment "Mechanisms exist to route all remote accesses through managed network access control points (e.g., VPN concentrator)." .


###  http://FYP-ASHS21/csonto/OPS-NET-14.5-WorkFromAnywhere-WFA--TelecommutingSecurity
:OPS-NET-14.5-WorkFromAnywhere-WFA--TelecommutingSecurity rdf:type owl:NamedIndividual ,
                                                                   :Security_Operations_Policies ;
                                                          :HasWeight 10 ;
                                                          rdfs:comment "Mechanisms exist to define secure telecommuting practices and govern remote access to systems and data for remote workers. " .


###  http://FYP-ASHS21/csonto/OPS-NET-14.6-Third-PartyRemoteAccessGovernance
:OPS-NET-14.6-Third-PartyRemoteAccessGovernance rdf:type owl:NamedIndividual ,
                                                         :Security_Operations_Policies ;
                                                :HasWeight 8 ;
                                                rdfs:comment "Mechanisms exist to proactively control and monitor third-party accounts used to access, support, or maintain system components via remote access." .


###  http://FYP-ASHS21/csonto/OPS-NET-14.7-EndpointSecurityValidation
:OPS-NET-14.7-EndpointSecurityValidation rdf:type owl:NamedIndividual ,
                                                  :Security_Operations_Policies ;
                                         :HasWeight 6 ;
                                         rdfs:comment "Mechanisms exist to validate software versions/patch levels and control remote devices connecting to corporate networks or storing and accessing organization information. " .


###  http://FYP-ASHS21/csonto/OPS-NET-14.8-ExpeditiousDisconnect-DisableCapability
:OPS-NET-14.8-ExpeditiousDisconnect-DisableCapability rdf:type owl:NamedIndividual ,
                                                               :Security_Operations_Policies ;
                                                      :HasWeight 8 ;
                                                      rdfs:comment "Mechanisms exist to provide the capability to expeditiously disconnect or disable a user's remote access session." .


###  http://FYP-ASHS21/csonto/OPS-NET-15-WirelessNetworking
:OPS-NET-15-WirelessNetworking rdf:type owl:NamedIndividual ,
                                        :Security_Operations_Policies ;
                               :HasWeight 9 ;
                               rdfs:comment "Mechanisms exist to control authorized wireless usage and monitor for unauthorized wireless access." .


###  http://FYP-ASHS21/csonto/OPS-NET-15.2-DisableWirelessNetworking
:OPS-NET-15.2-DisableWirelessNetworking rdf:type owl:NamedIndividual ,
                                                 :Security_Operations_Policies ;
                                        :HasWeight 5 ;
                                        rdfs:comment "Mechanisms exist to disable unnecessary wireless networking capabilities that are internally embedded within system components prior to issuance to end users. " .


###  http://FYP-ASHS21/csonto/OPS-NET-15.3-RestrictConfigurationByUsers
:OPS-NET-15.3-RestrictConfigurationByUsers rdf:type owl:NamedIndividual ,
                                                    :Security_Operations_Policies ;
                                           :HasWeight 8 ;
                                           rdfs:comment "Mechanisms exist to identify and explicitly authorize users who are allowed to independently configure wireless networking capabilities. " .


###  http://FYP-ASHS21/csonto/OPS-NET-15.4-WirelessBoundaries
:OPS-NET-15.4-WirelessBoundaries rdf:type owl:NamedIndividual ,
                                          :Security_Operations_Policies ;
                                 :HasWeight 5 ;
                                 rdfs:comment "Mechanisms exist to confine wireless communications to organization-controlled boundaries. " .


###  http://FYP-ASHS21/csonto/OPS-NET-15.5-RogueWirelessDetection
:OPS-NET-15.5-RogueWirelessDetection rdf:type owl:NamedIndividual ,
                                              :Security_Operations_Policies ;
                                     :HasWeight 8 ;
                                     rdfs:comment "Mechanisms exist to test for the presence of Wireless Access Points (WAPs) and identify all authorized and unauthorized WAPs within the facility(ies). " .


###  http://FYP-ASHS21/csonto/OPS-NET-16-Intranets
:OPS-NET-16-Intranets rdf:type owl:NamedIndividual ,
                               :Security_Operations_Policies ;
                      :HasWeight 8 ;
                      rdfs:comment """Mechanisms exist to establish trust relationships with other organizations owning, operating, and/or maintaining intranet systems, allowing authorized individuals to: 
  Access the intranet from external systems; and
  Process, store, and/or transmit organization-controlled information using the external systems.""" .


###  http://FYP-ASHS21/csonto/OPS-NET-17-DataLossPrevention-DLP-
:OPS-NET-17-DataLossPrevention-DLP- rdf:type owl:NamedIndividual ,
                                             :Security_Operations_Policies ;
                                    :HasWeight 8 ;
                                    rdfs:comment "Automated mechanisms exist to implement Data Loss Prevention (DLP) to protect sensitive information as it is stored, transmitted and processed." .


###  http://FYP-ASHS21/csonto/OPS-NET-18.1-RouteTraffictoProxyServers
:OPS-NET-18.1-RouteTraffictoProxyServers rdf:type owl:NamedIndividual ,
                                                  :Security_Operations_Policies ;
                                         :HasWeight 9 ;
                                         rdfs:comment "Mechanisms exist to route internal communications traffic to external networks through organization-approved proxy servers at managed interfaces. " .


###  http://FYP-ASHS21/csonto/OPS-NET-18.2-VisibilityofEncryptedCommunications
:OPS-NET-18.2-VisibilityofEncryptedCommunications rdf:type owl:NamedIndividual ,
                                                           :Security_Operations_Policies ;
                                                  :HasWeight 5 ;
                                                  rdfs:comment "Mechanisms exist to configure the proxy to make encrypted communications traffic visible to monitoring tools and mechanisms." .


###  http://FYP-ASHS21/csonto/OPS-NET-18.3-RoutePrivilegedNetworkAccess
:OPS-NET-18.3-RoutePrivilegedNetworkAccess rdf:type owl:NamedIndividual ,
                                                    :Security_Operations_Policies ;
                                           :HasWeight 1 ;
                                           rdfs:comment "Automated mechanisms exist to route networked, privileged accesses through a dedicated, managed interface for purposes of access control and auditing." .


###  http://FYP-ASHS21/csonto/OPS-OPS-01-OperationsSecurity
:OPS-OPS-01-OperationsSecurity rdf:type owl:NamedIndividual ,
                                        :Security_Operations_Policies ;
                               :HasWeight 8 ;
                               rdfs:comment "Mechanisms exist to facilitate the implementation of operational security controls." .


###  http://FYP-ASHS21/csonto/OPS-OPS-01.1-StandardizedOperatingProcedures-SOP-
:OPS-OPS-01.1-StandardizedOperatingProcedures-SOP- rdf:type owl:NamedIndividual ,
                                                            :Security_Operations_Policies ;
                                                   :HasWeight 9 ;
                                                   rdfs:comment "Mechanisms exist to identify and document Standardized Operating Procedures (SOP), or similar documentation, to enable the proper execution of day-to-day / assigned tasks." .


###  http://FYP-ASHS21/csonto/OPS-OPS-02-SecurityConceptOfOperations-CONOPS-
:OPS-OPS-02-SecurityConceptOfOperations-CONOPS- rdf:type owl:NamedIndividual ,
                                                         :Security_Operations_Policies ;
                                                :HasWeight 9 ;
                                                rdfs:comment "Mechanisms exist to develop a security Concept of Operations (CONOPS), or a similarly-defined plan for achieving cybersecurity objectives, that documents management, operational and technical measures implemented to apply defense-in-depth techniques that is communicated to all appropriate stakeholders. " .


###  http://FYP-ASHS21/csonto/OPS-OPS-03-ServiceDelivery-BusinessProcessSupport-
:OPS-OPS-03-ServiceDelivery-BusinessProcessSupport- rdf:type owl:NamedIndividual ,
                                                             :Security_Operations_Policies ;
                                                    :HasWeight 7 ;
                                                    rdfs:comment "Mechanisms exist to define supporting business processes and implement appropriate governance and service management to ensure appropriate planning, delivery and support of the organization's technology capabilities supporting business functions, workforce, and/or customers based on industry-recognized standards to achieve the specific goals of the process area." .


###  http://FYP-ASHS21/csonto/OPS-OPS-04-SecurityOperationsCenter-SOC-
:OPS-OPS-04-SecurityOperationsCenter-SOC- rdf:type owl:NamedIndividual ,
                                                   :Security_Operations_Policies ;
                                          :HasWeight 8 ;
                                          rdfs:comment "Mechanisms exist to establish and maintain a Security Operations Center (SOC) that facilitates a 24x7 response capability." .


###  http://FYP-ASHS21/csonto/OPS-OPS-05-SecurePracticesGuidelines
:OPS-OPS-05-SecurePracticesGuidelines rdf:type owl:NamedIndividual ,
                                               :Security_Operations_Policies ;
                                      :HasWeight 7 ;
                                      rdfs:comment "Mechanisms exist to provide guidelines and recommendations for the secure use of products and/or services to assist in the configuration, installation and use of the product and/or service." .


###  http://FYP-ASHS21/csonto/OPS-PRI-01-DataPrivacyProgram
:OPS-PRI-01-DataPrivacyProgram rdf:type owl:NamedIndividual ,
                                        :Security_Operations_Policies ;
                               :HasWeight 10 ;
                               rdfs:comment "Mechanisms exist to facilitate the implementation and operation of data privacy controls. " .


###  http://FYP-ASHS21/csonto/OPS-PRI-01.1-ChiefPrivacyOfficer-CPO-
:OPS-PRI-01.1-ChiefPrivacyOfficer-CPO- rdf:type owl:NamedIndividual ,
                                                :Security_Operations_Policies ;
                                       :HasWeight 3 ;
                                       rdfs:comment "Mechanisms exist to appoints a Chief Privacy Officer (CPO) or similar role, with the authority, mission, accountability and resources to coordinate, develop and implement, applicable data privacy requirements and manage data privacy risks through the organization-wide data privacy program." .


###  http://FYP-ASHS21/csonto/OPS-PRI-01.2-PrivacyActStatements
:OPS-PRI-01.2-PrivacyActStatements rdf:type owl:NamedIndividual ,
                                            :Security_Operations_Policies ;
                                   :HasWeight 2 ;
                                   rdfs:comment """Mechanisms exist to provide additional formal notice to individuals from whom the information is being collected that includes:
  Notice of the authority of organizations to collect Personal Data (PD); 
  Whether providing Personal Data (PD) is mandatory or optional; 
  The principal purpose or purposes for which the Personal Data (PD) is to be used; 
  The intended disclosures or routine uses of the information; and 
  The consequences of not providing all or some portion of the information requested.""" .


###  http://FYP-ASHS21/csonto/OPS-PRI-01.3-DisseminationofDataPrivacyProgramInformation
:OPS-PRI-01.3-DisseminationofDataPrivacyProgramInformation rdf:type owl:NamedIndividual ,
                                                                    :Security_Operations_Policies ;
                                                           :HasWeight 5 ;
                                                           rdfs:comment """Mechanisms exist to: 
  Ensure that the public has access to information about organizational data privacy activities and can communicate with its Chief Privacy Officer (CPO) or similar role;
  Ensure that organizational data privacy practices are publicly available through organizational websites or otherwise; and
  Utilize publicly facing email addresses and/or phone lines to enable the public to provide feedback and/or direct questions to data privacy office(s) regarding data privacy practices.""" .


###  http://FYP-ASHS21/csonto/OPS-PRI-01.4-DataProtectionOfficer-DPO-
:OPS-PRI-01.4-DataProtectionOfficer-DPO- rdf:type owl:NamedIndividual ,
                                                  :Security_Operations_Policies ;
                                         :HasWeight 7 ;
                                         rdfs:comment """Mechanisms exist to appoint a Data Protection Officer (DPO):
  Based on the basis of professional qualities; and
  To be involved in all issues related to the protection of personal data.""" .


###  http://FYP-ASHS21/csonto/OPS-PRI-01.5-BindingCorporateRules-BCR-
:OPS-PRI-01.5-BindingCorporateRules-BCR- rdf:type owl:NamedIndividual ,
                                                  :Security_Operations_Policies ;
                                         :HasWeight 5 ;
                                         rdfs:comment "Mechanisms exist to implement and manage Binding Corporate Rules (BCR) (e.g., data sharing agreement) to legally-bind all parties engaged in a joint economic activity that contractually states enforceable rights on data subjects with regard to the processing of their personal data." .


###  http://FYP-ASHS21/csonto/OPS-PRI-01.6-SecurityofPersonalData
:OPS-PRI-01.6-SecurityofPersonalData rdf:type owl:NamedIndividual ,
                                              :Security_Operations_Policies ;
                                     :HasWeight 7 ;
                                     rdfs:comment "Mechanisms exist to ensure Personal Data (PD) is protected by security safeguards that are sufficient and appropriately scoped to protect the confidentiality and integrity of the PD." .


###  http://FYP-ASHS21/csonto/OPS-PRI-01.7-LimitingPersonalDataDisclosures
:OPS-PRI-01.7-LimitingPersonalDataDisclosures rdf:type owl:NamedIndividual ,
                                                       :Security_Operations_Policies ;
                                              :HasWeight 7 ;
                                              rdfs:comment "Mechanisms exist to limit the disclosure of Personal Data (PD) to authorized parties for the sole purpose for which the PD was obtained." .


###  http://FYP-ASHS21/csonto/OPS-PRI-02-DataPrivacyNotice
:OPS-PRI-02-DataPrivacyNotice rdf:type owl:NamedIndividual ,
                                       :Security_Operations_Policies ;
                              :HasWeight 7 ;
                              rdfs:comment """Mechanisms exist to:
 Make data privacy notice(s) available to individuals upon first interacting with an organization and subsequently as necessary; 
 Ensure that data privacy notices are clear and easy-to-understand, expressing information about Personal Data (PD) processing in plain language that meet all legal obligations; and
 Define the scope of PD processing activities, including the geographic locations and third-party recipients that process the PD within the scope of the data privacy notice.""" .


###  http://FYP-ASHS21/csonto/OPS-PRI-02.1-PurposeSpecification
:OPS-PRI-02.1-PurposeSpecification rdf:type owl:NamedIndividual ,
                                            :Security_Operations_Policies ;
                                   :HasWeight 7 ;
                                   rdfs:comment "Mechanisms exist to identify and document the purpose(s) for which Personal Data (PD) is collected, used, maintained and shared in its data privacy notices." .


###  http://FYP-ASHS21/csonto/OPS-PRI-02.2-AutomatedDataManagementProcesses
:OPS-PRI-02.2-AutomatedDataManagementProcesses rdf:type owl:NamedIndividual ,
                                                        :Security_Operations_Policies ;
                                               :HasWeight 1 ;
                                               rdfs:comment "Automated mechanisms exist to adjust data that is able to be collected, created, used, disseminated, maintained, retained and/or disclosed, based on updated data subject authorization(s)." .


###  http://FYP-ASHS21/csonto/OPS-PRI-02.3-ComputerMatchingAgreements-CMA-
:OPS-PRI-02.3-ComputerMatchingAgreements-CMA- rdf:type owl:NamedIndividual ,
                                                       :Security_Operations_Policies ;
                                              :HasWeight 1 ;
                                              rdfs:comment "Mechanisms exist to publish Computer Matching Agreements (CMA) on the public website of the organization." .


###  http://FYP-ASHS21/csonto/OPS-PRI-02.4-SystemofRecordsNotice-SORN-
:OPS-PRI-02.4-SystemofRecordsNotice-SORN- rdf:type owl:NamedIndividual ,
                                                   :Security_Operations_Policies ;
                                          :HasWeight 1 ;
                                          rdfs:comment "Mechanisms exist to draft, publish and keep System of Records Notices (SORN) updated in accordance with regulatory guidance." .


###  http://FYP-ASHS21/csonto/OPS-PRI-02.5-SystemofRecordsNotice-SORN-ReviewProcess
:OPS-PRI-02.5-SystemofRecordsNotice-SORN-ReviewProcess rdf:type owl:NamedIndividual ,
                                                                :Security_Operations_Policies ;
                                                       :HasWeight 1 ;
                                                       rdfs:comment "Mechanisms exist to review all routine uses of data published in the System of Records Notices (SORN) to ensure continued accuracy and to ensure that routine uses continue to be compatible with the purpose for which the information was collected." .


###  http://FYP-ASHS21/csonto/OPS-PRI-02.6-PrivacyActExemptions
:OPS-PRI-02.6-PrivacyActExemptions rdf:type owl:NamedIndividual ,
                                            :Security_Operations_Policies ;
                                   :HasWeight 1 ;
                                   rdfs:comment "Mechanisms exist to review all Privacy Act exemptions claimed for the System of Records Notices (SORN) to ensure they remain appropriate and accurate." .


###  http://FYP-ASHS21/csonto/OPS-PRI-02.7-Real-TimeorLayeredNotice
:OPS-PRI-02.7-Real-TimeorLayeredNotice rdf:type owl:NamedIndividual ,
                                                :Security_Operations_Policies ;
                                       :HasWeight 2 ;
                                       rdfs:comment "Mechanisms exist to provide real-time and/or layered notice when Personal Data (PD) is collected that provides data subjects with a summary of key points or more detailed information that is specific to the organization's data privacy notice." .


###  http://FYP-ASHS21/csonto/OPS-PRI-03.1-TailoredConsent
:OPS-PRI-03.1-TailoredConsent rdf:type owl:NamedIndividual ,
                                       :Security_Operations_Policies ;
                              :HasWeight 1 ;
                              rdfs:comment "Mechanisms exist to allow data subjects to modify the use permissions to selected attributes of their Personal Data (PD)." .


###  http://FYP-ASHS21/csonto/OPS-PRI-03.3-ProhibitionOfSellingorSharingPersonalData
:OPS-PRI-03.3-ProhibitionOfSellingorSharingPersonalData rdf:type owl:NamedIndividual ,
                                                                 :Security_Operations_Policies ;
                                                        :HasWeight 5 ;
                                                        rdfs:comment "Mechanisms exist to prevent the sale or sharing of Personal Data (PD) when instructed by the data subject." .


###  http://FYP-ASHS21/csonto/OPS-PRI-03.4-RevokeConsent
:OPS-PRI-03.4-RevokeConsent rdf:type owl:NamedIndividual ,
                                     :Security_Operations_Policies ;
                            :HasWeight 3 ;
                            rdfs:comment "Mechanisms exist to allow data subjects to revoke consent to the processing of their Personal Data (PD)." .


###  http://FYP-ASHS21/csonto/OPS-PRI-03.5-ProductorServiceDeliveryRestrictions
:OPS-PRI-03.5-ProductorServiceDeliveryRestrictions rdf:type owl:NamedIndividual ,
                                                            :Security_Operations_Policies ;
                                                   :HasWeight 7 ;
                                                   rdfs:comment "Mechanisms exist to prohibit the refusal of products and/or services on the grounds that a data subject does not agree to the processing of Personal Data (PD) or withdraws consent." .


###  http://FYP-ASHS21/csonto/OPS-PRI-03.6-AuthorizedAgent
:OPS-PRI-03.6-AuthorizedAgent rdf:type owl:NamedIndividual ,
                                       :Security_Operations_Policies ;
                              :HasWeight 6 ;
                              rdfs:comment "Mechanisms exist to allow data subjects to authorize another person or entity, acting on the data subject's behalf, to make Personal Data (PD) processing decisions." .


###  http://FYP-ASHS21/csonto/OPS-PRI-03.7-ActiveParticipationByDataSubjects
:OPS-PRI-03.7-ActiveParticipationByDataSubjects rdf:type owl:NamedIndividual ,
                                                         :Security_Operations_Policies ;
                                                :HasWeight 3 ;
                                                rdfs:comment "Mechanisms exist to compel data subjects to select the level of consent deemed appropriate by the data subject for the relevant business purpose (e.g., opt-in, opt-out, accept all cookies, etc.)." .


###  http://FYP-ASHS21/csonto/OPS-PRI-03.8-GlobalPrivacyControl-GPC-
:OPS-PRI-03.8-GlobalPrivacyControl-GPC- rdf:type owl:NamedIndividual ,
                                                 :Security_Operations_Policies ;
                                        :HasWeight 5 ;
                                        rdfs:comment "Automated mechanisms exist to provide data subjects with functionality to exercise pre-selected opt-out preferences (e.g., opt-out signal)." .


###  http://FYP-ASHS21/csonto/OPS-PRI-04-RestrictCollectionToIdentifiedPurpose
:OPS-PRI-04-RestrictCollectionToIdentifiedPurpose rdf:type owl:NamedIndividual ,
                                                           :Security_Operations_Policies ;
                                                  :HasWeight 7 ;
                                                  rdfs:comment "Mechanisms exist to collect Personal Data (PD) only for the purposes identified in the data privacy notice and includes protections against collecting PD from minors without appropriate parental, or legal guardian, consent." .


###  http://FYP-ASHS21/csonto/OPS-PRI-04.2-PrimarySources
:OPS-PRI-04.2-PrimarySources rdf:type owl:NamedIndividual ,
                                      :Security_Operations_Policies ;
                             :HasWeight 7 ;
                             rdfs:comment "Mechanisms exist to ensure information is directly collected from the data subject, whenever possible." .


###  http://FYP-ASHS21/csonto/OPS-PRI-04.3-IdentifiableImageCollection
:OPS-PRI-04.3-IdentifiableImageCollection rdf:type owl:NamedIndividual ,
                                                   :Security_Operations_Policies ;
                                          :HasWeight 7 ;
                                          rdfs:comment "Mechanisms exist to restrict the collection, processing, storage and sharing of photographic and/or video surveillance image collection that can identify individuals to legitimate business needs." .


###  http://FYP-ASHS21/csonto/OPS-PRI-04.4-AcquiredPersonalData
:OPS-PRI-04.4-AcquiredPersonalData rdf:type owl:NamedIndividual ,
                                            :Security_Operations_Policies ;
                                   :HasWeight 6 ;
                                   rdfs:comment "Mechanisms exist to promptly inform data subjects of the utilization purpose when their Personal Data (PD) is acquired and not received directly from the data subject, except where that utilization purpose was disclosed in advance to the data subject." .


###  http://FYP-ASHS21/csonto/OPS-PRI-04.5-ValidateCollectedPersonalData
:OPS-PRI-04.5-ValidateCollectedPersonalData rdf:type owl:NamedIndividual ,
                                                     :Security_Operations_Policies ;
                                            :HasWeight 1 ;
                                            rdfs:comment "Mechanisms exist to ensure that the data subject, or authorized representative, validate Personal Data (PD) during the collection process." .


###  http://FYP-ASHS21/csonto/OPS-PRI-04.6-Re-ValidateCollectedPersonalData
:OPS-PRI-04.6-Re-ValidateCollectedPersonalData rdf:type owl:NamedIndividual ,
                                                        :Security_Operations_Policies ;
                                               :HasWeight 1 ;
                                               rdfs:comment "Mechanisms exist to ensure that the data subject, or authorized representative, re-validate that Personal Data (PD) acquired during the collection process is still accurate." .


###  http://FYP-ASHS21/csonto/OPS-PRI-05.1-InternalUseofPersonalDataForTesting-TrainingandResearch
:OPS-PRI-05.1-InternalUseofPersonalDataForTesting-TrainingandResearch rdf:type owl:NamedIndividual ,
                                                                               :Security_Operations_Policies ;
                                                                      :HasWeight 8 ;
                                                                      rdfs:comment """Mechanisms exist to address the use of Personal Data (PD) for internal testing, training and research that:
  Takes measures to limit or minimize the amount of PD used for internal testing, training and research purposes; and
  Authorizes the use of PD when such information is required for internal testing, training and research.""" .


###  http://FYP-ASHS21/csonto/OPS-PRI-05.3-DataMasking
:OPS-PRI-05.3-DataMasking rdf:type owl:NamedIndividual ,
                                   :Security_Operations_Policies ;
                          :HasWeight 8 ;
                          rdfs:comment "Mechanisms exist to mask sensitive information through data anonymization, pseudonymization, redaction or de-identification." .


###  http://FYP-ASHS21/csonto/OPS-PRI-05.4-UsageRestrictionsofSensitivePersonalData
:OPS-PRI-05.4-UsageRestrictionsofSensitivePersonalData rdf:type owl:NamedIndividual ,
                                                                :Security_Operations_Policies ;
                                                       :HasWeight 8 ;
                                                       rdfs:comment "Mechanisms exist to restrict the use of Personal Data (PD) to only the authorized purpose(s) consistent with applicable laws, regulations and in data privacy notices. " .


###  http://FYP-ASHS21/csonto/OPS-PRI-05.5-InventoryofPersonalData
:OPS-PRI-05.5-InventoryofPersonalData rdf:type owl:NamedIndividual ,
                                               :Security_Operations_Policies ;
                                      :HasWeight 8 ;
                                      rdfs:comment "Mechanisms exist to establish, maintain and update an inventory that contains a listing of all programs and systems identified as collecting, using, maintaining, or sharing Personal Data (PD). " .


###  http://FYP-ASHS21/csonto/OPS-PRI-05.6-PersonalDataInventoryAutomationSupport
:OPS-PRI-05.6-PersonalDataInventoryAutomationSupport rdf:type owl:NamedIndividual ,
                                                              :Security_Operations_Policies ;
                                                     :HasWeight 1 ;
                                                     rdfs:comment "Automated mechanisms exist to determine if Personal Data (PD) is maintained in electronic form." .


###  http://FYP-ASHS21/csonto/OPS-PRI-05.7-PersonalDataCategories
:OPS-PRI-05.7-PersonalDataCategories rdf:type owl:NamedIndividual ,
                                              :Security_Operations_Policies ;
                                     :HasWeight 5 ;
                                     rdfs:comment "Mechanisms exist to define and implement data handling and protection requirements for specific categories of sensitive Personal Data (PD)." .


###  http://FYP-ASHS21/csonto/OPS-PRI-06-DataSubjectAccess
:OPS-PRI-06-DataSubjectAccess rdf:type owl:NamedIndividual ,
                                       :Security_Operations_Policies ;
                              :HasWeight 6 ;
                              rdfs:comment "Mechanisms exist to provide data subjects the ability to access their Personal Data (PD) maintained in organizational systems of records." .


###  http://FYP-ASHS21/csonto/OPS-PRI-06.1-CorrectingInaccuratePersonalData
:OPS-PRI-06.1-CorrectingInaccuratePersonalData rdf:type owl:NamedIndividual ,
                                                        :Security_Operations_Policies ;
                                               :HasWeight 5 ;
                                               rdfs:comment """Mechanisms exist to establish and implement a process for:
  Data subjects to have inaccurate Personal Data (PD) maintained by the organization corrected or amended; and
  Disseminating corrections or amendments of PD to other authorized users of the PD.""" .


###  http://FYP-ASHS21/csonto/OPS-PRI-06.2-NoticeofCorrectionorProcessingChange
:OPS-PRI-06.2-NoticeofCorrectionorProcessingChange rdf:type owl:NamedIndividual ,
                                                            :Security_Operations_Policies ;
                                                   :HasWeight 4 ;
                                                   rdfs:comment "Mechanisms exist to notify affected data subjects if their Personal Data (PD) has been corrected or amended." .


###  http://FYP-ASHS21/csonto/OPS-PRI-06.3-AppealAdverseDecision
:OPS-PRI-06.3-AppealAdverseDecision rdf:type owl:NamedIndividual ,
                                             :Security_Operations_Policies ;
                                    :HasWeight 4 ;
                                    rdfs:comment "Mechanisms exist to provide an organization-defined process for data subjects to appeal an adverse decision and have incorrect information amended." .


###  http://FYP-ASHS21/csonto/OPS-PRI-06.4-UserFeedbackManagement
:OPS-PRI-06.4-UserFeedbackManagement rdf:type owl:NamedIndividual ,
                                              :Security_Operations_Policies ;
                                     :HasWeight 5 ;
                                     rdfs:comment "Mechanisms exist to implement a process for receiving and responding to complaints, concerns or questions from data subjects about the organizational data privacy practices." .


###  http://FYP-ASHS21/csonto/OPS-PRI-06.5-RighttoErasure
:OPS-PRI-06.5-RighttoErasure rdf:type owl:NamedIndividual ,
                                      :Security_Operations_Policies ;
                             :HasWeight 5 ;
                             rdfs:comment "Mechanisms exist to erase personal data of a data subject, without delay." .


###  http://FYP-ASHS21/csonto/OPS-PRI-06.6-DataPortability
:OPS-PRI-06.6-DataPortability rdf:type owl:NamedIndividual ,
                                       :Security_Operations_Policies ;
                              :HasWeight 3 ;
                              rdfs:comment "Mechanisms exist to export Personal Data (PD) in a structured, commonly used and machine-readable format that allows the data subject to transmit the data to another controller without hindrance." .


###  http://FYP-ASHS21/csonto/OPS-PRI-06.7-PersonalDataExportability
:OPS-PRI-06.7-PersonalDataExportability rdf:type owl:NamedIndividual ,
                                                 :Security_Operations_Policies ;
                                        :HasWeight 5 ;
                                        rdfs:comment "Mechanisms exist to digitally export Personal Data (PD) in a secure manner upon request by the data subject." .


###  http://FYP-ASHS21/csonto/OPS-PRI-07-InformationSharingWithThirdParties
:OPS-PRI-07-InformationSharingWithThirdParties rdf:type owl:NamedIndividual ,
                                                        :Security_Operations_Policies ;
                                               :HasWeight 9 ;
                                               rdfs:comment "Mechanisms exist to disclose Personal Data (PD) to third-parties only for the purposes identified in the data privacy notice and with the implicit or explicit consent of the data subject. " .


###  http://FYP-ASHS21/csonto/OPS-PRI-07.2-JointProcessingofPersonalData
:OPS-PRI-07.2-JointProcessingofPersonalData rdf:type owl:NamedIndividual ,
                                                     :Security_Operations_Policies ;
                                            :HasWeight 5 ;
                                            rdfs:comment "Mechanisms exist to clearly define and communicate the organization's role in processing Personal Data (PD) in the data processing ecosystem. " .


###  http://FYP-ASHS21/csonto/OPS-PRI-07.3-ObligationToInformThird-Parties
:OPS-PRI-07.3-ObligationToInformThird-Parties rdf:type owl:NamedIndividual ,
                                                       :Security_Operations_Policies ;
                                              :HasWeight 5 ;
                                              rdfs:comment "Mechanisms exist to inform applicable third-parties of any modification, deletion or other change that affects shared Personal Data (PD)." .


###  http://FYP-ASHS21/csonto/OPS-PRI-07.4-RejectUnauthorizedDisclosureRequests
:OPS-PRI-07.4-RejectUnauthorizedDisclosureRequests rdf:type owl:NamedIndividual ,
                                                            :Security_Operations_Policies ;
                                                   :HasWeight 5 ;
                                                   rdfs:comment "Mechanisms exist to reject unauthorized disclosure requests." .


###  http://FYP-ASHS21/csonto/OPS-PRI-09-PersonalDataLineage
:OPS-PRI-09-PersonalDataLineage rdf:type owl:NamedIndividual ,
                                         :Security_Operations_Policies ;
                                :HasWeight 5 ;
                                rdfs:comment "Mechanisms exist to utilize a record of processing activities to maintain a record of Personal Data (PD) that is stored, transmitted and/or processed under the organization's responsibility." .


###  http://FYP-ASHS21/csonto/OPS-PRI-10-DataQualityManagement
:OPS-PRI-10-DataQualityManagement rdf:type owl:NamedIndividual ,
                                           :Security_Operations_Policies ;
                                  :HasWeight 5 ;
                                  rdfs:comment "Mechanisms exist to issue guidelines ensuring and maximizing the quality, utility, objectivity, integrity, impact determination and de-identification of Personal Data (PD) across the information lifecycle." .


###  http://FYP-ASHS21/csonto/OPS-PRI-10.1-Automation
:OPS-PRI-10.1-Automation rdf:type owl:NamedIndividual ,
                                  :Security_Operations_Policies ;
                         :HasWeight 1 ;
                         rdfs:comment "Automated mechanisms exist to support the evaluation of data quality across the information lifecycle." .


###  http://FYP-ASHS21/csonto/OPS-PRI-10.2-DataAnalyticsBias
:OPS-PRI-10.2-DataAnalyticsBias rdf:type owl:NamedIndividual ,
                                         :Security_Operations_Policies ;
                                :HasWeight 5 ;
                                rdfs:comment "Mechanisms exist to evaluate its analytical processes for potential bias." .


###  http://FYP-ASHS21/csonto/OPS-PRI-11-DataTagging
:OPS-PRI-11-DataTagging rdf:type owl:NamedIndividual ,
                                 :Security_Operations_Policies ;
                        :HasWeight 3 ;
                        rdfs:comment "Mechanisms exist to issue data modeling guidelines to support tagging of sensitive/regulated data." .


###  http://FYP-ASHS21/csonto/OPS-PRI-12-UpdatingPersonalData-PD-
:OPS-PRI-12-UpdatingPersonalData-PD- rdf:type owl:NamedIndividual ,
                                              :Security_Operations_Policies ;
                                     :HasWeight 9 ;
                                     rdfs:comment "Mechanisms exist to develop processes to identify and record the method under which Personal Data (PD) is updated and the frequency that such updates occur." .


###  http://FYP-ASHS21/csonto/OPS-PRI-13-DataManagementBoard
:OPS-PRI-13-DataManagementBoard rdf:type owl:NamedIndividual ,
                                         :Security_Operations_Policies ;
                                :HasWeight 3 ;
                                rdfs:comment "Mechanisms exist to establish a written charter for a Data Management Board (DMB) and assigned organization-defined roles to the DMB." .


###  http://FYP-ASHS21/csonto/OPS-PRI-14.1-AccountingofDisclosures
:OPS-PRI-14.1-AccountingofDisclosures rdf:type owl:NamedIndividual ,
                                               :Security_Operations_Policies ;
                                      :HasWeight 8 ;
                                      rdfs:comment "Mechanisms exist to develop and maintain an accounting of disclosures of Personal Data (PD) held by the organization and make the accounting of disclosures available to the person named in the record, upon request." .


###  http://FYP-ASHS21/csonto/OPS-PRI-14.2-NotificationofDisclosureRequestToDataSubject
:OPS-PRI-14.2-NotificationofDisclosureRequestToDataSubject rdf:type owl:NamedIndividual ,
                                                                    :Security_Operations_Policies ;
                                                           :HasWeight 5 ;
                                                           rdfs:comment "Mechanisms exist to notify data subjects of applicable legal requests to disclose Personal Data (PD)." .


###  http://FYP-ASHS21/csonto/OPS-PRI-15-RegisterAsADataControllerand-orDataProcessor
:OPS-PRI-15-RegisterAsADataControllerand-orDataProcessor rdf:type owl:NamedIndividual ,
                                                                  :Security_Operations_Policies ;
                                                         :HasWeight 3 ;
                                                         rdfs:comment "Mechanisms exist to register as a data controller and/or data processor, including registering databases containing Personal Data (PD) with the appropriate Data Authority, when necessary." .


###  http://FYP-ASHS21/csonto/OPS-PRI-16-PotentialHumanRightsAbuses
:OPS-PRI-16-PotentialHumanRightsAbuses rdf:type owl:NamedIndividual ,
                                                :Security_Operations_Policies ;
                                       :HasWeight 10 ;
                                       rdfs:comment "Mechanisms exist to constrain the supply of physical and/or digital activity logs to the host government that can directly lead to contravention of the Universal Declaration of Human Rights (UDHR), as well as other applicable statutory, regulatory and/or contractual obligations." .


###  http://FYP-ASHS21/csonto/OPS-PRI-17-DataSubjectCommunications
:OPS-PRI-17-DataSubjectCommunications rdf:type owl:NamedIndividual ,
                                               :Security_Operations_Policies ;
                                      :HasWeight 6 ;
                                      rdfs:comment "Mechanisms exist to craft disclosures and communications to data subjects such that the material is readily accessible and written in a manner that is concise, unambiguous and understandable by a reasonable person." .


###  http://FYP-ASHS21/csonto/OPS-PRI-17.1-ConspicuousLinkToDataPrivacyNotice
:OPS-PRI-17.1-ConspicuousLinkToDataPrivacyNotice rdf:type owl:NamedIndividual ,
                                                          :Security_Operations_Policies ;
                                                 :HasWeight 4 ;
                                                 rdfs:comment "Mechanisms exist to include a conspicuous link to the organization's data privacy notice on all consumer-facing websites and mobile applications." .


###  http://FYP-ASHS21/csonto/OPS-PRI-17.2-NoticeofFinancialIncentive
:OPS-PRI-17.2-NoticeofFinancialIncentive rdf:type owl:NamedIndividual ,
                                                  :Security_Operations_Policies ;
                                         :HasWeight 2 ;
                                         rdfs:comment "Mechanisms exist to provide data subjects with a Notice of Financial Incentive that explains the material terms of a financial incentive, price or service difference so the data subject can make an informed decision about whether to participate." .


###  http://FYP-ASHS21/csonto/OPS-THR-01-ThreatIntelligenceProgram
:OPS-THR-01-ThreatIntelligenceProgram rdf:type owl:NamedIndividual ,
                                               :Security_Operations_Policies ;
                                      :HasWeight 8 ;
                                      rdfs:comment "Mechanisms exist to implement a threat intelligence program that includes a cross-organization information-sharing capability that can influence the development of the system and security architectures, selection of security solutions, monitoring, threat hunting, response and recovery activities." .


###  http://FYP-ASHS21/csonto/OPS-THR-02-IndicatorsofExposure-IOE-
:OPS-THR-02-IndicatorsofExposure-IOE- rdf:type owl:NamedIndividual ,
                                               :Security_Operations_Policies ;
                                      :HasWeight 8 ;
                                      rdfs:comment "Mechanisms exist to develop Indicators of Exposure (IOE) to understand the potential attack vectors that attackers could use to attack the organization. " .


###  http://FYP-ASHS21/csonto/OPS-THR-03-ThreatIntelligenceFeeds
:OPS-THR-03-ThreatIntelligenceFeeds rdf:type owl:NamedIndividual ,
                                             :Security_Operations_Policies ;
                                    :HasWeight 8 ;
                                    rdfs:comment "Mechanisms exist to maintain situational awareness of evolving threats by leveraging the knowledge of attacker tactics, techniques and procedures to facilitate the implementation of preventative and compensating controls." .


###  http://FYP-ASHS21/csonto/OPS-THR-04-InsiderThreatProgram
:OPS-THR-04-InsiderThreatProgram rdf:type owl:NamedIndividual ,
                                          :Security_Operations_Policies ;
                                 :HasWeight 8 ;
                                 rdfs:comment "Mechanisms exist to implement an insider threat program that includes a cross-discipline insider threat incident handling team. " .


###  http://FYP-ASHS21/csonto/OPS-THR-05-InsiderThreatAwareness
:OPS-THR-05-InsiderThreatAwareness rdf:type owl:NamedIndividual ,
                                            :Security_Operations_Policies ;
                                   :HasWeight 8 ;
                                   rdfs:comment "Mechanisms exist to utilize security awareness training on recognizing and reporting potential indicators of insider threat." .


###  http://FYP-ASHS21/csonto/OPS-THR-06-VulnerabilityDisclosureProgram-VDP-
:OPS-THR-06-VulnerabilityDisclosureProgram-VDP- rdf:type owl:NamedIndividual ,
                                                         :Security_Operations_Policies ;
                                                :HasWeight 8 ;
                                                rdfs:comment "Mechanisms exist to establish a Vulnerability Disclosure Program (VDP) to assist with the secure development and maintenance of products and services that receives unsolicited input from the public about vulnerabilities in organizational systems, services and processes." .


###  http://FYP-ASHS21/csonto/OPS-THR-07-ThreatHunting
:OPS-THR-07-ThreatHunting rdf:type owl:NamedIndividual ,
                                   :Security_Operations_Policies ;
                          :HasWeight 4 ;
                          rdfs:comment "Mechanisms exist to perform cyber threat hunting that uses Indicators of Compromise (IoC) to detect, track and disrupt threats that evade existing security controls." .


###  http://FYP-ASHS21/csonto/OPS-THR-08-Tainting
:OPS-THR-08-Tainting rdf:type owl:NamedIndividual ,
                              :Security_Operations_Policies ;
                     :HasWeight 1 ;
                     rdfs:comment "Mechanisms exist to embed false data or steganographic data in files to enable the organization to determine if data has been exfiltrated and provide a means to identify the individual(s) involved." .


###  http://FYP-ASHS21/csonto/OPS-THR-09-ThreatCatalog
:OPS-THR-09-ThreatCatalog rdf:type owl:NamedIndividual ,
                                   :Security_Operations_Policies ;
                          :HasWeight 5 ;
                          rdfs:comment "Mechanisms exist to develop and keep current a catalog of applicable internal and external threats to the organization, both natural and manmade." .


###  http://FYP-ASHS21/csonto/OPS-THR-10-ThreatAnalysis
:OPS-THR-10-ThreatAnalysis rdf:type owl:NamedIndividual ,
                                    :Security_Operations_Policies ;
                           :HasWeight 7 ;
                           rdfs:comment "Mechanisms exist to identify, assess, prioritize and document the potential impact(s) and likelihood(s) of applicable internal and external threats." .


###  http://FYP-ASHS21/csonto/OPS-VPM-01.1-AttackSurfaceScope
:OPS-VPM-01.1-AttackSurfaceScope rdf:type owl:NamedIndividual ,
                                          :Security_Operations_Policies ;
                                 :HasWeight 5 ;
                                 rdfs:comment "Mechanisms exist to define and manage the scope for its attack surface management activities." .


###  http://FYP-ASHS21/csonto/OPS-VPM-02-VulnerabilityRemediationProcess
:OPS-VPM-02-VulnerabilityRemediationProcess rdf:type owl:NamedIndividual ,
                                                     :Security_Operations_Policies ;
                                            :HasWeight 10 ;
                                            rdfs:comment "Mechanisms exist to ensure that vulnerabilities are properly identified, tracked and remediated." .


###  http://FYP-ASHS21/csonto/OPS-VPM-03-VulnerabilityRanking
:OPS-VPM-03-VulnerabilityRanking rdf:type owl:NamedIndividual ,
                                          :Security_Operations_Policies ;
                                 :HasWeight 8 ;
                                 rdfs:comment "Mechanisms exist to identify and assign a risk ranking to newly discovered security vulnerabilities using reputable outside sources for security vulnerability information. " .


###  http://FYP-ASHS21/csonto/OPS-VPM-03.1-VulnerabilityExploitationAnalysis
:OPS-VPM-03.1-VulnerabilityExploitationAnalysis rdf:type owl:NamedIndividual ,
                                                         :Security_Operations_Policies ;
                                                :HasWeight 5 ;
                                                rdfs:comment "Mechanisms exist to identify, assess, prioritize and document the potential impact(s) and likelihood(s) of applicable internal and external threats exploiting known vulnerabilities." .


###  http://FYP-ASHS21/csonto/OPS-VPM-04-ContinuousVulnerabilityRemediationActivities
:OPS-VPM-04-ContinuousVulnerabilityRemediationActivities rdf:type owl:NamedIndividual ,
                                                                  :Security_Operations_Policies ;
                                                         :HasWeight 8 ;
                                                         rdfs:comment "Mechanisms exist to address new threats and vulnerabilities on an ongoing basis and ensure assets are protected against known attacks. " .


###  http://FYP-ASHS21/csonto/OPS-VPM-04.1-StableVersions
:OPS-VPM-04.1-StableVersions rdf:type owl:NamedIndividual ,
                                      :Security_Operations_Policies ;
                             :HasWeight 8 ;
                             rdfs:comment "Mechanisms exist to install the latest stable version of any software and/or security-related updates on all applicable systems." .


###  http://FYP-ASHS21/csonto/OPS-VPM-04.2-FlawRemediationwithPersonalData-PD-
:OPS-VPM-04.2-FlawRemediationwithPersonalData-PD- rdf:type owl:NamedIndividual ,
                                                           :Security_Operations_Policies ;
                                                  :HasWeight 8 ;
                                                  rdfs:comment "Mechanisms exist to identify and correct flaws related to the collection, usage, processing or dissemination of Personal Data (PD)." .


###  http://FYP-ASHS21/csonto/OPS-VPM-05.1-CentralizedManagementofFlawRemediationProcesses
:OPS-VPM-05.1-CentralizedManagementofFlawRemediationProcesses rdf:type owl:NamedIndividual ,
                                                                       :Security_Operations_Policies ;
                                                              :HasWeight 9 ;
                                                              rdfs:comment "Mechanisms exist to centrally-manage the flaw remediation process. " .


###  http://FYP-ASHS21/csonto/OPS-VPM-05.2-AutomatedRemediationStatus
:OPS-VPM-05.2-AutomatedRemediationStatus rdf:type owl:NamedIndividual ,
                                                  :Security_Operations_Policies ;
                                         :HasWeight 9 ;
                                         rdfs:comment "Automated mechanisms exist to determine the state of system components with regard to flaw remediation. " .


###  http://FYP-ASHS21/csonto/OPS-VPM-05.3-TimeToRemediate-BenchmarksForCorrectiveAction
:OPS-VPM-05.3-TimeToRemediate-BenchmarksForCorrectiveAction rdf:type owl:NamedIndividual ,
                                                                     :Security_Operations_Policies ;
                                                            :HasWeight 6 ;
                                                            rdfs:comment "Mechanisms exist to track the effectiveness of remediation operations through metrics reporting." .


###  http://FYP-ASHS21/csonto/OPS-VPM-05.5-RemovalofPreviousVersions
:OPS-VPM-05.5-RemovalofPreviousVersions rdf:type owl:NamedIndividual ,
                                                 :Security_Operations_Policies ;
                                        :HasWeight 5 ;
                                        rdfs:comment "Mechanisms exist to remove old versions of software and firmware components after updated versions have been installed. " .


###  http://FYP-ASHS21/csonto/OPS-VPM-06-VulnerabilityScanning
:OPS-VPM-06-VulnerabilityScanning rdf:type owl:NamedIndividual ,
                                           :Security_Operations_Policies ;
                                  :HasWeight 9 ;
                                  rdfs:comment "Mechanisms exist to detect vulnerabilities and configuration errors by recurring vulnerability scanning of systems and web applications." .


###  http://FYP-ASHS21/csonto/OPS-VPM-06.1-UpdateToolCapability
:OPS-VPM-06.1-UpdateToolCapability rdf:type owl:NamedIndividual ,
                                            :Security_Operations_Policies ;
                                   :HasWeight 8 ;
                                   rdfs:comment "Mechanisms exist to update vulnerability scanning tools." .


###  http://FYP-ASHS21/csonto/OPS-VPM-06.2-Breadth-DepthofCoverage
:OPS-VPM-06.2-Breadth-DepthofCoverage rdf:type owl:NamedIndividual ,
                                               :Security_Operations_Policies ;
                                      :HasWeight 8 ;
                                      rdfs:comment "Mechanisms exist to identify the breadth and depth of coverage for vulnerability scanning that define the system components scanned and types of vulnerabilities that are checked for. " .


###  http://FYP-ASHS21/csonto/OPS-VPM-06.3-PrivilegedAccess
:OPS-VPM-06.3-PrivilegedAccess rdf:type owl:NamedIndividual ,
                                        :Security_Operations_Policies ;
                               :HasWeight 9 ;
                               rdfs:comment "Mechanisms exist to implement privileged access authorization for selected vulnerability scanning activities. " .


###  http://FYP-ASHS21/csonto/OPS-VPM-06.4-TrendAnalysis
:OPS-VPM-06.4-TrendAnalysis rdf:type owl:NamedIndividual ,
                                     :Security_Operations_Policies ;
                            :HasWeight 9 ;
                            rdfs:comment "Automated mechanisms exist to compare the results of vulnerability scans over time to determine trends in system vulnerabilities. " .


###  http://FYP-ASHS21/csonto/OPS-VPM-06.5-ReviewHistoricalAuditLogs
:OPS-VPM-06.5-ReviewHistoricalAuditLogs rdf:type owl:NamedIndividual ,
                                                 :Security_Operations_Policies ;
                                        :HasWeight 9 ;
                                        rdfs:comment "Mechanisms exist to review historical audit logs to determine if identified vulnerabilities have been previously exploited. " .


###  http://FYP-ASHS21/csonto/OPS-VPM-06.6-ExternalVulnerabilityAssessmentScans
:OPS-VPM-06.6-ExternalVulnerabilityAssessmentScans rdf:type owl:NamedIndividual ,
                                                            :Security_Operations_Policies ;
                                                   :HasWeight 9 ;
                                                   rdfs:comment "Mechanisms exist to perform quarterly external vulnerability scans (outside the organization's network looking inward) via a reputable vulnerability service provider, which include rescans until passing results are obtained or all high vulnerabilities are resolved, as defined by the Common Vulnerability Scoring System (CVSS)." .


###  http://FYP-ASHS21/csonto/OPS-VPM-06.7-InternalVulnerabilityAssessmentScans
:OPS-VPM-06.7-InternalVulnerabilityAssessmentScans rdf:type owl:NamedIndividual ,
                                                            :Security_Operations_Policies ;
                                                   :HasWeight 9 ;
                                                   rdfs:comment "Mechanisms exist to perform quarterly internal vulnerability scans, which includes all segments of the organization's internal network, as well as rescans until passing results are obtained or all high vulnerabilities are resolved, as defined by the Common Vulnerability Scoring System (CVSS)." .


###  http://FYP-ASHS21/csonto/OPS-VPM-06.8-AcceptableDiscoverableInformation
:OPS-VPM-06.8-AcceptableDiscoverableInformation rdf:type owl:NamedIndividual ,
                                                         :Security_Operations_Policies ;
                                                :HasWeight 5 ;
                                                rdfs:comment "Mechanisms exist to define what information is allowed to be discoverable by adversaries and take corrective actions to remediated non-compliant systems." .


###  http://FYP-ASHS21/csonto/OPS-VPM-06.9-CorrelateScanningInformation
:OPS-VPM-06.9-CorrelateScanningInformation rdf:type owl:NamedIndividual ,
                                                    :Security_Operations_Policies ;
                                           :HasWeight 5 ;
                                           rdfs:comment "Automated mechanisms exist to correlate the output from vulnerability scanning tools to determine the presence of multi-vulnerability/multi-hop attack vectors." .


###  http://FYP-ASHS21/csonto/OPS-VPM-07-PenetrationTesting
:OPS-VPM-07-PenetrationTesting rdf:type owl:NamedIndividual ,
                                        :Security_Operations_Policies ;
                               :HasWeight 9 ;
                               rdfs:comment "Mechanisms exist to conduct penetration testing on systems and web applications." .


###  http://FYP-ASHS21/csonto/OPS-VPM-07.1-IndependentPenetrationAgentorTeam
:OPS-VPM-07.1-IndependentPenetrationAgentorTeam rdf:type owl:NamedIndividual ,
                                                         :Security_Operations_Policies ;
                                                :HasWeight 6 ;
                                                rdfs:comment "Mechanisms exist to utilize an independent assessor or penetration team to perform penetration testing." .


###  http://FYP-ASHS21/csonto/OPS-VPM-08-TechnicalSurveillanceCountermeasuresSecurity
:OPS-VPM-08-TechnicalSurveillanceCountermeasuresSecurity rdf:type owl:NamedIndividual ,
                                                                  :Security_Operations_Policies ;
                                                         :HasWeight 1 ;
                                                         rdfs:comment "Mechanisms exist to utilize a technical surveillance countermeasures survey." .


###  http://FYP-ASHS21/csonto/OPS-VPM-09-ReviewingVulnerabilityScannerUsage
:OPS-VPM-09-ReviewingVulnerabilityScannerUsage rdf:type owl:NamedIndividual ,
                                                        :Security_Operations_Policies ;
                                               :HasWeight 3 ;
                                               rdfs:comment "Mechanisms exist to monitor logs associated with scanning activities and associated administrator accounts to ensure that those activities are limited to the timeframes of legitimate scans. " .


###  http://FYP-ASHS21/csonto/OPS-VPM-10-RedTeamExercises
:OPS-VPM-10-RedTeamExercises rdf:type owl:NamedIndividual ,
                                      :Security_Operations_Policies ;
                             :HasWeight 3 ;
                             rdfs:comment "Mechanisms exist to utilize \"red team\" exercises to simulate attempts by adversaries to compromise systems and applications in accordance with organization-defined rules of engagement. " .


###  http://FYP-ASHS21/csonto/OPS-WEB-01-WebSecurity
:OPS-WEB-01-WebSecurity rdf:type owl:NamedIndividual ,
                                 :Security_Operations_Policies ;
                        :HasWeight 8 ;
                        rdfs:comment "Mechanisms exist to facilitate the implementation of an enterprise-wide web management policy, as well as associated standards, controls and procedures." .


###  http://FYP-ASHS21/csonto/OPS-WEB-01.1-UnauthorizedCode
:OPS-WEB-01.1-UnauthorizedCode rdf:type owl:NamedIndividual ,
                                        :Security_Operations_Policies ;
                               :HasWeight 9 ;
                               rdfs:comment "Mechanisms exist to prevent unauthorized code from being present in a secure page as it is rendered in a clients browser." .


###  http://FYP-ASHS21/csonto/OPS-WEB-02-UseofDemilitarizedZones-DMZ-
:OPS-WEB-02-UseofDemilitarizedZones-DMZ- rdf:type owl:NamedIndividual ,
                                                  :Security_Operations_Policies ;
                                         :HasWeight 9 ;
                                         rdfs:comment "Mechanisms exist to utilize a Demilitarized Zone (DMZ) to restrict inbound traffic to authorized devices on certain services, protocols and ports." .


###  http://FYP-ASHS21/csonto/OPS-WEB-03-WebApplicationFirewall-WAF-
:OPS-WEB-03-WebApplicationFirewall-WAF- rdf:type owl:NamedIndividual ,
                                                 :Security_Operations_Policies ;
                                        :HasWeight 8 ;
                                        rdfs:comment "Mechanisms exist to deploy Web Application Firewalls (WAFs) to provide defense-in-depth protection for application-specific threats. " .


###  http://FYP-ASHS21/csonto/OPS-WEB-04-Client-FacingWebServices
:OPS-WEB-04-Client-FacingWebServices rdf:type owl:NamedIndividual ,
                                              :Security_Operations_Policies ;
                                     :HasWeight 10 ;
                                     rdfs:comment "Mechanisms exist to deploy reasonably-expected security controls to protect the confidentiality and availability of client data that is stored, transmitted or processed by the Internet-based service." .


###  http://FYP-ASHS21/csonto/OPS-WEB-05-CookieManagement
:OPS-WEB-05-CookieManagement rdf:type owl:NamedIndividual ,
                                      :Security_Operations_Policies ;
                             :HasWeight 5 ;
                             rdfs:comment "Mechanisms exist to provide individuals with clear and precise information about cookies, in accordance with applicable legal requirements for cookie management." .


###  http://FYP-ASHS21/csonto/OPS-WEB-06-StrongCustomerAuthentication-SCA-
:OPS-WEB-06-StrongCustomerAuthentication-SCA- rdf:type owl:NamedIndividual ,
                                                       :Security_Operations_Policies ;
                                              :HasWeight 8 ;
                                              rdfs:comment "Mechanisms exist to implement Strong Customer Authentication (SCA) for consumers to reasonably prove their identity." .


###  http://FYP-ASHS21/csonto/OPS-WEB-07-WebSecurityStandard
:OPS-WEB-07-WebSecurityStandard rdf:type owl:NamedIndividual ,
                                         :Security_Operations_Policies ;
                                :HasWeight 9 ;
                                rdfs:comment "Mechanisms exist to ensure the Open Web Application Security Project (OWASP) Application Security Verification Standard is incorporated into the organization's Secure Systems Development Lifecycle (SSDLC) process." .


###  http://FYP-ASHS21/csonto/OPS-WEB-08-WebApplicationFramework
:OPS-WEB-08-WebApplicationFramework rdf:type owl:NamedIndividual ,
                                             :Security_Operations_Policies ;
                                    :HasWeight 9 ;
                                    rdfs:comment "Mechanisms exist to ensure a robust Web Application Framework is used to aid in the development of secure web applications, including web services, web resources and web APIs." .


###  http://FYP-ASHS21/csonto/OPS-WEB-10-SecureWebTraffic
:OPS-WEB-10-SecureWebTraffic rdf:type owl:NamedIndividual ,
                                      :Security_Operations_Policies ;
                             :HasWeight 9 ;
                             rdfs:comment "Mechanisms exist to ensure all web application content is delivered using cryptographic mechanisms (e.g., TLS)." .


###  http://FYP-ASHS21/csonto/OPS-WEB-11-OutputEncoding
:OPS-WEB-11-OutputEncoding rdf:type owl:NamedIndividual ,
                                    :Security_Operations_Policies ;
                           :HasWeight 9 ;
                           rdfs:comment "Mechanisms exist to ensure output encoding is performed on all content produced by a web application to reduce the likelihood of cross-site scripting and other injection attacks." .


###  http://FYP-ASHS21/csonto/OPS-WEB-12-WebBrowserSecurity
:OPS-WEB-12-WebBrowserSecurity rdf:type owl:NamedIndividual ,
                                        :Security_Operations_Policies ;
                               :HasWeight 9 ;
                               rdfs:comment "Mechanisms exist to ensure web applications implement Content-Security-Policy, HSTS and X-Frame-Options response headers to protect both the web application and its users." .


###  http://FYP-ASHS21/csonto/OPS-WEB-13-WebsiteChangeDetection
:OPS-WEB-13-WebsiteChangeDetection rdf:type owl:NamedIndividual ,
                                            :Security_Operations_Policies ;
                                   :HasWeight 8 ;
                                   rdfs:comment "Mechanisms exist to detect and respond to Indicators of Compromise (IoC) for unauthorized alterations, additions, deletions or changes on websites that store, process and/or transmit sensitive / regulated data. " .


###  http://FYP-ASHS21/csonto/AAT-01-ArtificialIntelligence-AI-&AutonomousTechnologiesGovernance
<http://FYP-ASHS21/csonto/AAT-01-ArtificialIntelligence-AI-&AutonomousTechnologiesGovernance> rdf:type owl:NamedIndividual ,
                                                                                                       :Emerging_Technologies_Policies ;
                                                                                              :HasWeight 10 ;
                                                                                              rdfs:comment "Mechanisms exist to ensure policies, processes, procedures and practices related to the mapping, measuring and managing of Artificial Intelligence (AI) and Autonomous Technologies (AAT)-related risks are in place, transparent and implemented effectively." .


###  http://FYP-ASHS21/csonto/AAT-01.1-AI&AutonomousTechnologies-RelatedLegalRequirementsDefinition
<http://FYP-ASHS21/csonto/AAT-01.1-AI&AutonomousTechnologies-RelatedLegalRequirementsDefinition> rdf:type owl:NamedIndividual ,
                                                                                                          :Emerging_Technologies_Policies ;
                                                                                                 :HasWeight 8 ;
                                                                                                 rdfs:comment "Mechanisms exist to identify, understand, document and manage applicable statutory and regulatory requirements for Artificial Intelligence (AI) and Autonomous Technologies (AAT)." .


###  http://FYP-ASHS21/csonto/AAT-01.2-TrustworthyAI&AutonomousTechnologies
<http://FYP-ASHS21/csonto/AAT-01.2-TrustworthyAI&AutonomousTechnologies> rdf:type owl:NamedIndividual ,
                                                                                  :Emerging_Technologies_Policies ;
                                                                         :HasWeight 10 ;
                                                                         rdfs:comment "Mechanisms exist to ensure Artificial Intelligence (AI) and Autonomous Technologies (AAT) are designed to be reliable, safe, fair, secure, resilient, transparent, explainable and data privacy-enhanced to minimize emergent properties or unintended consequences." .


###  http://FYP-ASHS21/csonto/AAT-01.3-AI&AutonomousTechnologiesValueSustainment
<http://FYP-ASHS21/csonto/AAT-01.3-AI&AutonomousTechnologiesValueSustainment> rdf:type owl:NamedIndividual ,
                                                                                       :Emerging_Technologies_Policies ;
                                                                              :HasWeight 1 ;
                                                                              rdfs:comment "Mechanisms exist to sustain the value of deployed Artificial Intelligence (AI) and Autonomous Technologies (AAT)." .


###  http://FYP-ASHS21/csonto/AAT-02-SituationalAwarenessofAI&AutonomousTechnologies
<http://FYP-ASHS21/csonto/AAT-02-SituationalAwarenessofAI&AutonomousTechnologies> rdf:type owl:NamedIndividual ,
                                                                                           :Emerging_Technologies_Policies ;
                                                                                  :HasWeight 9 ;
                                                                                  rdfs:comment "Mechanisms exist to develop and maintain an inventory of Artificial Intelligence (AI) and Autonomous Technologies (AAT) (internal and third-party)." .


###  http://FYP-ASHS21/csonto/AAT-02.1-AI&AutonomousTechnologiesRiskMapping
<http://FYP-ASHS21/csonto/AAT-02.1-AI&AutonomousTechnologiesRiskMapping> rdf:type owl:NamedIndividual ,
                                                                                  :Emerging_Technologies_Policies ;
                                                                         :HasWeight 9 ;
                                                                         rdfs:comment "Mechanisms exist to identify Artificial Intelligence (AI) and Autonomous Technologies (AAT) in use and map those components to potential legal risks, including statutory and regulatory compliance requirements." .


###  http://FYP-ASHS21/csonto/AAT-02.2-AI&AutonomousTechnologiesInternalControls
<http://FYP-ASHS21/csonto/AAT-02.2-AI&AutonomousTechnologiesInternalControls> rdf:type owl:NamedIndividual ,
                                                                                       :Emerging_Technologies_Policies ;
                                                                              :HasWeight 9 ;
                                                                              rdfs:comment "Mechanisms exist to identify and document internal cybersecurity & data privacy controls for Artificial Intelligence (AI) and Autonomous Technologies (AAT)." .


###  http://FYP-ASHS21/csonto/AAT-03-AI&AutonomousTechnologiesContextDefinition
<http://FYP-ASHS21/csonto/AAT-03-AI&AutonomousTechnologiesContextDefinition> rdf:type owl:NamedIndividual ,
                                                                                      :Emerging_Technologies_Policies ;
                                                                             :HasWeight 8 ;
                                                                             rdfs:comment """Mechanisms exist to establish and document the context surrounding Artificial Intelligence (AI) and Autonomous Technologies (AAT), including:
  Intended purposes;
  Potentially beneficial uses;
  Context-specific laws and regulations;
  Norms and expectations; and
  Prospective settings in which the system(s) will be deployed.""" .


###  http://FYP-ASHS21/csonto/AAT-03.1-AI&AutonomousTechnologiesMissionandGoalsDefinition
<http://FYP-ASHS21/csonto/AAT-03.1-AI&AutonomousTechnologiesMissionandGoalsDefinition> rdf:type owl:NamedIndividual ,
                                                                                                :Emerging_Technologies_Policies ;
                                                                                       :HasWeight 8 ;
                                                                                       rdfs:comment "Mechanisms exist to define and document the organizations mission and defined goals for Artificial Intelligence (AI) and Autonomous Technologies (AAT)." .


###  http://FYP-ASHS21/csonto/AAT-04-AI&AutonomousTechnologiesBusinessCase
<http://FYP-ASHS21/csonto/AAT-04-AI&AutonomousTechnologiesBusinessCase> rdf:type owl:NamedIndividual ,
                                                                                 :Emerging_Technologies_Policies ;
                                                                        :HasWeight 8 ;
                                                                        rdfs:comment "Mechanisms exist to benchmark capabilities, targeted usage, goals and expected benefits and costs of Artificial Intelligence (AI) and Autonomous Technologies (AAT)." .


###  http://FYP-ASHS21/csonto/AAT-04.1-AI&AutonomousTechnologiesPotentialBenefitsAnalysis
<http://FYP-ASHS21/csonto/AAT-04.1-AI&AutonomousTechnologiesPotentialBenefitsAnalysis> rdf:type owl:NamedIndividual ,
                                                                                                :Emerging_Technologies_Policies ;
                                                                                       :HasWeight 2 ;
                                                                                       rdfs:comment "Mechanisms exist to assess the potential benefits of proposed Artificial Intelligence (AI) and Autonomous Technologies (AAT)." .


###  http://FYP-ASHS21/csonto/AAT-04.2-AI&AutonomousTechnologiesPotentialCostsAnalysis
<http://FYP-ASHS21/csonto/AAT-04.2-AI&AutonomousTechnologiesPotentialCostsAnalysis> rdf:type owl:NamedIndividual ,
                                                                                             :Emerging_Technologies_Policies ;
                                                                                    :HasWeight 2 ;
                                                                                    rdfs:comment "Mechanisms exist to assess potential costs, including non-monetary costs, resulting from expected or realized Artificial Intelligence (AI) and Autonomous Technologies (AAT)-related errors or system functionality and trustworthiness." .


###  http://FYP-ASHS21/csonto/AAT-04.3-AI&AutonomousTechnologiesTargetedApplicationScope
<http://FYP-ASHS21/csonto/AAT-04.3-AI&AutonomousTechnologiesTargetedApplicationScope> rdf:type owl:NamedIndividual ,
                                                                                               :Emerging_Technologies_Policies ;
                                                                                      :HasWeight 8 ;
                                                                                      rdfs:comment "Mechanisms exist to specify and document the targeted application scope of the proposed use and operation of Artificial Intelligence (AI) and Autonomous Technologies (AAT)." .


###  http://FYP-ASHS21/csonto/AAT-04.4-AI&AutonomousTechnologiesCost-BenefitMapping
<http://FYP-ASHS21/csonto/AAT-04.4-AI&AutonomousTechnologiesCost-BenefitMapping> rdf:type owl:NamedIndividual ,
                                                                                          :Emerging_Technologies_Policies ;
                                                                                 :HasWeight 2 ;
                                                                                 rdfs:comment "Mechanisms exist to map risks and benefits for all components of Artificial Intelligence (AI) and Autonomous Technologies (AAT), including third-party software and data." .


###  http://FYP-ASHS21/csonto/AAT-05-AI&AutonomousTechnologiesTraining
<http://FYP-ASHS21/csonto/AAT-05-AI&AutonomousTechnologiesTraining> rdf:type owl:NamedIndividual ,
                                                                             :Emerging_Technologies_Policies ;
                                                                    :HasWeight 5 ;
                                                                    rdfs:comment "Mechanisms exist to ensure personnel and external stakeholders are provided with position-specific risk management training for Artificial Intelligence (AI) and Autonomous Technologies (AAT)." .


###  http://FYP-ASHS21/csonto/AAT-06-AI&AutonomousTechnologiesFairness&Bias
<http://FYP-ASHS21/csonto/AAT-06-AI&AutonomousTechnologiesFairness&Bias> rdf:type owl:NamedIndividual ,
                                                                                  :Emerging_Technologies_Policies ;
                                                                         :HasWeight 9 ;
                                                                         rdfs:comment "Mechanisms exist to prevent Artificial Intelligence (AI) and Autonomous Technologies (AAT) from unfairly identifying, profiling and/or statistically singling out a segmented population defined by race, religion, gender identity, national origin, religion, disability or any other politically-charged identifier." .


###  http://FYP-ASHS21/csonto/AAT-07-AI&AutonomousTechnologiesRiskManagementDecisions
<http://FYP-ASHS21/csonto/AAT-07-AI&AutonomousTechnologiesRiskManagementDecisions> rdf:type owl:NamedIndividual ,
                                                                                            :Emerging_Technologies_Policies ;
                                                                                   :HasWeight 10 ;
                                                                                   rdfs:comment "Mechanisms exist to leverage decision makers from a diversity of demographics, disciplines, experience, expertise and backgrounds for mapping, measuring and managing Artificial Intelligence (AI) and Autonomous Technologies (AAT)-related risks." .


###  http://FYP-ASHS21/csonto/AAT-07.1-AI&AutonomousTechnologiesImpactCharacterization
<http://FYP-ASHS21/csonto/AAT-07.1-AI&AutonomousTechnologiesImpactCharacterization> rdf:type owl:NamedIndividual ,
                                                                                             :Emerging_Technologies_Policies ;
                                                                                    :HasWeight 8 ;
                                                                                    rdfs:comment "Mechanisms exist to characterize the impacts of proposed Artificial Intelligence (AI) and Autonomous Technologies (AAT) on individuals, groups, communities, organizations and society." .


###  http://FYP-ASHS21/csonto/AAT-07.2-AI&AutonomousTechnologiesLikelihood&ImpactRiskAnalysis
<http://FYP-ASHS21/csonto/AAT-07.2-AI&AutonomousTechnologiesLikelihood&ImpactRiskAnalysis> rdf:type owl:NamedIndividual ,
                                                                                                    :Emerging_Technologies_Policies ;
                                                                                           :HasWeight 10 ;
                                                                                           rdfs:comment "Mechanisms exist to define the potential likelihood and impact of each identified risk based on expected use and past uses of Artificial Intelligence (AI) and Autonomous Technologies (AAT) in similar contexts." .


###  http://FYP-ASHS21/csonto/AAT-07.3-AI&AutonomousTechnologiesContinuousImprovements
<http://FYP-ASHS21/csonto/AAT-07.3-AI&AutonomousTechnologiesContinuousImprovements> rdf:type owl:NamedIndividual ,
                                                                                             :Emerging_Technologies_Policies ;
                                                                                    :HasWeight 8 ;
                                                                                    rdfs:comment "Mechanisms exist to continuously improve Artificial Intelligence (AI) and Autonomous Technologies (AAT) capabilities to maximize benefits and minimize negative impacts associated with AAT." .


###  http://FYP-ASHS21/csonto/AAT-08-AssignedResponsibilitiesforAI&AutonomousTechnologies
<http://FYP-ASHS21/csonto/AAT-08-AssignedResponsibilitiesforAI&AutonomousTechnologies> rdf:type owl:NamedIndividual ,
                                                                                                :Emerging_Technologies_Policies ;
                                                                                       :HasWeight 9 ;
                                                                                       rdfs:comment "Mechanisms exist to define and differentiate roles and responsibilities for human-AI configurations and oversight of AI systems." .


###  http://FYP-ASHS21/csonto/AAT-09-AI&AutonomousTechnologiesRiskProfiling
<http://FYP-ASHS21/csonto/AAT-09-AI&AutonomousTechnologiesRiskProfiling> rdf:type owl:NamedIndividual ,
                                                                                  :Emerging_Technologies_Policies ;
                                                                         :HasWeight 9 ;
                                                                         rdfs:comment "Mechanisms exist to document the risks and potential impacts of Artificial Intelligence (AI) and Autonomous Technologies (AAT) designed, developed, deployed, evaluated and used." .


###  http://FYP-ASHS21/csonto/AAT-10-ArtificialIntelligenceTest-Evaluation-Validation&Verification-AITEVV-
<http://FYP-ASHS21/csonto/AAT-10-ArtificialIntelligenceTest-Evaluation-Validation&Verification-AITEVV-> rdf:type owl:NamedIndividual ,
                                                                                                                 :Emerging_Technologies_Policies ;
                                                                                                        :HasWeight 10 ;
                                                                                                        rdfs:comment "Mechanisms exist to implement Artificial Intelligence Test, Evaluation, Validation & Verification (AI TEVV) practices to enable Artificial Intelligence (AI) and Autonomous Technologies (AAT)-related testing, identification of incidents and information sharing." .


###  http://FYP-ASHS21/csonto/AAT-10.14-UpdatingAI&AutonomousTechnologies
<http://FYP-ASHS21/csonto/AAT-10.14-UpdatingAI&AutonomousTechnologies> rdf:type owl:NamedIndividual ,
                                                                                :Emerging_Technologies_Policies ;
                                                                       :HasWeight 9 ;
                                                                       rdfs:comment "Mechanisms exist to integrate continual improvements for deployed Artificial Intelligence (AI) and Autonomous Technologies (AAT)." .


###  http://FYP-ASHS21/csonto/AAT-10.6-AITEVVTransparency&AccountabilityAssessment
<http://FYP-ASHS21/csonto/AAT-10.6-AITEVVTransparency&AccountabilityAssessment> rdf:type owl:NamedIndividual ,
                                                                                         :Emerging_Technologies_Policies ;
                                                                                :HasWeight 7 ;
                                                                                rdfs:comment "Mechanisms exist to examine risks associated with transparency and accountability of Artificial Intelligence (AI) and Autonomous Technologies (AAT) to be deployed." .


###  http://FYP-ASHS21/csonto/AAT-10.8-AITEVVFairness&BiasAssessment
<http://FYP-ASHS21/csonto/AAT-10.8-AITEVVFairness&BiasAssessment> rdf:type owl:NamedIndividual ,
                                                                           :Emerging_Technologies_Policies ;
                                                                  :HasWeight 9 ;
                                                                  rdfs:comment "Mechanisms exist to examine fairness and bias of Artificial Intelligence (AI) and Autonomous Technologies (AAT) to be deployed." .


###  http://FYP-ASHS21/csonto/AAT-10.9-AI&AutonomousTechnologiesModelValidation
<http://FYP-ASHS21/csonto/AAT-10.9-AI&AutonomousTechnologiesModelValidation> rdf:type owl:NamedIndividual ,
                                                                                      :Emerging_Technologies_Policies ;
                                                                             :HasWeight 5 ;
                                                                             rdfs:comment "Mechanisms exist to validate the Artificial Intelligence (AI) and Autonomous Technologies (AAT) model." .


###  http://FYP-ASHS21/csonto/AAT-11-RobustStakeholderEngagementforAI&AutonomousTechnologies
<http://FYP-ASHS21/csonto/AAT-11-RobustStakeholderEngagementforAI&AutonomousTechnologies> rdf:type owl:NamedIndividual ,
                                                                                                   :Emerging_Technologies_Policies ;
                                                                                          :HasWeight 9 ;
                                                                                          rdfs:comment "Mechanisms exist to compel ongoing engagement with relevant Artificial Intelligence (AI) and Autonomous Technologies (AAT) stakeholders to encourage feedback about positive, negative and unanticipated impacts." .


###  http://FYP-ASHS21/csonto/AAT-11.1-AI&AutonomousTechnologiesStakeholderFeedbackIntegration
<http://FYP-ASHS21/csonto/AAT-11.1-AI&AutonomousTechnologiesStakeholderFeedbackIntegration> rdf:type owl:NamedIndividual ,
                                                                                                     :Emerging_Technologies_Policies ;
                                                                                            :HasWeight 9 ;
                                                                                            rdfs:comment "Mechanisms exist to regularly collect, consider, prioritize and integrate risk-related feedback from those external to the team that developed or deployed Artificial Intelligence (AI) and Autonomous Technologies (AAT)." .


###  http://FYP-ASHS21/csonto/AAT-11.2-AI&AutonomousTechnologiesOngoingAssessments
<http://FYP-ASHS21/csonto/AAT-11.2-AI&AutonomousTechnologiesOngoingAssessments> rdf:type owl:NamedIndividual ,
                                                                                         :Emerging_Technologies_Policies ;
                                                                                :HasWeight 9 ;
                                                                                rdfs:comment "Mechanisms exist to conduct regular assessments of Artificial Intelligence (AI) and Autonomous Technologies (AAT) with independent assessors and stakeholders not involved in the development of the AAT." .


###  http://FYP-ASHS21/csonto/AAT-11.3-AI&AutonomousTechnologiesEndUserFeedback
<http://FYP-ASHS21/csonto/AAT-11.3-AI&AutonomousTechnologiesEndUserFeedback> rdf:type owl:NamedIndividual ,
                                                                                      :Emerging_Technologies_Policies ;
                                                                             :HasWeight 7 ;
                                                                             rdfs:comment "Mechanisms exist to collect and integrate feedback from end users and impacted communities into Artificial Intelligence (AI) and Autonomous Technologies (AAT)-related system evaluation metrics." .


###  http://FYP-ASHS21/csonto/AAT-11.4-AI&AutonomousTechnologiesIncident&ErrorReporting
<http://FYP-ASHS21/csonto/AAT-11.4-AI&AutonomousTechnologiesIncident&ErrorReporting> rdf:type owl:NamedIndividual ,
                                                                                              :Emerging_Technologies_Policies ;
                                                                                     :HasWeight 9 ;
                                                                                     rdfs:comment "Mechanisms exist to communicate Artificial Intelligence (AI) and Autonomous Technologies (AAT)-related incidents and/or errors to relevant stakeholders, including affected communities. " .


###  http://FYP-ASHS21/csonto/AAT-12-AI&AutonomousTechnologiesIntellectualPropertyInfringementProtections
<http://FYP-ASHS21/csonto/AAT-12-AI&AutonomousTechnologiesIntellectualPropertyInfringementProtections> rdf:type owl:NamedIndividual ,
                                                                                                                :Emerging_Technologies_Policies ;
                                                                                                       :HasWeight 10 ;
                                                                                                       rdfs:comment "Mechanisms exist to identify data sources for Artificial Intelligence (AI) and Autonomous Technologies (AAT) to prevent third-party Intellectual Property (IP) rights infringement." .


###  http://FYP-ASHS21/csonto/AAT-13-AI&AutonomousTechnologiesStakeholderDiversity
<http://FYP-ASHS21/csonto/AAT-13-AI&AutonomousTechnologiesStakeholderDiversity> rdf:type owl:NamedIndividual ,
                                                                                         :Emerging_Technologies_Policies ;
                                                                                :HasWeight 8 ;
                                                                                rdfs:comment "Mechanisms exist to ensure Artificial Intelligence (AI) and Autonomous Technologies (AAT) stakeholder competencies, skills and capacities incorporate demographic diversity, broad domain and user experience expertise." .


###  http://FYP-ASHS21/csonto/AAT-13.1-AI&AutonomousTechnologiesStakeholderCompetencies
<http://FYP-ASHS21/csonto/AAT-13.1-AI&AutonomousTechnologiesStakeholderCompetencies> rdf:type owl:NamedIndividual ,
                                                                                              :Emerging_Technologies_Policies ;
                                                                                     :HasWeight 9 ;
                                                                                     rdfs:comment "Mechanisms exist to ensure Artificial Intelligence (AI) and Autonomous Technologies (AAT)-related operator and practitioner proficiency requirements for Artificial Intelligence (AI) and Autonomous Technologies (AAT) are defined, assessed and documented." .


###  http://FYP-ASHS21/csonto/AAT-14-AI&AutonomousTechnologiesRequirementsDefinitions
<http://FYP-ASHS21/csonto/AAT-14-AI&AutonomousTechnologiesRequirementsDefinitions> rdf:type owl:NamedIndividual ,
                                                                                            :Emerging_Technologies_Policies ;
                                                                                   :HasWeight 8 ;
                                                                                   rdfs:comment "Mechanisms exist to take socio-technical implications into account to address risks associated with Artificial Intelligence (AI) and Autonomous Technologies (AAT)." .


###  http://FYP-ASHS21/csonto/AAT-14.1-AI&AutonomousTechnologiesImplementationTasksDefinition
<http://FYP-ASHS21/csonto/AAT-14.1-AI&AutonomousTechnologiesImplementationTasksDefinition> rdf:type owl:NamedIndividual ,
                                                                                                    :Emerging_Technologies_Policies ;
                                                                                           :HasWeight 8 ;
                                                                                           rdfs:comment "Mechanisms exist to define the tasks that Artificial Intelligence (AI) and Autonomous Technologies (AAT) will support (e.g., classifiers, generative models, recommenders)." .


###  http://FYP-ASHS21/csonto/AAT-14.2-AI&AutonomousTechnologiesKnowledgeLimits
<http://FYP-ASHS21/csonto/AAT-14.2-AI&AutonomousTechnologiesKnowledgeLimits> rdf:type owl:NamedIndividual ,
                                                                                      :Emerging_Technologies_Policies ;
                                                                             :HasWeight 10 ;
                                                                             rdfs:comment "Mechanisms exist to identify and document knowledge limits of Artificial Intelligence (AI) and Autonomous Technologies (AAT) to provide sufficient information to assist relevant stakeholder decision making." .


###  http://FYP-ASHS21/csonto/AAT-15-AI&AutonomousTechnologiesViabilityDecisions
<http://FYP-ASHS21/csonto/AAT-15-AI&AutonomousTechnologiesViabilityDecisions> rdf:type owl:NamedIndividual ,
                                                                                       :Emerging_Technologies_Policies ;
                                                                              :HasWeight 10 ;
                                                                              rdfs:comment "Mechanisms exist to define the criteria as to whether Artificial Intelligence (AI) and Autonomous Technologies (AAT) achieved intended purposes and stated objectives to determine whether its development or deployment should proceed." .


###  http://FYP-ASHS21/csonto/AAT-15.1-AI&AutonomousTechnologiesNegativeResidualRisks
<http://FYP-ASHS21/csonto/AAT-15.1-AI&AutonomousTechnologiesNegativeResidualRisks> rdf:type owl:NamedIndividual ,
                                                                                            :Emerging_Technologies_Policies ;
                                                                                   :HasWeight 9 ;
                                                                                   rdfs:comment "Mechanisms exist to identify and document negative, residual risks (defined as the sum of all unmitigated risks) to both downstream acquirers and end users of Artificial Intelligence (AI) and Autonomous Technologies (AAT)." .


###  http://FYP-ASHS21/csonto/AAT-15.2-ResponsibilityToSupersede-Deactivateand-orDisengageAI&AutonomousTechnologies
<http://FYP-ASHS21/csonto/AAT-15.2-ResponsibilityToSupersede-Deactivateand-orDisengageAI&AutonomousTechnologies> rdf:type owl:NamedIndividual ,
                                                                                                                          :Emerging_Technologies_Policies ;
                                                                                                                 :HasWeight 10 ;
                                                                                                                 rdfs:comment "Mechanisms exist to define the criteria and responsible party(ies) for superseding, disengaging or deactivating Artificial Intelligence (AI) and Autonomous Technologies (AAT) that demonstrate performance or outcomes inconsistent with intended use." .


###  http://FYP-ASHS21/csonto/AAT-16-AI&AutonomousTechnologiesProductionMonitoring
<http://FYP-ASHS21/csonto/AAT-16-AI&AutonomousTechnologiesProductionMonitoring> rdf:type owl:NamedIndividual ,
                                                                                         :Emerging_Technologies_Policies ;
                                                                                :HasWeight 9 ;
                                                                                rdfs:comment "Mechanisms exist to monitor the functionality and behavior of the deployed Artificial Intelligence (AI) and Autonomous Technologies (AAT)." .


###  http://FYP-ASHS21/csonto/AAT-16.1-AI&AutonomousTechnologiesMeasurementApproaches
<http://FYP-ASHS21/csonto/AAT-16.1-AI&AutonomousTechnologiesMeasurementApproaches> rdf:type owl:NamedIndividual ,
                                                                                            :Emerging_Technologies_Policies ;
                                                                                   :HasWeight 8 ;
                                                                                   rdfs:comment "Mechanisms exist to measure Artificial Intelligence (AI) and Autonomous Technologies (AAT)-related risks to deployment context(s) through review and consultation with industry experts, domain specialists and end users." .


###  http://FYP-ASHS21/csonto/AAT-16.2-MeasuringAI&AutonomousTechnologiesEffectiveness
<http://FYP-ASHS21/csonto/AAT-16.2-MeasuringAI&AutonomousTechnologiesEffectiveness> rdf:type owl:NamedIndividual ,
                                                                                             :Emerging_Technologies_Policies ;
                                                                                    :HasWeight 5 ;
                                                                                    rdfs:comment "Mechanisms exist to regularly assess the effectiveness of existing controls, including reports of errors and potential impacts on affected communities." .


###  http://FYP-ASHS21/csonto/AAT-16.3-UnmeasurableAI&AutonomousTechnologiesRisks
<http://FYP-ASHS21/csonto/AAT-16.3-UnmeasurableAI&AutonomousTechnologiesRisks> rdf:type owl:NamedIndividual ,
                                                                                        :Emerging_Technologies_Policies ;
                                                                               :HasWeight 7 ;
                                                                               rdfs:comment "Mechanisms exist to identify and document unmeasurable risks or trustworthiness characteristics." .


###  http://FYP-ASHS21/csonto/AAT-16.4-EfficacyofAI&AutonomousTechnologiesMeasurement
<http://FYP-ASHS21/csonto/AAT-16.4-EfficacyofAI&AutonomousTechnologiesMeasurement> rdf:type owl:NamedIndividual ,
                                                                                            :Emerging_Technologies_Policies ;
                                                                                   :HasWeight 5 ;
                                                                                   rdfs:comment "Mechanisms exist to gather and assess feedback about the efficacy of Artificial Intelligence (AI) and Autonomous Technologies (AAT)-related measurements." .


###  http://FYP-ASHS21/csonto/AAT-16.5-AI&AutonomousTechnologiesDomainExpertReviews
<http://FYP-ASHS21/csonto/AAT-16.5-AI&AutonomousTechnologiesDomainExpertReviews> rdf:type owl:NamedIndividual ,
                                                                                          :Emerging_Technologies_Policies ;
                                                                                 :HasWeight 8 ;
                                                                                 rdfs:comment "Mechanisms exist to utilize input from domain experts and relevant stakeholders to validate whether the Artificial Intelligence (AI) and Autonomous Technologies (AAT) perform consistently, as intended." .


###  http://FYP-ASHS21/csonto/AAT-16.6-AI&AutonomousTechnologiesPerformanceChanges
<http://FYP-ASHS21/csonto/AAT-16.6-AI&AutonomousTechnologiesPerformanceChanges> rdf:type owl:NamedIndividual ,
                                                                                         :Emerging_Technologies_Policies ;
                                                                                :HasWeight 10 ;
                                                                                rdfs:comment "Mechanisms exist to evaluate performance improvements or declines with domain experts and relevant stakeholders to define context-relevant risks and trustworthiness issues." .


###  http://FYP-ASHS21/csonto/AAT-16.7-Pre-TrainedAI&AutonomousTechnologiesModels
<http://FYP-ASHS21/csonto/AAT-16.7-Pre-TrainedAI&AutonomousTechnologiesModels> rdf:type owl:NamedIndividual ,
                                                                                        :Emerging_Technologies_Policies ;
                                                                               :HasWeight 8 ;
                                                                               rdfs:comment "Mechanisms exist to validate the information sources and quality of pre-trained models used in Artificial Intelligence (AI) and Autonomous Technologies (AAT training, maintenance and improvement-related activities." .


###  http://FYP-ASHS21/csonto/AAT-17-AI&AutonomousTechnologiesHarmPrevention
<http://FYP-ASHS21/csonto/AAT-17-AI&AutonomousTechnologiesHarmPrevention> rdf:type owl:NamedIndividual ,
                                                                                   :Emerging_Technologies_Policies ;
                                                                          :HasWeight 10 ;
                                                                          rdfs:comment "Mechanisms exist to proactively prevent harm by regularly identifying and tracking existing, unanticipated and emergent Artificial Intelligence (AI) and Autonomous Technologies (AAT)-related risks." .


###  http://FYP-ASHS21/csonto/AAT-17.1-AI&AutonomousTechnologiesHumanSubjectProtections
<http://FYP-ASHS21/csonto/AAT-17.1-AI&AutonomousTechnologiesHumanSubjectProtections> rdf:type owl:NamedIndividual ,
                                                                                              :Emerging_Technologies_Policies ;
                                                                                     :HasWeight 10 ;
                                                                                     rdfs:comment "Mechanisms exist to protect human subjects from harm." .


###  http://FYP-ASHS21/csonto/AAT-17.2-AI&AutonomousTechnologiesEnvironmentalImpact&Sustainability
<http://FYP-ASHS21/csonto/AAT-17.2-AI&AutonomousTechnologiesEnvironmentalImpact&Sustainability> rdf:type owl:NamedIndividual ,
                                                                                                         :Emerging_Technologies_Policies ;
                                                                                                :HasWeight 9 ;
                                                                                                rdfs:comment "Mechanisms exist to assess and document the environmental impacts and sustainability of Artificial Intelligence (AI) and Autonomous Technologies (AAT)." .


###  http://FYP-ASHS21/csonto/AAT-17.3-PreviouslyUnknownAI&AutonomousTechnologiesThreats&Risks
<http://FYP-ASHS21/csonto/AAT-17.3-PreviouslyUnknownAI&AutonomousTechnologiesThreats&Risks> rdf:type owl:NamedIndividual ,
                                                                                                     :Emerging_Technologies_Policies ;
                                                                                            :HasWeight 9 ;
                                                                                            rdfs:comment "Mechanisms exist to respond to and recover from a previously unknown Artificial Intelligence (AI) and Autonomous Technologies (AAT)-related risk when it is identified." .


###  http://FYP-ASHS21/csonto/AAT-18-AI&AutonomousTechnologiesRiskTrackingApproaches
<http://FYP-ASHS21/csonto/AAT-18-AI&AutonomousTechnologiesRiskTrackingApproaches> rdf:type owl:NamedIndividual ,
                                                                                           :Emerging_Technologies_Policies ;
                                                                                  :HasWeight 9 ;
                                                                                  rdfs:comment "Mechanisms exist to track Artificial Intelligence (AI) and Autonomous Technologies (AAT)-related risks are difficult to assess using currently available measurement techniques or where metrics are not yet available." .


###  http://FYP-ASHS21/csonto/AAT-18.1-AI&AutonomousTechnologiesRiskResponse
<http://FYP-ASHS21/csonto/AAT-18.1-AI&AutonomousTechnologiesRiskResponse> rdf:type owl:NamedIndividual ,
                                                                                   :Emerging_Technologies_Policies ;
                                                                          :HasWeight 10 ;
                                                                          rdfs:comment "Mechanisms exist to prioritize, respond to and remediate Artificial Intelligence (AI) and Autonomous Technologies (AAT)-related risks based on assessments and other analytical output." .


###  http://FYP-ASHS21/csonto/AAT-CLD-04-Application&ProgramInterface-API-Security
<http://FYP-ASHS21/csonto/AAT-CLD-04-Application&ProgramInterface-API-Security> rdf:type owl:NamedIndividual ,
                                                                                         :Emerging_Technologies_Policies ;
                                                                                :HasWeight 9 ;
                                                                                rdfs:comment "Mechanisms exist to ensure support for secure interoperability between components with Application & Program Interfaces (APIs)." .


###  http://FYP-ASHS21/csonto/AAT-CLD-07-DataHandling&Portability
<http://FYP-ASHS21/csonto/AAT-CLD-07-DataHandling&Portability> rdf:type owl:NamedIndividual ,
                                                                        :Emerging_Technologies_Policies ;
                                                               :HasWeight 4 ;
                                                               rdfs:comment "Mechanisms exist to ensure cloud providers use secure protocols for the import, export and management of data in cloud-based services. " .


###  http://FYP-ASHS21/csonto/AST-01.2-StakeholderIdentification&Involvement
<http://FYP-ASHS21/csonto/AST-01.2-StakeholderIdentification&Involvement> rdf:type owl:NamedIndividual ,
                                                                                   :Asset_Management_Policies ;
                                                                          :HasWeight 5 ;
                                                                          rdfs:comment "Mechanisms exist to identify and involve pertinent stakeholders of critical systems, applications and services to support the ongoing secure management of those assets." .


###  http://FYP-ASHS21/csonto/AST-04-NetworkDiagrams&DataFlowDiagrams-DFDs-
<http://FYP-ASHS21/csonto/AST-04-NetworkDiagrams&DataFlowDiagrams-DFDs-> rdf:type owl:NamedIndividual ,
                                                                                  :Asset_Management_Policies ;
                                                                         :HasWeight 10 ;
                                                                         rdfs:comment """Mechanisms exist to maintain network architecture diagrams that: 
  Contain sufficient detail to assess the security of the network's architecture;
  Reflect the current architecture of the network environment; and
  Document all sensitive/regulated data flows.""" .


###  http://FYP-ASHS21/csonto/AST-05-SecurityofAssets&Media
<http://FYP-ASHS21/csonto/AST-05-SecurityofAssets&Media> rdf:type owl:NamedIndividual ,
                                                                  :Asset_Management_Policies ;
                                                         :HasWeight 8 ;
                                                         rdfs:comment "Mechanisms exist to maintain strict control over the internal or external distribution of any kind of sensitive/regulated media. " .


###  http://FYP-ASHS21/csonto/AST-07-Kiosks&PointofInteraction-PoI-Devices
<http://FYP-ASHS21/csonto/AST-07-Kiosks&PointofInteraction-PoI-Devices> rdf:type owl:NamedIndividual ,
                                                                                 :Asset_Management_Policies ;
                                                                        :HasWeight 8 ;
                                                                        rdfs:comment "Mechanisms exist to appropriately protect devices that capture sensitive/regulated data via direct physical interaction from tampering and substitution. " .


###  http://FYP-ASHS21/csonto/AST-14.1-Bluetooth&WirelessDevices
<http://FYP-ASHS21/csonto/AST-14.1-Bluetooth&WirelessDevices> rdf:type owl:NamedIndividual ,
                                                                       :Asset_Management_Policies ;
                                                              :HasWeight 7 ;
                                                              rdfs:comment "Mechanisms exist to prevent the usage of Bluetooth and wireless devices (e.g., Near Field Communications (NFC)) in sensitive areas or unless used in a Radio Frequency (RF)-screened building." .


###  http://FYP-ASHS21/csonto/AST-15.1-InspectionofSystems-Components&Devices
<http://FYP-ASHS21/csonto/AST-15.1-InspectionofSystems-Components&Devices> rdf:type owl:NamedIndividual ,
                                                                                    :Asset_Management_Policies ;
                                                                           :HasWeight 6 ;
                                                                           rdfs:comment "Mechanisms exist to physically and logically inspect critical technology assets to detect evidence of tampering. " .


###  http://FYP-ASHS21/csonto/AST-17-ProhibitedEquipment&Services
<http://FYP-ASHS21/csonto/AST-17-ProhibitedEquipment&Services> rdf:type owl:NamedIndividual ,
                                                                        :Asset_Management_Policies ;
                                                               :HasWeight 9 ;
                                                               rdfs:comment "Mechanisms exist to govern Supply Chain Risk Management (SCRM) sanctions that require the removal and prohibition of certain technology services and/or equipment that are designated as supply chain threats by a statutory or regulatory body." .


###  http://FYP-ASHS21/csonto/AST-22-Microphones&WebCameras
<http://FYP-ASHS21/csonto/AST-22-Microphones&WebCameras> rdf:type owl:NamedIndividual ,
                                                                  :Asset_Management_Policies ;
                                                         :HasWeight 8 ;
                                                         rdfs:comment "Mechanisms exist to configure assets to prohibit the use of endpoint-based microphones and web cameras in secure areas or where sensitive/regulated information is discussed." .


###  http://FYP-ASHS21/csonto/AST-CAP-01-Capacity&PerformanceManagement
<http://FYP-ASHS21/csonto/AST-CAP-01-Capacity&PerformanceManagement> rdf:type owl:NamedIndividual ,
                                                                              :Asset_Management_Policies ;
                                                                     :HasWeight 8 ;
                                                                     rdfs:comment "Mechanisms exist to facilitate the implementation of capacity management controls to ensure optimal system performance to meet expected and anticipated future capacity requirements." .


###  http://FYP-ASHS21/csonto/AST-CFG-02.1-Reviews&Updates
<http://FYP-ASHS21/csonto/AST-CFG-02.1-Reviews&Updates> rdf:type owl:NamedIndividual ,
                                                                 :Asset_Management_Policies ;
                                                        :HasWeight 8 ;
                                                        rdfs:comment """Mechanisms exist to review and update baseline configurations:
  At least annually;
  When required due to so; or
  As part of system component installations and upgrades.""" .


###  http://FYP-ASHS21/csonto/AST-CFG-02.2-AutomatedCentralManagement&Verification
<http://FYP-ASHS21/csonto/AST-CFG-02.2-AutomatedCentralManagement&Verification> rdf:type owl:NamedIndividual ,
                                                                                         :Asset_Management_Policies ;
                                                                                :HasWeight 7 ;
                                                                                rdfs:comment "Automated mechanisms exist to govern and report on baseline configurations of the systems. " .


###  http://FYP-ASHS21/csonto/AST-CFG-02.4-Development&TestEnvironmentConfigurations
<http://FYP-ASHS21/csonto/AST-CFG-02.4-Development&TestEnvironmentConfigurations> rdf:type owl:NamedIndividual ,
                                                                                           :Asset_Management_Policies ;
                                                                                  :HasWeight 5 ;
                                                                                  rdfs:comment "Mechanisms exist to manage baseline configurations for development and test environments separately from operational baseline configurations to minimize the risk of unintentional changes." .


###  http://FYP-ASHS21/csonto/AST-CFG-04.2-UnsupportedInternetBrowsers&EmailClients
<http://FYP-ASHS21/csonto/AST-CFG-04.2-UnsupportedInternetBrowsers&EmailClients> rdf:type owl:NamedIndividual ,
                                                                                          :Asset_Management_Policies ;
                                                                                 :HasWeight 7 ;
                                                                                 rdfs:comment "Mechanisms exist to allow only approved Internet browsers and email clients to run on systems." .


###  http://FYP-ASHS21/csonto/AST-MDM-03-FullDevice&Container-BasedEncryption
<http://FYP-ASHS21/csonto/AST-MDM-03-FullDevice&Container-BasedEncryption> rdf:type owl:NamedIndividual ,
                                                                                    :Asset_Management_Policies ;
                                                                           :HasWeight 9 ;
                                                                           rdfs:comment "Cryptographic mechanisms exist to protect the confidentiality and integrity of information on mobile devices through full-device or container encryption." .


###  http://FYP-ASHS21/csonto/CHG-CHG-02.2-Test-Validate&DocumentChanges
<http://FYP-ASHS21/csonto/CHG-CHG-02.2-Test-Validate&DocumentChanges> rdf:type owl:NamedIndividual ,
                                                                               :Change_Management_Policies ;
                                                                      :HasWeight 9 ;
                                                                      rdfs:comment "Mechanisms exist to appropriately test and document proposed changes in a non-production environment before changes are implemented in a production environment." .


###  http://FYP-ASHS21/csonto/CHG-CHG-02.3-Cybersecurity&DataPrivacyRepresentativeforAssetLifecycleChanges
<http://FYP-ASHS21/csonto/CHG-CHG-02.3-Cybersecurity&DataPrivacyRepresentativeforAssetLifecycleChanges> rdf:type owl:NamedIndividual ,
                                                                                                                 :Change_Management_Policies ;
                                                                                                        :HasWeight 7 ;
                                                                                                        rdfs:comment "Mechanisms exist to include a cybersecurity and/or data privacy representative in the configuration change control review process." .


###  http://FYP-ASHS21/csonto/CHG-RSK-09.2-AI&AutonomousTechnologiesSupplyChainImpacts
<http://FYP-ASHS21/csonto/CHG-RSK-09.2-AI&AutonomousTechnologiesSupplyChainImpacts> rdf:type owl:NamedIndividual ,
                                                                                             :Change_Management_Policies ;
                                                                                    :HasWeight 8 ;
                                                                                    rdfs:comment "Mechanisms exist to address Artificial Intelligence (AI) and Autonomous Technologies (AAT)-related risks and benefits arising from the organization's supply chain, including third-party software and data." .


###  http://FYP-ASHS21/csonto/CHG-SEA-01.1-CentralizedManagementofCybersecurity&DataPrivacyControls
<http://FYP-ASHS21/csonto/CHG-SEA-01.1-CentralizedManagementofCybersecurity&DataPrivacyControls> rdf:type owl:NamedIndividual ,
                                                                                                          :Change_Management_Policies ;
                                                                                                 :HasWeight 9 ;
                                                                                                 rdfs:comment "Mechanisms exist to centrally-manage the organization-wide management and implementation of cybersecurity & data privacy controls and related processes." .


###  http://FYP-ASHS21/csonto/CHG-SEA-14-Concealment&Misdirection
<http://FYP-ASHS21/csonto/CHG-SEA-14-Concealment&Misdirection> rdf:type owl:NamedIndividual ,
                                                                        :Change_Management_Policies ;
                                                               :HasWeight 2 ;
                                                               rdfs:comment "Mechanisms exist to utilize concealment and misdirection techniques for systems to confuse and mislead adversaries. " .


###  http://FYP-ASHS21/csonto/CHG-SEA-14.2-ChangeProcessing&StorageLocations
<http://FYP-ASHS21/csonto/CHG-SEA-14.2-ChangeProcessing&StorageLocations> rdf:type owl:NamedIndividual ,
                                                                                   :Change_Management_Policies ;
                                                                          :HasWeight 5 ;
                                                                          rdfs:comment "Automated mechanisms exist to change the location of processing and/or storage at random time intervals." .


###  http://FYP-ASHS21/csonto/CHG-SEA-15-DistributedProcessing&Storage
<http://FYP-ASHS21/csonto/CHG-SEA-15-DistributedProcessing&Storage> rdf:type owl:NamedIndividual ,
                                                                             :Change_Management_Policies ;
                                                                    :HasWeight 4 ;
                                                                    rdfs:comment "Mechanisms exist to distribute processing and storage across multiple physical locations. " .


###  http://FYP-ASHS21/csonto/CHG-TDA-01-TechnologyDevelopment&Acquisition
<http://FYP-ASHS21/csonto/CHG-TDA-01-TechnologyDevelopment&Acquisition> rdf:type owl:NamedIndividual ,
                                                                                 :Change_Management_Policies ;
                                                                        :HasWeight 10 ;
                                                                        rdfs:comment "Mechanisms exist to facilitate the implementation of tailored development and acquisition strategies, contract tools and procurement methods to meet unique business needs." .


###  http://FYP-ASHS21/csonto/CHG-TDA-02.1-Ports-Protocols&ServicesInUse
<http://FYP-ASHS21/csonto/CHG-TDA-02.1-Ports-Protocols&ServicesInUse> rdf:type owl:NamedIndividual ,
                                                                               :Change_Management_Policies ;
                                                                      :HasWeight 8 ;
                                                                      rdfs:comment "Mechanisms exist to require the developers of systems, system components or services to identify early in the Secure Development Life Cycle (SDLC), the functions, ports, protocols and services intended for use. " .


###  http://FYP-ASHS21/csonto/CHG-TDA-02.3-DevelopmentMethods-Techniques&Processes
<http://FYP-ASHS21/csonto/CHG-TDA-02.3-DevelopmentMethods-Techniques&Processes> rdf:type owl:NamedIndividual ,
                                                                                         :Change_Management_Policies ;
                                                                                :HasWeight 5 ;
                                                                                rdfs:comment "Mechanisms exist to require software vendors / manufacturers to demonstrate that their software development processes employ industry-recognized secure practices for secure programming, engineering methods, quality control processes and validation techniques to minimize flawed or malformed software." .


###  http://FYP-ASHS21/csonto/CHG-TDA-02.5-Identification&JustificationofPorts-Protocols&Services
<http://FYP-ASHS21/csonto/CHG-TDA-02.5-Identification&JustificationofPorts-Protocols&Services> rdf:type owl:NamedIndividual ,
                                                                                                        :Change_Management_Policies ;
                                                                                               :HasWeight 8 ;
                                                                                               rdfs:comment "Mechanisms exist to require process owners to identify, document and justify the business need for the ports, protocols and other services necessary to operate their technology solutions. " .


###  http://FYP-ASHS21/csonto/CHG-TDA-02.6-InsecurePorts-Protocols&Services
<http://FYP-ASHS21/csonto/CHG-TDA-02.6-InsecurePorts-Protocols&Services> rdf:type owl:NamedIndividual ,
                                                                                  :Change_Management_Policies ;
                                                                         :HasWeight 9 ;
                                                                         rdfs:comment "Mechanisms exist to mitigate the risk associated with the use of insecure ports, protocols and services necessary to operate technology solutions. " .


###  http://FYP-ASHS21/csonto/CHG-TDA-02.7-Cybersecurity&DataPrivacyRepresentativesForProductChanges
<http://FYP-ASHS21/csonto/CHG-TDA-02.7-Cybersecurity&DataPrivacyRepresentativesForProductChanges> rdf:type owl:NamedIndividual ,
                                                                                                           :Change_Management_Policies ;
                                                                                                  :HasWeight 10 ;
                                                                                                  rdfs:comment "Mechanisms exist to include appropriate cybersecurity & data privacy representatives in the product feature and/or functionality change control review process." .


###  http://FYP-ASHS21/csonto/CHG-TDA-05-DeveloperArchitecture&Design
<http://FYP-ASHS21/csonto/CHG-TDA-05-DeveloperArchitecture&Design> rdf:type owl:NamedIndividual ,
                                                                            :Change_Management_Policies ;
                                                                   :HasWeight 8 ;
                                                                   rdfs:comment """Mechanisms exist to require the developers of systems, system components or services to produce a design specification and security architecture that: 
  Is consistent with and supportive of the organizations security architecture which is established within and is an integrated part of the organizations enterprise architecture;
  Accurately and completely describes the required security functionality and the allocation of security controls among physical and logical components; and
  Expresses how individual security functions, mechanisms and services work together to provide required security capabilities and a unified approach to protection.""" .


###  http://FYP-ASHS21/csonto/CHG-TDA-05.1-PhysicalDiagnostic&TestInterfaces
<http://FYP-ASHS21/csonto/CHG-TDA-05.1-PhysicalDiagnostic&TestInterfaces> rdf:type owl:NamedIndividual ,
                                                                                   :Change_Management_Policies ;
                                                                          :HasWeight 5 ;
                                                                          rdfs:comment "Mechanisms exist to secure physical diagnostic and test interfaces to prevent misuse." .


###  http://FYP-ASHS21/csonto/CHG-TDA-05.2-Diagnostic&TestInterfaceMonitoring
<http://FYP-ASHS21/csonto/CHG-TDA-05.2-Diagnostic&TestInterfaceMonitoring> rdf:type owl:NamedIndividual ,
                                                                                    :Change_Management_Policies ;
                                                                           :HasWeight 3 ;
                                                                           rdfs:comment "Mechanisms exist to enable endpoint devices to log events and generate alerts for attempts to access diagnostic and test interfaces." .


###  http://FYP-ASHS21/csonto/CHG-TDA-09-Cybersecurity&DataPrivacyTestingThroughoutDevelopment
<http://FYP-ASHS21/csonto/CHG-TDA-09-Cybersecurity&DataPrivacyTestingThroughoutDevelopment> rdf:type owl:NamedIndividual ,
                                                                                                     :Change_Management_Policies ;
                                                                                            :HasWeight 9 ;
                                                                                            rdfs:comment """Mechanisms exist to require system developers/integrators consult with cybersecurity & data privacy personnel to: 
  Create and implement a Security Test and Evaluation (ST&E) plan;
  Implement a verifiable flaw remediation process to correct weaknesses and deficiencies identified during the security testing and evaluation process; and
  Document the results of the security testing/evaluation and flaw remediation processes.""" .


###  http://FYP-ASHS21/csonto/CHG-TDA-15-DeveloperThreatAnalysis&FlawRemediation
<http://FYP-ASHS21/csonto/CHG-TDA-15-DeveloperThreatAnalysis&FlawRemediation> rdf:type owl:NamedIndividual ,
                                                                                       :Change_Management_Policies ;
                                                                              :HasWeight 9 ;
                                                                              rdfs:comment "Mechanisms exist to require system developers and integrators to create a Security Test and Evaluation (ST&E) plan and implement the plan under the witness of an independent party. " .


###  http://FYP-ASHS21/csonto/CHG-TPM-03.1-AcquisitionStrategies-Tools&Methods
<http://FYP-ASHS21/csonto/CHG-TPM-03.1-AcquisitionStrategies-Tools&Methods> rdf:type owl:NamedIndividual ,
                                                                                     :Change_Management_Policies ;
                                                                            :HasWeight 9 ;
                                                                            rdfs:comment "Mechanisms exist to utilize tailored acquisition strategies, contract tools and procurement methods for the purchase of unique systems, system components or services." .


###  http://FYP-ASHS21/csonto/CHG-TPM-04.1-Third-PartyRiskAssessments&Approvals
<http://FYP-ASHS21/csonto/CHG-TPM-04.1-Third-PartyRiskAssessments&Approvals> rdf:type owl:NamedIndividual ,
                                                                                      :Change_Management_Policies ;
                                                                             :HasWeight 9 ;
                                                                             rdfs:comment "Mechanisms exist to conduct a risk assessment prior to the acquisition or outsourcing of technology-related services." .


###  http://FYP-ASHS21/csonto/CHG-TPM-04.2-ExternalConnectivityRequirements-IdentificationofPorts-Protocols&Services
<http://FYP-ASHS21/csonto/CHG-TPM-04.2-ExternalConnectivityRequirements-IdentificationofPorts-Protocols&Services> rdf:type owl:NamedIndividual ,
                                                                                                                           :Change_Management_Policies ;
                                                                                                                  :HasWeight 7 ;
                                                                                                                  rdfs:comment "Mechanisms exist to require External Service Providers (ESPs) to identify and document the business need for ports, protocols and other services it requires to operate its processes and technologies." .


###  http://FYP-ASHS21/csonto/CHG-TPM-05.4-Responsible-Accountable-Supportive-Consulted&Informed-RASCI-Matrix
<http://FYP-ASHS21/csonto/CHG-TPM-05.4-Responsible-Accountable-Supportive-Consulted&Informed-RASCI-Matrix> rdf:type owl:NamedIndividual ,
                                                                                                                    :Change_Management_Policies ;
                                                                                                           :HasWeight 8 ;
                                                                                                           rdfs:comment "Mechanisms exist to document and maintain a Responsible, Accountable, Supportive, Consulted & Informed (RASCI) matrix, or similar documentation, to delineate assignment for cybersecurity & data privacy controls between internal stakeholders and External Service Providers (ESPs). " .


###  http://FYP-ASHS21/csonto/CHG-TPM-11-Third-PartyIncidentResponse&RecoveryCapabilities
<http://FYP-ASHS21/csonto/CHG-TPM-11-Third-PartyIncidentResponse&RecoveryCapabilities> rdf:type owl:NamedIndividual ,
                                                                                                :Change_Management_Policies ;
                                                                                       :HasWeight 8 ;
                                                                                       rdfs:comment "Mechanisms exist to ensure response/recovery planning and testing are conducted with critical suppliers/providers. " .


###  http://FYP-ASHS21/csonto/GOV-01-Cybersecurity&DataProtectionGovernanceProgram
<http://FYP-ASHS21/csonto/GOV-01-Cybersecurity&DataProtectionGovernanceProgram> rdf:type owl:NamedIndividual ,
                                                                                         :Governance_Policies ;
                                                                                :HasWeight 10 ;
                                                                                rdfs:comment "Mechanisms exist to facilitate the implementation of cybersecurity & data protection governance controls." .


###  http://FYP-ASHS21/csonto/GOV-01.1-SteeringCommittee&ProgramOversight
<http://FYP-ASHS21/csonto/GOV-01.1-SteeringCommittee&ProgramOversight> rdf:type owl:NamedIndividual ,
                                                                                :Governance_Policies ;
                                                                       :HasWeight 7 ;
                                                                       rdfs:comment "Mechanisms exist to coordinate cybersecurity, data protection and business alignment through a steering committee or advisory board, comprised of key cybersecurity, data privacy and business executives, which meets formally and on a regular basis." .


###  http://FYP-ASHS21/csonto/GOV-02-PublishingCybersecurity&DataProtectionDocumentation
<http://FYP-ASHS21/csonto/GOV-02-PublishingCybersecurity&DataProtectionDocumentation> rdf:type owl:NamedIndividual ,
                                                                                               :Governance_Policies ;
                                                                                      :HasWeight 10 ;
                                                                                      rdfs:comment "Mechanisms exist to establish, maintain and disseminate cybersecurity & data protection policies, standards and procedures." .


###  http://FYP-ASHS21/csonto/GOV-03-PeriodicReview&UpdateofCybersecurity&DataProtectionProgram
<http://FYP-ASHS21/csonto/GOV-03-PeriodicReview&UpdateofCybersecurity&DataProtectionProgram> rdf:type owl:NamedIndividual ,
                                                                                                      :Governance_Policies ;
                                                                                             :HasWeight 7 ;
                                                                                             rdfs:comment "Mechanisms exist to review the cybersecurity & data privacy program, including policies, standards and procedures, at planned intervals or if significant changes occur to ensure their continuing suitability, adequacy and effectiveness. " .


###  http://FYP-ASHS21/csonto/GOV-04-AssignedCybersecurity&DataProtectionResponsibilities
<http://FYP-ASHS21/csonto/GOV-04-AssignedCybersecurity&DataProtectionResponsibilities> rdf:type owl:NamedIndividual ,
                                                                                                :Governance_Policies ;
                                                                                       :HasWeight 10 ;
                                                                                       rdfs:comment "Mechanisms exist to assign one or more qualified individuals with the mission and resources to centrally-manage, coordinate, develop, implement and maintain an enterprise-wide cybersecurity & data protection program. " .


###  http://FYP-ASHS21/csonto/GOV-07-ContactsWithGroups&Associations
<http://FYP-ASHS21/csonto/GOV-07-ContactsWithGroups&Associations> rdf:type owl:NamedIndividual ,
                                                                           :Governance_Policies ;
                                                                  :HasWeight 7 ;
                                                                  rdfs:comment """Mechanisms exist to establish contact with selected groups and associations within the cybersecurity & data privacy communities to: 
  Facilitate ongoing cybersecurity & data privacy education and training for organizational personnel;
  Maintain currency with recommended cybersecurity & data privacy practices, techniques and technologies; and
  Share current cybersecurity and/or data privacy-related information including threats, vulnerabilities and incidents.
""" .


###  http://FYP-ASHS21/csonto/GOV-08-DefiningBusinessContext&Mission
<http://FYP-ASHS21/csonto/GOV-08-DefiningBusinessContext&Mission> rdf:type owl:NamedIndividual ,
                                                                           :Governance_Policies ;
                                                                  :HasWeight 5 ;
                                                                  rdfs:comment "Mechanisms exist to define the context of its business model and document the mission of the organization." .


###  http://FYP-ASHS21/csonto/GOV-15-OperationalizingCybersecurity&DataProtectionPractices
<http://FYP-ASHS21/csonto/GOV-15-OperationalizingCybersecurity&DataProtectionPractices> rdf:type owl:NamedIndividual ,
                                                                                                 :Governance_Policies ;
                                                                                        :HasWeight 9 ;
                                                                                        rdfs:comment "Mechanisms exist to compel data and/or process owners to operationalize cybersecurity & data privacy practices for each system, application and/or service under their control." .


###  http://FYP-ASHS21/csonto/GOV-15.4-AuthorizeSystems-Applications&Services
<http://FYP-ASHS21/csonto/GOV-15.4-AuthorizeSystems-Applications&Services> rdf:type owl:NamedIndividual ,
                                                                                    :Governance_Policies ;
                                                                           :HasWeight 8 ;
                                                                           rdfs:comment "Mechanisms exist to compel data and/or process owners to obtain authorization for the production use of each system, application and/or service under their control." .


###  http://FYP-ASHS21/csonto/GOV-PRM-01-Cybersecurity&DataPrivacyPortfolioManagement
<http://FYP-ASHS21/csonto/GOV-PRM-01-Cybersecurity&DataPrivacyPortfolioManagement> rdf:type owl:NamedIndividual ,
                                                                                            :Governance_Policies ;
                                                                                   :HasWeight 8 ;
                                                                                   rdfs:comment "Mechanisms exist to facilitate the implementation of cybersecurity & data privacy-related resource planning controls that define a viable plan for achieving cybersecurity & data privacy objectives." .


###  http://FYP-ASHS21/csonto/GOV-PRM-01.1-StrategicPlan&Objectives
<http://FYP-ASHS21/csonto/GOV-PRM-01.1-StrategicPlan&Objectives> rdf:type owl:NamedIndividual ,
                                                                          :Governance_Policies ;
                                                                 :HasWeight 5 ;
                                                                 rdfs:comment "Mechanisms exist to establish a strategic cybersecurity & data privacy-specific business plan and set of objectives to achieve that plan." .


###  http://FYP-ASHS21/csonto/GOV-PRM-02-Cybersecurity&DataPrivacyResourceManagement
<http://FYP-ASHS21/csonto/GOV-PRM-02-Cybersecurity&DataPrivacyResourceManagement> rdf:type owl:NamedIndividual ,
                                                                                           :Governance_Policies ;
                                                                                  :HasWeight 8 ;
                                                                                  rdfs:comment "Mechanisms exist to address all capital planning and investment requests, including the resources needed to implement the cybersecurity & data privacy programs and document all exceptions to this requirement. " .


###  http://FYP-ASHS21/csonto/GOV-PRM-04-Cybersecurity&DataPrivacyInProjectManagement
<http://FYP-ASHS21/csonto/GOV-PRM-04-Cybersecurity&DataPrivacyInProjectManagement> rdf:type owl:NamedIndividual ,
                                                                                            :Governance_Policies ;
                                                                                   :HasWeight 10 ;
                                                                                   rdfs:comment "Mechanisms exist to assess cybersecurity & data privacy controls in system project development to determine the extent to which the controls are implemented correctly, operating as intended and producing the desired outcome with respect to meeting the requirements." .


###  http://FYP-ASHS21/csonto/GOV-PRM-05-Cybersecurity&DataPrivacyRequirementsDefinition
<http://FYP-ASHS21/csonto/GOV-PRM-05-Cybersecurity&DataPrivacyRequirementsDefinition> rdf:type owl:NamedIndividual ,
                                                                                               :Governance_Policies ;
                                                                                      :HasWeight 9 ;
                                                                                      rdfs:comment "Mechanisms exist to identify critical system components and functions by performing a criticality analysis for critical systems, system components or services at pre-defined decision points in the Secure Development Life Cycle (SDLC). " .


###  http://FYP-ASHS21/csonto/IAO-03-SystemSecurity&PrivacyPlan-SSPP-
<http://FYP-ASHS21/csonto/IAO-03-SystemSecurity&PrivacyPlan-SSPP-> rdf:type owl:NamedIndividual ,
                                                                            :Assurance_Policies ;
                                                                   :HasWeight 7 ;
                                                                   rdfs:comment "Mechanisms exist to generate System Security & Privacy Plans (SSPPs), or similar document repositories, to identify and maintain key architectural information on each critical system, application or service, as well as influence inputs, entities, systems, applications and processes, providing a historical record of the data and its origins." .


###  http://FYP-ASHS21/csonto/IAO-04-ThreatAnalysis&FlawRemediationDuringDevelopment
<http://FYP-ASHS21/csonto/IAO-04-ThreatAnalysis&FlawRemediationDuringDevelopment> rdf:type owl:NamedIndividual ,
                                                                                           :Assurance_Policies ;
                                                                                  :HasWeight 10 ;
                                                                                  rdfs:comment "Mechanisms exist to require system developers and integrators to create and execute a Security Test and Evaluation (ST&E) plan to identify and remediate flaws during development." .


###  http://FYP-ASHS21/csonto/IAO-05-PlanofAction&Milestones-POA&M-
<http://FYP-ASHS21/csonto/IAO-05-PlanofAction&Milestones-POA&M-> rdf:type owl:NamedIndividual ,
                                                                          :Assurance_Policies ;
                                                                 :HasWeight 9 ;
                                                                 rdfs:comment "Mechanisms exist to generate a Plan of Action and Milestones (POA&M), or similar risk register, to document planned remedial actions to correct weaknesses or deficiencies noted during the assessment of the security controls and to reduce or eliminate known vulnerabilities." .


###  http://FYP-ASHS21/csonto/IAO-05.1-PlanofAction&Milestones-POA&M-Automation
<http://FYP-ASHS21/csonto/IAO-05.1-PlanofAction&Milestones-POA&M-Automation> rdf:type owl:NamedIndividual ,
                                                                                      :Assurance_Policies ;
                                                                             :HasWeight 2 ;
                                                                             rdfs:comment "Automated mechanisms exist to help ensure the Plan of Action and Milestones (POA&M), or similar risk register, is accurate, up-to-date and readily-available." .


###  http://FYP-ASHS21/csonto/IAO-CPL-01-Statutory-Regulatory&ContractualCompliance
<http://FYP-ASHS21/csonto/IAO-CPL-01-Statutory-Regulatory&ContractualCompliance> rdf:type owl:NamedIndividual ,
                                                                                          :Assurance_Policies ;
                                                                                 :HasWeight 10 ;
                                                                                 rdfs:comment "Mechanisms exist to facilitate the identification and implementation of relevant statutory, regulatory and contractual controls." .


###  http://FYP-ASHS21/csonto/IAO-CPL-02-Cybersecurity&DataPrivacyControlsOversight
<http://FYP-ASHS21/csonto/IAO-CPL-02-Cybersecurity&DataPrivacyControlsOversight> rdf:type owl:NamedIndividual ,
                                                                                          :Assurance_Policies ;
                                                                                 :HasWeight 10 ;
                                                                                 rdfs:comment "Mechanisms exist to provide a security & data privacy controls oversight function that reports to the organization's executive leadership." .


###  http://FYP-ASHS21/csonto/IAO-CPL-03-Cybersecurity&DataPrivacyAssessments
<http://FYP-ASHS21/csonto/IAO-CPL-03-Cybersecurity&DataPrivacyAssessments> rdf:type owl:NamedIndividual ,
                                                                                    :Assurance_Policies ;
                                                                           :HasWeight 10 ;
                                                                           rdfs:comment "Mechanisms exist to ensure managers regularly review the processes and documented procedures within their area of responsibility to adhere to appropriate security policies, standards and other applicable requirements." .


###  http://FYP-ASHS21/csonto/IAO-CPL-03.2-FunctionalReviewOfCybersecurity&DataPrivacyControls
<http://FYP-ASHS21/csonto/IAO-CPL-03.2-FunctionalReviewOfCybersecurity&DataPrivacyControls> rdf:type owl:NamedIndividual ,
                                                                                                     :Assurance_Policies ;
                                                                                            :HasWeight 8 ;
                                                                                            rdfs:comment "Mechanisms exist to regularly review technology assets for adherence to the organizations cybersecurity & data privacy policies and standards. " .


###  http://FYP-ASHS21/csonto/IAO-SAT-01-Cybersecurity&DataPrivacy-MindedWorkforce
<http://FYP-ASHS21/csonto/IAO-SAT-01-Cybersecurity&DataPrivacy-MindedWorkforce> rdf:type owl:NamedIndividual ,
                                                                                         :Assurance_Policies ;
                                                                                :HasWeight 8 ;
                                                                                rdfs:comment "Mechanisms exist to facilitate the implementation of security workforce development and awareness controls. " .


###  http://FYP-ASHS21/csonto/IAO-SAT-02-Cybersecurity&DataPrivacyAwarenessTraining
<http://FYP-ASHS21/csonto/IAO-SAT-02-Cybersecurity&DataPrivacyAwarenessTraining> rdf:type owl:NamedIndividual ,
                                                                                          :Assurance_Policies ;
                                                                                 :HasWeight 8 ;
                                                                                 rdfs:comment "Mechanisms exist to provide all employees and contractors appropriate awareness education and training that is relevant for their job function. " .


###  http://FYP-ASHS21/csonto/IAO-SAT-02.2-SocialEngineering&Mining
<http://FYP-ASHS21/csonto/IAO-SAT-02.2-SocialEngineering&Mining> rdf:type owl:NamedIndividual ,
                                                                          :Assurance_Policies ;
                                                                 :HasWeight 5 ;
                                                                 rdfs:comment "Mechanisms exist to include awareness training on recognizing and reporting potential and actual instances of social engineering and social mining." .


###  http://FYP-ASHS21/csonto/IAO-SAT-03-Role-BasedCybersecurity&DataPrivacyTraining
<http://FYP-ASHS21/csonto/IAO-SAT-03-Role-BasedCybersecurity&DataPrivacyTraining> rdf:type owl:NamedIndividual ,
                                                                                           :Assurance_Policies ;
                                                                                  :HasWeight 8 ;
                                                                                  rdfs:comment """Mechanisms exist to provide role-based cybersecurity & data privacy-related training: 
  Before authorizing access to the system or performing assigned duties; 
  When required by system changes; and 
  Annually thereafter.""" .


###  http://FYP-ASHS21/csonto/IAO-SAT-03.2-SuspiciousCommunications&AnomalousSystemBehavior
<http://FYP-ASHS21/csonto/IAO-SAT-03.2-SuspiciousCommunications&AnomalousSystemBehavior> rdf:type owl:NamedIndividual ,
                                                                                                  :Assurance_Policies ;
                                                                                         :HasWeight 9 ;
                                                                                         rdfs:comment "Mechanisms exist to provide training to personnel on organization-defined indicators of malware to recognize suspicious communications and anomalous behavior." .


###  http://FYP-ASHS21/csonto/IAO-SAT-03.3-SensitiveInformationStorage-Handling&Processing
<http://FYP-ASHS21/csonto/IAO-SAT-03.3-SensitiveInformationStorage-Handling&Processing> rdf:type owl:NamedIndividual ,
                                                                                                 :Assurance_Policies ;
                                                                                        :HasWeight 9 ;
                                                                                        rdfs:comment "Mechanisms exist to ensure that every user accessing a system processing, storing or transmitting sensitive information is formally trained in data handling requirements." .


###  http://FYP-ASHS21/csonto/IAO-SAT-03.4-VendorCybersecurity&DataPrivacyTraining
<http://FYP-ASHS21/csonto/IAO-SAT-03.4-VendorCybersecurity&DataPrivacyTraining> rdf:type owl:NamedIndividual ,
                                                                                         :Assurance_Policies ;
                                                                                :HasWeight 7 ;
                                                                                rdfs:comment "Mechanisms exist to incorporate vendor-specific security training in support of new technology initiatives. " .


###  http://FYP-ASHS21/csonto/IAO-SAT-03.7-ContinuingProfessionalEducation-CPE--Cybersecurity&DataPrivacyPersonnel
<http://FYP-ASHS21/csonto/IAO-SAT-03.7-ContinuingProfessionalEducation-CPE--Cybersecurity&DataPrivacyPersonnel> rdf:type owl:NamedIndividual ,
                                                                                                                         :Assurance_Policies ;
                                                                                                                :HasWeight 8 ;
                                                                                                                rdfs:comment "Mechanisms exist to ensure cybersecurity & data privacy personnel receive Continuing Professional Education (CPE) training to maintain currency and proficiency with industry-recognized secure practices that are pertinent to their assigned roles and responsibilities." .


###  http://FYP-ASHS21/csonto/IAO-SAT-04-Cybersecurity&DataPrivacyTrainingRecords
<http://FYP-ASHS21/csonto/IAO-SAT-04-Cybersecurity&DataPrivacyTrainingRecords> rdf:type owl:NamedIndividual ,
                                                                                        :Assurance_Policies ;
                                                                               :HasWeight 9 ;
                                                                               rdfs:comment "Mechanisms exist to document, retain and monitor individual training activities, including basic cybersecurity & data privacy awareness training, ongoing awareness training and specific-system training." .


###  http://FYP-ASHS21/csonto/OPS-BCD-02.1-ResumeAllMissions&BusinessFunctions
<http://FYP-ASHS21/csonto/OPS-BCD-02.1-ResumeAllMissions&BusinessFunctions> rdf:type owl:NamedIndividual ,
                                                                                     :Security_Operations_Policies ;
                                                                            :HasWeight 8 ;
                                                                            rdfs:comment "Mechanisms exist to resume all missions and business functions within Recovery Time Objectives (RTOs) of the contingency plan's activation." .


###  http://FYP-ASHS21/csonto/OPS-BCD-02.2-ContinueEssentialMission&BusinessFunctions
<http://FYP-ASHS21/csonto/OPS-BCD-02.2-ContinueEssentialMission&BusinessFunctions> rdf:type owl:NamedIndividual ,
                                                                                            :Security_Operations_Policies ;
                                                                                   :HasWeight 8 ;
                                                                                   rdfs:comment "Mechanisms exist to continue essential missions and business functions with little or no loss of operational continuity and sustain that continuity until full system restoration at primary processing and/or storage sites." .


###  http://FYP-ASHS21/csonto/OPS-BCD-02.3-ResumeEssentialMissions&BusinessFunctions
<http://FYP-ASHS21/csonto/OPS-BCD-02.3-ResumeEssentialMissions&BusinessFunctions> rdf:type owl:NamedIndividual ,
                                                                                           :Security_Operations_Policies ;
                                                                                  :HasWeight 8 ;
                                                                                  rdfs:comment "Mechanisms exist to resume essential missions and business functions within an organization-defined time period of contingency plan activation. " .


###  http://FYP-ASHS21/csonto/OPS-BCD-04-ContingencyPlanTesting&Exercises
<http://FYP-ASHS21/csonto/OPS-BCD-04-ContingencyPlanTesting&Exercises> rdf:type owl:NamedIndividual ,
                                                                                :Security_Operations_Policies ;
                                                                       :HasWeight 6 ;
                                                                       rdfs:comment "Mechanisms exist to conduct tests and/or exercises to evaluate the contingency plan's effectiveness and the organizations readiness to execute the plan. " .


###  http://FYP-ASHS21/csonto/OPS-BCD-04.2-AlternateStorage&ProcessingSites
<http://FYP-ASHS21/csonto/OPS-BCD-04.2-AlternateStorage&ProcessingSites> rdf:type owl:NamedIndividual ,
                                                                                  :Security_Operations_Policies ;
                                                                         :HasWeight 5 ;
                                                                         rdfs:comment "Mechanisms exist to test contingency plans at alternate storage & processing sites to both familiarize contingency personnel with the facility and evaluate the capabilities of the alternate processing site to support contingency operations. " .


###  http://FYP-ASHS21/csonto/OPS-BCD-05-ContingencyPlanRootCauseAnalysis-RCA-&LessonsLearned
<http://FYP-ASHS21/csonto/OPS-BCD-05-ContingencyPlanRootCauseAnalysis-RCA-&LessonsLearned> rdf:type owl:NamedIndividual ,
                                                                                                    :Security_Operations_Policies ;
                                                                                           :HasWeight 9 ;
                                                                                           rdfs:comment "Mechanisms exist to conduct a Root Cause Analysis (RCA) and \"lessons learned\" activity every time the contingency plan is activated." .


###  http://FYP-ASHS21/csonto/OPS-BCD-06-ContingencyPlanning&Updates
<http://FYP-ASHS21/csonto/OPS-BCD-06-ContingencyPlanning&Updates> rdf:type owl:NamedIndividual ,
                                                                           :Security_Operations_Policies ;
                                                                  :HasWeight 8 ;
                                                                  rdfs:comment "Mechanisms exist to keep contingency plans current with business needs, technology changes and feedback from contingency plan testing activities." .


###  http://FYP-ASHS21/csonto/OPS-BCD-11.1-TestingforReliability&Integrity
<http://FYP-ASHS21/csonto/OPS-BCD-11.1-TestingforReliability&Integrity> rdf:type owl:NamedIndividual ,
                                                                                 :Security_Operations_Policies ;
                                                                        :HasWeight 9 ;
                                                                        rdfs:comment "Mechanisms exist to routinely test backups that verify the reliability of the backup process, as well as the integrity and availability of the data. " .


###  http://FYP-ASHS21/csonto/OPS-BCD-12-InformationSystemRecovery&Reconstitution
<http://FYP-ASHS21/csonto/OPS-BCD-12-InformationSystemRecovery&Reconstitution> rdf:type owl:NamedIndividual ,
                                                                                        :Security_Operations_Policies ;
                                                                               :HasWeight 9 ;
                                                                               rdfs:comment "Mechanisms exist to ensure the secure recovery and reconstitution of systems to a known state after a disruption, compromise or failure." .


###  http://FYP-ASHS21/csonto/OPS-BCD-13-Backup&RestorationHardwareProtection
<http://FYP-ASHS21/csonto/OPS-BCD-13-Backup&RestorationHardwareProtection> rdf:type owl:NamedIndividual ,
                                                                                    :Security_Operations_Policies ;
                                                                           :HasWeight 8 ;
                                                                           rdfs:comment "Mechanisms exist to protect backup and restoration hardware and software." .


###  http://FYP-ASHS21/csonto/OPS-BCD-16-AI&AutonomousTechnologiesIncidents
<http://FYP-ASHS21/csonto/OPS-BCD-16-AI&AutonomousTechnologiesIncidents> rdf:type owl:NamedIndividual ,
                                                                                  :Security_Operations_Policies ;
                                                                         :HasWeight 10 ;
                                                                         rdfs:comment "Mechanisms exist to handle failures or incidents with Artificial Intelligence (AI) and Autonomous Technologies (AAT) deemed to be high-risk." .


###  http://FYP-ASHS21/csonto/OPS-CRY-07-WirelessAccessAuthentication&Encryption
<http://FYP-ASHS21/csonto/OPS-CRY-07-WirelessAccessAuthentication&Encryption> rdf:type owl:NamedIndividual ,
                                                                                       :Security_Operations_Policies ;
                                                                              :HasWeight 9 ;
                                                                              rdfs:comment "Mechanisms exist to protect wireless access via secure authentication and encryption." .


###  http://FYP-ASHS21/csonto/OPS-CRY-09.4-Control&DistributionofCryptographicKeys
<http://FYP-ASHS21/csonto/OPS-CRY-09.4-Control&DistributionofCryptographicKeys> rdf:type owl:NamedIndividual ,
                                                                                         :Security_Operations_Policies ;
                                                                                :HasWeight 9 ;
                                                                                rdfs:comment "Mechanisms exist to facilitate the secure distribution of symmetric and asymmetric cryptographic keys using industry recognized key management technology and processes. " .


###  http://FYP-ASHS21/csonto/OPS-CRY-10-TransmissionofCybersecurity&DataPrivacyAttributes
<http://FYP-ASHS21/csonto/OPS-CRY-10-TransmissionofCybersecurity&DataPrivacyAttributes> rdf:type owl:NamedIndividual ,
                                                                                                 :Security_Operations_Policies ;
                                                                                        :HasWeight 5 ;
                                                                                        rdfs:comment "Mechanisms exist to ensure systems associate security attributes with information exchanged between systems. " .


###  http://FYP-ASHS21/csonto/OPS-DCH-02-Data&AssetClassification
<http://FYP-ASHS21/csonto/OPS-DCH-02-Data&AssetClassification> rdf:type owl:NamedIndividual ,
                                                                        :Security_Operations_Policies ;
                                                               :HasWeight 10 ;
                                                               rdfs:comment "Mechanisms exist to ensure data and assets are categorized in accordance with applicable statutory, regulatory and contractual requirements. " .


###  http://FYP-ASHS21/csonto/OPS-DCH-05-Cybersecurity&DataPrivacyAttributes
<http://FYP-ASHS21/csonto/OPS-DCH-05-Cybersecurity&DataPrivacyAttributes> rdf:type owl:NamedIndividual ,
                                                                                   :Security_Operations_Policies ;
                                                                          :HasWeight 2 ;
                                                                          rdfs:comment "Mechanisms exist to bind cybersecurity & data privacy attributes to information as it is stored, transmitted and processed." .


###  http://FYP-ASHS21/csonto/OPS-DCH-05.8-IdentityAssociationTechniques&Technologies
<http://FYP-ASHS21/csonto/OPS-DCH-05.8-IdentityAssociationTechniques&Technologies> rdf:type owl:NamedIndividual ,
                                                                                            :Security_Operations_Policies ;
                                                                                   :HasWeight 2 ;
                                                                                   rdfs:comment "Mechanisms exist to associate cybersecurity & data privacy attributes to information." .


###  http://FYP-ASHS21/csonto/OPS-DCH-14.1-InformationSearch&Retrieval
<http://FYP-ASHS21/csonto/OPS-DCH-14.1-InformationSearch&Retrieval> rdf:type owl:NamedIndividual ,
                                                                             :Security_Operations_Policies ;
                                                                    :HasWeight 5 ;
                                                                    rdfs:comment "Mechanisms exist to ensure information systems implement data search and retrieval functions that properly enforce data protection / sharing restrictions." .


###  http://FYP-ASHS21/csonto/OPS-DCH-18-Media&DataRetention
<http://FYP-ASHS21/csonto/OPS-DCH-18-Media&DataRetention> rdf:type owl:NamedIndividual ,
                                                                   :Security_Operations_Policies ;
                                                          :HasWeight 8 ;
                                                          rdfs:comment "Mechanisms exist to retain media and data in accordance with applicable statutory, regulatory and contractual obligations. " .


###  http://FYP-ASHS21/csonto/OPS-DCH-18.2-LimitPersonalData-PD-ElementsInTesting-Training&Research
<http://FYP-ASHS21/csonto/OPS-DCH-18.2-LimitPersonalData-PD-ElementsInTesting-Training&Research> rdf:type owl:NamedIndividual ,
                                                                                                          :Security_Operations_Policies ;
                                                                                                 :HasWeight 8 ;
                                                                                                 rdfs:comment "Mechanisms exist to minimize the use of Personal Data (PD) for research, testing, or training, in accordance with the Data Protection Impact Assessment (DPIA)." .


###  http://FYP-ASHS21/csonto/OPS-DCH-22.1-Updating&CorrectingPersonalData-PD-
<http://FYP-ASHS21/csonto/OPS-DCH-22.1-Updating&CorrectingPersonalData-PD-> rdf:type owl:NamedIndividual ,
                                                                                     :Security_Operations_Policies ;
                                                                            :HasWeight 6 ;
                                                                            rdfs:comment "Mechanisms exist to utilize technical controls to correct Personal Data (PD) that is inaccurate or outdated, incorrectly determined regarding impact, or incorrectly de-identified." .


###  http://FYP-ASHS21/csonto/OPS-END-06.2-IntegrationofDetection&Response
<http://FYP-ASHS21/csonto/OPS-END-06.2-IntegrationofDetection&Response> rdf:type owl:NamedIndividual ,
                                                                                 :Security_Operations_Policies ;
                                                                        :HasWeight 9 ;
                                                                        rdfs:comment "Mechanisms exist to detect and respond to unauthorized configuration changes as cybersecurity incidents." .


###  http://FYP-ASHS21/csonto/OPS-END-08-Phishing&SpamProtection
<http://FYP-ASHS21/csonto/OPS-END-08-Phishing&SpamProtection> rdf:type owl:NamedIndividual ,
                                                                       :Security_Operations_Policies ;
                                                              :HasWeight 10 ;
                                                              rdfs:comment "Mechanisms exist to utilize anti-phishing and spam protection technologies to detect and take action on unsolicited messages transported by electronic mail." .


###  http://FYP-ASHS21/csonto/OPS-END-12-Port&Input-Output-I-O-DeviceAccess
<http://FYP-ASHS21/csonto/OPS-END-12-Port&Input-Output-I-O-DeviceAccess> rdf:type owl:NamedIndividual ,
                                                                                  :Security_Operations_Policies ;
                                                                         :HasWeight 6 ;
                                                                         rdfs:comment "Mechanisms exist to physically disable or remove unnecessary connection ports or input/output devices from sensitive systems." .


###  http://FYP-ASHS21/csonto/OPS-IAC-01-Identity&AccessManagement-IAM-
<http://FYP-ASHS21/csonto/OPS-IAC-01-Identity&AccessManagement-IAM-> rdf:type owl:NamedIndividual ,
                                                                              :Security_Operations_Policies ;
                                                                     :HasWeight 10 ;
                                                                     rdfs:comment "Mechanisms exist to facilitate the implementation of identification and access management controls." .


###  http://FYP-ASHS21/csonto/OPS-IAC-02-Identification&AuthenticationforOrganizationalUsers
<http://FYP-ASHS21/csonto/OPS-IAC-02-Identification&AuthenticationforOrganizationalUsers> rdf:type owl:NamedIndividual ,
                                                                                                   :Security_Operations_Policies ;
                                                                                          :HasWeight 9 ;
                                                                                          rdfs:comment "Mechanisms exist to uniquely identify and centrally Authenticate, Authorize and Audit (AAA) organizational users and processes acting on behalf of organizational users. " .


###  http://FYP-ASHS21/csonto/OPS-IAC-03-Identification&AuthenticationforNon-OrganizationalUsers
<http://FYP-ASHS21/csonto/OPS-IAC-03-Identification&AuthenticationforNon-OrganizationalUsers> rdf:type owl:NamedIndividual ,
                                                                                                       :Security_Operations_Policies ;
                                                                                              :HasWeight 9 ;
                                                                                              rdfs:comment "Mechanisms exist to uniquely identify and centrally Authenticate, Authorize and Audit (AAA) third-party users and processes that provide services to the organization." .


###  http://FYP-ASHS21/csonto/OPS-IAC-04-Identification&AuthenticationforDevices
<http://FYP-ASHS21/csonto/OPS-IAC-04-Identification&AuthenticationforDevices> rdf:type owl:NamedIndividual ,
                                                                                       :Security_Operations_Policies ;
                                                                              :HasWeight 9 ;
                                                                              rdfs:comment "Mechanisms exist to uniquely identify and centrally Authenticate, Authorize and Audit (AAA) devices before establishing a connection using bidirectional authentication that is cryptographically- based and replay resistant." .


###  http://FYP-ASHS21/csonto/OPS-IAC-05-Identification&AuthenticationforThirdPartySystems&Services
<http://FYP-ASHS21/csonto/OPS-IAC-05-Identification&AuthenticationforThirdPartySystems&Services> rdf:type owl:NamedIndividual ,
                                                                                                          :Security_Operations_Policies ;
                                                                                                 :HasWeight 9 ;
                                                                                                 rdfs:comment "Mechanisms exist to identify and authenticate third-party systems and services." .


###  http://FYP-ASHS21/csonto/OPS-IAC-05.1-SharingIdentification&AuthenticationInformation
<http://FYP-ASHS21/csonto/OPS-IAC-05.1-SharingIdentification&AuthenticationInformation> rdf:type owl:NamedIndividual ,
                                                                                                 :Security_Operations_Policies ;
                                                                                        :HasWeight 5 ;
                                                                                        rdfs:comment "Mechanisms exist to ensure external service providers provide current and accurate information for any third-party user with access to the organization's data or assets." .


###  http://FYP-ASHS21/csonto/OPS-IAC-07-UserProvisioning&De-Provisioning
<http://FYP-ASHS21/csonto/OPS-IAC-07-UserProvisioning&De-Provisioning> rdf:type owl:NamedIndividual ,
                                                                                :Security_Operations_Policies ;
                                                                       :HasWeight 10 ;
                                                                       rdfs:comment "Mechanisms exist to utilize a formal user registration and de-registration process that governs the assignment of access rights. " .


###  http://FYP-ASHS21/csonto/OPS-IAC-07.1-ChangeofRoles&Duties
<http://FYP-ASHS21/csonto/OPS-IAC-07.1-ChangeofRoles&Duties> rdf:type owl:NamedIndividual ,
                                                                      :Security_Operations_Policies ;
                                                             :HasWeight 10 ;
                                                             rdfs:comment "Mechanisms exist to revoke user access rights following changes in personnel roles and duties, if no longer necessary or permitted. " .


###  http://FYP-ASHS21/csonto/OPS-IAC-13-AdaptiveIdentification&Authentication
<http://FYP-ASHS21/csonto/OPS-IAC-13-AdaptiveIdentification&Authentication> rdf:type owl:NamedIndividual ,
                                                                                     :Security_Operations_Policies ;
                                                                            :HasWeight 5 ;
                                                                            rdfs:comment "Mechanisms exist to allow individuals to utilize alternative methods of authentication under specific circumstances or situations." .


###  http://FYP-ASHS21/csonto/OPS-IAC-28.3-IdentityEvidenceValidation&Verification
<http://FYP-ASHS21/csonto/OPS-IAC-28.3-IdentityEvidenceValidation&Verification> rdf:type owl:NamedIndividual ,
                                                                                         :Security_Operations_Policies ;
                                                                                :HasWeight 5 ;
                                                                                rdfs:comment "Mechanisms exist to require that the presented identity evidence be validated and verified through organizational-defined methods of validation and verification." .


###  http://FYP-ASHS21/csonto/OPS-IAC-28.4-In-PersonValidation&Verification
<http://FYP-ASHS21/csonto/OPS-IAC-28.4-In-PersonValidation&Verification> rdf:type owl:NamedIndividual ,
                                                                                  :Security_Operations_Policies ;
                                                                         :HasWeight 5 ;
                                                                         rdfs:comment "Mechanisms exist to require that the validation and verification of identity evidence be conducted in person before a designated registration authority." .


###  http://FYP-ASHS21/csonto/OPS-IRO-02.4-IncidentClassification&Prioritization
<http://FYP-ASHS21/csonto/OPS-IRO-02.4-IncidentClassification&Prioritization> rdf:type owl:NamedIndividual ,
                                                                                       :Security_Operations_Policies ;
                                                                              :HasWeight 5 ;
                                                                              rdfs:comment "Mechanisms exist to identify classes of incidents and actions to take to ensure the continuation of organizational missions and business functions." .


###  http://FYP-ASHS21/csonto/OPS-IRO-08-ChainofCustody&Forensics
<http://FYP-ASHS21/csonto/OPS-IRO-08-ChainofCustody&Forensics> rdf:type owl:NamedIndividual ,
                                                                        :Security_Operations_Policies ;
                                                               :HasWeight 9 ;
                                                               rdfs:comment "Mechanisms exist to perform digital forensics and maintain the integrity of the chain of custody, in accordance with applicable laws, regulations and industry-recognized secure practices." .


###  http://FYP-ASHS21/csonto/OPS-IRO-09.1-AutomatedTracking-DataCollection&Analysis
<http://FYP-ASHS21/csonto/OPS-IRO-09.1-AutomatedTracking-DataCollection&Analysis> rdf:type owl:NamedIndividual ,
                                                                                           :Security_Operations_Policies ;
                                                                                  :HasWeight 1 ;
                                                                                  rdfs:comment "Automated mechanisms exist to assist in the tracking, collection and analysis of information from actual and potential cybersecurity & data privacy incidents." .


###  http://FYP-ASHS21/csonto/OPS-IRO-13-RootCauseAnalysis-RCA-&LessonsLearned
<http://FYP-ASHS21/csonto/OPS-IRO-13-RootCauseAnalysis-RCA-&LessonsLearned> rdf:type owl:NamedIndividual ,
                                                                                     :Security_Operations_Policies ;
                                                                            :HasWeight 8 ;
                                                                            rdfs:comment "Mechanisms exist to incorporate lessons learned from analyzing and resolving cybersecurity & data privacy incidents to reduce the likelihood or impact of future incidents. " .


###  http://FYP-ASHS21/csonto/OPS-IRO-14-Regulatory&LawEnforcementContacts
<http://FYP-ASHS21/csonto/OPS-IRO-14-Regulatory&LawEnforcementContacts> rdf:type owl:NamedIndividual ,
                                                                                 :Security_Operations_Policies ;
                                                                        :HasWeight 9 ;
                                                                        rdfs:comment "Mechanisms exist to maintain incident response contacts with applicable regulatory and law enforcement agencies. " .


###  http://FYP-ASHS21/csonto/OPS-IRO-16-PublicRelations&ReputationRepair
<http://FYP-ASHS21/csonto/OPS-IRO-16-PublicRelations&ReputationRepair> rdf:type owl:NamedIndividual ,
                                                                                :Security_Operations_Policies ;
                                                                       :HasWeight 6 ;
                                                                       rdfs:comment "Mechanisms exist to proactively manage public relations associated with incidents and employ appropriate measures to prevent further reputational damage and develop plans to repair any damage to the organization's reputation." .


###  http://FYP-ASHS21/csonto/OPS-MON-01.1-IntrusionDetection&PreventionSystems-IDS&IPS-
<http://FYP-ASHS21/csonto/OPS-MON-01.1-IntrusionDetection&PreventionSystems-IDS&IPS-> rdf:type owl:NamedIndividual ,
                                                                                               :Security_Operations_Policies ;
                                                                                      :HasWeight 9 ;
                                                                                      rdfs:comment "Mechanisms exist to implement Intrusion Detection / Prevention Systems (IDS / IPS) technologies on critical systems, key network segments and network choke points." .


###  http://FYP-ASHS21/csonto/OPS-MON-01.3-Inbound&OutboundCommunicationsTraffic
<http://FYP-ASHS21/csonto/OPS-MON-01.3-Inbound&OutboundCommunicationsTraffic> rdf:type owl:NamedIndividual ,
                                                                                       :Security_Operations_Policies ;
                                                                              :HasWeight 9 ;
                                                                              rdfs:comment "Mechanisms exist to continuously monitor inbound and outbound communications traffic for unusual or unauthorized activities or conditions." .


###  http://FYP-ASHS21/csonto/OPS-MON-01.8-Reviews&Updates
<http://FYP-ASHS21/csonto/OPS-MON-01.8-Reviews&Updates> rdf:type owl:NamedIndividual ,
                                                                 :Security_Operations_Policies ;
                                                        :HasWeight 10 ;
                                                        rdfs:comment "Mechanisms exist to review event logs on an ongoing basis and escalate incidents in accordance with established timelines and procedures." .


###  http://FYP-ASHS21/csonto/OPS-MON-02.2-CentralReview&Analysis
<http://FYP-ASHS21/csonto/OPS-MON-02.2-CentralReview&Analysis> rdf:type owl:NamedIndividual ,
                                                                        :Security_Operations_Policies ;
                                                               :HasWeight 5 ;
                                                               rdfs:comment "Automated mechanisms exist to centrally collect, review and analyze audit records from multiple sources." .


###  http://FYP-ASHS21/csonto/OPS-MON-02.3-IntegrationofScanning&OtherMonitoringInformation
<http://FYP-ASHS21/csonto/OPS-MON-02.3-IntegrationofScanning&OtherMonitoringInformation> rdf:type owl:NamedIndividual ,
                                                                                                  :Security_Operations_Policies ;
                                                                                         :HasWeight 5 ;
                                                                                         rdfs:comment "Automated mechanisms exist to integrate the analysis of audit records with analysis of vulnerability scanners, network performance, system monitoring and other sources to further enhance the ability to identify inappropriate or unusual activity." .


###  http://FYP-ASHS21/csonto/OPS-NET-03.6-DynamicIsolation&Segregation-Sandboxing-
<http://FYP-ASHS21/csonto/OPS-NET-03.6-DynamicIsolation&Segregation-Sandboxing-> rdf:type owl:NamedIndividual ,
                                                                                          :Security_Operations_Policies ;
                                                                                 :HasWeight 5 ;
                                                                                 rdfs:comment "Automated mechanisms exist to dynamically isolate (e.g., sandbox) untrusted components during runtime, where the component is isolated in a fault-contained environment but it can still collaborate with the application. " .


###  http://FYP-ASHS21/csonto/OPS-NET-04-DataFlowEnforcementAccessControlLists-ACLs-
<http://FYP-ASHS21/csonto/OPS-NET-04-DataFlowEnforcementAccessControlLists-ACLs-> rdf:type owl:NamedIndividual ,
                                                                                            :Security_Operations_Policies ;
                                                                                   :HasWeight 10 ;
                                                                                   rdfs:comment "Mechanisms exist to design, implement and review firewall and router configurations to restrict connections between untrusted networks and internal systems. " .


###  http://FYP-ASHS21/csonto/OPS-NET-04.1-DenyTrafficbyDefault&AllowTrafficbyException
<http://FYP-ASHS21/csonto/OPS-NET-04.1-DenyTrafficbyDefault&AllowTrafficbyException> rdf:type owl:NamedIndividual ,
                                                                                              :Security_Operations_Policies ;
                                                                                     :HasWeight 10 ;
                                                                                     rdfs:comment "Mechanisms exist to configure firewall and router configurations to deny network traffic by default and allow network traffic by exception (e.g., deny all, permit by exception). " .


###  http://FYP-ASHS21/csonto/OPS-NET-10.1-Architecture&ProvisioningforName-AddressResolutionService
<http://FYP-ASHS21/csonto/OPS-NET-10.1-Architecture&ProvisioningforName-AddressResolutionService> rdf:type owl:NamedIndividual ,
                                                                                                           :Security_Operations_Policies ;
                                                                                                  :HasWeight 9 ;
                                                                                                  rdfs:comment "Mechanisms exist to ensure systems that collectively provide Domain Name Service (DNS) resolution service are fault-tolerant and implement internal/external role separation. " .


###  http://FYP-ASHS21/csonto/OPS-NET-14.1-AutomatedMonitoring&Control
<http://FYP-ASHS21/csonto/OPS-NET-14.1-AutomatedMonitoring&Control> rdf:type owl:NamedIndividual ,
                                                                             :Security_Operations_Policies ;
                                                                    :HasWeight 1 ;
                                                                    rdfs:comment "Automated mechanisms exist to monitor and control remote access sessions. " .


###  http://FYP-ASHS21/csonto/OPS-NET-14.4-RemotePrivilegedCommands&SensitiveDataAccess
<http://FYP-ASHS21/csonto/OPS-NET-14.4-RemotePrivilegedCommands&SensitiveDataAccess> rdf:type owl:NamedIndividual ,
                                                                                              :Security_Operations_Policies ;
                                                                                     :HasWeight 8 ;
                                                                                     rdfs:comment "Mechanisms exist to restrict the execution of privileged commands and access to security-relevant information via remote access only for compelling operational needs. " .


###  http://FYP-ASHS21/csonto/OPS-NET-15.1-Authentication&Encryption
<http://FYP-ASHS21/csonto/OPS-NET-15.1-Authentication&Encryption> rdf:type owl:NamedIndividual ,
                                                                           :Security_Operations_Policies ;
                                                                  :HasWeight 9 ;
                                                                  rdfs:comment "Mechanisms exist to protect wireless access through authentication and strong encryption. " .


###  http://FYP-ASHS21/csonto/OPS-NET-18-DNS&ContentFiltering
<http://FYP-ASHS21/csonto/OPS-NET-18-DNS&ContentFiltering> rdf:type owl:NamedIndividual ,
                                                                    :Security_Operations_Policies ;
                                                           :HasWeight 9 ;
                                                           rdfs:comment "Mechanisms exist to force Internet-bound network traffic through a proxy device for URL content filtering and DNS filtering to limit a user's ability to connect to dangerous or prohibited Internet sites." .


###  http://FYP-ASHS21/csonto/OPS-PRI-03-Choice&Consent
<http://FYP-ASHS21/csonto/OPS-PRI-03-Choice&Consent> rdf:type owl:NamedIndividual ,
                                                              :Security_Operations_Policies ;
                                                     :HasWeight 7 ;
                                                     rdfs:comment """Mechanisms exist to authorize the processing of their Personal Data (PD) prior to its collection that:
 Uses plain language and provide examples to illustrate the potential data privacy risks of the authorization; and
 Provides a means for users to decline the authorization.
""" .


###  http://FYP-ASHS21/csonto/OPS-PRI-03.2-Just-In-TimeNotice&UpdatedConsent
<http://FYP-ASHS21/csonto/OPS-PRI-03.2-Just-In-TimeNotice&UpdatedConsent> rdf:type owl:NamedIndividual ,
                                                                                   :Security_Operations_Policies ;
                                                                          :HasWeight 1 ;
                                                                          rdfs:comment """Mechanisms exist to present authorizations to process Personal Data (PD) in conjunction with the data action, when:
 The original circumstances under which an individual gave consent have changed; or
 A significant amount of time has passed since an individual gave consent.""" .


###  http://FYP-ASHS21/csonto/OPS-PRI-04.1-AuthorityToCollect-Use-Maintain&SharePersonalData
<http://FYP-ASHS21/csonto/OPS-PRI-04.1-AuthorityToCollect-Use-Maintain&SharePersonalData> rdf:type owl:NamedIndividual ,
                                                                                                   :Security_Operations_Policies ;
                                                                                          :HasWeight 7 ;
                                                                                          rdfs:comment "Mechanisms exist to determine and document the legal authority that permits the collection, use, maintenance and sharing of Personal Data (PD), either generally or in support of a specific program or system need." .


###  http://FYP-ASHS21/csonto/OPS-PRI-05-PersonalDataRetention&Disposal
<http://FYP-ASHS21/csonto/OPS-PRI-05-PersonalDataRetention&Disposal> rdf:type owl:NamedIndividual ,
                                                                              :Security_Operations_Policies ;
                                                                     :HasWeight 8 ;
                                                                     rdfs:comment """Mechanisms exist to: 
  Retain Personal Data (PD), including metadata, for an organization-defined time period to fulfill the purpose(s) identified in the notice or as required by law;
  Dispose of, destroys, erases, and/or anonymizes the PD, regardless of the method of storage; and
  Use organization-defined techniques or methods to ensure secure deletion or destruction of PD (including originals, copies and archived records).""" .


###  http://FYP-ASHS21/csonto/OPS-PRI-05.2-PersonalDataAccuracy&Integrity
<http://FYP-ASHS21/csonto/OPS-PRI-05.2-PersonalDataAccuracy&Integrity> rdf:type owl:NamedIndividual ,
                                                                                :Security_Operations_Policies ;
                                                                       :HasWeight 5 ;
                                                                       rdfs:comment "Mechanisms exist to confirm the accuracy and relevance of Personal Data (PD) throughout the information lifecycle." .


###  http://FYP-ASHS21/csonto/OPS-PRI-07.1-DataPrivacyRequirementsforContractors&ServiceProviders
<http://FYP-ASHS21/csonto/OPS-PRI-07.1-DataPrivacyRequirementsforContractors&ServiceProviders> rdf:type owl:NamedIndividual ,
                                                                                                        :Security_Operations_Policies ;
                                                                                               :HasWeight 10 ;
                                                                                               rdfs:comment "Mechanisms exist to include data privacy requirements in contracts and other acquisition-related documents that establish data privacy roles and responsibilities for contractors and service providers. " .


###  http://FYP-ASHS21/csonto/OPS-PRI-08-Testing-Training&Monitoring
<http://FYP-ASHS21/csonto/OPS-PRI-08-Testing-Training&Monitoring> rdf:type owl:NamedIndividual ,
                                                                           :Security_Operations_Policies ;
                                                                  :HasWeight 8 ;
                                                                  rdfs:comment """Mechanisms exist to conduct cybersecurity & data privacy testing, training and monitoring activities
""" .


###  http://FYP-ASHS21/csonto/OPS-PRI-14-DataPrivacyRecords&Reporting
<http://FYP-ASHS21/csonto/OPS-PRI-14-DataPrivacyRecords&Reporting> rdf:type owl:NamedIndividual ,
                                                                            :Security_Operations_Policies ;
                                                                   :HasWeight 8 ;
                                                                   rdfs:comment "Mechanisms exist to maintain data privacy-related records and develop, disseminate and update reports to internal senior management, as well as external oversight bodies, as appropriate, to demonstrate accountability with specific statutory and regulatory data privacy program mandates." .


###  http://FYP-ASHS21/csonto/OPS-VPM-01-Vulnerability&PatchManagementProgram-VPMP-
<http://FYP-ASHS21/csonto/OPS-VPM-01-Vulnerability&PatchManagementProgram-VPMP-> rdf:type owl:NamedIndividual ,
                                                                                          :Security_Operations_Policies ;
                                                                                 :HasWeight 9 ;
                                                                                 rdfs:comment "Mechanisms exist to facilitate the implementation and monitoring of vulnerability management controls." .


###  http://FYP-ASHS21/csonto/OPS-VPM-05-Software&FirmwarePatching
<http://FYP-ASHS21/csonto/OPS-VPM-05-Software&FirmwarePatching> rdf:type owl:NamedIndividual ,
                                                                         :Security_Operations_Policies ;
                                                                :HasWeight 10 ;
                                                                rdfs:comment "Mechanisms exist to conduct software patching for all deployed operating systems, applications and firmware." .


###  http://FYP-ASHS21/csonto/OPS-VPM-05.4-AutomatedSoftware&FirmwareUpdates
<http://FYP-ASHS21/csonto/OPS-VPM-05.4-AutomatedSoftware&FirmwareUpdates> rdf:type owl:NamedIndividual ,
                                                                                   :Security_Operations_Policies ;
                                                                          :HasWeight 5 ;
                                                                          rdfs:comment "Automated mechanisms exist to install the latest stable versions of security-relevant software and firmware updates." .


###  http://FYP-ASHS21/csonto/OPS-WEB-09-Validation&Sanitization
<http://FYP-ASHS21/csonto/OPS-WEB-09-Validation&Sanitization> rdf:type owl:NamedIndividual ,
                                                                       :Security_Operations_Policies ;
                                                              :HasWeight 9 ;
                                                              rdfs:comment "Mechanisms exist to ensure all input handled by a web application is validated and/or sanitized." .


#################################################################
#    General axioms
#################################################################

[ rdf:type owl:AllDisjointClasses ;
  owl:members ( :BusinessContinuity_And_DiasterRecovery
                :Continuous_Monitoring
                :Incident_Response
              )
] .


[ rdf:type owl:AllDisjointClasses ;
  owl:members ( :Capacity_And_Performance_PLanning
                :Configuration_Management
                :Mobile_Device_Management
              )
] .


[ rdf:type owl:AllDisjointClasses ;
  owl:members ( :Data_Protection
                :Embdded_Technologies
                :Infrastructure_And_Identity_And_Access_Management
                :Threat_Management
                :Vulnerability_And_Web_Management
              )
] .


[ rdf:type owl:AllDisjointClasses ;
  owl:members ( :Asset_Management_Policies
                :Assurance_Policies
                :Change_Management_Policies
                :Emerging_Technologies_Policies
                :Governance_Policies
                :Security_Operations_Policies
              )
] .


###  Generated by the OWL API (version 4.5.26.2023-07-17T20:34:13Z) https://github.com/owlcs/owlapi
